<?xml version="1.0" encoding="UTF-8"?>
<rdf:RDF xmlns:rdf="http://www.w3.org/1999/02/22-rdf-syntax-ns#"
  xmlns:dct="http://purl.org/dc/terms/"
  xmlns:schema="http://schema.org/"
  xmlns:skos="http://www.w3.org/2004/02/skos/core#"
  xmlns:sdmx-attribute="http://purl.org/linked-data/sdmx/2009/attribute#"
  xmlns:rdfs="http://www.w3.org/2000/01/rdf-schema#">

  <rdf:Description rdf:about="http://data.landportal.info/indicator/OECD-SIGI2019.SIGI.RCL">
    <rdf:type rdf:resource="http://www.w3.org/2004/02/skos/core#Concept"/>
    <rdf:type rdf:resource="http://purl.org/weso/ontology/computex#Indicator"/>
    <dct:subject rdf:resource="http://aims.fao.org/aos/agrovoc/c_8420"/>
    <dct:subject rdf:resource="http://data.landportal.info/voc/landvoc/overarching-category/OA-ACCESS"/>
    <dct:subject rdf:resource="http://data.landportal.info/voc/landvoc/overarching-category/OA-LAW"/>
    <dct:subject rdf:resource="http://data.landportal.info/voc/landvoc/theme/T-GENDER"/>
    <dct:subject rdf:resource="http://data.landportal.info/voc/landvoc/theme/T-INST"/>
    <schema:about rdf:resource="http://aims.fao.org/aos/agrovoc/c_8420"/>
    <schema:about rdf:resource="http://data.landportal.info/voc/landvoc/overarching-category/OA-ACCESS"/>
    <schema:about rdf:resource="http://data.landportal.info/voc/landvoc/overarching-category/OA-LAW"/>
    <schema:about rdf:resource="http://data.landportal.info/voc/landvoc/theme/T-GENDER"/>
    <schema:about rdf:resource="http://data.landportal.info/voc/landvoc/theme/T-INST"/>
    <dct:identifier>OECD-SIGI2019.SIGI.RCL</dct:identifier>
    <skos:notation>OECD-SIGI2019.SIGI.RCL</skos:notation>
    <dct:source rdf:resource="http://data.landportal.info/dataset/OECD-SIGI2019"/>
    <sdmx-attribute:unitMeasure>Index (0; 100)</sdmx-attribute:unitMeasure>
    <rdfs:label>Restricted civil liberties (SIGI2019)</rdfs:label>
    <skos:prefLabel>Restricted civil liberties (SIGI2019)</skos:prefLabel>
    <dct:title>Restricted civil liberties (SIGI2019)</dct:title>
    <skos:definition>This sub-index captures discriminatory laws and practices that restrict women’s access to public space, their political voice and their participation in all aspects of public life. This includes a lack of freedom of movement, the inability to vote or run for election, and negative attitudes toward women as public figures or as leaders. This sub-index highlights the importance of women’s participation in community actions and public decision making for a range of development outcomes such as governance, health and education. Source: OECD Development Centre’s Social Institutions and Gender Index (SIGI) website</skos:definition>
    <dct:description>This sub-index captures discriminatory laws and practices that restrict women’s access to public space, their political voice and their participation in all aspects of public life. This includes a lack of freedom of movement, the inability to vote or run for election, and negative attitudes toward women as public figures or as leaders. This sub-index highlights the importance of women’s participation in community actions and public decision making for a range of development outcomes such as governance, health and education. Source: OECD Development Centre’s Social Institutions and Gender Index (SIGI) website</dct:description>
    <rdfs:comment>This sub-index captures discriminatory laws and practices that restrict women’s access to public space, their political voice and their participation in all aspects of public life. This includes a lack of freedom of movement, the inability to vote or run for election, and negative attitudes toward women as public figures or as leaders. This sub-index highlights the importance of women’s participation in community actions and public decision making for a range of development outcomes such as governance, health and education. Source: OECD Development Centre’s Social Institutions and Gender Index (SIGI) website</rdfs:comment>
    <skos:inScheme rdf:resource="http://data.landportal.info/vocabulary/25"/>
    <rdfs:seeAlso rdf:resource="https://landportal.org/book/indicator/oecd-sigi2019sigircl"/>
  </rdf:Description>

</rdf:RDF>