<?xml version="1.0" encoding="UTF-8"?>
<rdf:RDF xmlns:rdf="http://www.w3.org/1999/02/22-rdf-syntax-ns#"
  xmlns:dct="http://purl.org/dc/terms/"
  xmlns:schema="http://schema.org/"
  xmlns:skos="http://www.w3.org/2004/02/skos/core#"
  xmlns:sdmx-attribute="http://purl.org/linked-data/sdmx/2009/attribute#"
  xmlns:rdfs="http://www.w3.org/2000/01/rdf-schema#">

  <rdf:Description rdf:about="http://data.landportal.info/indicator/OECD-SIGI2019.SALA.PRACT">
    <rdf:type rdf:resource="http://www.w3.org/2004/02/skos/core#Concept"/>
    <rdf:type rdf:resource="http://purl.org/weso/ontology/computex#Indicator"/>
    <dct:subject rdf:resource="http://aims.fao.org/aos/agrovoc/c_8420"/>
    <dct:subject rdf:resource="http://data.landportal.info/voc/landvoc/overarching-category/OA-ACCESS"/>
    <dct:subject rdf:resource="http://data.landportal.info/voc/landvoc/overarching-category/OA-LAW"/>
    <dct:subject rdf:resource="http://data.landportal.info/voc/landvoc/theme/T-GENDER"/>
    <dct:subject rdf:resource="http://data.landportal.info/voc/landvoc/theme/T-INST"/>
    <schema:about rdf:resource="http://aims.fao.org/aos/agrovoc/c_8420"/>
    <schema:about rdf:resource="http://data.landportal.info/voc/landvoc/overarching-category/OA-ACCESS"/>
    <schema:about rdf:resource="http://data.landportal.info/voc/landvoc/overarching-category/OA-LAW"/>
    <schema:about rdf:resource="http://data.landportal.info/voc/landvoc/theme/T-GENDER"/>
    <schema:about rdf:resource="http://data.landportal.info/voc/landvoc/theme/T-INST"/>
    <dct:identifier>OECD-SIGI2019.SALA.PRACT</dct:identifier>
    <skos:notation>OECD-SIGI2019.SALA.PRACT</skos:notation>
    <dct:source rdf:resource="http://data.landportal.info/dataset/OECD-SIGI2019"/>
    <sdmx-attribute:unitMeasure>Index (0; 1)</sdmx-attribute:unitMeasure>
    <rdfs:label>Secure access to land assets - Practice (SIGI2019)</rdfs:label>
    <skos:prefLabel>Secure access to land assets - Practice (SIGI2019)</skos:prefLabel>
    <dct:title>Secure access to land assets - Practice (SIGI2019)</dct:title>
    <skos:definition>Laws on access to land assets: Whether women and men have the same legal rights and secure access to land assets 0: Women and men have the same legal rights and secure access to land assets, without legal exceptions regarding some groups of women. Customary, religious and traditional laws or practices do not discriminate against women’s legal rights. 0.25: Women and men have the same legal rights and secure access to land assets, without legal exceptions regarding some groups of women. However, some customary, religious or traditional practices or laws discriminate against women’s legal right. 0.5: Women and men have the same legal rights and secure access to land assets. However, this does not apply to all groups of women. 0.75: Women and men have the same legal rights to own land assets; but not to use, make decisions and/or use land assets as collateral. 1: Women do not have the same legal rights as men to own land assets. Source: OECD Development Centre’s Social Institutions and Gender Index (SIGI) website</skos:definition>
    <dct:description>Laws on access to land assets: Whether women and men have the same legal rights and secure access to land assets 0: Women and men have the same legal rights and secure access to land assets, without legal exceptions regarding some groups of women. Customary, religious and traditional laws or practices do not discriminate against women’s legal rights. 0.25: Women and men have the same legal rights and secure access to land assets, without legal exceptions regarding some groups of women. However, some customary, religious or traditional practices or laws discriminate against women’s legal right. 0.5: Women and men have the same legal rights and secure access to land assets. However, this does not apply to all groups of women. 0.75: Women and men have the same legal rights to own land assets; but not to use, make decisions and/or use land assets as collateral. 1: Women do not have the same legal rights as men to own land assets. Source: OECD Development Centre’s Social Institutions and Gender Index (SIGI) website</dct:description>
    <rdfs:comment>Laws on access to land assets: Whether women and men have the same legal rights and secure access to land assets 0: Women and men have the same legal rights and secure access to land assets, without legal exceptions regarding some groups of women. Customary, religious and traditional laws or practices do not discriminate against women’s legal rights. 0.25: Women and men have the same legal rights and secure access to land assets, without legal exceptions regarding some groups of women. However, some customary, religious or traditional practices or laws discriminate against women’s legal right. 0.5: Women and men have the same legal rights and secure access to land assets. However, this does not apply to all groups of women. 0.75: Women and men have the same legal rights to own land assets; but not to use, make decisions and/or use land assets as collateral. 1: Women do not have the same legal rights as men to own land assets. Source: OECD Development Centre’s Social Institutions and Gender Index (SIGI) website</rdfs:comment>
    <skos:inScheme rdf:resource="http://data.landportal.info/vocabulary/25"/>
    <rdfs:seeAlso rdf:resource="https://landportal.org/book/indicator/oecd-sigi2019salapract"/>
  </rdf:Description>

</rdf:RDF>