<?xml version="1.0" encoding="UTF-8"?>
<rdf:RDF xmlns:rdf="http://www.w3.org/1999/02/22-rdf-syntax-ns#"
  xmlns:dct="http://purl.org/dc/terms/"
  xmlns:skos="http://www.w3.org/2004/02/skos/core#"
  xmlns:sdmx-attribute="http://purl.org/linked-data/sdmx/2009/attribute#"
  xmlns:schema="http://schema.org/"
  xmlns:rdfs="http://www.w3.org/2000/01/rdf-schema#">

  <rdf:Description rdf:about="http://data.landportal.info/indicator/FAO-6655-5110">
    <rdf:type rdf:resource="http://www.w3.org/2004/02/skos/core#Concept"/>
    <rdf:type rdf:resource="http://purl.org/weso/ontology/computex#Indicator"/>
    <dct:source rdf:resource="http://data.landportal.info/dataset/FAO-LU"/>
    <sdmx-attribute:unitMeasure>1'000 Ha</sdmx-attribute:unitMeasure>
    <dct:identifier>FAO-6655-5110</dct:identifier>
    <skos:notation>FAO-6655-5110</skos:notation>
    <dct:subject rdf:resource="http://aims.fao.org/aos/agrovoc/c_16112"/>
    <dct:subject rdf:resource="http://aims.fao.org/aos/agrovoc/c_4182"/>
    <dct:subject rdf:resource="http://aims.fao.org/aos/agrovoc/c_8e487587"/>
    <dct:subject rdf:resource="http://data.landportal.info/voc/landvoc/theme/T-PASTOR"/>
    <schema:about rdf:resource="http://aims.fao.org/aos/agrovoc/c_16112"/>
    <schema:about rdf:resource="http://aims.fao.org/aos/agrovoc/c_4182"/>
    <schema:about rdf:resource="http://aims.fao.org/aos/agrovoc/c_8e487587"/>
    <schema:about rdf:resource="http://data.landportal.info/voc/landvoc/theme/T-PASTOR"/>
    <rdfs:label>Land under perm. meadows and pastures</rdfs:label>
    <skos:prefLabel>Land under perm. meadows and pastures</skos:prefLabel>
    <dct:title>Land under perm. meadows and pastures</dct:title>
    <skos:definition>Land used permanently (five years or more) to grow herbaceous forage crops through cultivation or naturally (wild prairie or grazing land). Permanent meadows and pastures on which trees and shrubs are grown should be recorded under this heading only if the growing of forage crops is the most important use of the area. Measures may be taken to keep or increase productivity of the land (i.e., use of fertilizers, mowing or systematic grazing by domestic animals.) This class includes: Grazing in wooded areas (agroforestry areas, for example) Grazing in shrubby zones (heath, maquis, garigue) Grassland in the plain or low mountain areas used for grazing: land crossed during transhumance where the animals spend a part of the year (approximately 100 days) without returning to the holding in the evening: mountain and subalpine meadows and similar; and steppes and dry meadows used for pasture. Previously known as &quot;Permanent meadows and pastures&quot;</skos:definition>
    <dct:description>Land used permanently (five years or more) to grow herbaceous forage crops through cultivation or naturally (wild prairie or grazing land). Permanent meadows and pastures on which trees and shrubs are grown should be recorded under this heading only if the growing of forage crops is the most important use of the area. Measures may be taken to keep or increase productivity of the land (i.e., use of fertilizers, mowing or systematic grazing by domestic animals.) This class includes: Grazing in wooded areas (agroforestry areas, for example) Grazing in shrubby zones (heath, maquis, garigue) Grassland in the plain or low mountain areas used for grazing: land crossed during transhumance where the animals spend a part of the year (approximately 100 days) without returning to the holding in the evening: mountain and subalpine meadows and similar; and steppes and dry meadows used for pasture. Previously known as &quot;Permanent meadows and pastures&quot;</dct:description>
    <rdfs:comment>Land used permanently (five years or more) to grow herbaceous forage crops through cultivation or naturally (wild prairie or grazing land). Permanent meadows and pastures on which trees and shrubs are grown should be recorded under this heading only if the growing of forage crops is the most important use of the area. Measures may be taken to keep or increase productivity of the land (i.e., use of fertilizers, mowing or systematic grazing by domestic animals.) This class includes: Grazing in wooded areas (agroforestry areas, for example) Grazing in shrubby zones (heath, maquis, garigue) Grassland in the plain or low mountain areas used for grazing: land crossed during transhumance where the animals spend a part of the year (approximately 100 days) without returning to the holding in the evening: mountain and subalpine meadows and similar; and steppes and dry meadows used for pasture. Previously known as &quot;Permanent meadows and pastures&quot;</rdfs:comment>
    <skos:inScheme rdf:resource="http://data.landportal.info/vocabulary/25"/>
    <rdfs:seeAlso rdf:resource="https://landportal.org/book/indicators/fao-6655-5110"/>
  </rdf:Description>

</rdf:RDF>