<?xml version="1.0" encoding="UTF-8"?>
<rdf:RDF xmlns:rdf="http://www.w3.org/1999/02/22-rdf-syntax-ns#"
  xmlns:dct="http://purl.org/dc/terms/"
  xmlns:skos="http://www.w3.org/2004/02/skos/core#"
  xmlns:sdmx-attribute="http://purl.org/linked-data/sdmx/2009/attribute#"
  xmlns:schema="http://schema.org/"
  xmlns:rdfs="http://www.w3.org/2000/01/rdf-schema#">

  <rdf:Description rdf:about="http://data.landportal.info/indicator/FAO-6620-5110">
    <rdf:type rdf:resource="http://www.w3.org/2004/02/skos/core#Concept"/>
    <rdf:type rdf:resource="http://purl.org/weso/ontology/computex#Indicator"/>
    <dct:source rdf:resource="http://data.landportal.info/dataset/FAO-LU"/>
    <sdmx-attribute:unitMeasure>1'000 Ha</sdmx-attribute:unitMeasure>
    <dct:identifier>FAO-6620-5110</dct:identifier>
    <skos:notation>FAO-6620-5110</skos:notation>
    <dct:subject rdf:resource="http://aims.fao.org/aos/agrovoc/c_203"/>
    <dct:subject rdf:resource="http://aims.fao.org/aos/agrovoc/c_2593"/>
    <dct:subject rdf:resource="http://aims.fao.org/aos/agrovoc/c_10967"/>
    <dct:subject rdf:resource="http://aims.fao.org/aos/agrovoc/c_4182"/>
    <dct:subject rdf:resource="http://data.landportal.info/voc/landvoc/theme/T-FOOD"/>
    <dct:subject rdf:resource="http://data.landportal.info/voc/landvoc/theme/T-ENVIR"/>
    <schema:about rdf:resource="http://aims.fao.org/aos/agrovoc/c_203"/>
    <schema:about rdf:resource="http://aims.fao.org/aos/agrovoc/c_2593"/>
    <schema:about rdf:resource="http://aims.fao.org/aos/agrovoc/c_10967"/>
    <schema:about rdf:resource="http://aims.fao.org/aos/agrovoc/c_4182"/>
    <schema:about rdf:resource="http://data.landportal.info/voc/landvoc/theme/T-FOOD"/>
    <schema:about rdf:resource="http://data.landportal.info/voc/landvoc/theme/T-ENVIR"/>
    <rdfs:label>Cropland</rdfs:label>
    <skos:prefLabel>Cropland</skos:prefLabel>
    <dct:title>Cropland</dct:title>
    <skos:definition>Land used for cultivation of crops. The total of areas under &amp;#039;&amp;#039;Arable land&amp;#039;&amp;#039; and &amp;#039;&amp;#039;Permanent crops&amp;#039;&amp;#039;. Previously known as &amp;quot;Arable land and Permanent crops&amp;quot;</skos:definition>
    <dct:description>Land used for cultivation of crops. The total of areas under &amp;#039;&amp;#039;Arable land&amp;#039;&amp;#039; and &amp;#039;&amp;#039;Permanent crops&amp;#039;&amp;#039;. Previously known as &amp;quot;Arable land and Permanent crops&amp;quot;</dct:description>
    <rdfs:comment>Land used for cultivation of crops. The total of areas under &amp;#039;&amp;#039;Arable land&amp;#039;&amp;#039; and &amp;#039;&amp;#039;Permanent crops&amp;#039;&amp;#039;. Previously known as &amp;quot;Arable land and Permanent crops&amp;quot;</rdfs:comment>
    <skos:inScheme rdf:resource="http://data.landportal.info/vocabulary/25"/>
    <rdfs:seeAlso rdf:resource="https://landportal.org/book/indicator/fao-6620-5110"/>
  </rdf:Description>

</rdf:RDF>