<?xml version="1.0" encoding="UTF-8"?>
<rdf:RDF xmlns:rdf="http://www.w3.org/1999/02/22-rdf-syntax-ns#"
  xmlns:dct="http://purl.org/dc/terms/"
  xmlns:skos="http://www.w3.org/2004/02/skos/core#"
  xmlns:schema="http://schema.org/"
  xmlns:rdfs="http://www.w3.org/2000/01/rdf-schema#">

  <rdf:Description rdf:about="http://data.landportal.info/indicator/FAO-23045-6084">
    <rdf:type rdf:resource="http://www.w3.org/2004/02/skos/core#Concept"/>
    <rdf:type rdf:resource="http://purl.org/weso/ontology/computex#Indicator"/>
    <dct:identifier>FAO-23045-6084</dct:identifier>
    <skos:notation>FAO-23045-6084</skos:notation>
    <dct:subject rdf:resource="http://aims.fao.org/aos/agrovoc/c_203"/>
    <dct:subject rdf:resource="http://aims.fao.org/aos/agrovoc/c_6513"/>
    <dct:subject rdf:resource="http://aims.fao.org/aos/agrovoc/c_35332"/>
    <dct:subject rdf:resource="http://data.landportal.info/voc/landvoc/theme/T-INST"/>
    <schema:about rdf:resource="http://aims.fao.org/aos/agrovoc/c_203"/>
    <schema:about rdf:resource="http://aims.fao.org/aos/agrovoc/c_6513"/>
    <schema:about rdf:resource="http://aims.fao.org/aos/agrovoc/c_35332"/>
    <schema:about rdf:resource="http://data.landportal.info/voc/landvoc/theme/T-INST"/>
    <dct:source rdf:resource="http://data.landportal.info/dataset/FAO-ASTI"/>
    <rdfs:label>Agriculture research spending (2011 PPP$)</rdfs:label>
    <skos:prefLabel>Agriculture research spending (2011 PPP$)</skos:prefLabel>
    <dct:title>Agriculture research spending (2011 PPP$)</dct:title>
    <skos:definition>Total spending for agricultural reserch measured in 2011 PPP$.</skos:definition>
    <dct:description>Total spending for agricultural reserch measured in 2011 PPP$.</dct:description>
    <rdfs:comment>Total spending for agricultural reserch measured in 2011 PPP$.</rdfs:comment>
    <skos:inScheme rdf:resource="http://data.landportal.info/vocabulary/25"/>
    <rdfs:seeAlso rdf:resource="https://landportal.org/book/indicators/fao-23045-6084"/>
  </rdf:Description>

</rdf:RDF>