<?xml version="1.0" encoding="UTF-8"?>
<rdf:RDF xmlns:rdf="http://www.w3.org/1999/02/22-rdf-syntax-ns#"
  xmlns:dct="http://purl.org/dc/terms/"
  xmlns:schema="http://schema.org/"
  xmlns:skos="http://www.w3.org/2004/02/skos/core#"
  xmlns:sdmx-attribute="http://purl.org/linked-data/sdmx/2009/attribute#"
  xmlns:rdfs="http://www.w3.org/2000/01/rdf-schema#">

  <rdf:Description rdf:about="http://data.landportal.info/indicator/NKT-VGGT16-1C">
    <rdf:type rdf:resource="http://www.w3.org/2004/02/skos/core#Concept"/>
    <rdf:type rdf:resource="http://purl.org/weso/ontology/computex#Indicator"/>
    <dct:subject rdf:resource="http://aims.fao.org/aos/agrovoc/c_ff890f6b"/>
    <dct:subject rdf:resource="http://aims.fao.org/aos/agrovoc/c_331524"/>
    <dct:subject rdf:resource="http://aims.fao.org/aos/agrovoc/c_37898"/>
    <dct:subject rdf:resource="http://aims.fao.org/aos/agrovoc/c_66afb052"/>
    <dct:subject rdf:resource="http://aims.fao.org/aos/agrovoc/c_45cd8441"/>
    <dct:subject rdf:resource="http://aims.fao.org/aos/agrovoc/c_7fc44e33"/>
    <dct:subject rdf:resource="http://data.landportal.info/voc/landvoc/theme/T-INDIG"/>
    <dct:subject rdf:resource="http://data.landportal.info/voc/landvoc/theme/T-INVEST"/>
    <schema:about rdf:resource="http://aims.fao.org/aos/agrovoc/c_ff890f6b"/>
    <schema:about rdf:resource="http://aims.fao.org/aos/agrovoc/c_331524"/>
    <schema:about rdf:resource="http://aims.fao.org/aos/agrovoc/c_37898"/>
    <schema:about rdf:resource="http://aims.fao.org/aos/agrovoc/c_66afb052"/>
    <schema:about rdf:resource="http://aims.fao.org/aos/agrovoc/c_45cd8441"/>
    <schema:about rdf:resource="http://aims.fao.org/aos/agrovoc/c_7fc44e33"/>
    <schema:about rdf:resource="http://data.landportal.info/voc/landvoc/theme/T-INDIG"/>
    <schema:about rdf:resource="http://data.landportal.info/voc/landvoc/theme/T-INVEST"/>
    <dct:identifier>NKT-VGGT16-1C</dct:identifier>
    <skos:notation>NKT-VGGT16-1C</skos:notation>
    <dct:source rdf:resource="http://data.landportal.info/dataset/NKT-VGGT16"/>
    <sdmx-attribute:unitMeasure>Index (A; C)</sdmx-attribute:unitMeasure>
    <rdfs:label>Compensation for formally recognized customary tenure rights</rdfs:label>
    <skos:prefLabel>Compensation for formally recognized customary tenure rights</skos:prefLabel>
    <dct:title>Compensation for formally recognized customary tenure rights</dct:title>
    <skos:definition>This indicator asks whether national laws adopt VGGT principle 16.1 by providing compensation for formally recognized tenure rights held by Indigenous Peoples and local communities. Section 16. 1 provides that States should respect legitimate tenure rights by providing just compensation. Principle 9 of the VGGTs calls for States to respect and protect the legitimate tenure rights of Indigenous Peoples and local communities with customary tenure. Answering the question posed by the indicator entailed reviewing a broad range of legally binding statutes, regulations, and some court decisions at the national level. For more info, see: http://www.wri.org/publication/encroaching-on-land-and-livelihoods</skos:definition>
    <dct:description>This indicator asks whether national laws adopt VGGT principle 16.1 by providing compensation for formally recognized tenure rights held by Indigenous Peoples and local communities. Section 16. 1 provides that States should respect legitimate tenure rights by providing just compensation. Principle 9 of the VGGTs calls for States to respect and protect the legitimate tenure rights of Indigenous Peoples and local communities with customary tenure. Answering the question posed by the indicator entailed reviewing a broad range of legally binding statutes, regulations, and some court decisions at the national level. For more info, see: http://www.wri.org/publication/encroaching-on-land-and-livelihoods</dct:description>
    <rdfs:comment>This indicator asks whether national laws adopt VGGT principle 16.1 by providing compensation for formally recognized tenure rights held by Indigenous Peoples and local communities. Section 16. 1 provides that States should respect legitimate tenure rights by providing just compensation. Principle 9 of the VGGTs calls for States to respect and protect the legitimate tenure rights of Indigenous Peoples and local communities with customary tenure. Answering the question posed by the indicator entailed reviewing a broad range of legally binding statutes, regulations, and some court decisions at the national level. For more info, see: http://www.wri.org/publication/encroaching-on-land-and-livelihoods</rdfs:comment>
    <skos:inScheme rdf:resource="http://data.landportal.info/vocabulary/25"/>
    <skos:broader rdf:resource="http://data.landportal.info/indicator/VGGT-16-1"/>
    <rdfs:seeAlso rdf:resource="https://landportal.org/book/indicator/nkt-vggt16-1c"/>
  </rdf:Description>

</rdf:RDF>