<?xml version="1.0" encoding="UTF-8"?>
<rdf:RDF xmlns:rdf="http://www.w3.org/1999/02/22-rdf-syntax-ns#"
  xmlns:dct="http://purl.org/dc/terms/"
  xmlns:schema="http://schema.org/"
  xmlns:skos="http://www.w3.org/2004/02/skos/core#"
  xmlns:sdmx-attribute="http://purl.org/linked-data/sdmx/2009/attribute#"
  xmlns:rdfs="http://www.w3.org/2000/01/rdf-schema#">

  <rdf:Description rdf:about="http://data.landportal.info/indicator/NKT-VGGT16-9D">
    <rdf:type rdf:resource="http://www.w3.org/2004/02/skos/core#Concept"/>
    <rdf:type rdf:resource="http://purl.org/weso/ontology/computex#Indicator"/>
    <dct:subject rdf:resource="http://aims.fao.org/aos/agrovoc/c_1791"/>
    <dct:subject rdf:resource="http://aims.fao.org/aos/agrovoc/c_65c7772b"/>
    <dct:subject rdf:resource="http://aims.fao.org/aos/agrovoc/c_1798"/>
    <dct:subject rdf:resource="http://aims.fao.org/aos/agrovoc/c_aca7ac6d"/>
    <dct:subject rdf:resource="http://aims.fao.org/aos/agrovoc/c_9a4f48b4"/>
    <dct:subject rdf:resource="http://aims.fao.org/aos/agrovoc/c_12069"/>
    <dct:subject rdf:resource="http://data.landportal.info/voc/landvoc/theme/T-INVEST"/>
    <dct:subject rdf:resource="http://data.landportal.info/voc/landvoc/theme/T-CONFLICT"/>
    <dct:subject rdf:resource="http://data.landportal.info/voc/landvoc/theme/T-INST"/>
    <schema:about rdf:resource="http://aims.fao.org/aos/agrovoc/c_1791"/>
    <schema:about rdf:resource="http://aims.fao.org/aos/agrovoc/c_65c7772b"/>
    <schema:about rdf:resource="http://aims.fao.org/aos/agrovoc/c_1798"/>
    <schema:about rdf:resource="http://aims.fao.org/aos/agrovoc/c_aca7ac6d"/>
    <schema:about rdf:resource="http://aims.fao.org/aos/agrovoc/c_9a4f48b4"/>
    <schema:about rdf:resource="http://aims.fao.org/aos/agrovoc/c_12069"/>
    <schema:about rdf:resource="http://data.landportal.info/voc/landvoc/theme/T-INVEST"/>
    <schema:about rdf:resource="http://data.landportal.info/voc/landvoc/theme/T-CONFLICT"/>
    <schema:about rdf:resource="http://data.landportal.info/voc/landvoc/theme/T-INST"/>
    <dct:identifier>NKT-VGGT16-9D</dct:identifier>
    <skos:notation>NKT-VGGT16-9D</skos:notation>
    <dct:source rdf:resource="http://data.landportal.info/dataset/NKT-VGGT16"/>
    <sdmx-attribute:unitMeasure>Index (A; C)</sdmx-attribute:unitMeasure>
    <rdfs:label>A right to productive alternative land or suitable alternative housing for all displaced persons</rdfs:label>
    <skos:prefLabel>A right to productive alternative land or suitable alternative housing for all displaced persons</skos:prefLabel>
    <dct:title>A right to productive alternative land or suitable alternative housing for all displaced persons</dct:title>
    <skos:definition>This indicator asks whether national laws provide all populations displaced by expropriation with a right to productive alternative land or suitable alternative housing. This indicator is based on Section 16.8 of the VGGTs, which establishes that &amp;quot;evictions and relocations should not result in individuals being rendered homeless or vulnerable to the violation of human rights. Where those affected are unable to provide for themselves, States should, to the extent that resources permit, take appropriate measures to provide adequate alternative housing, resettlement or access to productive land, fisheries and forests as the case may be.&amp;quot;</skos:definition>
    <dct:description>This indicator asks whether national laws provide all populations displaced by expropriation with a right to productive alternative land or suitable alternative housing. This indicator is based on Section 16.8 of the VGGTs, which establishes that &amp;quot;evictions and relocations should not result in individuals being rendered homeless or vulnerable to the violation of human rights. Where those affected are unable to provide for themselves, States should, to the extent that resources permit, take appropriate measures to provide adequate alternative housing, resettlement or access to productive land, fisheries and forests as the case may be.&amp;quot;</dct:description>
    <rdfs:comment>This indicator asks whether national laws provide all populations displaced by expropriation with a right to productive alternative land or suitable alternative housing. This indicator is based on Section 16.8 of the VGGTs, which establishes that &amp;quot;evictions and relocations should not result in individuals being rendered homeless or vulnerable to the violation of human rights. Where those affected are unable to provide for themselves, States should, to the extent that resources permit, take appropriate measures to provide adequate alternative housing, resettlement or access to productive land, fisheries and forests as the case may be.&amp;quot;</rdfs:comment>
    <skos:inScheme rdf:resource="http://data.landportal.info/vocabulary/25"/>
    <skos:broader rdf:resource="http://data.landportal.info/indicator/VGGT-16-9"/>
    <rdfs:seeAlso rdf:resource="https://landportal.org/book/indicator/nkt-vggt16-9d"/>
  </rdf:Description>

</rdf:RDF>