<?xml version="1.0" encoding="UTF-8"?>
<rdf:RDF xmlns:rdf="http://www.w3.org/1999/02/22-rdf-syntax-ns#"
  xmlns:dct="http://purl.org/dc/terms/"
  xmlns:schema="http://schema.org/"
  xmlns:skos="http://www.w3.org/2004/02/skos/core#"
  xmlns:sdmx-attribute="http://purl.org/linked-data/sdmx/2009/attribute#"
  xmlns:rdfs="http://www.w3.org/2000/01/rdf-schema#">

  <rdf:Description rdf:about="http://data.landportal.info/indicator/NKT-VGGT16-9A">
    <rdf:type rdf:resource="http://www.w3.org/2004/02/skos/core#Concept"/>
    <rdf:type rdf:resource="http://purl.org/weso/ontology/computex#Indicator"/>
    <dct:subject rdf:resource="http://aims.fao.org/aos/agrovoc/c_1791"/>
    <dct:subject rdf:resource="http://aims.fao.org/aos/agrovoc/c_1798"/>
    <dct:subject rdf:resource="http://aims.fao.org/aos/agrovoc/c_1ada969a"/>
    <dct:subject rdf:resource="http://aims.fao.org/aos/agrovoc/c_aca7ac6d"/>
    <dct:subject rdf:resource="http://aims.fao.org/aos/agrovoc/c_9a4f48b4"/>
    <dct:subject rdf:resource="http://aims.fao.org/aos/agrovoc/c_195"/>
    <dct:subject rdf:resource="http://aims.fao.org/aos/agrovoc/c_12069"/>
    <dct:subject rdf:resource="http://data.landportal.info/voc/landvoc/theme/T-INVEST"/>
    <dct:subject rdf:resource="http://data.landportal.info/voc/landvoc/theme/T-CONFLICT"/>
    <dct:subject rdf:resource="http://data.landportal.info/voc/landvoc/theme/T-INST"/>
    <schema:about rdf:resource="http://aims.fao.org/aos/agrovoc/c_1791"/>
    <schema:about rdf:resource="http://aims.fao.org/aos/agrovoc/c_1798"/>
    <schema:about rdf:resource="http://aims.fao.org/aos/agrovoc/c_1ada969a"/>
    <schema:about rdf:resource="http://aims.fao.org/aos/agrovoc/c_aca7ac6d"/>
    <schema:about rdf:resource="http://aims.fao.org/aos/agrovoc/c_9a4f48b4"/>
    <schema:about rdf:resource="http://aims.fao.org/aos/agrovoc/c_195"/>
    <schema:about rdf:resource="http://aims.fao.org/aos/agrovoc/c_12069"/>
    <schema:about rdf:resource="http://data.landportal.info/voc/landvoc/theme/T-INVEST"/>
    <schema:about rdf:resource="http://data.landportal.info/voc/landvoc/theme/T-CONFLICT"/>
    <schema:about rdf:resource="http://data.landportal.info/voc/landvoc/theme/T-INST"/>
    <dct:identifier>NKT-VGGT16-9A</dct:identifier>
    <skos:notation>NKT-VGGT16-9A</skos:notation>
    <dct:source rdf:resource="http://data.landportal.info/dataset/NKT-VGGT16"/>
    <sdmx-attribute:unitMeasure>Index (A; C)</sdmx-attribute:unitMeasure>
    <rdfs:label>Laws or regulations with robust resettlement and rehabilitation procedures</rdfs:label>
    <skos:prefLabel>Laws or regulations with robust resettlement and rehabilitation procedures</skos:prefLabel>
    <dct:title>Laws or regulations with robust resettlement and rehabilitation procedures</dct:title>
    <skos:definition>This indicator asks whether countries have enacted national laws with robust provisions for resettling and rehabilitating populations displaced by development projects involving the expropriation of land. For purposes of this indicator, the term “robust provisions” refers to provisions which grant alternative land or housing, relocation allowance, a right to consultation during the resettlement process, and other measures that ensure the livelihoods of displaced populations are adequately revitalized. This indicator is based on Section 16.8 of the VGGTs, which establishes that &amp;quot;evictions and relocations should not result in individuals being rendered homeless or vulnerable to the violation of human rights. Where those affected are unable to provide for themselves, States should, to the extent that resources permit, take appropriate measures to provide adequate alternative housing, resettlement or access to productive land, fisheries and forests as the case may be.&amp;quot;</skos:definition>
    <dct:description>This indicator asks whether countries have enacted national laws with robust provisions for resettling and rehabilitating populations displaced by development projects involving the expropriation of land. For purposes of this indicator, the term “robust provisions” refers to provisions which grant alternative land or housing, relocation allowance, a right to consultation during the resettlement process, and other measures that ensure the livelihoods of displaced populations are adequately revitalized. This indicator is based on Section 16.8 of the VGGTs, which establishes that &amp;quot;evictions and relocations should not result in individuals being rendered homeless or vulnerable to the violation of human rights. Where those affected are unable to provide for themselves, States should, to the extent that resources permit, take appropriate measures to provide adequate alternative housing, resettlement or access to productive land, fisheries and forests as the case may be.&amp;quot;</dct:description>
    <rdfs:comment>This indicator asks whether countries have enacted national laws with robust provisions for resettling and rehabilitating populations displaced by development projects involving the expropriation of land. For purposes of this indicator, the term “robust provisions” refers to provisions which grant alternative land or housing, relocation allowance, a right to consultation during the resettlement process, and other measures that ensure the livelihoods of displaced populations are adequately revitalized. This indicator is based on Section 16.8 of the VGGTs, which establishes that &amp;quot;evictions and relocations should not result in individuals being rendered homeless or vulnerable to the violation of human rights. Where those affected are unable to provide for themselves, States should, to the extent that resources permit, take appropriate measures to provide adequate alternative housing, resettlement or access to productive land, fisheries and forests as the case may be.&amp;quot;</rdfs:comment>
    <skos:inScheme rdf:resource="http://data.landportal.info/vocabulary/25"/>
    <skos:broader rdf:resource="http://data.landportal.info/indicator/VGGT-16-9"/>
    <rdfs:seeAlso rdf:resource="https://landportal.org/book/indicator/nkt-vggt16-9a"/>
  </rdf:Description>

</rdf:RDF>