<?xml version="1.0" encoding="UTF-8"?>
<rdf:RDF xmlns:rdf="http://www.w3.org/1999/02/22-rdf-syntax-ns#"
  xmlns:dct="http://purl.org/dc/terms/"
  xmlns:schema="http://schema.org/"
  xmlns:skos="http://www.w3.org/2004/02/skos/core#"
  xmlns:sdmx-attribute="http://purl.org/linked-data/sdmx/2009/attribute#"
  xmlns:rdfs="http://www.w3.org/2000/01/rdf-schema#">

  <rdf:Description rdf:about="http://data.landportal.info/indicator/NKT-VGGT16-3I">
    <rdf:type rdf:resource="http://www.w3.org/2004/02/skos/core#Concept"/>
    <rdf:type rdf:resource="http://purl.org/weso/ontology/computex#Indicator"/>
    <dct:subject rdf:resource="http://aims.fao.org/aos/agrovoc/c_1791"/>
    <dct:subject rdf:resource="http://aims.fao.org/aos/agrovoc/c_1798"/>
    <dct:subject rdf:resource="http://aims.fao.org/aos/agrovoc/c_1ada969a"/>
    <dct:subject rdf:resource="http://aims.fao.org/aos/agrovoc/c_aca7ac6d"/>
    <dct:subject rdf:resource="http://aims.fao.org/aos/agrovoc/c_9a4f48b4"/>
    <dct:subject rdf:resource="http://aims.fao.org/aos/agrovoc/c_195"/>
    <dct:subject rdf:resource="http://aims.fao.org/aos/agrovoc/c_12069"/>
    <dct:subject rdf:resource="http://aims.fao.org/aos/agrovoc/c_45cd8441"/>
    <dct:subject rdf:resource="http://data.landportal.info/voc/landvoc/theme/T-INVEST"/>
    <dct:subject rdf:resource="http://data.landportal.info/voc/landvoc/theme/T-CONFLICT"/>
    <dct:subject rdf:resource="http://data.landportal.info/voc/landvoc/theme/T-INST"/>
    <schema:about rdf:resource="http://aims.fao.org/aos/agrovoc/c_1791"/>
    <schema:about rdf:resource="http://aims.fao.org/aos/agrovoc/c_1798"/>
    <schema:about rdf:resource="http://aims.fao.org/aos/agrovoc/c_1ada969a"/>
    <schema:about rdf:resource="http://aims.fao.org/aos/agrovoc/c_aca7ac6d"/>
    <schema:about rdf:resource="http://aims.fao.org/aos/agrovoc/c_9a4f48b4"/>
    <schema:about rdf:resource="http://aims.fao.org/aos/agrovoc/c_195"/>
    <schema:about rdf:resource="http://aims.fao.org/aos/agrovoc/c_12069"/>
    <schema:about rdf:resource="http://aims.fao.org/aos/agrovoc/c_45cd8441"/>
    <schema:about rdf:resource="http://data.landportal.info/voc/landvoc/theme/T-INVEST"/>
    <schema:about rdf:resource="http://data.landportal.info/voc/landvoc/theme/T-CONFLICT"/>
    <schema:about rdf:resource="http://data.landportal.info/voc/landvoc/theme/T-INST"/>
    <dct:identifier>NKT-VGGT16-3I</dct:identifier>
    <skos:notation>NKT-VGGT16-3I</skos:notation>
    <dct:source rdf:resource="http://data.landportal.info/dataset/NKT-VGGT16"/>
    <sdmx-attribute:unitMeasure>Index (A; C)</sdmx-attribute:unitMeasure>
    <rdfs:label>A right to challenge compensation decisions in court</rdfs:label>
    <skos:prefLabel>A right to challenge compensation decisions in court</skos:prefLabel>
    <dct:title>A right to challenge compensation decisions in court</dct:title>
    <skos:definition>This indicator asks whether national laws provide affected landholders with the right to appeal or challenge compensation decisions in court. This indicator is based on Section 16.3 of the VGGTs, which provides that &quot;States should ensure a fair valuation and prompt compensation in accordance with national law.&quot; Furthermore, section 16.6 of the VGGTs provides &quot;All parties should endeavour to prevent corruption, particularly through use of objectively assessed values, transparent and decentralized processes and services, and a right to appeal.&quot;Answering the question posed by the indicator entailed reviewing a broad range of legally binding laws, regulations, and court decisions at the national level.</skos:definition>
    <dct:description>This indicator asks whether national laws provide affected landholders with the right to appeal or challenge compensation decisions in court. This indicator is based on Section 16.3 of the VGGTs, which provides that &quot;States should ensure a fair valuation and prompt compensation in accordance with national law.&quot; Furthermore, section 16.6 of the VGGTs provides &quot;All parties should endeavour to prevent corruption, particularly through use of objectively assessed values, transparent and decentralized processes and services, and a right to appeal.&quot;Answering the question posed by the indicator entailed reviewing a broad range of legally binding laws, regulations, and court decisions at the national level.</dct:description>
    <rdfs:comment>This indicator asks whether national laws provide affected landholders with the right to appeal or challenge compensation decisions in court. This indicator is based on Section 16.3 of the VGGTs, which provides that &quot;States should ensure a fair valuation and prompt compensation in accordance with national law.&quot; Furthermore, section 16.6 of the VGGTs provides &quot;All parties should endeavour to prevent corruption, particularly through use of objectively assessed values, transparent and decentralized processes and services, and a right to appeal.&quot;Answering the question posed by the indicator entailed reviewing a broad range of legally binding laws, regulations, and court decisions at the national level.</rdfs:comment>
    <skos:inScheme rdf:resource="http://data.landportal.info/vocabulary/25"/>
    <skos:broader rdf:resource="http://data.landportal.info/indicator/VGGT-16-3"/>
    <rdfs:seeAlso rdf:resource="https://landportal.org/book/indicator/nkt-vggt16-3i"/>
  </rdf:Description>

</rdf:RDF>