<?xml version="1.0" encoding="UTF-8"?>
<rdf:RDF xmlns:rdf="http://www.w3.org/1999/02/22-rdf-syntax-ns#"
  xmlns:dct="http://purl.org/dc/terms/"
  xmlns:schema="http://schema.org/"
  xmlns:skos="http://www.w3.org/2004/02/skos/core#"
  xmlns:sdmx-attribute="http://purl.org/linked-data/sdmx/2009/attribute#"
  xmlns:rdfs="http://www.w3.org/2000/01/rdf-schema#">

  <rdf:Description rdf:about="http://data.landportal.info/indicator/LS-VGGT.END.GFFA2015">
    <rdf:type rdf:resource="http://www.w3.org/2004/02/skos/core#Concept"/>
    <rdf:type rdf:resource="http://purl.org/weso/ontology/computex#Indicator"/>
    <dct:subject rdf:resource="http://data.landportal.info/voc/landvoc/overarching-category/OA-ACCESS"/>
    <dct:subject rdf:resource="http://data.landportal.info/voc/landvoc/overarching-category/OA-USE"/>
    <schema:about rdf:resource="http://data.landportal.info/voc/landvoc/overarching-category/OA-ACCESS"/>
    <schema:about rdf:resource="http://data.landportal.info/voc/landvoc/overarching-category/OA-USE"/>
    <dct:identifier>LS-VGGT.END.GFFA2015</dct:identifier>
    <skos:notation>LS-VGGT.END.GFFA2015</skos:notation>
    <dct:source rdf:resource="http://data.landportal.info/dataset/LS-VGGT"/>
    <sdmx-attribute:unitMeasure>Index (0; 1=endorsed)</sdmx-attribute:unitMeasure>
    <rdfs:label>VGGT endorsement at GFFA 2015</rdfs:label>
    <skos:prefLabel>VGGT endorsement at GFFA 2015</skos:prefLabel>
    <dct:title>VGGT endorsement at GFFA 2015</dct:title>
    <skos:definition>This indicator lists the cuntries that endorsed the VGGT during the Global Forum for Food and Agriculture 2015. The GFFA Communiqué of the 7th Berlin Agriculture Ministers´ Summit 2015, states among other things: We, the agriculture ministers assembled at the GFFA 2015, advocate: […]implementing and applying the &quot;Voluntary Guidelines on the Responsible Governance of Tenure of Land, Fisheries and Forests in the Context of National Food Security&quot; and the &quot;Principles for Responsible Investment in Agriculture and Food Systems&quot; at regional, national and local level, and we support the FAO in its efforts; [...]</skos:definition>
    <dct:description>This indicator lists the cuntries that endorsed the VGGT during the Global Forum for Food and Agriculture 2015. The GFFA Communiqué of the 7th Berlin Agriculture Ministers´ Summit 2015, states among other things: We, the agriculture ministers assembled at the GFFA 2015, advocate: […]implementing and applying the &quot;Voluntary Guidelines on the Responsible Governance of Tenure of Land, Fisheries and Forests in the Context of National Food Security&quot; and the &quot;Principles for Responsible Investment in Agriculture and Food Systems&quot; at regional, national and local level, and we support the FAO in its efforts; [...]</dct:description>
    <rdfs:comment>This indicator lists the cuntries that endorsed the VGGT during the Global Forum for Food and Agriculture 2015. The GFFA Communiqué of the 7th Berlin Agriculture Ministers´ Summit 2015, states among other things: We, the agriculture ministers assembled at the GFFA 2015, advocate: […]implementing and applying the &quot;Voluntary Guidelines on the Responsible Governance of Tenure of Land, Fisheries and Forests in the Context of National Food Security&quot; and the &quot;Principles for Responsible Investment in Agriculture and Food Systems&quot; at regional, national and local level, and we support the FAO in its efforts; [...]</rdfs:comment>
    <skos:inScheme rdf:resource="http://data.landportal.info/vocabulary/25"/>
    <rdfs:seeAlso rdf:resource="https://landportal.org/book/indicator/ls-vggtendgffa2015"/>
  </rdf:Description>

</rdf:RDF>