<?xml version="1.0" encoding="UTF-8"?>
<rdf:RDF xmlns:rdf="http://www.w3.org/1999/02/22-rdf-syntax-ns#"
  xmlns:dct="http://purl.org/dc/terms/"
  xmlns:schema="http://schema.org/"
  xmlns:skos="http://www.w3.org/2004/02/skos/core#"
  xmlns:sdmx-attribute="http://purl.org/linked-data/sdmx/2009/attribute#"
  xmlns:rdfs="http://www.w3.org/2000/01/rdf-schema#">

  <rdf:Description rdf:about="http://data.landportal.info/indicator/AFRB-Q48F.DN">
    <rdf:type rdf:resource="http://www.w3.org/2004/02/skos/core#Concept"/>
    <rdf:type rdf:resource="http://purl.org/weso/ontology/computex#Indicator"/>
    <dct:subject rdf:resource="http://data.landportal.info/voc/landvoc/overarching-category/OA-ACCESS"/>
    <dct:subject rdf:resource="http://data.landportal.info/voc/landvoc/theme/T-CORRUPT"/>
    <dct:subject rdf:resource="http://data.landportal.info/voc/landvoc/theme/T-INST"/>
    <dct:subject rdf:resource="http://data.landportal.info/voc/landvoc/theme/T-INVEST"/>
    <schema:about rdf:resource="http://data.landportal.info/voc/landvoc/overarching-category/OA-ACCESS"/>
    <schema:about rdf:resource="http://data.landportal.info/voc/landvoc/theme/T-CORRUPT"/>
    <schema:about rdf:resource="http://data.landportal.info/voc/landvoc/theme/T-INST"/>
    <schema:about rdf:resource="http://data.landportal.info/voc/landvoc/theme/T-INVEST"/>
    <dct:identifier>AFRB-Q48F.DN</dct:identifier>
    <skos:notation>AFRB-Q48F.DN</skos:notation>
    <dct:source rdf:resource="http://data.landportal.info/dataset/AFRB-SURV"/>
    <sdmx-attribute:unitMeasure>Percentage (%)</sdmx-attribute:unitMeasure>
    <rdfs:label>Q48F - Rich person pay bribe to register land not theirs -- Don't Know (%)</rdfs:label>
    <skos:prefLabel>Q48F - Rich person pay bribe to register land not theirs -- Don't Know (%)</skos:prefLabel>
    <dct:title>Q48F - Rich person pay bribe to register land not theirs -- Don't Know (%)</dct:title>
    <skos:definition>This indicator from round 7 of the Afrobarometer shows the share of respondents, in a given country, that responded &quot;Don't know&quot; to the following question: - Rich person pay bribe to register land not theirs (Q48f) -- And in this country, how likely do you think it is that a rich person could pay a bribe or use personal connections to get away with: Registering land that does not belong to them? (Not at all likely; Not very likely; Somewhat likely; Very likely; Refused; Don’t know) For more information on the Afrobarometer, please visit: http://afrobarometer.org/</skos:definition>
    <dct:description>This indicator from round 7 of the Afrobarometer shows the share of respondents, in a given country, that responded &quot;Don't know&quot; to the following question: - Rich person pay bribe to register land not theirs (Q48f) -- And in this country, how likely do you think it is that a rich person could pay a bribe or use personal connections to get away with: Registering land that does not belong to them? (Not at all likely; Not very likely; Somewhat likely; Very likely; Refused; Don’t know) For more information on the Afrobarometer, please visit: http://afrobarometer.org/</dct:description>
    <rdfs:comment>This indicator from round 7 of the Afrobarometer shows the share of respondents, in a given country, that responded &quot;Don't know&quot; to the following question: - Rich person pay bribe to register land not theirs (Q48f) -- And in this country, how likely do you think it is that a rich person could pay a bribe or use personal connections to get away with: Registering land that does not belong to them? (Not at all likely; Not very likely; Somewhat likely; Very likely; Refused; Don’t know) For more information on the Afrobarometer, please visit: http://afrobarometer.org/</rdfs:comment>
    <skos:inScheme rdf:resource="http://data.landportal.info/vocabulary/25"/>
    <rdfs:seeAlso rdf:resource="https://landportal.org/book/indicator/afrb-q48fdn"/>
  </rdf:Description>

</rdf:RDF>