<?xml version="1.0" encoding="UTF-8"?>
<rdf:RDF xmlns:rdf="http://www.w3.org/1999/02/22-rdf-syntax-ns#"
  xmlns:schema="http://schema.org/"
  xmlns:dct="http://purl.org/dc/terms/"
  xmlns:skos="http://www.w3.org/2004/02/skos/core#"
  xmlns:dc="http://purl.org/dc/elements/1.1/"
  xmlns:rdfs="http://www.w3.org/2000/01/rdf-schema#">

  <rdf:Description rdf:about="http://data.landportal.info/dataset/FAO-FS.2011">
    <rdf:type rdf:resource="http://www.w3.org/2004/02/skos/core#Concept"/>
    <rdf:type rdf:resource="http://purl.org/linked-data/cube#DataSet"/>
    <rdf:type rdf:resource="http://www.w3.org/ns/dcat#Dataset"/>
    <schema:image rdf:resource="https://landportal.org/sites/landportal.org/files/FAO-FS.2011.png"/>
    <schema:logo rdf:resource="https://landportal.org/sites/landportal.org/files/FAO-FS.2011.png"/>
    <dct:subject rdf:resource="http://aims.fao.org/aos/agrovoc/c_10967"/>
    <dct:subject rdf:resource="http://data.landportal.info/voc/landvoc/overarching-category/OA-USE"/>
    <dct:subject rdf:resource="http://data.landportal.info/voc/landvoc/theme/T-FOOD"/>
    <dct:subject rdf:resource="http://data.landportal.info/voc/landvoc/theme/T-SOCEC"/>
    <schema:about rdf:resource="http://aims.fao.org/aos/agrovoc/c_10967"/>
    <schema:about rdf:resource="http://data.landportal.info/voc/landvoc/overarching-category/OA-USE"/>
    <schema:about rdf:resource="http://data.landportal.info/voc/landvoc/theme/T-FOOD"/>
    <schema:about rdf:resource="http://data.landportal.info/voc/landvoc/theme/T-SOCEC"/>
    <dct:publisher rdf:resource="http://data.landportal.info/organization/11005528-e13b-45b2-814a-5bb54c84bdfe"/>
    <dct:identifier>FAO-FS.2011</dct:identifier>
    <skos:notation>FAO-FS.2011</skos:notation>
    <dc:rights rdf:datatype="http://www.w3.org/2001/XMLSchema#string">To ensure wide dissemination of its information, FAO is committed to making its content freely available and encourages the use, reproduction and dissemination of the text, multimedia and data presented. Except where otherwise indicated, content may be copied, printed and downloaded for private study, research and teaching purposes, and for use in non-commercial products or services, provided that appropriate acknowledgement of FAO as the source and copyright holder is given and that FAO's endorsement of users' views, products or services is not stated or implied in any way. More details in the FAO Terms and conditions webpage.</dc:rights>
    <skos:prefLabel>FAO - Food Security (2011 suite)</skos:prefLabel>
    <rdfs:label>FAO - Food Security (2011 suite)</rdfs:label>
    <dct:title>FAO - Food Security (2011 suite)</dct:title>
    <skos:definition>This dataset contains a subset of the suite of indicators (suite 2011) on the level of food security in several countries as provided by FAO. Following the recommendation of experts gathered in the Committee on World Food Security (CFS) Round Table on hunger measurement, hosted at FAO headquarters in September 2011, an initial set of indicators aiming to capture various aspects of food insecurity was selected and called FAO suite of food security indicators.  The indicators (30) were grouped along the four dimension of food security: Availability Access Stability Utilization Due to the change in 2017 to a new suite of indicators, in this dataset remains the indicators that are not part of the new dataset FAO - Food Security (2017 suite)   Data from the FAO suite of food security indicators was able to be accessed on FAOSTAT.</skos:definition>
    <dct:description>This dataset contains a subset of the suite of indicators (suite 2011) on the level of food security in several countries as provided by FAO. Following the recommendation of experts gathered in the Committee on World Food Security (CFS) Round Table on hunger measurement, hosted at FAO headquarters in September 2011, an initial set of indicators aiming to capture various aspects of food insecurity was selected and called FAO suite of food security indicators.  The indicators (30) were grouped along the four dimension of food security: Availability Access Stability Utilization Due to the change in 2017 to a new suite of indicators, in this dataset remains the indicators that are not part of the new dataset FAO - Food Security (2017 suite)   Data from the FAO suite of food security indicators was able to be accessed on FAOSTAT.</dct:description>
    <rdfs:comment>This dataset contains a subset of the suite of indicators (suite 2011) on the level of food security in several countries as provided by FAO. Following the recommendation of experts gathered in the Committee on World Food Security (CFS) Round Table on hunger measurement, hosted at FAO headquarters in September 2011, an initial set of indicators aiming to capture various aspects of food insecurity was selected and called FAO suite of food security indicators.  The indicators (30) were grouped along the four dimension of food security: Availability Access Stability Utilization Due to the change in 2017 to a new suite of indicators, in this dataset remains the indicators that are not part of the new dataset FAO - Food Security (2017 suite)   Data from the FAO suite of food security indicators was able to be accessed on FAOSTAT.</rdfs:comment>
    <skos:inScheme rdf:resource="http://data.landportal.info/vocabulary/24"/>
    <rdfs:seeAlso rdf:resource="https://landportal.org/book/dataset/fao-fs2011"/>
  </rdf:Description>

</rdf:RDF>