<?xml version="1.0" encoding="UTF-8"?>
<rdf:RDF xmlns:rdf="http://www.w3.org/1999/02/22-rdf-syntax-ns#"
  xmlns:dct="http://purl.org/dc/terms/"
  xmlns:schema="http://schema.org/"
  xmlns:skos="http://www.w3.org/2004/02/skos/core#"
  xmlns:dc="http://purl.org/dc/elements/1.1/"
  xmlns:rdfs="http://www.w3.org/2000/01/rdf-schema#">

  <rdf:Description rdf:about="http://data.landportal.info/dataset/WB-GENDER">
    <rdf:type rdf:resource="http://www.w3.org/2004/02/skos/core#Concept"/>
    <rdf:type rdf:resource="http://purl.org/linked-data/cube#DataSet"/>
    <rdf:type rdf:resource="http://www.w3.org/ns/dcat#Dataset"/>
    <dct:subject rdf:resource="http://aims.fao.org/aos/agrovoc/c_1dfe5bfe"/>
    <dct:subject rdf:resource="http://data.landportal.info/voc/landvoc/theme/T-GENDER"/>
    <schema:about rdf:resource="http://aims.fao.org/aos/agrovoc/c_1dfe5bfe"/>
    <schema:about rdf:resource="http://data.landportal.info/voc/landvoc/theme/T-GENDER"/>
    <dct:identifier>WB-GENDER</dct:identifier>
    <skos:notation>WB-GENDER</skos:notation>
    <dct:license rdf:resource="http://purl.org/NET/rdflicense/cc-by4.0"/>
    <schema:license rdf:resource="http://purl.org/NET/rdflicense/cc-by4.0"/>
    <dct:publisher rdf:resource="http://data.landportal.info/organization/78e2ad5a-ed53-4bc5-aafe-2d39f19da353"/>
    <dc:rights rdf:datatype="http://www.w3.org/2001/XMLSchema#string">The World Bank Group is committed to open access and strives to enhance public access to and use of data that it collects and publishes. For more information read the Terms of Use for Datasets Listed in The World Bank Data Catalog</dc:rights>
    <skos:prefLabel>WB - Gender Indicators</skos:prefLabel>
    <rdfs:label>WB - Gender Indicators</rdfs:label>
    <dct:title>WB - Gender Indicators</dct:title>
    <skos:definition>This dataset contains gender indicators (such as women/men who own land alone or women/men who own land both alone and jointly) as provided by the World Bank.</skos:definition>
    <dct:description>This dataset contains gender indicators (such as women/men who own land alone or women/men who own land both alone and jointly) as provided by the World Bank.</dct:description>
    <rdfs:comment>This dataset contains gender indicators (such as women/men who own land alone or women/men who own land both alone and jointly) as provided by the World Bank.</rdfs:comment>
    <skos:inScheme rdf:resource="http://data.landportal.info/vocabulary/24"/>
    <rdfs:seeAlso rdf:resource="https://landportal.org/book/dataset/wb-gender"/>
  </rdf:Description>

</rdf:RDF>