<?xml version="1.0" encoding="UTF-8"?>
<rdf:RDF xmlns:rdf="http://www.w3.org/1999/02/22-rdf-syntax-ns#"
  xmlns:dct="http://purl.org/dc/terms/"
  xmlns:skos="http://www.w3.org/2004/02/skos/core#"
  xmlns:schema="http://schema.org/"
  xmlns:sdmx-attribute="http://purl.org/linked-data/sdmx/2009/attribute#"
  xmlns:rdfs="http://www.w3.org/2000/01/rdf-schema#">

  <rdf:Description rdf:about="http://data.landportal.info/indicator/DP-MOD-O-F-VGGT.7">
    <rdf:type rdf:resource="http://www.w3.org/2004/02/skos/core#Concept"/>
    <rdf:type rdf:resource="http://purl.org/weso/ontology/computex#Indicator"/>
    <dct:identifier>DP-MOD-O-F-VGGT.7</dct:identifier>
    <skos:notation>DP-MOD-O-F-VGGT.7</skos:notation>
    <dct:subject rdf:resource="http://data.landportal.info/voc/landvoc/overarching-category/OA-LAW"/>
    <dct:subject rdf:resource="http://data.landportal.info/voc/landvoc/overarching-category/OA-USE"/>
    <dct:subject rdf:resource="http://data.landportal.info/voc/landvoc/theme/T-INST"/>
    <dct:subject rdf:resource="http://data.landportal.info/voc/landvoc/theme/T-INVEST"/>
    <schema:about rdf:resource="http://data.landportal.info/voc/landvoc/overarching-category/OA-LAW"/>
    <schema:about rdf:resource="http://data.landportal.info/voc/landvoc/overarching-category/OA-USE"/>
    <schema:about rdf:resource="http://data.landportal.info/voc/landvoc/theme/T-INST"/>
    <schema:about rdf:resource="http://data.landportal.info/voc/landvoc/theme/T-INVEST"/>
    <dct:source rdf:resource="http://data.landportal.info/dataset/DP-MOD"/>
    <sdmx-attribute:unitMeasure>US$ (Current)</sdmx-attribute:unitMeasure>
    <rdfs:label>Ongoing Projects - Funding (VGGT chapter 7 - Promotion, implementation, M &amp; E)</rdfs:label>
    <skos:prefLabel>Ongoing Projects - Funding (VGGT chapter 7 - Promotion, implementation, M &amp; E)</skos:prefLabel>
    <dct:title>Ongoing Projects - Funding (VGGT chapter 7 - Promotion, implementation, M &amp; E)</dct:title>
    <skos:definition>Total funding for programmes related to VGGT chapter 7 (Promotion, implementation, M &amp;amp; E) and still ongoing in January 2019 (US $), according to the Land Governance Programme Map &amp;amp; Database (https://landgov.donorplatform.org/). Last updated on the 31st of January, 2019.</skos:definition>
    <dct:description>Total funding for programmes related to VGGT chapter 7 (Promotion, implementation, M &amp;amp; E) and still ongoing in January 2019 (US $), according to the Land Governance Programme Map &amp;amp; Database (https://landgov.donorplatform.org/). Last updated on the 31st of January, 2019.</dct:description>
    <rdfs:comment>Total funding for programmes related to VGGT chapter 7 (Promotion, implementation, M &amp;amp; E) and still ongoing in January 2019 (US $), according to the Land Governance Programme Map &amp;amp; Database (https://landgov.donorplatform.org/). Last updated on the 31st of January, 2019.</rdfs:comment>
    <skos:inScheme rdf:resource="http://data.landportal.info/vocabulary/25"/>
    <rdfs:seeAlso rdf:resource="https://landportal.org/book/indicator/dp-mod-o-f-vggt7"/>
  </rdf:Description>

</rdf:RDF>