<?xml version="1.0" encoding="UTF-8"?>
<rdf:RDF xmlns:rdf="http://www.w3.org/1999/02/22-rdf-syntax-ns#"
  xmlns:dct="http://purl.org/dc/terms/"
  xmlns:schema="http://schema.org/"
  xmlns:skos="http://www.w3.org/2004/02/skos/core#"
  xmlns:rdfs="http://www.w3.org/2000/01/rdf-schema#">

  <rdf:Description rdf:about="http://data.landportal.info/indicator/FAO-22013-6126">
    <rdf:type rdf:resource="http://www.w3.org/2004/02/skos/core#Concept"/>
    <rdf:type rdf:resource="http://purl.org/weso/ontology/computex#Indicator"/>
    <dct:subject rdf:resource="http://aims.fao.org/aos/agrovoc/c_203"/>
    <dct:subject rdf:resource="http://aims.fao.org/aos/agrovoc/c_10967"/>
    <dct:subject rdf:resource="http://aims.fao.org/aos/agrovoc/c_aca7ac6d"/>
    <dct:subject rdf:resource="http://data.landportal.info/voc/landvoc/theme/T-FOOD"/>
    <dct:subject rdf:resource="http://data.landportal.info/voc/landvoc/theme/T-SOCEC"/>
    <schema:about rdf:resource="http://aims.fao.org/aos/agrovoc/c_203"/>
    <schema:about rdf:resource="http://aims.fao.org/aos/agrovoc/c_10967"/>
    <schema:about rdf:resource="http://aims.fao.org/aos/agrovoc/c_aca7ac6d"/>
    <schema:about rdf:resource="http://data.landportal.info/voc/landvoc/theme/T-FOOD"/>
    <schema:about rdf:resource="http://data.landportal.info/voc/landvoc/theme/T-SOCEC"/>
    <dct:identifier>FAO-22013-6126</dct:identifier>
    <skos:notation>FAO-22013-6126</skos:notation>
    <dct:source rdf:resource="http://data.landportal.info/dataset/FAO-FS"/>
    <rdfs:label>Gross domestic product per capita, PPP (constant 2011 international $)</rdfs:label>
    <skos:prefLabel>Gross domestic product per capita, PPP (constant 2011 international $)</skos:prefLabel>
    <dct:title>Gross domestic product per capita, PPP (constant 2011 international $)</dct:title>
    <skos:definition>This indicator is part of the FAO Suite of Food Security Indicators (2017) in the dimension &quot;access&quot;. GDP per capita based on purchasing power parity (PPP). PPP GDP is gross domestic product converted to international dollars using purchasing power parity rates. An international dollar has the same purchasing power over GDP as the U.S. dollar has in the United States. GDP at purchaser's prices is the sum of gross value added by all resident producers in the economy plus any product taxes and minus any subsidies not included in the value of the products. It is calculated without making deductions for depreciation of fabricated assets or for depletion and degradation of natural resources. Data are in constant 2011 international dollars. This indicator provides information on the possibility of economical access to markets. Original data can be retrieved from the World Bank (World Bank: http://data.worldbank.org/indicator/NY.GDP.PCAP.PP.KD)  </skos:definition>
    <dct:description>This indicator is part of the FAO Suite of Food Security Indicators (2017) in the dimension &quot;access&quot;. GDP per capita based on purchasing power parity (PPP). PPP GDP is gross domestic product converted to international dollars using purchasing power parity rates. An international dollar has the same purchasing power over GDP as the U.S. dollar has in the United States. GDP at purchaser's prices is the sum of gross value added by all resident producers in the economy plus any product taxes and minus any subsidies not included in the value of the products. It is calculated without making deductions for depreciation of fabricated assets or for depletion and degradation of natural resources. Data are in constant 2011 international dollars. This indicator provides information on the possibility of economical access to markets. Original data can be retrieved from the World Bank (World Bank: http://data.worldbank.org/indicator/NY.GDP.PCAP.PP.KD)  </dct:description>
    <rdfs:comment>This indicator is part of the FAO Suite of Food Security Indicators (2017) in the dimension &quot;access&quot;. GDP per capita based on purchasing power parity (PPP). PPP GDP is gross domestic product converted to international dollars using purchasing power parity rates. An international dollar has the same purchasing power over GDP as the U.S. dollar has in the United States. GDP at purchaser's prices is the sum of gross value added by all resident producers in the economy plus any product taxes and minus any subsidies not included in the value of the products. It is calculated without making deductions for depreciation of fabricated assets or for depletion and degradation of natural resources. Data are in constant 2011 international dollars. This indicator provides information on the possibility of economical access to markets. Original data can be retrieved from the World Bank (World Bank: http://data.worldbank.org/indicator/NY.GDP.PCAP.PP.KD)  </rdfs:comment>
    <skos:inScheme rdf:resource="http://data.landportal.info/vocabulary/25"/>
    <rdfs:seeAlso rdf:resource="https://landportal.org/book/indicator/fao-22013-6126"/>
  </rdf:Description>

</rdf:RDF>