<?xml version="1.0" encoding="UTF-8"?>
<rdf:RDF xmlns:rdf="http://www.w3.org/1999/02/22-rdf-syntax-ns#"
  xmlns:dct="http://purl.org/dc/terms/"
  xmlns:schema="http://schema.org/"
  xmlns:skos="http://www.w3.org/2004/02/skos/core#"
  xmlns:sdmx-attribute="http://purl.org/linked-data/sdmx/2009/attribute#"
  xmlns:rdfs="http://www.w3.org/2000/01/rdf-schema#">

  <rdf:Description rdf:about="http://data.landportal.info/indicator/WB-LGAF2016-3.3.1">
    <rdf:type rdf:resource="http://www.w3.org/2004/02/skos/core#Concept"/>
    <rdf:type rdf:resource="http://purl.org/weso/ontology/computex#Indicator"/>
    <dct:subject rdf:resource="http://aims.fao.org/aos/agrovoc/c_9000091"/>
    <dct:subject rdf:resource="http://aims.fao.org/aos/agrovoc/c_aca7ac6d"/>
    <dct:subject rdf:resource="http://aims.fao.org/aos/agrovoc/c_37948"/>
    <dct:subject rdf:resource="http://aims.fao.org/aos/agrovoc/c_8086"/>
    <dct:subject rdf:resource="http://data.landportal.info/voc/landvoc/theme/T-INST"/>
    <dct:subject rdf:resource="http://data.landportal.info/voc/landvoc/theme/T-URBAN"/>
    <schema:about rdf:resource="http://aims.fao.org/aos/agrovoc/c_9000091"/>
    <schema:about rdf:resource="http://aims.fao.org/aos/agrovoc/c_aca7ac6d"/>
    <schema:about rdf:resource="http://aims.fao.org/aos/agrovoc/c_37948"/>
    <schema:about rdf:resource="http://aims.fao.org/aos/agrovoc/c_8086"/>
    <schema:about rdf:resource="http://data.landportal.info/voc/landvoc/theme/T-INST"/>
    <schema:about rdf:resource="http://data.landportal.info/voc/landvoc/theme/T-URBAN"/>
    <dct:identifier>WB-LGAF2016-3.3.1</dct:identifier>
    <skos:notation>WB-LGAF2016-3.3.1</skos:notation>
    <dct:source rdf:resource="http://data.landportal.info/dataset/WB-LGAF2016"/>
<sdmx-attribute:unitMeasure>Index (A; D)</sdmx-attribute:unitMeasure>
    <rdfs:label>Policy for low-cost housing &amp; services exists, implemented</rdfs:label>
    <skos:prefLabel>Policy for low-cost housing &amp; services exists, implemented</skos:prefLabel>
    <dct:title>Policy for low-cost housing &amp; services exists, implemented</dct:title>
    <skos:definition>Policy for low-cost housing &amp;amp; services exists, implemented measured on a scale from A - which stands for good practices - to D - reflecting weak practices. For more information please visit http://go.worldbank.org/21M7S7AZO0</skos:definition>
    <dct:description>Policy for low-cost housing &amp;amp; services exists, implemented measured on a scale from A - which stands for good practices - to D - reflecting weak practices. For more information please visit http://go.worldbank.org/21M7S7AZO0</dct:description>
    <rdfs:comment>Policy for low-cost housing &amp;amp; services exists, implemented measured on a scale from A - which stands for good practices - to D - reflecting weak practices. For more information please visit http://go.worldbank.org/21M7S7AZO0</rdfs:comment>
    <skos:inScheme rdf:resource="http://data.landportal.info/vocabulary/25"/>
    <rdfs:seeAlso rdf:resource="https://landportal.org/book/indicators/wb-lgaf2016-331"/>
  </rdf:Description>

</rdf:RDF>