<?xml version="1.0" encoding="UTF-8"?>
<rdf:RDF xmlns:rdf="http://www.w3.org/1999/02/22-rdf-syntax-ns#"
  xmlns:dct="http://purl.org/dc/terms/"
  xmlns:schema="http://schema.org/"
  xmlns:skos="http://www.w3.org/2004/02/skos/core#"
  xmlns:sdmx-attribute="http://purl.org/linked-data/sdmx/2009/attribute#"
  xmlns:rdfs="http://www.w3.org/2000/01/rdf-schema#">

  <rdf:Description rdf:about="http://data.landportal.info/indicator/UN-SI_AGR_SSFP">
    <rdf:type rdf:resource="http://www.w3.org/2004/02/skos/core#Concept"/>
    <rdf:type rdf:resource="http://purl.org/weso/ontology/computex#Indicator"/>
    <dct:subject rdf:resource="http://data.landportal.info/voc/landvoc/theme/T-FOOD"/>
    <dct:subject rdf:resource="http://data.landportal.info/voc/landvoc/theme/T-INST"/>
    <dct:subject rdf:resource="http://data.landportal.info/voc/landvoc/theme/T-SOCEC"/>
    <schema:about rdf:resource="http://data.landportal.info/voc/landvoc/theme/T-FOOD"/>
    <schema:about rdf:resource="http://data.landportal.info/voc/landvoc/theme/T-INST"/>
    <schema:about rdf:resource="http://data.landportal.info/voc/landvoc/theme/T-SOCEC"/>
    <dct:identifier>UN-SI_AGR_SSFP</dct:identifier>
    <skos:notation>UN-SI_AGR_SSFP</skos:notation>
    <dct:source rdf:resource="http://data.landportal.info/dataset/UN-SDG_2.3.2"/>
    <sdmx-attribute:unitMeasure>Constant 2011 international $</sdmx-attribute:unitMeasure>
    <rdfs:label>Average income of small-scale food producers, PPP (constant 2011 international $)</rdfs:label>
    <skos:prefLabel>Average income of small-scale food producers, PPP (constant 2011 international $)</skos:prefLabel>
    <dct:title>Average income of small-scale food producers, PPP (constant 2011 international $)</dct:title>
    <skos:definition>The data series presented here measures average income of small-scale food producers, PPP (constant 2011 international $). This data series contributes to the measurement of SDG Indicator 2.3.2, classified as Tier II in September 2018, which is officially defined as follows: SDG indicator 2.3.2 measures income from on-farm production activities, which is related to the production of food and agricultural products. This includes income from crop production, livestock production, fisheries and aquaculture production, and from forestry production. The indicator is computed as annual income.  According to Food and Agriculture Organization of the United Nations (FAO) -- the Custodian Agency for this indicator -- the rationale behind this indicator can be summarised as follows:  The 2030 Sustainable Development Agenda has emphasized the importance of enhancing income of small-scale food producers, as these producers play an important role in the global production of food. The indicator monitors progress in this area, where the target is to double income by year 2030. The enhancement of income of small-scale production units also has implications on poverty reduction, as small-scale food producers are often poor, and are frequently found to be close to subsistence conditions. The full official metadata for this Tier II indicator are available at UN SDG Metadata website. For more information, check also this indicator's page on Land Portal SDG porfolio. For more information on this data series, please visit UN SDG website.</skos:definition>
    <dct:description>The data series presented here measures average income of small-scale food producers, PPP (constant 2011 international $). This data series contributes to the measurement of SDG Indicator 2.3.2, classified as Tier II in September 2018, which is officially defined as follows: SDG indicator 2.3.2 measures income from on-farm production activities, which is related to the production of food and agricultural products. This includes income from crop production, livestock production, fisheries and aquaculture production, and from forestry production. The indicator is computed as annual income.  According to Food and Agriculture Organization of the United Nations (FAO) -- the Custodian Agency for this indicator -- the rationale behind this indicator can be summarised as follows:  The 2030 Sustainable Development Agenda has emphasized the importance of enhancing income of small-scale food producers, as these producers play an important role in the global production of food. The indicator monitors progress in this area, where the target is to double income by year 2030. The enhancement of income of small-scale production units also has implications on poverty reduction, as small-scale food producers are often poor, and are frequently found to be close to subsistence conditions. The full official metadata for this Tier II indicator are available at UN SDG Metadata website. For more information, check also this indicator's page on Land Portal SDG porfolio. For more information on this data series, please visit UN SDG website.</dct:description>
    <rdfs:comment>The data series presented here measures average income of small-scale food producers, PPP (constant 2011 international $). This data series contributes to the measurement of SDG Indicator 2.3.2, classified as Tier II in September 2018, which is officially defined as follows: SDG indicator 2.3.2 measures income from on-farm production activities, which is related to the production of food and agricultural products. This includes income from crop production, livestock production, fisheries and aquaculture production, and from forestry production. The indicator is computed as annual income.  According to Food and Agriculture Organization of the United Nations (FAO) -- the Custodian Agency for this indicator -- the rationale behind this indicator can be summarised as follows:  The 2030 Sustainable Development Agenda has emphasized the importance of enhancing income of small-scale food producers, as these producers play an important role in the global production of food. The indicator monitors progress in this area, where the target is to double income by year 2030. The enhancement of income of small-scale production units also has implications on poverty reduction, as small-scale food producers are often poor, and are frequently found to be close to subsistence conditions. The full official metadata for this Tier II indicator are available at UN SDG Metadata website. For more information, check also this indicator's page on Land Portal SDG porfolio. For more information on this data series, please visit UN SDG website.</rdfs:comment>
    <skos:inScheme rdf:resource="http://data.landportal.info/vocabulary/25"/>
    <rdfs:seeAlso rdf:resource="https://landportal.org/book/indicator/un-siagrssfp"/>
  </rdf:Description>

</rdf:RDF>