<?xml version="1.0" encoding="UTF-8"?>
<rdf:RDF xmlns:rdf="http://www.w3.org/1999/02/22-rdf-syntax-ns#"
  xmlns:schema="http://schema.org/"
  xmlns:dct="http://purl.org/dc/terms/"
  xmlns:skos="http://www.w3.org/2004/02/skos/core#"
  xmlns:rdfs="http://www.w3.org/2000/01/rdf-schema#">

  <rdf:Description rdf:about="http://data.landportal.info/dataset/LM-LANDMATRIX">
    <rdf:type rdf:resource="http://www.w3.org/2004/02/skos/core#Concept"/>
    <rdf:type rdf:resource="http://purl.org/linked-data/cube#DataSet"/>
    <rdf:type rdf:resource="http://www.w3.org/ns/dcat#Dataset"/>
    <schema:image rdf:resource="https://landportal.org/sites/landportal.org/files/land-matrix.png"/>
    <schema:logo rdf:resource="https://landportal.org/sites/landportal.org/files/land-matrix.png"/>
    <dct:identifier>LM-LANDMATRIX</dct:identifier>
    <skos:notation>LM-LANDMATRIX</skos:notation>
    <dct:subject rdf:resource="http://aims.fao.org/aos/agrovoc/c_89d3dcbb"/>
    <dct:subject rdf:resource="http://aims.fao.org/aos/agrovoc/c_37734"/>
    <dct:subject rdf:resource="http://aims.fao.org/aos/agrovoc/c_24866"/>
    <dct:subject rdf:resource="http://aims.fao.org/aos/agrovoc/c_28718"/>
    <dct:subject rdf:resource="http://aims.fao.org/aos/agrovoc/c_37898"/>
    <dct:subject rdf:resource="http://aims.fao.org/aos/agrovoc/c_4182"/>
    <dct:subject rdf:resource="http://data.landportal.info/voc/landvoc/theme/T-INVEST"/>
    <dct:subject rdf:resource="http://data.landportal.info/voc/landvoc/theme/T-INST"/>
    <schema:about rdf:resource="http://aims.fao.org/aos/agrovoc/c_89d3dcbb"/>
    <schema:about rdf:resource="http://aims.fao.org/aos/agrovoc/c_37734"/>
    <schema:about rdf:resource="http://aims.fao.org/aos/agrovoc/c_24866"/>
    <schema:about rdf:resource="http://aims.fao.org/aos/agrovoc/c_28718"/>
    <schema:about rdf:resource="http://aims.fao.org/aos/agrovoc/c_37898"/>
    <schema:about rdf:resource="http://aims.fao.org/aos/agrovoc/c_4182"/>
    <schema:about rdf:resource="http://data.landportal.info/voc/landvoc/theme/T-INVEST"/>
    <schema:about rdf:resource="http://data.landportal.info/voc/landvoc/theme/T-INST"/>
    <dct:license rdf:resource="http://purl.org/NET/rdflicense/cc-by4.0"/>
    <schema:license rdf:resource="http://purl.org/NET/rdflicense/cc-by4.0"/>
    <dct:publisher rdf:resource="http://data.landportal.info/organization/f8184144-8687-48d8-b0de-c91045c27f43"/>
    <skos:prefLabel>Land Matrix - Large-Scale Land Acquisitions</skos:prefLabel>
    <rdfs:label>Land Matrix - Large-Scale Land Acquisitions</rdfs:label>
    <dct:title>Land Matrix - Large-Scale Land Acquisitions</dct:title>
    <skos:definition>This dataset contains information provided by the Land Matrix on the size, nature, state and purpose of Large-Scale Land Aquisitions around the world.</skos:definition>
    <dct:description>This dataset contains information provided by the Land Matrix on the size, nature, state and purpose of Large-Scale Land Aquisitions around the world.</dct:description>
    <rdfs:comment>This dataset contains information provided by the Land Matrix on the size, nature, state and purpose of Large-Scale Land Aquisitions around the world.</rdfs:comment>
    <skos:inScheme rdf:resource="http://data.landportal.info/vocabulary/24"/>
    <rdfs:seeAlso rdf:resource="https://landportal.org/book/datasets/datlm0"/>
  </rdf:Description>

</rdf:RDF>