<?xml version="1.0" encoding="UTF-8"?>
<rdf:RDF xmlns:rdf="http://www.w3.org/1999/02/22-rdf-syntax-ns#"
  xmlns:dct="http://purl.org/dc/terms/"
  xmlns:schema="http://schema.org/"
  xmlns:skos="http://www.w3.org/2004/02/skos/core#"
  xmlns:sdmx-attribute="http://purl.org/linked-data/sdmx/2009/attribute#"
  xmlns:rdfs="http://www.w3.org/2000/01/rdf-schema#">

  <rdf:Description rdf:about="http://data.landportal.info/indicator/WB-ER.PTD.TOTL.ZS">
    <rdf:type rdf:resource="http://www.w3.org/2004/02/skos/core#Concept"/>
    <rdf:type rdf:resource="http://purl.org/weso/ontology/computex#Indicator"/>
    <dct:subject rdf:resource="http://aims.fao.org/aos/agrovoc/c_2593"/>
    <dct:subject rdf:resource="http://aims.fao.org/aos/agrovoc/c_37952"/>
    <dct:subject rdf:resource="http://data.landportal.info/voc/landvoc/theme/T-ENVIR"/>
    <schema:about rdf:resource="http://aims.fao.org/aos/agrovoc/c_2593"/>
    <schema:about rdf:resource="http://aims.fao.org/aos/agrovoc/c_37952"/>
    <schema:about rdf:resource="http://data.landportal.info/voc/landvoc/theme/T-ENVIR"/>
    <dct:identifier>WB-ER.PTD.TOTL.ZS</dct:identifier>
    <skos:notation>WB-ER.PTD.TOTL.ZS</skos:notation>
    <dct:source rdf:resource="http://data.landportal.info/dataset/WB-ENV"/>
    <sdmx-attribute:unitMeasure>% of total territorial area</sdmx-attribute:unitMeasure>
    <rdfs:label>Terrestrial and marine protected areas (% of total territorial area)</rdfs:label>
    <skos:prefLabel>Terrestrial and marine protected areas (% of total territorial area)</skos:prefLabel>
    <dct:title>Terrestrial and marine protected areas (% of total territorial area)</dct:title>
    <skos:definition>This indicator measures the proportion of terrestrial and marine protected areas as a share of the total territorial area, including territorial waters, in a country. Terrestrial protected areas are totally or partially protected areas of at least 1,000 hectares that are designated by national authorities as scientific reserves with limited public access, national parks, natural monuments, nature reserves or wildlife sanctuaries, protected landscapes, and areas managed mainly for sustainable use. Marine protected areas are areas of intertidal or subtidal terrain--and overlying water and associated flora and fauna and historical and cultural features--that have been reserved by law or other effective means to protect part or all of the enclosed environment. Sites protected under local or provincial law are excluded. The International Union for Conservation of Nature (IUCN) defines a protected area as &quot;a clearly defined geographical space, recognized, dedicated and managed, through legal or other effective means, to achieve the long-term conservation of nature with associated ecosystem services and cultural values&quot;. Protected areas remain the fundamental building blocks of virtually all national and international conservation strategies, supported by governments and international institutions. They provide the core of efforts to protect the world's threatened species and are increasingly recognized as essential providers of ecosystem services and biological resources. Some sites are owned and managed by governments, others by private individuals, companies, communities and faith groups. Currently about a tenth of the world's land surface is under some form of protected area, (Source: http://databank.worldbank.org/data/reports.aspx?source=2&amp;amp;type=metadata&amp;amp;series=ER.PTD.TOTL.ZS)</skos:definition>
    <dct:description>This indicator measures the proportion of terrestrial and marine protected areas as a share of the total territorial area, including territorial waters, in a country. Terrestrial protected areas are totally or partially protected areas of at least 1,000 hectares that are designated by national authorities as scientific reserves with limited public access, national parks, natural monuments, nature reserves or wildlife sanctuaries, protected landscapes, and areas managed mainly for sustainable use. Marine protected areas are areas of intertidal or subtidal terrain--and overlying water and associated flora and fauna and historical and cultural features--that have been reserved by law or other effective means to protect part or all of the enclosed environment. Sites protected under local or provincial law are excluded. The International Union for Conservation of Nature (IUCN) defines a protected area as &quot;a clearly defined geographical space, recognized, dedicated and managed, through legal or other effective means, to achieve the long-term conservation of nature with associated ecosystem services and cultural values&quot;. Protected areas remain the fundamental building blocks of virtually all national and international conservation strategies, supported by governments and international institutions. They provide the core of efforts to protect the world's threatened species and are increasingly recognized as essential providers of ecosystem services and biological resources. Some sites are owned and managed by governments, others by private individuals, companies, communities and faith groups. Currently about a tenth of the world's land surface is under some form of protected area, (Source: http://databank.worldbank.org/data/reports.aspx?source=2&amp;amp;type=metadata&amp;amp;series=ER.PTD.TOTL.ZS)</dct:description>
    <rdfs:comment>This indicator measures the proportion of terrestrial and marine protected areas as a share of the total territorial area, including territorial waters, in a country. Terrestrial protected areas are totally or partially protected areas of at least 1,000 hectares that are designated by national authorities as scientific reserves with limited public access, national parks, natural monuments, nature reserves or wildlife sanctuaries, protected landscapes, and areas managed mainly for sustainable use. Marine protected areas are areas of intertidal or subtidal terrain--and overlying water and associated flora and fauna and historical and cultural features--that have been reserved by law or other effective means to protect part or all of the enclosed environment. Sites protected under local or provincial law are excluded. The International Union for Conservation of Nature (IUCN) defines a protected area as &quot;a clearly defined geographical space, recognized, dedicated and managed, through legal or other effective means, to achieve the long-term conservation of nature with associated ecosystem services and cultural values&quot;. Protected areas remain the fundamental building blocks of virtually all national and international conservation strategies, supported by governments and international institutions. They provide the core of efforts to protect the world's threatened species and are increasingly recognized as essential providers of ecosystem services and biological resources. Some sites are owned and managed by governments, others by private individuals, companies, communities and faith groups. Currently about a tenth of the world's land surface is under some form of protected area, (Source: http://databank.worldbank.org/data/reports.aspx?source=2&amp;amp;type=metadata&amp;amp;series=ER.PTD.TOTL.ZS)</rdfs:comment>
    <skos:inScheme rdf:resource="http://data.landportal.info/vocabulary/25"/>
    <rdfs:seeAlso rdf:resource="https://landportal.org/book/indicator/wb-erptdtotlzs"/>
  </rdf:Description>

</rdf:RDF>