<?xml version="1.0" encoding="UTF-8"?>
<rdf:RDF
   xmlns:rdf="http://www.w3.org/1999/02/22-rdf-syntax-ns#"
   xmlns:rdfs="http://www.w3.org/2000/01/rdf-schema#"
   xmlns:schema="http://schema.org/"
   xmlns:skos="http://www.w3.org/2004/02/skos/core#"
>
  <rdf:Description rdf:about="http://data.landportal.info/voc/landvoc/theme/T-CONFLICT">
    <skos:related rdf:resource="http://aims.fao.org/aos/agrovoc/c_1ada969a"/>
    <skos:related rdf:resource="http://aims.fao.org/aos/agrovoc/c_6f79699c"/>
    <skos:inScheme rdf:resource="http://data.landportal.info/vocabulary/26"/>
    <skos:prefLabel>Land Conflicts</skos:prefLabel>
    <skos:related rdf:resource="http://aims.fao.org/aos/agrovoc/c_e236b2b1"/>
    <skos:definition>A “land conflict” involves competing claims to large areas of land by groups, of a breadth and depth not easily resolved within existing law. There is often no consensus on the rules to be applied, and the parties may have quite different understandings of the nature of the conflict. As used in this paper, “conflict” implies tension and the danger of violence, but not violence unless this is specified. Longstanding potentials for conflict based in structural or other fundamental problems may be the result of “trigger” events turned violent.  Source: USAID</skos:definition>
    <skos:related rdf:resource="http://aims.fao.org/aos/agrovoc/c_ee93bbbe"/>
    <skos:notation>T-CONFLICT</skos:notation>
    <schema:image rdf:resource="https://landportal.org/sites/landportal.org/files/icons-landportal-05-transparent.png"/>
    <rdf:type rdf:resource="http://www.w3.org/2004/02/skos/core#Concept"/>
    <rdfs:seeAlso rdf:resource="https://landportal.org/voc/themes/land-conflicts"/>
    <skos:related rdf:resource="http://aims.fao.org/aos/agrovoc/c_95fedfc9"/>
    <rdfs:label>Land Conflicts</rdfs:label>
  </rdf:Description>
  <rdf:Description rdf:about="http://data.landportal.info/voc/landvoc/theme/T-FOREST">
    <skos:related rdf:resource="http://aims.fao.org/aos/agrovoc/c_1882e93f"/>
    <skos:related rdf:resource="http://aims.fao.org/aos/agrovoc/c_3060"/>
    <skos:related rdf:resource="http://aims.fao.org/aos/agrovoc/c_3055"/>
    <skos:related rdf:resource="http://aims.fao.org/aos/agrovoc/c_3046"/>
    <skos:prefLabel>Posse Florestal</skos:prefLabel>
    <skos:related rdf:resource="http://aims.fao.org/aos/agrovoc/c_15590"/>
    <skos:related rdf:resource="http://aims.fao.org/aos/agrovoc/c_28079"/>
    <skos:related rdf:resource="http://aims.fao.org/aos/agrovoc/c_8c59c597"/>
    <skos:related rdf:resource="http://aims.fao.org/aos/agrovoc/c_330982"/>
    <skos:related rdf:resource="http://aims.fao.org/aos/agrovoc/c_16532"/>
    <skos:related rdf:resource="http://aims.fao.org/aos/agrovoc/c_1374158672853"/>
    <skos:related rdf:resource="http://aims.fao.org/aos/agrovoc/c_1374070277659"/>
    <schema:image rdf:resource="https://landportal.org/sites/landportal.org/files/icons-landportal-01-transparent.png"/>
    <rdf:type rdf:resource="http://www.w3.org/2004/02/skos/core#Concept"/>
    <rdfs:label>Posse Florestal</rdfs:label>
    <skos:definition>Responsible forest governance and secure forest rights are needed to reduce deforestation, combat climate change, and sustain the planet.</skos:definition>
    <skos:related rdf:resource="http://aims.fao.org/aos/agrovoc/c_14569"/>
    <skos:inScheme rdf:resource="http://data.landportal.info/vocabulary/26"/>
    <skos:notation>T-FOREST</skos:notation>
    <skos:related rdf:resource="http://aims.fao.org/aos/agrovoc/c_32620"/>
    <skos:related rdf:resource="http://aims.fao.org/aos/agrovoc/c_c0a7f4fb"/>
    <skos:related rdf:resource="http://aims.fao.org/aos/agrovoc/c_24843"/>
    <skos:related rdf:resource="http://aims.fao.org/aos/agrovoc/c_1374155312641"/>
    <rdfs:seeAlso rdf:resource="https://landportal.org/voc/themes/forestry"/>
  </rdf:Description>
  <rdf:Description rdf:about="http://data.landportal.info/voc/landvoc/theme/T-URBAN">
    <skos:definition>With the expansion of cities and urban infrastructure comes a growing need to better understand the relationship between people and land in urban and peri-urban areas.</skos:definition>
    <skos:related rdf:resource="http://aims.fao.org/aos/agrovoc/c_ba3b2ea7"/>
    <skos:related rdf:resource="http://aims.fao.org/aos/agrovoc/c_9f542492"/>
    <rdfs:label>Urban Tenure</rdfs:label>
    <schema:image rdf:resource="https://landportal.org/sites/landportal.org/files/icons-landportal-10-transparent.png"/>
    <skos:prefLabel>Urban Tenure</skos:prefLabel>
    <skos:related rdf:resource="http://aims.fao.org/aos/agrovoc/c_37948"/>
    <skos:notation>T-URBAN</skos:notation>
    <skos:related rdf:resource="http://aims.fao.org/aos/agrovoc/c_32620"/>
    <skos:related rdf:resource="http://aims.fao.org/aos/agrovoc/c_8085"/>
    <skos:related rdf:resource="http://aims.fao.org/aos/agrovoc/c_34ea1b1e"/>
    <skos:related rdf:resource="http://aims.fao.org/aos/agrovoc/c_4174"/>
    <rdf:type rdf:resource="http://www.w3.org/2004/02/skos/core#Concept"/>
    <skos:related rdf:resource="http://aims.fao.org/aos/agrovoc/c_9001019"/>
    <rdfs:seeAlso rdf:resource="https://landportal.org/voc/themes/urbanisation"/>
    <skos:related rdf:resource="http://aims.fao.org/aos/agrovoc/c_8086"/>
    <skos:related rdf:resource="http://aims.fao.org/aos/agrovoc/c_8088"/>
    <skos:related rdf:resource="http://aims.fao.org/aos/agrovoc/c_18389"/>
    <skos:inScheme rdf:resource="http://data.landportal.info/vocabulary/26"/>
  </rdf:Description>
  <rdf:Description rdf:about="http://data.landportal.info/voc/landvoc/theme/T-INST">
    <schema:image rdf:resource="https://landportal.org/sites/landportal.org/files/icons-landportal-06-transparent.png"/>
    <rdf:type rdf:resource="http://www.w3.org/2004/02/skos/core#Concept"/>
    <skos:prefLabel>Land Stakeholders &amp; Institutions</skos:prefLabel>
    <skos:inScheme rdf:resource="http://data.landportal.info/vocabulary/26"/>
    <skos:definition>A stakeholder is anyone or any institution who has interests in, or is affected by, an issue or activity or transaction, and therefore has a natural right to participate in decisions relating to it.  There may be more than one stakeholder, or stakeholder group, claiming an interest in the land use on a particular area of land. As examples, a farmer is a stakeholder in relation to the distribution or management of irrigation water from a common source, or as regards decisions on grazing rights on communal land. The term can also be applied to groups, as when several groups have an interest in, or are affected by, the exploitation of the water from a reservoir or products extracted from a forest. Stakeholders include those individuals or groups, such as women or indigenous communities, who have genuine and legitimate claims on use, but whose opinion may not be valued in current negotiations for cultural or religious reasons. Groups resident outside the area, such as non-governmental organizations (NGOs) and research institutions, can also be stakeholders. Also the government of a country may have ministries with the position of stakeholders. The concept can be extended to include unborn generations who have a future interest in the resource. Source: FAO</skos:definition>
    <skos:notation>T-INST</skos:notation>
    <skos:related rdf:resource="http://aims.fao.org/aos/agrovoc/c_2224"/>
    <rdfs:seeAlso rdf:resource="https://landportal.org/voc/themes/land-stakeholders-institutions"/>
    <rdfs:label>Land Stakeholders &amp; Institutions</rdfs:label>
  </rdf:Description>
  <rdf:Description rdf:about="http://data.landportal.info/voc/landvoc/theme/T-FOOD">
    <skos:inScheme rdf:resource="http://data.landportal.info/vocabulary/26"/>
    <skos:related rdf:resource="http://aims.fao.org/aos/agrovoc/c_10967"/>
    <skos:prefLabel>Land &amp; Food Security</skos:prefLabel>
    <rdfs:label>Land &amp; Food Security</rdfs:label>
    <rdf:type rdf:resource="http://www.w3.org/2004/02/skos/core#Concept"/>
    <rdfs:seeAlso rdf:resource="https://landportal.org/voc/themes/land-food-security"/>
    <skos:notation>T-FOOD</skos:notation>
    <schema:image rdf:resource="https://landportal.org/sites/landportal.org/files/icons-landportal-03-transparent.png"/>
    <skos:definition>Food security exists when all people, at all times, have physical and economic access to sufficient, safe and nutritious food to meet their dietary needs and foodpreferences for an active and healthy life. Source: FAO</skos:definition>
  </rdf:Description>
  <rdf:Description rdf:about="http://data.landportal.info/voc/landvoc/theme/T-POSTCONFLICT">
    <rdf:type rdf:resource="http://www.w3.org/2004/02/skos/core#Concept"/>
    <skos:inScheme rdf:resource="http://data.landportal.info/vocabulary/26"/>
    <rdfs:seeAlso rdf:resource="https://landportal.org/voc/landvoc/theme/land-post-conflict-settings"/>
    <rdfs:label>Land in post-conflict settings</rdfs:label>
    <skos:prefLabel>Land in post-conflict settings</skos:prefLabel>
    <skos:notation>T-POSTCONFLICT</skos:notation>
    <skos:definition>Post-war societies not only have to deal with continuing unpeaceful relations but also land-related conflict legacies, farmland and forest degradation, heavily exploited natural resources, land mines, a destroyed infrastructure, as well as returning refugees and ex-combatants. In the aftermath of war, access to and control of land often remains a sensitive issue which may precipitate tensions and lead to a renewed destabilization of volatile post-conflict situations.</skos:definition>
  </rdf:Description>
  <rdf:Description rdf:about="http://data.landportal.info/voc/landvoc/theme/T-PASTOR">
    <skos:prefLabel>Rangelands, Drylands &amp; Pastoralism</skos:prefLabel>
    <skos:related rdf:resource="http://aims.fao.org/aos/agrovoc/c_8e487587"/>
    <skos:inScheme rdf:resource="http://data.landportal.info/vocabulary/26"/>
    <skos:notation>T-PASTOR</skos:notation>
    <skos:related rdf:resource="http://aims.fao.org/aos/agrovoc/c_653f04fe"/>
    <skos:related rdf:resource="http://aims.fao.org/aos/agrovoc/c_3369"/>
    <schema:image rdf:resource="https://landportal.org/sites/landportal.org/files/icons-landportal-09-transparent.png"/>
    <rdfs:label>Rangelands, Drylands &amp; Pastoralism</rdfs:label>
    <rdf:type rdf:resource="http://www.w3.org/2004/02/skos/core#Concept"/>
    <skos:related rdf:resource="http://aims.fao.org/aos/agrovoc/c_6b8a1f45"/>
    <skos:related rdf:resource="http://aims.fao.org/aos/agrovoc/c_bac66d94"/>
    <skos:related rdf:resource="http://aims.fao.org/aos/agrovoc/c_25243"/>
    <skos:related rdf:resource="http://aims.fao.org/aos/agrovoc/c_6448"/>
    <rdfs:seeAlso rdf:resource="https://landportal.org/voc/themes/rangelands-drylands-pastoralism"/>
    <skos:definition>Rangelands are grasslands, shrublands, woodlands, wetlands, and deserts that are grazed by domestic livestock or wild animals. Types of rangelands include tallgrass and shortgrass prairies, desert grasslands and shrublands, woodlands, savannas, chaparrals, steppes, and tundras. Pastoralism is the branch of agriculture concerned with the raising of livestock. "Pastoralism" generally has a mobile aspect, moving the herds in search of fresh pasture and water (in contrast to pastoral farming, in which non-nomadic farmers grow crops and improve pastures for their livestock).    Drylands conventionally are defined in terms of water stress: as terrestrial areas where the mean annual rainfall (including snow, fog, hail, etc) is lower than the total amount of water evaporated to the atmosphere. Sources: GlobalRangelands.org &amp;amp; Wikipedia &amp;amp; IUCN  </skos:definition>
    <skos:related rdf:resource="http://aims.fao.org/aos/agrovoc/c_16112"/>
    <skos:related rdf:resource="http://aims.fao.org/aos/agrovoc/c_4d6b6100"/>
    <skos:related rdf:resource="http://aims.fao.org/aos/agrovoc/c_97241aeb"/>
  </rdf:Description>
  <rdf:Description rdf:about="http://data.landportal.info/voc/landvoc/theme/T-INVEST">
    <skos:related rdf:resource="http://aims.fao.org/aos/agrovoc/c_8b6d895f"/>
    <skos:related rdf:resource="http://aims.fao.org/aos/agrovoc/c_a4f67d48"/>
    <skos:related rdf:resource="http://aims.fao.org/aos/agrovoc/c_15d85712"/>
    <skos:definition>Investments in agricultural land may be essential for achieving food security and promoting economic growth, but what are the potential costs and benefits for local landholders and the environment?</skos:definition>
    <skos:related rdf:resource="http://aims.fao.org/aos/agrovoc/c_666dbc26"/>
    <skos:inScheme rdf:resource="http://data.landportal.info/vocabulary/26"/>
    <skos:related rdf:resource="http://aims.fao.org/aos/agrovoc/c_0d7ef890"/>
    <skos:related rdf:resource="http://aims.fao.org/aos/agrovoc/c_357653f9"/>
    <skos:related rdf:resource="http://aims.fao.org/aos/agrovoc/c_9a4f48b4"/>
    <schema:image rdf:resource="https://landportal.org/sites/landportal.org/files/icons-landportal-08-transparent.png"/>
    <skos:related rdf:resource="http://aims.fao.org/aos/agrovoc/c_4181"/>
    <skos:related rdf:resource="http://aims.fao.org/aos/agrovoc/c_cc39a497"/>
    <skos:related rdf:resource="http://aims.fao.org/aos/agrovoc/c_4175"/>
    <rdf:type rdf:resource="http://www.w3.org/2004/02/skos/core#Concept"/>
    <skos:related rdf:resource="http://aims.fao.org/aos/agrovoc/c_89d3dcbb"/>
    <rdfs:label>Land &amp; Investments</rdfs:label>
    <skos:notation>T-INVEST</skos:notation>
    <skos:prefLabel>Land &amp; Investments</skos:prefLabel>
    <rdfs:seeAlso rdf:resource="https://landportal.org/voc/themes/large-scale-land-acquisitions"/>
    <skos:related rdf:resource="http://aims.fao.org/aos/agrovoc/c_45ce1b52"/>
  </rdf:Description>
  <rdf:Description rdf:about="http://data.landportal.info/voc/landvoc/theme/T-INDIG">
    <skos:related rdf:resource="http://aims.fao.org/aos/agrovoc/c_16532"/>
    <skos:definition>Secure community land rights are an essential condition for Indigenous Peoples and local communities to enjoy human rights, socio-economic development, and cultural protection.</skos:definition>
    <skos:related rdf:resource="http://aims.fao.org/aos/agrovoc/c_9904d265"/>
    <skos:related rdf:resource="http://aims.fao.org/aos/agrovoc/c_28e0dafa"/>
    <schema:image rdf:resource="https://landportal.org/sites/landportal.org/files/icons-landportal-02-transparent.png"/>
    <skos:related rdf:resource="http://aims.fao.org/aos/agrovoc/c_1782"/>
    <skos:related rdf:resource="http://aims.fao.org/aos/agrovoc/c_45cd8441"/>
    <skos:inScheme rdf:resource="http://data.landportal.info/vocabulary/26"/>
    <skos:notation>T-INDIG</skos:notation>
    <rdfs:label>Indigenous &amp; Community Land Rights</rdfs:label>
    <skos:related rdf:resource="http://aims.fao.org/aos/agrovoc/c_86524ff8"/>
    <skos:related rdf:resource="http://aims.fao.org/aos/agrovoc/c_331524"/>
    <skos:prefLabel>Indigenous &amp; Community Land Rights</skos:prefLabel>
    <skos:related rdf:resource="http://aims.fao.org/aos/agrovoc/c_a291ae58"/>
    <skos:related rdf:resource="http://aims.fao.org/aos/agrovoc/c_ff890f6b"/>
    <rdf:type rdf:resource="http://www.w3.org/2004/02/skos/core#Concept"/>
    <skos:related rdf:resource="http://aims.fao.org/aos/agrovoc/c_d42b49e7"/>
    <rdfs:seeAlso rdf:resource="https://landportal.org/voc/themes/indigenous-community-land-rights"/>
    <skos:related rdf:resource="http://aims.fao.org/aos/agrovoc/c_9000022"/>
  </rdf:Description>
  <rdf:Description rdf:about="http://data.landportal.info/voc/landvoc/theme/T-CORRUPT">
    <skos:related rdf:resource="http://aims.fao.org/aos/agrovoc/c_28663"/>
    <skos:notation>T-CORRUPT</skos:notation>
    <rdfs:seeAlso rdf:resource="https://landportal.org/voc/landvoc/theme/land-corruption"/>
    <skos:prefLabel>Land &amp; Corruption</skos:prefLabel>
    <skos:inScheme rdf:resource="http://data.landportal.info/vocabulary/26"/>
    <rdfs:label>Land &amp; Corruption</rdfs:label>
    <schema:image rdf:resource="https://landportal.org/sites/landportal.org/files/icons-landportal-107.png"/>
    <rdf:type rdf:resource="http://www.w3.org/2004/02/skos/core#Concept"/>
  </rdf:Description>
  <rdf:Description rdf:about="http://data.landportal.info/voc/landvoc/theme/T-ENVIR">
    <skos:related rdf:resource="http://aims.fao.org/aos/agrovoc/c_36580"/>
    <skos:related rdf:resource="http://aims.fao.org/aos/agrovoc/c_a6fdfb0e"/>
    <skos:related rdf:resource="http://aims.fao.org/aos/agrovoc/c_2593"/>
    <rdfs:seeAlso rdf:resource="https://landportal.org/voc/themes/land-climate-change-and-environment"/>
    <skos:related rdf:resource="http://aims.fao.org/aos/agrovoc/c_1666"/>
    <skos:related rdf:resource="http://aims.fao.org/aos/agrovoc/c_1374158672853"/>
    <skos:related rdf:resource="http://aims.fao.org/aos/agrovoc/c_62487b4a"/>
    <schema:image rdf:resource="https://landportal.org/sites/landportal.org/files/icons-landportal-07-transparent.png"/>
    <skos:inScheme rdf:resource="http://data.landportal.info/vocabulary/26"/>
    <rdfs:label>Land, Climate Change &amp; Environment</rdfs:label>
    <skos:related rdf:resource="http://aims.fao.org/aos/agrovoc/c_34823"/>
    <skos:related rdf:resource="http://aims.fao.org/aos/agrovoc/c_7ffc9d69"/>
    <rdf:type rdf:resource="http://www.w3.org/2004/02/skos/core#Concept"/>
    <skos:related rdf:resource="http://aims.fao.org/aos/agrovoc/c_6887"/>
    <skos:related rdf:resource="http://aims.fao.org/aos/agrovoc/c_35332"/>
    <skos:related rdf:resource="http://aims.fao.org/aos/agrovoc/c_37720"/>
    <skos:related rdf:resource="http://aims.fao.org/aos/agrovoc/c_bdedf48c"/>
    <skos:prefLabel>Land, Climate Change &amp; Environment</skos:prefLabel>
    <skos:related rdf:resource="http://aims.fao.org/aos/agrovoc/c_15590"/>
    <skos:definition>Climate change can destabilize existing land and resource governance institutions and associated property rights across the spectrum of landscape types. Transformed climatic conditions, manifested in either rapid-onset or slow-onset ways, can change how land and natural resources are accessed and used as geographical shifts in resource productivity, resource scarcity, and therefore land use patterns occur.</skos:definition>
    <skos:related rdf:resource="http://aims.fao.org/aos/agrovoc/c_37952"/>
    <skos:notation>T-ENVIR</skos:notation>
  </rdf:Description>
  <rdf:Description rdf:about="http://data.landportal.info/voc/landvoc/theme/T-GENDER">
    <skos:related rdf:resource="http://aims.fao.org/aos/agrovoc/c_64d8574a"/>
    <skos:related rdf:resource="http://aims.fao.org/aos/agrovoc/c_70a14ab3"/>
    <skos:related rdf:resource="http://aims.fao.org/aos/agrovoc/c_a0982198"/>
    <skos:prefLabel>Land &amp; Gender</skos:prefLabel>
    <skos:notation>T-GENDER</skos:notation>
    <skos:related rdf:resource="http://aims.fao.org/aos/agrovoc/c_8420"/>
    <skos:related rdf:resource="http://aims.fao.org/aos/agrovoc/c_85dfd05c"/>
    <rdfs:seeAlso rdf:resource="https://landportal.org/categories/land-gender"/>
    <skos:related rdf:resource="http://aims.fao.org/aos/agrovoc/c_1dfe5bfe"/>
    <skos:inScheme rdf:resource="http://data.landportal.info/vocabulary/26"/>
    <skos:related rdf:resource="http://aims.fao.org/aos/agrovoc/c_958edb9d"/>
    <skos:definition>To achieve the Sustainable Development Goals and promote gender equity in access to land, laws, institutions, and customary practices that are gender discriminatory need to be addressed.</skos:definition>
    <rdf:type rdf:resource="http://www.w3.org/2004/02/skos/core#Concept"/>
    <skos:related rdf:resource="http://aims.fao.org/aos/agrovoc/c_b3372020"/>
    <schema:image rdf:resource="https://landportal.org/sites/landportal.org/files/icons-landportal-04-transparent.png"/>
    <rdfs:label>Land &amp; Gender</rdfs:label>
  </rdf:Description>
  <rdf:Description rdf:about="http://data.landportal.info/voc/landvoc/theme/T-SOCEC">
    <skos:related rdf:resource="http://aims.fao.org/aos/agrovoc/c_25195"/>
    <rdfs:seeAlso rdf:resource="https://landportal.org/voc/landvoc/theme/socio-economic-institutional-context"/>
    <rdf:type rdf:resource="http://www.w3.org/2004/02/skos/core#Concept"/>
    <skos:notation>T-SOCEC</skos:notation>
    <skos:definition>This theme include all information which are not directly related to land issues, but are important to understand the general context in which land dynamics occur. For instance, this theme includes socio-economic, demographic and institutional information.</skos:definition>
    <schema:image rdf:resource="https://landportal.org/sites/landportal.org/files/icons-landportal-11-transparent.png"/>
    <skos:prefLabel>Socio-Economic &amp; Institutional Context</skos:prefLabel>
    <skos:inScheme rdf:resource="http://data.landportal.info/vocabulary/26"/>
    <rdfs:label>Socio-Economic &amp; Institutional Context</rdfs:label>
    <skos:related rdf:resource="http://aims.fao.org/aos/agrovoc/c_6705"/>
  </rdf:Description>
  <rdf:Description rdf:about="http://data.landportal.info/voc/landvoc/theme/T-FLR">
    <skos:notation>T-FLR</skos:notation>
    <skos:prefLabel>Forest Landscape Restoration</skos:prefLabel>
    <rdf:type rdf:resource="http://www.w3.org/2004/02/skos/core#Concept"/>
    <skos:inScheme rdf:resource="http://data.landportal.info/vocabulary/26"/>
    <rdfs:label>Forest Landscape Restoration</rdfs:label>
    <rdfs:seeAlso rdf:resource="https://landportal.org/voc/landvoc/theme/forest-landscape-restoration"/>
    <skos:definition>Forest landscape restoration (FLR) is the ongoing process of regaining ecological functionality and enhancing human well-being across deforested or degraded forest landscapes. FLR is more than just planting trees – it is restoring a whole landscape to meet present and future needs and to offer multiple benefits and land uses over time. Source: IUCN (https://www.iucn.org/theme/forests/our-work/forest-landscape-restoration)</skos:definition>
  </rdf:Description>
</rdf:RDF>
