<?xml version="1.0" encoding="UTF-8"?>
<rdf:RDF xmlns:rdf="http://www.w3.org/1999/02/22-rdf-syntax-ns#"
  xmlns:dct="http://purl.org/dc/terms/"
  xmlns:schema="http://schema.org/"
  xmlns:skos="http://www.w3.org/2004/02/skos/core#"
  xmlns:sdmx-attribute="http://purl.org/linked-data/sdmx/2009/attribute#"
  xmlns:rdfs="http://www.w3.org/2000/01/rdf-schema#">

  <rdf:Description rdf:about="http://data.landportal.info/indicator/UN-AG_LND_DGRD">
    <rdf:type rdf:resource="http://www.w3.org/2004/02/skos/core#Concept"/>
    <rdf:type rdf:resource="http://purl.org/weso/ontology/computex#Indicator"/>
    <dct:subject rdf:resource="http://data.landportal.info/voc/landvoc/theme/T-FLR"/>
    <dct:subject rdf:resource="http://data.landportal.info/voc/landvoc/theme/T-ENVIR"/>
    <dct:subject rdf:resource="http://data.landportal.info/voc/landvoc/theme/T-PASTOR"/>
    <schema:about rdf:resource="http://data.landportal.info/voc/landvoc/theme/T-FLR"/>
    <schema:about rdf:resource="http://data.landportal.info/voc/landvoc/theme/T-ENVIR"/>
    <schema:about rdf:resource="http://data.landportal.info/voc/landvoc/theme/T-PASTOR"/>
    <dct:identifier>UN-AG_LND_DGRD</dct:identifier>
    <skos:notation>UN-AG_LND_DGRD</skos:notation>
    <dct:source rdf:resource="http://data.landportal.info/dataset/UN-SDG_15.3.1"/>
    <sdmx-attribute:unitMeasure>Percentage (%)</sdmx-attribute:unitMeasure>
    <rdfs:label>Proportion of land that is degraded over total land area (%)</rdfs:label>
    <skos:prefLabel>Proportion of land that is degraded over total land area (%)</skos:prefLabel>
    <dct:title>Proportion of land that is degraded over total land area (%)</dct:title>
    <skos:definition>The data series presented here measures proportion of land that is degraded over total land area (%). This data series contributes to the measurement of SDG Indicator 15.3.1, classified as Tier II in September 2018, which is officially defined as follows: The measurement unit for this indicator is the spatial extent (hectares or km2) expressed as the proportion (percentage or %) of land that is degraded over total land area. SDG indicator 15.3.1 is a binary - degraded/not degraded - quantification based on the analysis of available data for three sub-indicators to be validated and reported by national authorities. The sub-indicators (Trends in Land Cover, Land Productivity and Carbon Stocks) were adopted by the UNCCD’s governing body in 2013 as part of its monitoring and evaluation approach.  According to United Nations Convention to Combat Desertification (UNCCD) and partners (Food and Agriculture Organization of the United Nations (FAO), United Nations Statistics Division (UNSD), United Nations Environment Programme (UNEP), United Nations Framework Convention on Climate Change (UNFCCC), Convention on Biological Diversity (CBD)) -- the Custodian Agencies for this indicator -- the rationale behind this indicator can be summarised as follows:  In the last decade, there have been a number of global/regional targets and initiatives to halt and reverse land degradation and restore degraded land. Starting in 2010, these include the Aichi Biodiversity Targets, one of which aims to restore at least 15% of degraded ecosystems; the Bonn Challenge and its regional initiatives to restore more than 150 million hectares; and most recently the Sustainable Development Goals (SDGs), in particular SDG target 15.3. For each of the sub-indicators, countries can access a wide range of data sources, including Earth observation and geospatial information, while at the same time ensuring national ownership.18 The use of the existing national reporting templates of the UNCCD, 19 which include the indicator and subindicators, provides a practical and harmonized approach to reporting on this indicator beginning in 2018 and every four years thereafter. SDG indicator 15.3.1 is a binary -- degraded/not degraded -- quantification based on the analysis of available data that is validated and reported by national authorities. The full official metadata for this Tier II indicator are available at UN SDG Metadata website. For more information, check also this indicator's page on Land Portal SDG porfolio. For more information on this data series, please visit UN SDG website.</skos:definition>
    <dct:description>The data series presented here measures proportion of land that is degraded over total land area (%). This data series contributes to the measurement of SDG Indicator 15.3.1, classified as Tier II in September 2018, which is officially defined as follows: The measurement unit for this indicator is the spatial extent (hectares or km2) expressed as the proportion (percentage or %) of land that is degraded over total land area. SDG indicator 15.3.1 is a binary - degraded/not degraded - quantification based on the analysis of available data for three sub-indicators to be validated and reported by national authorities. The sub-indicators (Trends in Land Cover, Land Productivity and Carbon Stocks) were adopted by the UNCCD’s governing body in 2013 as part of its monitoring and evaluation approach.  According to United Nations Convention to Combat Desertification (UNCCD) and partners (Food and Agriculture Organization of the United Nations (FAO), United Nations Statistics Division (UNSD), United Nations Environment Programme (UNEP), United Nations Framework Convention on Climate Change (UNFCCC), Convention on Biological Diversity (CBD)) -- the Custodian Agencies for this indicator -- the rationale behind this indicator can be summarised as follows:  In the last decade, there have been a number of global/regional targets and initiatives to halt and reverse land degradation and restore degraded land. Starting in 2010, these include the Aichi Biodiversity Targets, one of which aims to restore at least 15% of degraded ecosystems; the Bonn Challenge and its regional initiatives to restore more than 150 million hectares; and most recently the Sustainable Development Goals (SDGs), in particular SDG target 15.3. For each of the sub-indicators, countries can access a wide range of data sources, including Earth observation and geospatial information, while at the same time ensuring national ownership.18 The use of the existing national reporting templates of the UNCCD, 19 which include the indicator and subindicators, provides a practical and harmonized approach to reporting on this indicator beginning in 2018 and every four years thereafter. SDG indicator 15.3.1 is a binary -- degraded/not degraded -- quantification based on the analysis of available data that is validated and reported by national authorities. The full official metadata for this Tier II indicator are available at UN SDG Metadata website. For more information, check also this indicator's page on Land Portal SDG porfolio. For more information on this data series, please visit UN SDG website.</dct:description>
    <rdfs:comment>The data series presented here measures proportion of land that is degraded over total land area (%). This data series contributes to the measurement of SDG Indicator 15.3.1, classified as Tier II in September 2018, which is officially defined as follows: The measurement unit for this indicator is the spatial extent (hectares or km2) expressed as the proportion (percentage or %) of land that is degraded over total land area. SDG indicator 15.3.1 is a binary - degraded/not degraded - quantification based on the analysis of available data for three sub-indicators to be validated and reported by national authorities. The sub-indicators (Trends in Land Cover, Land Productivity and Carbon Stocks) were adopted by the UNCCD’s governing body in 2013 as part of its monitoring and evaluation approach.  According to United Nations Convention to Combat Desertification (UNCCD) and partners (Food and Agriculture Organization of the United Nations (FAO), United Nations Statistics Division (UNSD), United Nations Environment Programme (UNEP), United Nations Framework Convention on Climate Change (UNFCCC), Convention on Biological Diversity (CBD)) -- the Custodian Agencies for this indicator -- the rationale behind this indicator can be summarised as follows:  In the last decade, there have been a number of global/regional targets and initiatives to halt and reverse land degradation and restore degraded land. Starting in 2010, these include the Aichi Biodiversity Targets, one of which aims to restore at least 15% of degraded ecosystems; the Bonn Challenge and its regional initiatives to restore more than 150 million hectares; and most recently the Sustainable Development Goals (SDGs), in particular SDG target 15.3. For each of the sub-indicators, countries can access a wide range of data sources, including Earth observation and geospatial information, while at the same time ensuring national ownership.18 The use of the existing national reporting templates of the UNCCD, 19 which include the indicator and subindicators, provides a practical and harmonized approach to reporting on this indicator beginning in 2018 and every four years thereafter. SDG indicator 15.3.1 is a binary -- degraded/not degraded -- quantification based on the analysis of available data that is validated and reported by national authorities. The full official metadata for this Tier II indicator are available at UN SDG Metadata website. For more information, check also this indicator's page on Land Portal SDG porfolio. For more information on this data series, please visit UN SDG website.</rdfs:comment>
    <skos:inScheme rdf:resource="http://data.landportal.info/vocabulary/25"/>
    <rdfs:seeAlso rdf:resource="https://landportal.org/book/indicator/un-aglnddgrd"/>
  </rdf:Description>

</rdf:RDF>