<?xml version="1.0" encoding="UTF-8"?>
<rdf:RDF xmlns:rdf="http://www.w3.org/1999/02/22-rdf-syntax-ns#"
  xmlns:dct="http://purl.org/dc/terms/"
  xmlns:skos="http://www.w3.org/2004/02/skos/core#"
  xmlns:sdmx-attribute="http://purl.org/linked-data/sdmx/2009/attribute#"
  xmlns:schema="http://schema.org/"
  xmlns:rdfs="http://www.w3.org/2000/01/rdf-schema#">

  <rdf:Description rdf:about="http://data.landportal.info/indicator/WB-SH.H2O.SAFE.RU.ZS">
    <rdf:type rdf:resource="http://www.w3.org/2004/02/skos/core#Concept"/>
    <rdf:type rdf:resource="http://purl.org/weso/ontology/computex#Indicator"/>
    <dct:identifier>WB-SH.H2O.SAFE.RU.ZS</dct:identifier>
    <skos:notation>WB-SH.H2O.SAFE.RU.ZS</skos:notation>
    <dct:subject rdf:resource="http://aims.fao.org/aos/agrovoc/c_aca7ac6d"/>
    <dct:subject rdf:resource="http://aims.fao.org/aos/agrovoc/c_4182"/>
    <dct:subject rdf:resource="http://aims.fao.org/aos/agrovoc/c_6699"/>
    <dct:subject rdf:resource="http://aims.fao.org/aos/agrovoc/c_16062"/>
    <dct:subject rdf:resource="http://data.landportal.info/voc/landvoc/theme/T-SOCEC"/>
    <schema:about rdf:resource="http://aims.fao.org/aos/agrovoc/c_aca7ac6d"/>
    <schema:about rdf:resource="http://aims.fao.org/aos/agrovoc/c_4182"/>
    <schema:about rdf:resource="http://aims.fao.org/aos/agrovoc/c_6699"/>
    <schema:about rdf:resource="http://aims.fao.org/aos/agrovoc/c_16062"/>
    <schema:about rdf:resource="http://data.landportal.info/voc/landvoc/theme/T-SOCEC"/>
    <dct:source rdf:resource="http://data.landportal.info/dataset/WB-HN"/>
    <sdmx-attribute:unitMeasure>Percentage (%)</sdmx-attribute:unitMeasure>
    <rdfs:label>Improved water source, rural (% of rural population with access)</rdfs:label>
    <skos:prefLabel>Improved water source, rural (% of rural population with access)</skos:prefLabel>
    <dct:title>Improved water source, rural (% of rural population with access)</dct:title>
    <skos:definition>Access to an improved water source refers to the percentage of the population using an improved drinking water source. The improved drinking water source includes piped water on premises (piped household water connection located inside the user’s dwelling, plot or yard), and other improved drinking water sources (public taps or standpipes, tube wells or boreholes, protected dug wells, protected springs, and rainwater collection).   Please note that the data for this indicator have not been updated since 2015. The WHO/UNICEF Joint Monitoring Programme for Water Supply and Sanitation has introduced updated water and sanitation indicators. For the most recent data on water access, please see the following indicators: People using safely managed drinking water services (% of population) (SH.H2O.SMDW.ZS) and People using basic drinking water services (% of population) (SH.H2O.BASW.ZS).</skos:definition>
    <dct:description>Access to an improved water source refers to the percentage of the population using an improved drinking water source. The improved drinking water source includes piped water on premises (piped household water connection located inside the user’s dwelling, plot or yard), and other improved drinking water sources (public taps or standpipes, tube wells or boreholes, protected dug wells, protected springs, and rainwater collection).   Please note that the data for this indicator have not been updated since 2015. The WHO/UNICEF Joint Monitoring Programme for Water Supply and Sanitation has introduced updated water and sanitation indicators. For the most recent data on water access, please see the following indicators: People using safely managed drinking water services (% of population) (SH.H2O.SMDW.ZS) and People using basic drinking water services (% of population) (SH.H2O.BASW.ZS).</dct:description>
    <rdfs:comment>Access to an improved water source refers to the percentage of the population using an improved drinking water source. The improved drinking water source includes piped water on premises (piped household water connection located inside the user’s dwelling, plot or yard), and other improved drinking water sources (public taps or standpipes, tube wells or boreholes, protected dug wells, protected springs, and rainwater collection).   Please note that the data for this indicator have not been updated since 2015. The WHO/UNICEF Joint Monitoring Programme for Water Supply and Sanitation has introduced updated water and sanitation indicators. For the most recent data on water access, please see the following indicators: People using safely managed drinking water services (% of population) (SH.H2O.SMDW.ZS) and People using basic drinking water services (% of population) (SH.H2O.BASW.ZS).</rdfs:comment>
    <skos:inScheme rdf:resource="http://data.landportal.info/vocabulary/25"/>
    <rdfs:seeAlso rdf:resource="https://landportal.org/book/indicators/wb-shh2osaferuzs"/>
  </rdf:Description>

</rdf:RDF>