<?xml version="1.0" encoding="UTF-8"?>
<rdf:RDF xmlns:rdf="http://www.w3.org/1999/02/22-rdf-syntax-ns#"
  xmlns:dct="http://purl.org/dc/terms/"
  xmlns:skos="http://www.w3.org/2004/02/skos/core#"
  xmlns:sdmx-attribute="http://purl.org/linked-data/sdmx/2009/attribute#"
  xmlns:schema="http://schema.org/"
  xmlns:rdfs="http://www.w3.org/2000/01/rdf-schema#">

  <rdf:Description rdf:about="http://data.landportal.info/indicator/WB-SH.H2O.SMDW.RU.ZS">
    <rdf:type rdf:resource="http://www.w3.org/2004/02/skos/core#Concept"/>
    <rdf:type rdf:resource="http://purl.org/weso/ontology/computex#Indicator"/>
    <dct:identifier>WB-SH.H2O.SMDW.RU.ZS</dct:identifier>
    <skos:notation>WB-SH.H2O.SMDW.RU.ZS</skos:notation>
    <dct:subject rdf:resource="http://aims.fao.org/aos/agrovoc/c_aca7ac6d"/>
    <dct:subject rdf:resource="http://aims.fao.org/aos/agrovoc/c_4182"/>
    <dct:subject rdf:resource="http://aims.fao.org/aos/agrovoc/c_6699"/>
    <dct:subject rdf:resource="http://aims.fao.org/aos/agrovoc/c_16062"/>
    <dct:subject rdf:resource="http://data.landportal.info/voc/landvoc/theme/T-SOCEC"/>
    <schema:about rdf:resource="http://aims.fao.org/aos/agrovoc/c_aca7ac6d"/>
    <schema:about rdf:resource="http://aims.fao.org/aos/agrovoc/c_4182"/>
    <schema:about rdf:resource="http://aims.fao.org/aos/agrovoc/c_6699"/>
    <schema:about rdf:resource="http://aims.fao.org/aos/agrovoc/c_16062"/>
    <schema:about rdf:resource="http://data.landportal.info/voc/landvoc/theme/T-SOCEC"/>
    <dct:source rdf:resource="http://data.landportal.info/dataset/WB-HN"/>
    <sdmx-attribute:unitMeasure>Percentage (%)</sdmx-attribute:unitMeasure>
    <rdfs:label>People using safely managed drinking water services, rural (% of rural population)</rdfs:label>
    <skos:prefLabel>People using safely managed drinking water services, rural (% of rural population)</skos:prefLabel>
    <dct:title>People using safely managed drinking water services, rural (% of rural population)</dct:title>
    <skos:definition>The percentage of people using drinking water from an improved source that is accessible on premises, available when needed and free from faecal and priority chemical contamination. Improved water sources include piped water, boreholes or tubewells, protected dug wells, protected springs, and packaged or delivered water.   More information on World Bank website</skos:definition>
    <dct:description>The percentage of people using drinking water from an improved source that is accessible on premises, available when needed and free from faecal and priority chemical contamination. Improved water sources include piped water, boreholes or tubewells, protected dug wells, protected springs, and packaged or delivered water.   More information on World Bank website</dct:description>
    <rdfs:comment>The percentage of people using drinking water from an improved source that is accessible on premises, available when needed and free from faecal and priority chemical contamination. Improved water sources include piped water, boreholes or tubewells, protected dug wells, protected springs, and packaged or delivered water.   More information on World Bank website</rdfs:comment>
    <skos:inScheme rdf:resource="http://data.landportal.info/vocabulary/25"/>
    <rdfs:seeAlso rdf:resource="https://landportal.org/book/indicator/shh2osmdwruzs"/>
  </rdf:Description>

</rdf:RDF>