<?xml version="1.0" encoding="UTF-8"?>
<rdf:RDF xmlns:rdf="http://www.w3.org/1999/02/22-rdf-syntax-ns#"
  xmlns:dct="http://purl.org/dc/terms/"
  xmlns:schema="http://schema.org/"
  xmlns:skos="http://www.w3.org/2004/02/skos/core#"
  xmlns:sdmx-attribute="http://purl.org/linked-data/sdmx/2009/attribute#"
  xmlns:rdfs="http://www.w3.org/2000/01/rdf-schema#">

  <rdf:Description rdf:about="http://data.landportal.info/indicator/LMM-LSIC-9CL">
    <rdf:type rdf:resource="http://www.w3.org/2004/02/skos/core#Concept"/>
    <rdf:type rdf:resource="http://purl.org/weso/ontology/computex#Indicator"/>
    <dct:subject rdf:resource="http://aims.fao.org/aos/agrovoc/c_ff890f6b"/>
    <dct:subject rdf:resource="http://aims.fao.org/aos/agrovoc/c_86524ff8"/>
    <dct:subject rdf:resource="http://aims.fao.org/aos/agrovoc/c_331524"/>
    <dct:subject rdf:resource="http://aims.fao.org/aos/agrovoc/c_37898"/>
    <dct:subject rdf:resource="http://aims.fao.org/aos/agrovoc/c_45cd8441"/>
    <dct:subject rdf:resource="http://aims.fao.org/aos/agrovoc/c_7fc44e33"/>
    <dct:subject rdf:resource="http://aims.fao.org/aos/agrovoc/c_16062"/>
    <dct:subject rdf:resource="http://data.landportal.info/voc/landvoc/theme/T-INDIG"/>
    <dct:subject rdf:resource="http://data.landportal.info/voc/landvoc/theme/T-INST"/>
    <schema:about rdf:resource="http://aims.fao.org/aos/agrovoc/c_ff890f6b"/>
    <schema:about rdf:resource="http://aims.fao.org/aos/agrovoc/c_86524ff8"/>
    <schema:about rdf:resource="http://aims.fao.org/aos/agrovoc/c_331524"/>
    <schema:about rdf:resource="http://aims.fao.org/aos/agrovoc/c_37898"/>
    <schema:about rdf:resource="http://aims.fao.org/aos/agrovoc/c_45cd8441"/>
    <schema:about rdf:resource="http://aims.fao.org/aos/agrovoc/c_7fc44e33"/>
    <schema:about rdf:resource="http://aims.fao.org/aos/agrovoc/c_16062"/>
    <schema:about rdf:resource="http://data.landportal.info/voc/landvoc/theme/T-INDIG"/>
    <schema:about rdf:resource="http://data.landportal.info/voc/landvoc/theme/T-INST"/>
    <dct:identifier>LMM-LSIC-9CL</dct:identifier>
    <skos:notation>LMM-LSIC-9CL</skos:notation>
    <dct:source rdf:resource="http://data.landportal.info/dataset/LMM-LSIC"/>
    <sdmx-attribute:unitMeasure>Index (1; 4)</sdmx-attribute:unitMeasure>
    <rdfs:label>IX - Rights to water - Community Lands</rdfs:label>
    <skos:prefLabel>IX - Rights to water - Community Lands</skos:prefLabel>
    <dct:title>IX - Rights to water - Community Lands</dct:title>
    <skos:definition>This indicator is part of the set of Indicators of the Legal Security of Indigenous and Community Lands estimated by LandMark (http://www.landmarkmap.org/). It answers to the following question: Does the law explicitly recognize that communities land rights include the rights to local water sources on the land? Each indicator is assigned a score from 1 (-&amp;gt; Yes, the law addresses the issue fully) to 4 (-&amp;gt; No, the law does not address the issue.) ot Not applicable (-&amp;gt; N/A Not applicable is used in cases where the subject matter in question is non-existent.). The scoring of indicators is based exclusively on express legal provisions.</skos:definition>
    <dct:description>This indicator is part of the set of Indicators of the Legal Security of Indigenous and Community Lands estimated by LandMark (http://www.landmarkmap.org/). It answers to the following question: Does the law explicitly recognize that communities land rights include the rights to local water sources on the land? Each indicator is assigned a score from 1 (-&amp;gt; Yes, the law addresses the issue fully) to 4 (-&amp;gt; No, the law does not address the issue.) ot Not applicable (-&amp;gt; N/A Not applicable is used in cases where the subject matter in question is non-existent.). The scoring of indicators is based exclusively on express legal provisions.</dct:description>
    <rdfs:comment>This indicator is part of the set of Indicators of the Legal Security of Indigenous and Community Lands estimated by LandMark (http://www.landmarkmap.org/). It answers to the following question: Does the law explicitly recognize that communities land rights include the rights to local water sources on the land? Each indicator is assigned a score from 1 (-&amp;gt; Yes, the law addresses the issue fully) to 4 (-&amp;gt; No, the law does not address the issue.) ot Not applicable (-&amp;gt; N/A Not applicable is used in cases where the subject matter in question is non-existent.). The scoring of indicators is based exclusively on express legal provisions.</rdfs:comment>
    <skos:inScheme rdf:resource="http://data.landportal.info/vocabulary/25"/>
    <rdfs:seeAlso rdf:resource="https://landportal.org/book/indicator/lmm-lsic-9cl"/>
  </rdf:Description>

</rdf:RDF>