<?xml version="1.0" encoding="UTF-8"?>
<rdf:RDF xmlns:rdf="http://www.w3.org/1999/02/22-rdf-syntax-ns#"
  xmlns:dct="http://purl.org/dc/terms/"
  xmlns:schema="http://schema.org/"
  xmlns:skos="http://www.w3.org/2004/02/skos/core#"
  xmlns:sdmx-attribute="http://purl.org/linked-data/sdmx/2009/attribute#"
  xmlns:rdfs="http://www.w3.org/2000/01/rdf-schema#">

  <rdf:Description rdf:about="http://data.landportal.info/indicator/FAO-6773-5110">
    <rdf:type rdf:resource="http://www.w3.org/2004/02/skos/core#Concept"/>
    <rdf:type rdf:resource="http://purl.org/weso/ontology/computex#Indicator"/>
    <dct:subject rdf:resource="http://data.landportal.info/voc/landvoc/overarching-category/OA-USE"/>
    <schema:about rdf:resource="http://data.landportal.info/voc/landvoc/overarching-category/OA-USE"/>
    <dct:identifier>FAO-6773-5110</dct:identifier>
    <skos:notation>FAO-6773-5110</skos:notation>
    <dct:source rdf:resource="http://data.landportal.info/dataset/FAO-LU"/>
    <sdmx-attribute:unitMeasure>1'000 Ha</sdmx-attribute:unitMeasure>
    <rdfs:label>Coastal waters</rdfs:label>
    <skos:prefLabel>Coastal waters</skos:prefLabel>
    <dct:title>Coastal waters</dct:title>
    <skos:definition>Waters located in between the land territory and the outer limit of the territorial sea. They comprise &quot;Internal waters&quot; and &quot;Territorial sea,&quot; and where applicable, &quot;Archipelagic waters.&quot;</skos:definition>
    <dct:description>Waters located in between the land territory and the outer limit of the territorial sea. They comprise &quot;Internal waters&quot; and &quot;Territorial sea,&quot; and where applicable, &quot;Archipelagic waters.&quot;</dct:description>
    <rdfs:comment>Waters located in between the land territory and the outer limit of the territorial sea. They comprise &quot;Internal waters&quot; and &quot;Territorial sea,&quot; and where applicable, &quot;Archipelagic waters.&quot;</rdfs:comment>
    <skos:inScheme rdf:resource="http://data.landportal.info/vocabulary/25"/>
    <rdfs:seeAlso rdf:resource="https://landportal.org/book/indicator/fao-6773-5110"/>
  </rdf:Description>

</rdf:RDF>