<?xml version="1.0" encoding="UTF-8"?>
<rdf:RDF xmlns:rdf="http://www.w3.org/1999/02/22-rdf-syntax-ns#"
  xmlns:dct="http://purl.org/dc/terms/"
  xmlns:schema="http://schema.org/"
  xmlns:skos="http://www.w3.org/2004/02/skos/core#"
  xmlns:sdmx-attribute="http://purl.org/linked-data/sdmx/2009/attribute#"
  xmlns:rdfs="http://www.w3.org/2000/01/rdf-schema#">

  <rdf:Description rdf:about="http://data.landportal.info/indicator/FAO-6643-5110">
    <rdf:type rdf:resource="http://www.w3.org/2004/02/skos/core#Concept"/>
    <rdf:type rdf:resource="http://purl.org/weso/ontology/computex#Indicator"/>
    <dct:subject rdf:resource="http://data.landportal.info/voc/landvoc/overarching-category/OA-USE"/>
    <schema:about rdf:resource="http://data.landportal.info/voc/landvoc/overarching-category/OA-USE"/>
    <dct:identifier>FAO-6643-5110</dct:identifier>
    <skos:notation>FAO-6643-5110</skos:notation>
    <dct:source rdf:resource="http://data.landportal.info/dataset/FAO-LU"/>
    <sdmx-attribute:unitMeasure>1'000 Ha</sdmx-attribute:unitMeasure>
    <rdfs:label>Exclusive Economic Zone (EEZ)</rdfs:label>
    <skos:prefLabel>Exclusive Economic Zone (EEZ)</skos:prefLabel>
    <dct:title>Exclusive Economic Zone (EEZ)</dct:title>
    <skos:definition>Waters beyond and adjacent to the territorial sea, not extending beyond 200 nautical miles from the baselines from which the breadth of the territorial sea is measured, determined in accordance with part V of UNCLOS (1982).</skos:definition>
    <dct:description>Waters beyond and adjacent to the territorial sea, not extending beyond 200 nautical miles from the baselines from which the breadth of the territorial sea is measured, determined in accordance with part V of UNCLOS (1982).</dct:description>
    <rdfs:comment>Waters beyond and adjacent to the territorial sea, not extending beyond 200 nautical miles from the baselines from which the breadth of the territorial sea is measured, determined in accordance with part V of UNCLOS (1982).</rdfs:comment>
    <skos:inScheme rdf:resource="http://data.landportal.info/vocabulary/25"/>
    <rdfs:seeAlso rdf:resource="https://landportal.org/book/indicator/fao-6643-5110"/>
  </rdf:Description>

</rdf:RDF>