<?xml version="1.0" encoding="UTF-8"?>
<rdf:RDF xmlns:rdf="http://www.w3.org/1999/02/22-rdf-syntax-ns#"
  xmlns:dct="http://purl.org/dc/terms/"
  xmlns:skos="http://www.w3.org/2004/02/skos/core#"
  xmlns:sdmx-attribute="http://purl.org/linked-data/sdmx/2009/attribute#"
  xmlns:rdfs="http://www.w3.org/2000/01/rdf-schema#">

  <rdf:Description rdf:about="http://data.landportal.info/indicator/FAO-6646-72151">
    <rdf:type rdf:resource="http://www.w3.org/2004/02/skos/core#Concept"/>
    <rdf:type rdf:resource="http://purl.org/weso/ontology/computex#Indicator"/>
    <dct:identifier>FAO-6646-72151</dct:identifier>
    <skos:notation>FAO-6646-72151</skos:notation>
    <dct:source rdf:resource="http://data.landportal.info/dataset/FAO-LU"/>
    <sdmx-attribute:unitMeasure>Million tonnes</sdmx-attribute:unitMeasure>
    <rdfs:label>Forest land (million tonnes)</rdfs:label>
    <skos:prefLabel>Forest land (million tonnes)</skos:prefLabel>
    <dct:title>Forest land (million tonnes)</dct:title>
    <skos:definition>Land spanning more than 0.5 hectares with trees higher than 5 metres and a canopy cover of more than 10 per cent, or trees able to reach these thresholds in situ. Excludes land that is predominantly under agricultural or urban land use, and land that is predominantly used for maintenance and restoration of environmental function. Explanatory notes: Forest land is determined both by the presence of trees and by the absence of other predominant land uses. The trees should be able to reach a minimum height of 5 metres in situ Includes areas with young trees that have not yet reached but that are expected to reach a canopy cover of 10 per cent and tree height of 5 metres. It also includes areas that are temporarily unstocked owing to clear-cutting as part of a forest management practice or natural disasters, and that are expected to be regenerated within five years. Local conditions may, in exceptional cases, justify the use of a longer time frame Includes forest roads, firebreaks and other small open areas May include forest land in national parks, nature reserves and other protected areas, such as those of specific environmental, scientific, historical, cultural or spiritual interest Includes windbreaks, shelter belts and corridors of trees with an area of more than 0.5 hectares and width of more than 20 metres Includes abandoned shifting cultivation land with a regeneration of trees that have, or is expected to reach, a canopy cover of 10 per cent and tree height of 5 metres Includes areas with mangroves in tidal zones, regardless of whether this area is classified as land area or not Includes areas with bamboo and palms provided that land use, height and canopy cover criteria are met Some agroforestry systems such as the taungya system, where crops are grown only during the first years of the forest rotation should be classified as forest Excludes: tree stands in agricultural production systems, such as fruit-tree plantations (→Permanent crops), oil palm plantations, rubber and Christmas trees (→Permanent crops) and agroforestry systems when crops are grown under tree cover     The previous code used for this indicator was FAO-6661-5110 (Item code 6661, Element code 5110)</skos:definition>
    <dct:description>Land spanning more than 0.5 hectares with trees higher than 5 metres and a canopy cover of more than 10 per cent, or trees able to reach these thresholds in situ. Excludes land that is predominantly under agricultural or urban land use, and land that is predominantly used for maintenance and restoration of environmental function. Explanatory notes: Forest land is determined both by the presence of trees and by the absence of other predominant land uses. The trees should be able to reach a minimum height of 5 metres in situ Includes areas with young trees that have not yet reached but that are expected to reach a canopy cover of 10 per cent and tree height of 5 metres. It also includes areas that are temporarily unstocked owing to clear-cutting as part of a forest management practice or natural disasters, and that are expected to be regenerated within five years. Local conditions may, in exceptional cases, justify the use of a longer time frame Includes forest roads, firebreaks and other small open areas May include forest land in national parks, nature reserves and other protected areas, such as those of specific environmental, scientific, historical, cultural or spiritual interest Includes windbreaks, shelter belts and corridors of trees with an area of more than 0.5 hectares and width of more than 20 metres Includes abandoned shifting cultivation land with a regeneration of trees that have, or is expected to reach, a canopy cover of 10 per cent and tree height of 5 metres Includes areas with mangroves in tidal zones, regardless of whether this area is classified as land area or not Includes areas with bamboo and palms provided that land use, height and canopy cover criteria are met Some agroforestry systems such as the taungya system, where crops are grown only during the first years of the forest rotation should be classified as forest Excludes: tree stands in agricultural production systems, such as fruit-tree plantations (→Permanent crops), oil palm plantations, rubber and Christmas trees (→Permanent crops) and agroforestry systems when crops are grown under tree cover     The previous code used for this indicator was FAO-6661-5110 (Item code 6661, Element code 5110)</dct:description>
    <rdfs:comment>Land spanning more than 0.5 hectares with trees higher than 5 metres and a canopy cover of more than 10 per cent, or trees able to reach these thresholds in situ. Excludes land that is predominantly under agricultural or urban land use, and land that is predominantly used for maintenance and restoration of environmental function. Explanatory notes: Forest land is determined both by the presence of trees and by the absence of other predominant land uses. The trees should be able to reach a minimum height of 5 metres in situ Includes areas with young trees that have not yet reached but that are expected to reach a canopy cover of 10 per cent and tree height of 5 metres. It also includes areas that are temporarily unstocked owing to clear-cutting as part of a forest management practice or natural disasters, and that are expected to be regenerated within five years. Local conditions may, in exceptional cases, justify the use of a longer time frame Includes forest roads, firebreaks and other small open areas May include forest land in national parks, nature reserves and other protected areas, such as those of specific environmental, scientific, historical, cultural or spiritual interest Includes windbreaks, shelter belts and corridors of trees with an area of more than 0.5 hectares and width of more than 20 metres Includes abandoned shifting cultivation land with a regeneration of trees that have, or is expected to reach, a canopy cover of 10 per cent and tree height of 5 metres Includes areas with mangroves in tidal zones, regardless of whether this area is classified as land area or not Includes areas with bamboo and palms provided that land use, height and canopy cover criteria are met Some agroforestry systems such as the taungya system, where crops are grown only during the first years of the forest rotation should be classified as forest Excludes: tree stands in agricultural production systems, such as fruit-tree plantations (→Permanent crops), oil palm plantations, rubber and Christmas trees (→Permanent crops) and agroforestry systems when crops are grown under tree cover     The previous code used for this indicator was FAO-6661-5110 (Item code 6661, Element code 5110)</rdfs:comment>
    <skos:inScheme rdf:resource="http://data.landportal.info/vocabulary/25"/>
    <rdfs:seeAlso rdf:resource="https://landportal.org/book/indicator/fao-6646-72151"/>
  </rdf:Description>

</rdf:RDF>