<?xml version="1.0" encoding="UTF-8"?>
<rdf:RDF xmlns:rdf="http://www.w3.org/1999/02/22-rdf-syntax-ns#"
  xmlns:dct="http://purl.org/dc/terms/"
  xmlns:schema="http://schema.org/"
  xmlns:skos="http://www.w3.org/2004/02/skos/core#"
  xmlns:sdmx-attribute="http://purl.org/linked-data/sdmx/2009/attribute#"
  xmlns:rdfs="http://www.w3.org/2000/01/rdf-schema#">

  <rdf:Description rdf:about="http://data.landportal.info/indicator/FAO-6762-5110">
    <rdf:type rdf:resource="http://www.w3.org/2004/02/skos/core#Concept"/>
    <rdf:type rdf:resource="http://purl.org/weso/ontology/computex#Indicator"/>
    <dct:subject rdf:resource="http://data.landportal.info/voc/landvoc/overarching-category/OA-USE"/>
    <schema:about rdf:resource="http://data.landportal.info/voc/landvoc/overarching-category/OA-USE"/>
    <dct:identifier>FAO-6762-5110</dct:identifier>
    <skos:notation>FAO-6762-5110</skos:notation>
    <dct:source rdf:resource="http://data.landportal.info/dataset/FAO-LU"/>
    <sdmx-attribute:unitMeasure>1'000 Ha</sdmx-attribute:unitMeasure>
    <rdfs:label>Land used for aquaculture</rdfs:label>
    <skos:prefLabel>Land used for aquaculture</skos:prefLabel>
    <dct:title>Land used for aquaculture</dct:title>
    <skos:definition>Land used for aquaculture facilities and fish-farming activities. Aquaculture refers to the farming of aquatic organisms: fish, molluscs, crustaceans, aquatic plants, crocodiles, alligators, turtles and amphibians. Farming implying some form of intervention in the rearing process to enhance production, such as regular stocking, feeding, protection from predators, etc. Land used for aquaculture facilities and fish-farming activities includes housing facilities for breeding, nursing and rearing seed of fish, invertebrates or aquatic plants to fry, fingerling or juvenile stages.</skos:definition>
    <dct:description>Land used for aquaculture facilities and fish-farming activities. Aquaculture refers to the farming of aquatic organisms: fish, molluscs, crustaceans, aquatic plants, crocodiles, alligators, turtles and amphibians. Farming implying some form of intervention in the rearing process to enhance production, such as regular stocking, feeding, protection from predators, etc. Land used for aquaculture facilities and fish-farming activities includes housing facilities for breeding, nursing and rearing seed of fish, invertebrates or aquatic plants to fry, fingerling or juvenile stages.</dct:description>
    <rdfs:comment>Land used for aquaculture facilities and fish-farming activities. Aquaculture refers to the farming of aquatic organisms: fish, molluscs, crustaceans, aquatic plants, crocodiles, alligators, turtles and amphibians. Farming implying some form of intervention in the rearing process to enhance production, such as regular stocking, feeding, protection from predators, etc. Land used for aquaculture facilities and fish-farming activities includes housing facilities for breeding, nursing and rearing seed of fish, invertebrates or aquatic plants to fry, fingerling or juvenile stages.</rdfs:comment>
    <skos:inScheme rdf:resource="http://data.landportal.info/vocabulary/25"/>
    <rdfs:seeAlso rdf:resource="https://landportal.org/book/indicator/fao-6762-5110"/>
  </rdf:Description>

</rdf:RDF>