<?xml version="1.0" encoding="UTF-8"?>
<rdf:RDF xmlns:rdf="http://www.w3.org/1999/02/22-rdf-syntax-ns#"
  xmlns:dct="http://purl.org/dc/terms/"
  xmlns:schema="http://schema.org/"
  xmlns:skos="http://www.w3.org/2004/02/skos/core#"
  xmlns:sdmx-attribute="http://purl.org/linked-data/sdmx/2009/attribute#"
  xmlns:rdfs="http://www.w3.org/2000/01/rdf-schema#">

  <rdf:Description rdf:about="http://data.landportal.info/indicator/FAO-6767-5110">
    <rdf:type rdf:resource="http://www.w3.org/2004/02/skos/core#Concept"/>
    <rdf:type rdf:resource="http://purl.org/weso/ontology/computex#Indicator"/>
    <dct:subject rdf:resource="http://data.landportal.info/voc/landvoc/overarching-category/OA-USE"/>
    <schema:about rdf:resource="http://data.landportal.info/voc/landvoc/overarching-category/OA-USE"/>
    <dct:identifier>FAO-6767-5110</dct:identifier>
    <skos:notation>FAO-6767-5110</skos:notation>
    <dct:source rdf:resource="http://data.landportal.info/dataset/FAO-LU"/>
    <sdmx-attribute:unitMeasure>1'000 Ha</sdmx-attribute:unitMeasure>
    <rdfs:label>Inland waters used for aquac. or holding facilities</rdfs:label>
    <skos:prefLabel>Inland waters used for aquac. or holding facilities</skos:prefLabel>
    <dct:title>Inland waters used for aquac. or holding facilities</dct:title>
    <skos:definition>Inland water areas that are used for aquaculture facilities including supporting facilities. Aquaculture facilities include enclosures and pens (water areas confined by net, mesh and other barriers allowing uncontrolled water interchange), cages (open or covered enclosed structure constructed with net, mesh or any porous materials allowing natural water interchange), barrages (semi-permanent or seasonal enclosures formed by impervious man-made barriers and appropriate natural features) and rafts, ropes and stakes (raft, long lines or stakes used to culture shellfish and seaweeds).</skos:definition>
    <dct:description>Inland water areas that are used for aquaculture facilities including supporting facilities. Aquaculture facilities include enclosures and pens (water areas confined by net, mesh and other barriers allowing uncontrolled water interchange), cages (open or covered enclosed structure constructed with net, mesh or any porous materials allowing natural water interchange), barrages (semi-permanent or seasonal enclosures formed by impervious man-made barriers and appropriate natural features) and rafts, ropes and stakes (raft, long lines or stakes used to culture shellfish and seaweeds).</dct:description>
    <rdfs:comment>Inland water areas that are used for aquaculture facilities including supporting facilities. Aquaculture facilities include enclosures and pens (water areas confined by net, mesh and other barriers allowing uncontrolled water interchange), cages (open or covered enclosed structure constructed with net, mesh or any porous materials allowing natural water interchange), barrages (semi-permanent or seasonal enclosures formed by impervious man-made barriers and appropriate natural features) and rafts, ropes and stakes (raft, long lines or stakes used to culture shellfish and seaweeds).</rdfs:comment>
    <skos:inScheme rdf:resource="http://data.landportal.info/vocabulary/25"/>
    <rdfs:seeAlso rdf:resource="https://landportal.org/book/indicator/fao-6767-5110"/>
  </rdf:Description>

</rdf:RDF>