<?xml version="1.0" encoding="UTF-8"?>
<rdf:RDF xmlns:rdf="http://www.w3.org/1999/02/22-rdf-syntax-ns#"
  xmlns:dct="http://purl.org/dc/terms/"
  xmlns:schema="http://schema.org/"
  xmlns:skos="http://www.w3.org/2004/02/skos/core#"
  xmlns:sdmx-attribute="http://purl.org/linked-data/sdmx/2009/attribute#"
  xmlns:rdfs="http://www.w3.org/2000/01/rdf-schema#">

  <rdf:Description rdf:about="http://data.landportal.info/indicator/TI-GCB-GPCL">
    <rdf:type rdf:resource="http://www.w3.org/2004/02/skos/core#Concept"/>
    <rdf:type rdf:resource="http://purl.org/weso/ontology/computex#Indicator"/>
    <dct:subject rdf:resource="http://aims.fao.org/aos/agrovoc/c_28663"/>
    <dct:subject rdf:resource="http://data.landportal.info/voc/landvoc/theme/T-INST"/>
    <schema:about rdf:resource="http://aims.fao.org/aos/agrovoc/c_28663"/>
    <schema:about rdf:resource="http://data.landportal.info/voc/landvoc/theme/T-INST"/>
    <dct:identifier>TI-GCB-GPCL</dct:identifier>
    <skos:notation>TI-GCB-GPCL</skos:notation>
    <dct:source rdf:resource="http://data.landportal.info/dataset/TI-GCB"/>
    <sdmx-attribute:unitMeasure>Percentage (%)</sdmx-attribute:unitMeasure>
    <rdfs:label>Perception of &quot;grand&quot; or political corruption in land matters</rdfs:label>
    <skos:prefLabel>Perception of &quot;grand&quot; or political corruption in land matters</skos:prefLabel>
    <dct:title>Perception of &quot;grand&quot; or political corruption in land matters</dct:title>
    <skos:definition>This indicator measures respondent's perception about &quot;grand&quot; or political corruption in land matters. In particuar, the 2009 round of the Global Corruption Barometer included the following question: &quot;How serious do you think the problem of grand or political corruption in land matters is in this country?&quot; Possible answer were the followings: - Not a problem at all - Moderate - Average - Serious - Very serious problem - Don’t know/ No answer (NA) We used the weights provided in the original dataset provided by TI and calculated the weighted proportion of repondants chosing each answer, by country. For more information around the TI's GCB please visit: https://www.transparency.org/news/feature/global_corruption_barometer_ci...</skos:definition>
    <dct:description>This indicator measures respondent's perception about &quot;grand&quot; or political corruption in land matters. In particuar, the 2009 round of the Global Corruption Barometer included the following question: &quot;How serious do you think the problem of grand or political corruption in land matters is in this country?&quot; Possible answer were the followings: - Not a problem at all - Moderate - Average - Serious - Very serious problem - Don’t know/ No answer (NA) We used the weights provided in the original dataset provided by TI and calculated the weighted proportion of repondants chosing each answer, by country. For more information around the TI's GCB please visit: https://www.transparency.org/news/feature/global_corruption_barometer_ci...</dct:description>
    <rdfs:comment>This indicator measures respondent's perception about &quot;grand&quot; or political corruption in land matters. In particuar, the 2009 round of the Global Corruption Barometer included the following question: &quot;How serious do you think the problem of grand or political corruption in land matters is in this country?&quot; Possible answer were the followings: - Not a problem at all - Moderate - Average - Serious - Very serious problem - Don’t know/ No answer (NA) We used the weights provided in the original dataset provided by TI and calculated the weighted proportion of repondants chosing each answer, by country. For more information around the TI's GCB please visit: https://www.transparency.org/news/feature/global_corruption_barometer_ci...</rdfs:comment>
    <skos:inScheme rdf:resource="http://data.landportal.info/vocabulary/25"/>
    <rdfs:seeAlso rdf:resource="https://landportal.org/book/indicator/ti-gcb-gpcl"/>
  </rdf:Description>

</rdf:RDF>