<?xml version="1.0" encoding="UTF-8"?>
<rdf:RDF xmlns:rdf="http://www.w3.org/1999/02/22-rdf-syntax-ns#"
  xmlns:dct="http://purl.org/dc/terms/"
  xmlns:skos="http://www.w3.org/2004/02/skos/core#"
  xmlns:schema="http://schema.org/"
  xmlns:sdmx-attribute="http://purl.org/linked-data/sdmx/2009/attribute#"
  xmlns:rdfs="http://www.w3.org/2000/01/rdf-schema#">

  <rdf:Description rdf:about="http://data.landportal.info/indicator/IUCN-BCB-S.JOBS">
    <rdf:type rdf:resource="http://www.w3.org/2004/02/skos/core#Concept"/>
    <rdf:type rdf:resource="http://purl.org/weso/ontology/computex#Indicator"/>
    <dct:identifier>IUCN-BCB-S.JOBS</dct:identifier>
    <skos:notation>IUCN-BCB-S.JOBS</skos:notation>
    <dct:source rdf:resource="http://data.landportal.info/dataset/IUCN-BCB"/>
    <dct:subject rdf:resource="http://data.landportal.info/voc/landvoc/theme/T-FLR"/>
    <dct:subject rdf:resource="http://data.landportal.info/voc/landvoc/theme/T-SOCEC"/>
    <schema:about rdf:resource="http://data.landportal.info/voc/landvoc/theme/T-FLR"/>
    <schema:about rdf:resource="http://data.landportal.info/voc/landvoc/theme/T-SOCEC"/>
    <sdmx-attribute:unitMeasure>Number of jobs created</sdmx-attribute:unitMeasure>
    <rdfs:label>Number of jobs created resulting from FLR activities included under Bonn Challenge Commitment</rdfs:label>
    <skos:prefLabel>Number of jobs created resulting from FLR activities included under Bonn Challenge Commitment</skos:prefLabel>
    <dct:title>Number of jobs created resulting from FLR activities included under Bonn Challenge Commitment</dct:title>
    <skos:definition>This indicator reflects one of the socioeconomic impacts of FLR activities under the Bonn Challenge. In particular, it measures the number of jobs created resulting from FLR activities included under Bonn Challenge Commitment For more information, please visit the Bonn Challenge Barometer.</skos:definition>
    <dct:description>This indicator reflects one of the socioeconomic impacts of FLR activities under the Bonn Challenge. In particular, it measures the number of jobs created resulting from FLR activities included under Bonn Challenge Commitment For more information, please visit the Bonn Challenge Barometer.</dct:description>
    <rdfs:comment>This indicator reflects one of the socioeconomic impacts of FLR activities under the Bonn Challenge. In particular, it measures the number of jobs created resulting from FLR activities included under Bonn Challenge Commitment For more information, please visit the Bonn Challenge Barometer.</rdfs:comment>
    <skos:inScheme rdf:resource="http://data.landportal.info/vocabulary/25"/>
    <rdfs:seeAlso rdf:resource="https://landportal.org/book/indicator/iucn-bcb-sjobs"/>
  </rdf:Description>

</rdf:RDF>