<?xml version="1.0" encoding="UTF-8"?>
<rdf:RDF xmlns:rdf="http://www.w3.org/1999/02/22-rdf-syntax-ns#"
  xmlns:dct="http://purl.org/dc/terms/"
  xmlns:schema="http://schema.org/"
  xmlns:skos="http://www.w3.org/2004/02/skos/core#"
  xmlns:rdfs="http://www.w3.org/2000/01/rdf-schema#">

  <rdf:Description rdf:about="http://data.landportal.info/dataset/UN-SDG_15.2.1">
    <rdf:type rdf:resource="http://www.w3.org/2004/02/skos/core#Concept"/>
    <rdf:type rdf:resource="http://purl.org/linked-data/cube#DataSet"/>
    <rdf:type rdf:resource="http://www.w3.org/ns/dcat#Dataset"/>
    <dct:license rdf:resource="http://purl.org/NET/rdflicense/allrightsreserved"/>
    <schema:license rdf:resource="http://purl.org/NET/rdflicense/allrightsreserved"/>
    <dct:subject rdf:resource="http://data.landportal.info/voc/landvoc/theme/T-FLR"/>
    <dct:subject rdf:resource="http://data.landportal.info/voc/landvoc/theme/T-FOREST"/>
    <dct:subject rdf:resource="http://data.landportal.info/voc/landvoc/theme/T-ENVIR"/>
    <schema:about rdf:resource="http://data.landportal.info/voc/landvoc/theme/T-FLR"/>
    <schema:about rdf:resource="http://data.landportal.info/voc/landvoc/theme/T-FOREST"/>
    <schema:about rdf:resource="http://data.landportal.info/voc/landvoc/theme/T-ENVIR"/>
    <dct:publisher rdf:resource="http://data.landportal.info/organization/e82f9624-3a20-4f31-a61f-861982f6f1c5"/>
    <schema:image rdf:resource="https://landportal.org/sites/landportal.org/files/2019/08/sdg15.2.1.png"/>
    <schema:logo rdf:resource="https://landportal.org/sites/landportal.org/files/2019/08/sdg15.2.1.png"/>
    <dct:identifier>UN-SDG_15.2.1</dct:identifier>
    <skos:notation>UN-SDG_15.2.1</skos:notation>
    <skos:prefLabel>SDG 15.2.1 - Progress towards sustainable forest management</skos:prefLabel>
    <rdfs:label>SDG 15.2.1 - Progress towards sustainable forest management</rdfs:label>
    <dct:title>SDG 15.2.1 - Progress towards sustainable forest management</dct:title>
    <skos:definition>The data included in this dataset reflects indicator 15.2.1 of the Sustainable Development Goals (SDGs), which measures the progresses towards sustainable forest management. This indicator is under &quot;Goal 15: Life on Land&quot; of the SDGs and it refers to Target 15.2, which focuses on sustainable management of forests: By 2020, promote the implementation of sustainable management of all types of forests, halt deforestation, restore degraded forests and substantially increase afforestation and reforestation globally. This indicator is currently classified as Tier I. Food and Agriculture Organization of the United Nations (FAO) is the Custodian agency for this indicator and official metadata are available at SDG UN Metadata website. Please note that according to their official formulation, several SDGs indicators needs to be disaggregated, therefore the related datasets that appear on our website might contain more than one data series for a given SDGs indicator. In particular: SDG indicator 15.2.1 is composed of five sub-indicators that measure progress towards all dimensions of sustainable forestmanagement. The environmental values of forests are covered by three sub-indicators focused on the extension of forest area, biomass within the forest area and protection and maintenance of biological diversity, and of natural and associated cultural resources. Social and economic values of forests are reconciled with environmental values through sustainable management plans. The subindicator provides further qualification to the management of forest areas, by assessing areas which are independently verified for compliance with a set of national or international standards. The SDG indicator 15.2.1 is composed of five sub-indicators: Forest area annual net change rate Above-ground biomass stock in forest Proportion of forest area located within legally established protect areas Proportion of forest area under a long term forest management plan Forest area under an independently verified forest management certification scheme</skos:definition>
    <dct:description>The data included in this dataset reflects indicator 15.2.1 of the Sustainable Development Goals (SDGs), which measures the progresses towards sustainable forest management. This indicator is under &quot;Goal 15: Life on Land&quot; of the SDGs and it refers to Target 15.2, which focuses on sustainable management of forests: By 2020, promote the implementation of sustainable management of all types of forests, halt deforestation, restore degraded forests and substantially increase afforestation and reforestation globally. This indicator is currently classified as Tier I. Food and Agriculture Organization of the United Nations (FAO) is the Custodian agency for this indicator and official metadata are available at SDG UN Metadata website. Please note that according to their official formulation, several SDGs indicators needs to be disaggregated, therefore the related datasets that appear on our website might contain more than one data series for a given SDGs indicator. In particular: SDG indicator 15.2.1 is composed of five sub-indicators that measure progress towards all dimensions of sustainable forestmanagement. The environmental values of forests are covered by three sub-indicators focused on the extension of forest area, biomass within the forest area and protection and maintenance of biological diversity, and of natural and associated cultural resources. Social and economic values of forests are reconciled with environmental values through sustainable management plans. The subindicator provides further qualification to the management of forest areas, by assessing areas which are independently verified for compliance with a set of national or international standards. The SDG indicator 15.2.1 is composed of five sub-indicators: Forest area annual net change rate Above-ground biomass stock in forest Proportion of forest area located within legally established protect areas Proportion of forest area under a long term forest management plan Forest area under an independently verified forest management certification scheme</dct:description>
    <rdfs:comment>The data included in this dataset reflects indicator 15.2.1 of the Sustainable Development Goals (SDGs), which measures the progresses towards sustainable forest management. This indicator is under &quot;Goal 15: Life on Land&quot; of the SDGs and it refers to Target 15.2, which focuses on sustainable management of forests: By 2020, promote the implementation of sustainable management of all types of forests, halt deforestation, restore degraded forests and substantially increase afforestation and reforestation globally. This indicator is currently classified as Tier I. Food and Agriculture Organization of the United Nations (FAO) is the Custodian agency for this indicator and official metadata are available at SDG UN Metadata website. Please note that according to their official formulation, several SDGs indicators needs to be disaggregated, therefore the related datasets that appear on our website might contain more than one data series for a given SDGs indicator. In particular: SDG indicator 15.2.1 is composed of five sub-indicators that measure progress towards all dimensions of sustainable forestmanagement. The environmental values of forests are covered by three sub-indicators focused on the extension of forest area, biomass within the forest area and protection and maintenance of biological diversity, and of natural and associated cultural resources. Social and economic values of forests are reconciled with environmental values through sustainable management plans. The subindicator provides further qualification to the management of forest areas, by assessing areas which are independently verified for compliance with a set of national or international standards. The SDG indicator 15.2.1 is composed of five sub-indicators: Forest area annual net change rate Above-ground biomass stock in forest Proportion of forest area located within legally established protect areas Proportion of forest area under a long term forest management plan Forest area under an independently verified forest management certification scheme</rdfs:comment>
    <skos:inScheme rdf:resource="http://data.landportal.info/vocabulary/24"/>
    <rdfs:seeAlso rdf:resource="https://landportal.org/book/dataset/un-sdg1521"/>
  </rdf:Description>

</rdf:RDF>