<?xml version="1.0" encoding="UTF-8"?>
<rdf:RDF xmlns:rdf="http://www.w3.org/1999/02/22-rdf-syntax-ns#"
  xmlns:dct="http://purl.org/dc/terms/"
  xmlns:schema="http://schema.org/"
  xmlns:skos="http://www.w3.org/2004/02/skos/core#"
  xmlns:sdmx-attribute="http://purl.org/linked-data/sdmx/2009/attribute#"
  xmlns:rdfs="http://www.w3.org/2000/01/rdf-schema#">

  <rdf:Description rdf:about="http://data.landportal.info/indicator/LM-N13">
    <rdf:type rdf:resource="http://www.w3.org/2004/02/skos/core#Concept"/>
    <rdf:type rdf:resource="http://purl.org/weso/ontology/computex#Indicator"/>
    <dct:subject rdf:resource="http://aims.fao.org/aos/agrovoc/c_89d3dcbb"/>
    <dct:subject rdf:resource="http://aims.fao.org/aos/agrovoc/c_666dbc26"/>
    <dct:subject rdf:resource="http://aims.fao.org/aos/agrovoc/c_9a4f48b4"/>
    <dct:subject rdf:resource="http://data.landportal.info/voc/landvoc/theme/T-INVEST"/>
    <schema:about rdf:resource="http://aims.fao.org/aos/agrovoc/c_89d3dcbb"/>
    <schema:about rdf:resource="http://aims.fao.org/aos/agrovoc/c_666dbc26"/>
    <schema:about rdf:resource="http://aims.fao.org/aos/agrovoc/c_9a4f48b4"/>
    <schema:about rdf:resource="http://data.landportal.info/voc/landvoc/theme/T-INVEST"/>
    <dct:identifier>LM-N13</dct:identifier>
    <skos:notation>LM-N13</skos:notation>
    <dct:source rdf:resource="http://data.landportal.info/dataset/LM-LANDMATRIX"/>
    <sdmx-attribute:unitMeasure>Number</sdmx-attribute:unitMeasure>
    <rdfs:label>Total Number of Deals of Unknown Topic</rdfs:label>
    <skos:prefLabel>Total Number of Deals of Unknown Topic</skos:prefLabel>
    <dct:title>Total Number of Deals of Unknown Topic</dct:title>
    <skos:definition>Total number of deals having as main object purposes related to an Unknown Topic, in a given country over the period 2000-2015. A &quot;deal&quot; is referred to as an intended, concluded or failed attempt to acquire at least 200 Ha of land through purchase, lease or concession. It can be compared to the Total Number of Deals.</skos:definition>
    <dct:description>Total number of deals having as main object purposes related to an Unknown Topic, in a given country over the period 2000-2015. A &quot;deal&quot; is referred to as an intended, concluded or failed attempt to acquire at least 200 Ha of land through purchase, lease or concession. It can be compared to the Total Number of Deals.</dct:description>
    <rdfs:comment>Total number of deals having as main object purposes related to an Unknown Topic, in a given country over the period 2000-2015. A &quot;deal&quot; is referred to as an intended, concluded or failed attempt to acquire at least 200 Ha of land through purchase, lease or concession. It can be compared to the Total Number of Deals.</rdfs:comment>
    <skos:inScheme rdf:resource="http://data.landportal.info/vocabulary/25"/>
    <rdfs:seeAlso rdf:resource="https://landportal.org/book/indicators/indlm8"/>
  </rdf:Description>

</rdf:RDF>