<?xml version="1.0" encoding="UTF-8"?>
<rdf:RDF xmlns:rdf="http://www.w3.org/1999/02/22-rdf-syntax-ns#"
  xmlns:dct="http://purl.org/dc/terms/"
  xmlns:schema="http://schema.org/"
  xmlns:skos="http://www.w3.org/2004/02/skos/core#"
  xmlns:sdmx-attribute="http://purl.org/linked-data/sdmx/2009/attribute#"
  xmlns:rdfs="http://www.w3.org/2000/01/rdf-schema#">

  <rdf:Description rdf:about="http://data.landportal.info/indicator/LM-N16">
    <rdf:type rdf:resource="http://www.w3.org/2004/02/skos/core#Concept"/>
    <rdf:type rdf:resource="http://purl.org/weso/ontology/computex#Indicator"/>
    <dct:subject rdf:resource="http://aims.fao.org/aos/agrovoc/c_203"/>
    <dct:subject rdf:resource="http://aims.fao.org/aos/agrovoc/c_89d3dcbb"/>
    <dct:subject rdf:resource="http://aims.fao.org/aos/agrovoc/c_666dbc26"/>
    <dct:subject rdf:resource="http://aims.fao.org/aos/agrovoc/c_9a4f48b4"/>
    <dct:subject rdf:resource="http://data.landportal.info/voc/landvoc/theme/T-INVEST"/>
    <schema:about rdf:resource="http://aims.fao.org/aos/agrovoc/c_203"/>
    <schema:about rdf:resource="http://aims.fao.org/aos/agrovoc/c_89d3dcbb"/>
    <schema:about rdf:resource="http://aims.fao.org/aos/agrovoc/c_666dbc26"/>
    <schema:about rdf:resource="http://aims.fao.org/aos/agrovoc/c_9a4f48b4"/>
    <schema:about rdf:resource="http://data.landportal.info/voc/landvoc/theme/T-INVEST"/>
    <dct:identifier>LM-N16</dct:identifier>
    <skos:notation>LM-N16</skos:notation>
    <dct:source rdf:resource="http://data.landportal.info/dataset/LM-LANDMATRIX"/>
    <sdmx-attribute:unitMeasure>Number</sdmx-attribute:unitMeasure>
    <rdfs:label>Total number of livestock (Agriculture) deals</rdfs:label>
    <skos:prefLabel>Total number of livestock (Agriculture) deals</skos:prefLabel>
    <dct:title>Total number of livestock (Agriculture) deals</dct:title>
    <skos:definition>Total number of livestock (Agriculture) deals in a gven country over the overall time period 2000-2015. A &quot;deal&quot; is referred to as an intended, concluded or failed attempt to acquire at least 200 Ha of land through purchase, lease or concession. For more information, please see: http://www.landmatrix.org/en/about/.</skos:definition>
    <dct:description>Total number of livestock (Agriculture) deals in a gven country over the overall time period 2000-2015. A &quot;deal&quot; is referred to as an intended, concluded or failed attempt to acquire at least 200 Ha of land through purchase, lease or concession. For more information, please see: http://www.landmatrix.org/en/about/.</dct:description>
    <rdfs:comment>Total number of livestock (Agriculture) deals in a gven country over the overall time period 2000-2015. A &quot;deal&quot; is referred to as an intended, concluded or failed attempt to acquire at least 200 Ha of land through purchase, lease or concession. For more information, please see: http://www.landmatrix.org/en/about/.</rdfs:comment>
    <skos:inScheme rdf:resource="http://data.landportal.info/vocabulary/25"/>
    <rdfs:seeAlso rdf:resource="https://landportal.org/book/indicators/lm-n16"/>
  </rdf:Description>

</rdf:RDF>