<?xml version="1.0" encoding="UTF-8"?>
<rdf:RDF xmlns:rdf="http://www.w3.org/1999/02/22-rdf-syntax-ns#"
  xmlns:dct="http://purl.org/dc/terms/"
  xmlns:schema="http://schema.org/"
  xmlns:skos="http://www.w3.org/2004/02/skos/core#"
  xmlns:sdmx-attribute="http://purl.org/linked-data/sdmx/2009/attribute#"
  xmlns:rdfs="http://www.w3.org/2000/01/rdf-schema#">

  <rdf:Description rdf:about="http://data.landportal.info/indicator/LM-N3">
    <rdf:type rdf:resource="http://www.w3.org/2004/02/skos/core#Concept"/>
    <rdf:type rdf:resource="http://purl.org/weso/ontology/computex#Indicator"/>
    <dct:subject rdf:resource="http://aims.fao.org/aos/agrovoc/c_89d3dcbb"/>
    <dct:subject rdf:resource="http://aims.fao.org/aos/agrovoc/c_666dbc26"/>
    <dct:subject rdf:resource="http://aims.fao.org/aos/agrovoc/c_9a4f48b4"/>
    <dct:subject rdf:resource="http://data.landportal.info/voc/landvoc/theme/T-INVEST"/>
    <schema:about rdf:resource="http://aims.fao.org/aos/agrovoc/c_89d3dcbb"/>
    <schema:about rdf:resource="http://aims.fao.org/aos/agrovoc/c_666dbc26"/>
    <schema:about rdf:resource="http://aims.fao.org/aos/agrovoc/c_9a4f48b4"/>
    <schema:about rdf:resource="http://data.landportal.info/voc/landvoc/theme/T-INVEST"/>
    <dct:identifier>LM-N3</dct:identifier>
    <skos:notation>LM-N3</skos:notation>
    <dct:source rdf:resource="http://data.landportal.info/dataset/LM-LANDMATRIX"/>
    <sdmx-attribute:unitMeasure>Number</sdmx-attribute:unitMeasure>
    <rdfs:label>Total Number of Intended Deals</rdfs:label>
    <skos:prefLabel>Total Number of Intended Deals</skos:prefLabel>
    <dct:title>Total Number of Intended Deals</dct:title>
    <skos:definition>Total number of Intended deals, in a gven country in a given year. A &quot;deal&quot; is referred to as an intended, concluded or failed attempt to acquire at least 200 Ha of land through purchase, lease or concession. It can be compared to the Total Number of Deals.</skos:definition>
    <dct:description>Total number of Intended deals, in a gven country in a given year. A &quot;deal&quot; is referred to as an intended, concluded or failed attempt to acquire at least 200 Ha of land through purchase, lease or concession. It can be compared to the Total Number of Deals.</dct:description>
    <rdfs:comment>Total number of Intended deals, in a gven country in a given year. A &quot;deal&quot; is referred to as an intended, concluded or failed attempt to acquire at least 200 Ha of land through purchase, lease or concession. It can be compared to the Total Number of Deals.</rdfs:comment>
    <skos:inScheme rdf:resource="http://data.landportal.info/vocabulary/25"/>
    <rdfs:seeAlso rdf:resource="https://landportal.org/book/indicators/indlm9"/>
  </rdf:Description>

</rdf:RDF>