<?xml version="1.0" encoding="UTF-8"?>
<rdf:RDF xmlns:rdf="http://www.w3.org/1999/02/22-rdf-syntax-ns#"
  xmlns:dct="http://purl.org/dc/terms/"
  xmlns:schema="http://schema.org/"
  xmlns:skos="http://www.w3.org/2004/02/skos/core#"
  xmlns:sdmx-attribute="http://purl.org/linked-data/sdmx/2009/attribute#"
  xmlns:rdfs="http://www.w3.org/2000/01/rdf-schema#">

  <rdf:Description rdf:about="http://data.landportal.info/indicator/LM-HA1">
    <rdf:type rdf:resource="http://www.w3.org/2004/02/skos/core#Concept"/>
    <rdf:type rdf:resource="http://purl.org/weso/ontology/computex#Indicator"/>
    <dct:subject rdf:resource="http://aims.fao.org/aos/agrovoc/c_89d3dcbb"/>
    <dct:subject rdf:resource="http://aims.fao.org/aos/agrovoc/c_666dbc26"/>
    <dct:subject rdf:resource="http://aims.fao.org/aos/agrovoc/c_9a4f48b4"/>
    <dct:subject rdf:resource="http://aims.fao.org/aos/agrovoc/c_4182"/>
    <dct:subject rdf:resource="http://data.landportal.info/voc/landvoc/theme/T-INVEST"/>
    <schema:about rdf:resource="http://aims.fao.org/aos/agrovoc/c_89d3dcbb"/>
    <schema:about rdf:resource="http://aims.fao.org/aos/agrovoc/c_666dbc26"/>
    <schema:about rdf:resource="http://aims.fao.org/aos/agrovoc/c_9a4f48b4"/>
    <schema:about rdf:resource="http://aims.fao.org/aos/agrovoc/c_4182"/>
    <schema:about rdf:resource="http://data.landportal.info/voc/landvoc/theme/T-INVEST"/>
    <dct:identifier>LM-HA1</dct:identifier>
    <skos:notation>LM-HA1</skos:notation>
    <dct:source rdf:resource="http://data.landportal.info/dataset/LM-LANDMATRIX"/>
    <sdmx-attribute:unitMeasure>Hectares (ha)</sdmx-attribute:unitMeasure>
    <rdfs:label>Total Hectares in deals</rdfs:label>
    <skos:prefLabel>Total Hectares in deals</skos:prefLabel>
    <dct:title>Total Hectares in deals</dct:title>
    <skos:definition>Total Area (ha) calculated as the sum of all deals, in a gven country over the period 2000-2015. A &quot;deal&quot; is referred to as an intended, concluded or failed attempt to acquire at least 200 Ha of land through purchase, lease or concession. It can be compared to the Total Number of Deals.</skos:definition>
    <dct:description>Total Area (ha) calculated as the sum of all deals, in a gven country over the period 2000-2015. A &quot;deal&quot; is referred to as an intended, concluded or failed attempt to acquire at least 200 Ha of land through purchase, lease or concession. It can be compared to the Total Number of Deals.</dct:description>
    <rdfs:comment>Total Area (ha) calculated as the sum of all deals, in a gven country over the period 2000-2015. A &quot;deal&quot; is referred to as an intended, concluded or failed attempt to acquire at least 200 Ha of land through purchase, lease or concession. It can be compared to the Total Number of Deals.</rdfs:comment>
    <skos:inScheme rdf:resource="http://data.landportal.info/vocabulary/25"/>
    <rdfs:seeAlso rdf:resource="https://landportal.org/book/indicators/indlm12"/>
  </rdf:Description>

</rdf:RDF>