<?xml version="1.0" encoding="UTF-8"?>
<rdf:RDF xmlns:rdf="http://www.w3.org/1999/02/22-rdf-syntax-ns#"
  xmlns:dct="http://purl.org/dc/terms/"
  xmlns:schema="http://schema.org/"
  xmlns:skos="http://www.w3.org/2004/02/skos/core#"
  xmlns:sdmx-attribute="http://purl.org/linked-data/sdmx/2009/attribute#"
  xmlns:rdfs="http://www.w3.org/2000/01/rdf-schema#">

  <rdf:Description rdf:about="http://data.landportal.info/indicator/WB-SG.OWN.LDAJ.FE.ZS">
    <rdf:type rdf:resource="http://www.w3.org/2004/02/skos/core#Concept"/>
    <rdf:type rdf:resource="http://purl.org/weso/ontology/computex#Indicator"/>
    <dct:subject rdf:resource="http://aims.fao.org/aos/agrovoc/c_1dfe5bfe"/>
    <dct:subject rdf:resource="http://aims.fao.org/aos/agrovoc/c_bafa787a"/>
    <dct:subject rdf:resource="http://aims.fao.org/aos/agrovoc/c_9000090"/>
    <dct:subject rdf:resource="http://data.landportal.info/voc/landvoc/theme/T-GENDER"/>
    <schema:about rdf:resource="http://aims.fao.org/aos/agrovoc/c_1dfe5bfe"/>
    <schema:about rdf:resource="http://aims.fao.org/aos/agrovoc/c_bafa787a"/>
    <schema:about rdf:resource="http://aims.fao.org/aos/agrovoc/c_9000090"/>
    <schema:about rdf:resource="http://data.landportal.info/voc/landvoc/theme/T-GENDER"/>
    <dct:identifier>WB-SG.OWN.LDAJ.FE.ZS</dct:identifier>
    <skos:notation>WB-SG.OWN.LDAJ.FE.ZS</skos:notation>
    <dct:source rdf:resource="http://data.landportal.info/dataset/WB-GENDER"/>
    <sdmx-attribute:unitMeasure>Percentage (%)</sdmx-attribute:unitMeasure>
    <rdfs:label>Women who own land both alone and jointly (% of women age 15-49)</rdfs:label>
    <skos:prefLabel>Women who own land both alone and jointly (% of women age 15-49)</skos:prefLabel>
    <dct:title>Women who own land both alone and jointly (% of women age 15-49)</dct:title>
    <skos:definition>Women who own land both alone and jointly (% of women age 15-49) is the percentage of women age 15-49 who both solely and jointly with someone else own a land which is legally registered with their name or cannot be sold without their signature. &quot;Both alone and jointly&quot; Implies a woman owns a land alone and another land jointly with someone else. Women who own land both alone and jointly is the number of women age 15-49 who say the type of lands they own are the one they own alone as well as the one they own jointly with someone else, expressed as percentage of women age 15-49 who have been interviewed and It’s derived by dividing the number of women age 15-49 who responded they both alone and jointly with someone else own a land which legally registered with their name or can’t be sold without their signature by total number of women age 15-49 who have been interviewed. ‘Ownership’ implies that the land is legally registered in the woman’s name or, since official property records do not always exist or are not maintained, the land is recognized as hers and cannot be sold without her signature or equivalent. ‘land’ includes all agricultural or non-agricultural land. Non-agricultural land refers to rural land that is not used for growing crops, and most land in urban areas.</skos:definition>
    <dct:description>Women who own land both alone and jointly (% of women age 15-49) is the percentage of women age 15-49 who both solely and jointly with someone else own a land which is legally registered with their name or cannot be sold without their signature. &quot;Both alone and jointly&quot; Implies a woman owns a land alone and another land jointly with someone else. Women who own land both alone and jointly is the number of women age 15-49 who say the type of lands they own are the one they own alone as well as the one they own jointly with someone else, expressed as percentage of women age 15-49 who have been interviewed and It’s derived by dividing the number of women age 15-49 who responded they both alone and jointly with someone else own a land which legally registered with their name or can’t be sold without their signature by total number of women age 15-49 who have been interviewed. ‘Ownership’ implies that the land is legally registered in the woman’s name or, since official property records do not always exist or are not maintained, the land is recognized as hers and cannot be sold without her signature or equivalent. ‘land’ includes all agricultural or non-agricultural land. Non-agricultural land refers to rural land that is not used for growing crops, and most land in urban areas.</dct:description>
    <rdfs:comment>Women who own land both alone and jointly (% of women age 15-49) is the percentage of women age 15-49 who both solely and jointly with someone else own a land which is legally registered with their name or cannot be sold without their signature. &quot;Both alone and jointly&quot; Implies a woman owns a land alone and another land jointly with someone else. Women who own land both alone and jointly is the number of women age 15-49 who say the type of lands they own are the one they own alone as well as the one they own jointly with someone else, expressed as percentage of women age 15-49 who have been interviewed and It’s derived by dividing the number of women age 15-49 who responded they both alone and jointly with someone else own a land which legally registered with their name or can’t be sold without their signature by total number of women age 15-49 who have been interviewed. ‘Ownership’ implies that the land is legally registered in the woman’s name or, since official property records do not always exist or are not maintained, the land is recognized as hers and cannot be sold without her signature or equivalent. ‘land’ includes all agricultural or non-agricultural land. Non-agricultural land refers to rural land that is not used for growing crops, and most land in urban areas.</rdfs:comment>
    <skos:inScheme rdf:resource="http://data.landportal.info/vocabulary/25"/>
    <rdfs:seeAlso rdf:resource="https://landportal.org/book/indicator/wb-sgownldajfezs"/>
  </rdf:Description>

</rdf:RDF>