<?xml version="1.0" encoding="UTF-8"?>
<rdf:RDF xmlns:rdf="http://www.w3.org/1999/02/22-rdf-syntax-ns#"
  xmlns:dct="http://purl.org/dc/terms/"
  xmlns:schema="http://schema.org/"
  xmlns:skos="http://www.w3.org/2004/02/skos/core#"
  xmlns:sdmx-attribute="http://purl.org/linked-data/sdmx/2009/attribute#"
  xmlns:rdfs="http://www.w3.org/2000/01/rdf-schema#">

  <rdf:Description rdf:about="http://data.landportal.info/indicator/WB-SG.OWN.LDAL.MA.ZS">
    <rdf:type rdf:resource="http://www.w3.org/2004/02/skos/core#Concept"/>
    <rdf:type rdf:resource="http://purl.org/weso/ontology/computex#Indicator"/>
    <dct:subject rdf:resource="http://aims.fao.org/aos/agrovoc/c_1dfe5bfe"/>
    <dct:subject rdf:resource="http://aims.fao.org/aos/agrovoc/c_28718"/>
    <dct:subject rdf:resource="http://data.landportal.info/voc/landvoc/theme/T-GENDER"/>
    <schema:about rdf:resource="http://aims.fao.org/aos/agrovoc/c_1dfe5bfe"/>
    <schema:about rdf:resource="http://aims.fao.org/aos/agrovoc/c_28718"/>
    <schema:about rdf:resource="http://data.landportal.info/voc/landvoc/theme/T-GENDER"/>
    <dct:identifier>WB-SG.OWN.LDAL.MA.ZS</dct:identifier>
    <skos:notation>WB-SG.OWN.LDAL.MA.ZS</skos:notation>
    <dct:source rdf:resource="http://data.landportal.info/dataset/WB-GENDER"/>
    <sdmx-attribute:unitMeasure>Percentage (%)</sdmx-attribute:unitMeasure>
    <rdfs:label>Men who own land alone (% of men)</rdfs:label>
    <skos:prefLabel>Men who own land alone (% of men)</skos:prefLabel>
    <dct:title>Men who own land alone (% of men)</dct:title>
    <skos:definition>Men who own land alone is the number of men who say the only type of land they own is the one they own alone or don't share ownership with anyone, expressed as percentage of men who have been interviewed and It’s derived by dividing the number of men who responded they alone own a land, which legally registered with their name or can’t be sold without their signature, by total number of men who have been interviewed. ‘Ownership’ implies that the land is legally registered in the man's name or, since official property records do not always exist or are not maintained, the land is recognized as his and cannot be sold without his signature or equivalent. ‘land’ includes all agricultural or non-agricultural land. Non-agricultural land refers to rural land that is not used for growing crops, and most land in urban areas.</skos:definition>
    <dct:description>Men who own land alone is the number of men who say the only type of land they own is the one they own alone or don't share ownership with anyone, expressed as percentage of men who have been interviewed and It’s derived by dividing the number of men who responded they alone own a land, which legally registered with their name or can’t be sold without their signature, by total number of men who have been interviewed. ‘Ownership’ implies that the land is legally registered in the man's name or, since official property records do not always exist or are not maintained, the land is recognized as his and cannot be sold without his signature or equivalent. ‘land’ includes all agricultural or non-agricultural land. Non-agricultural land refers to rural land that is not used for growing crops, and most land in urban areas.</dct:description>
    <rdfs:comment>Men who own land alone is the number of men who say the only type of land they own is the one they own alone or don't share ownership with anyone, expressed as percentage of men who have been interviewed and It’s derived by dividing the number of men who responded they alone own a land, which legally registered with their name or can’t be sold without their signature, by total number of men who have been interviewed. ‘Ownership’ implies that the land is legally registered in the man's name or, since official property records do not always exist or are not maintained, the land is recognized as his and cannot be sold without his signature or equivalent. ‘land’ includes all agricultural or non-agricultural land. Non-agricultural land refers to rural land that is not used for growing crops, and most land in urban areas.</rdfs:comment>
    <skos:inScheme rdf:resource="http://data.landportal.info/vocabulary/25"/>
    <rdfs:seeAlso rdf:resource="https://landportal.org/book/indicator/wb-sgownldalmazs"/>
  </rdf:Description>

</rdf:RDF>