<?xml version="1.0" encoding="UTF-8"?>
<rdf:RDF xmlns:rdf="http://www.w3.org/1999/02/22-rdf-syntax-ns#"
  xmlns:dct="http://purl.org/dc/terms/"
  xmlns:schema="http://schema.org/"
  xmlns:skos="http://www.w3.org/2004/02/skos/core#"
  xmlns:sdmx-attribute="http://purl.org/linked-data/sdmx/2009/attribute#"
  xmlns:rdfs="http://www.w3.org/2000/01/rdf-schema#">

  <rdf:Description rdf:about="http://data.landportal.info/indicator/WB-CC.EST">
    <rdf:type rdf:resource="http://www.w3.org/2004/02/skos/core#Concept"/>
    <rdf:type rdf:resource="http://purl.org/weso/ontology/computex#Indicator"/>
    <dct:subject rdf:resource="http://aims.fao.org/aos/agrovoc/c_28663"/>
    <dct:subject rdf:resource="http://aims.fao.org/aos/agrovoc/c_9000091"/>
    <dct:subject rdf:resource="http://aims.fao.org/aos/agrovoc/c_aca7ac6d"/>
    <dct:subject rdf:resource="http://data.landportal.info/voc/landvoc/theme/T-SOCEC"/>
    <schema:about rdf:resource="http://aims.fao.org/aos/agrovoc/c_28663"/>
    <schema:about rdf:resource="http://aims.fao.org/aos/agrovoc/c_9000091"/>
    <schema:about rdf:resource="http://aims.fao.org/aos/agrovoc/c_aca7ac6d"/>
    <schema:about rdf:resource="http://data.landportal.info/voc/landvoc/theme/T-SOCEC"/>
    <dct:identifier>WB-CC.EST</dct:identifier>
    <skos:notation>WB-CC.EST</skos:notation>
    <dct:source rdf:resource="http://data.landportal.info/dataset/WB-WGI"/>
    <sdmx-attribute:unitMeasure>Index (-2.5; 2.5)</sdmx-attribute:unitMeasure>
    <rdfs:label>Control of Corruption</rdfs:label>
    <skos:prefLabel>Control of Corruption</skos:prefLabel>
    <dct:title>Control of Corruption</dct:title>
    <skos:definition>Control of corruption captures perceptions of the extent to which public power is exercised for private gain, including both petty and grand forms of corruption, as well as &quot;capture&quot; of the state by elites and private interests. This indicator is part of the Worldwide Governance Indicators.</skos:definition>
    <dct:description>Control of corruption captures perceptions of the extent to which public power is exercised for private gain, including both petty and grand forms of corruption, as well as &quot;capture&quot; of the state by elites and private interests. This indicator is part of the Worldwide Governance Indicators.</dct:description>
    <rdfs:comment>Control of corruption captures perceptions of the extent to which public power is exercised for private gain, including both petty and grand forms of corruption, as well as &quot;capture&quot; of the state by elites and private interests. This indicator is part of the Worldwide Governance Indicators.</rdfs:comment>
    <skos:inScheme rdf:resource="http://data.landportal.info/vocabulary/25"/>
    <rdfs:seeAlso rdf:resource="https://landportal.org/book/indicators/wb-ccest"/>
  </rdf:Description>

</rdf:RDF>