<?xml version="1.0" encoding="UTF-8"?>
<rdf:RDF xmlns:rdf="http://www.w3.org/1999/02/22-rdf-syntax-ns#"
  xmlns:dct="http://purl.org/dc/terms/"
  xmlns:skos="http://www.w3.org/2004/02/skos/core#"
  xmlns:schema="http://schema.org/"
  xmlns:rdfs="http://www.w3.org/2000/01/rdf-schema#">

  <rdf:Description rdf:about="http://data.landportal.info/dataset/AFRB-SURV">
    <rdf:type rdf:resource="http://www.w3.org/2004/02/skos/core#Concept"/>
    <rdf:type rdf:resource="http://purl.org/linked-data/cube#DataSet"/>
    <rdf:type rdf:resource="http://www.w3.org/ns/dcat#Dataset"/>
    <dct:identifier>AFRB-SURV</dct:identifier>
    <skos:notation>AFRB-SURV</skos:notation>
    <dct:publisher rdf:resource="http://data.landportal.info/organization/cd6c218b-3242-49ff-95cf-11a61137b380"/>
    <dct:subject rdf:resource="http://data.landportal.info/voc/landvoc/overarching-category/OA-LAW"/>
    <dct:subject rdf:resource="http://data.landportal.info/voc/landvoc/overarching-category/OA-USE"/>
    <dct:subject rdf:resource="http://data.landportal.info/voc/landvoc/theme/T-CORRUPT"/>
    <dct:subject rdf:resource="http://data.landportal.info/voc/landvoc/theme/T-GENDER"/>
    <dct:subject rdf:resource="http://data.landportal.info/voc/landvoc/theme/T-INVEST"/>
    <dct:subject rdf:resource="http://data.landportal.info/voc/landvoc/theme/T-INST"/>
    <schema:about rdf:resource="http://data.landportal.info/voc/landvoc/overarching-category/OA-LAW"/>
    <schema:about rdf:resource="http://data.landportal.info/voc/landvoc/overarching-category/OA-USE"/>
    <schema:about rdf:resource="http://data.landportal.info/voc/landvoc/theme/T-CORRUPT"/>
    <schema:about rdf:resource="http://data.landportal.info/voc/landvoc/theme/T-GENDER"/>
    <schema:about rdf:resource="http://data.landportal.info/voc/landvoc/theme/T-INVEST"/>
    <schema:about rdf:resource="http://data.landportal.info/voc/landvoc/theme/T-INST"/>
    <schema:image rdf:resource="https://landportal.org/sites/landportal.org/files/2019/04/afro-barometer.png"/>
    <schema:logo rdf:resource="https://landportal.org/sites/landportal.org/files/2019/04/afro-barometer.png"/>
    <skos:prefLabel>Afrobarometer Survey</skos:prefLabel>
    <rdfs:label>Afrobarometer Survey</rdfs:label>
    <dct:title>Afrobarometer Survey</dct:title>
    <skos:definition>Afrobarometer is a pan-African, non-partisan research network that conducts public attitude surveys on democracy, governance, economic conditions, and related issues in more than 35 countries in Africa. Afrobarometer surveys collect and publish high-quality, reliable statistical data on Africa, which is freely available to the public. The latest round of the Afrobarometer Survey (Round 7 - 2016/2018) collected opinions and perceptions around land-related issues, including women land rights and corruption in the land sector. In particular, the selection of indicator is based on the follwing questions : Access to information: land ownership (Q18b): How likely is it that you could get the following information from government or other public institutions, or haven’t you heard enough to say? If you went to the local council to find out who owns a piece of land in your community? (Not at all likely; Not very likely; Somewhat likely; Very likely; Don’t know) Women should have equal right to land (Q38e): For each of the following statements, please tell me whether you disagree or agree: Women should have the same rights as men to own and inherit land. (Strongly disagree; Disagree; Neither agree nor disagree; Agree; Strongly agree; Don’t know) Ordinary person: pay bribe to register land not theirs (Q48c): In this country, how likely do you think it is that an ordinary person could pay a bribe or use personal connections to get away with: Registering land that does not belong to them? (Not at all likely; Not very likely; Somewhat likely; Very likely; Don’t know) Rich person pay bribe to register land not theirs (Q48f): And in this country, how likely do you think it is that a rich person could pay a bribe or use personal connections to get away with: Registering land that does not belong to them? (Not at all likely; Not very likely; Somewhat likely; Very likely; Refused; Don’t know) Women and men have equal chance to own/inherit land (Q77d): For each of the following statements, please tell me whether you disagree or agree, or haven’t you heard enough to say? In our country today, women and men have equal opportunities to own and inherit land. (Strongly disagree; Disagree; Neither agree nor disagree; Agree; Strongly agree; Don’t know) For more information on the Afrobarometer, please visit the website afrobarometer.org</skos:definition>
    <dct:description>Afrobarometer is a pan-African, non-partisan research network that conducts public attitude surveys on democracy, governance, economic conditions, and related issues in more than 35 countries in Africa. Afrobarometer surveys collect and publish high-quality, reliable statistical data on Africa, which is freely available to the public. The latest round of the Afrobarometer Survey (Round 7 - 2016/2018) collected opinions and perceptions around land-related issues, including women land rights and corruption in the land sector. In particular, the selection of indicator is based on the follwing questions : Access to information: land ownership (Q18b): How likely is it that you could get the following information from government or other public institutions, or haven’t you heard enough to say? If you went to the local council to find out who owns a piece of land in your community? (Not at all likely; Not very likely; Somewhat likely; Very likely; Don’t know) Women should have equal right to land (Q38e): For each of the following statements, please tell me whether you disagree or agree: Women should have the same rights as men to own and inherit land. (Strongly disagree; Disagree; Neither agree nor disagree; Agree; Strongly agree; Don’t know) Ordinary person: pay bribe to register land not theirs (Q48c): In this country, how likely do you think it is that an ordinary person could pay a bribe or use personal connections to get away with: Registering land that does not belong to them? (Not at all likely; Not very likely; Somewhat likely; Very likely; Don’t know) Rich person pay bribe to register land not theirs (Q48f): And in this country, how likely do you think it is that a rich person could pay a bribe or use personal connections to get away with: Registering land that does not belong to them? (Not at all likely; Not very likely; Somewhat likely; Very likely; Refused; Don’t know) Women and men have equal chance to own/inherit land (Q77d): For each of the following statements, please tell me whether you disagree or agree, or haven’t you heard enough to say? In our country today, women and men have equal opportunities to own and inherit land. (Strongly disagree; Disagree; Neither agree nor disagree; Agree; Strongly agree; Don’t know) For more information on the Afrobarometer, please visit the website afrobarometer.org</dct:description>
    <rdfs:comment>Afrobarometer is a pan-African, non-partisan research network that conducts public attitude surveys on democracy, governance, economic conditions, and related issues in more than 35 countries in Africa. Afrobarometer surveys collect and publish high-quality, reliable statistical data on Africa, which is freely available to the public. The latest round of the Afrobarometer Survey (Round 7 - 2016/2018) collected opinions and perceptions around land-related issues, including women land rights and corruption in the land sector. In particular, the selection of indicator is based on the follwing questions : Access to information: land ownership (Q18b): How likely is it that you could get the following information from government or other public institutions, or haven’t you heard enough to say? If you went to the local council to find out who owns a piece of land in your community? (Not at all likely; Not very likely; Somewhat likely; Very likely; Don’t know) Women should have equal right to land (Q38e): For each of the following statements, please tell me whether you disagree or agree: Women should have the same rights as men to own and inherit land. (Strongly disagree; Disagree; Neither agree nor disagree; Agree; Strongly agree; Don’t know) Ordinary person: pay bribe to register land not theirs (Q48c): In this country, how likely do you think it is that an ordinary person could pay a bribe or use personal connections to get away with: Registering land that does not belong to them? (Not at all likely; Not very likely; Somewhat likely; Very likely; Don’t know) Rich person pay bribe to register land not theirs (Q48f): And in this country, how likely do you think it is that a rich person could pay a bribe or use personal connections to get away with: Registering land that does not belong to them? (Not at all likely; Not very likely; Somewhat likely; Very likely; Refused; Don’t know) Women and men have equal chance to own/inherit land (Q77d): For each of the following statements, please tell me whether you disagree or agree, or haven’t you heard enough to say? In our country today, women and men have equal opportunities to own and inherit land. (Strongly disagree; Disagree; Neither agree nor disagree; Agree; Strongly agree; Don’t know) For more information on the Afrobarometer, please visit the website afrobarometer.org</rdfs:comment>
    <skos:inScheme rdf:resource="http://data.landportal.info/vocabulary/24"/>
    <rdfs:seeAlso rdf:resource="https://landportal.org/book/dataset/afrb-surv"/>
  </rdf:Description>

</rdf:RDF>