<?xml version="1.0" encoding="UTF-8"?>
<rdf:RDF xmlns:rdf="http://www.w3.org/1999/02/22-rdf-syntax-ns#"
  xmlns:dct="http://purl.org/dc/terms/"
  xmlns:schema="http://schema.org/"
  xmlns:skos="http://www.w3.org/2004/02/skos/core#"
  xmlns:sdmx-attribute="http://purl.org/linked-data/sdmx/2009/attribute#"
  xmlns:rdfs="http://www.w3.org/2000/01/rdf-schema#">

  <rdf:Description rdf:about="http://data.landportal.info/indicator/UN-AG_LND_FRSTBIOPHA">
    <rdf:type rdf:resource="http://www.w3.org/2004/02/skos/core#Concept"/>
    <rdf:type rdf:resource="http://purl.org/weso/ontology/computex#Indicator"/>
    <dct:subject rdf:resource="http://data.landportal.info/voc/landvoc/theme/T-FLR"/>
    <dct:subject rdf:resource="http://data.landportal.info/voc/landvoc/theme/T-ENVIR"/>
    <schema:about rdf:resource="http://data.landportal.info/voc/landvoc/theme/T-FLR"/>
    <schema:about rdf:resource="http://data.landportal.info/voc/landvoc/theme/T-ENVIR"/>
    <dct:identifier>UN-AG_LND_FRSTBIOPHA</dct:identifier>
    <skos:notation>UN-AG_LND_FRSTBIOPHA</skos:notation>
    <dct:source rdf:resource="http://data.landportal.info/dataset/UN-SDG_15.2.1"/>
    <sdmx-attribute:unitMeasure>Tonnes per hectare</sdmx-attribute:unitMeasure>
    <rdfs:label>Above-ground biomass stock in forest</rdfs:label>
    <skos:prefLabel>Above-ground biomass stock in forest</skos:prefLabel>
    <dct:title>Above-ground biomass stock in forest</dct:title>
    <skos:definition>The data series presented here measures the above-ground biomass in forest per hectare (tonnes per hectare). This data series contributes to the measurement of SDG Indicator 15.2.1, classified as Tier I in September 2018, which is officially defined as follows: Proportion of important sites for terrestrial and freshwater biodiversity that are covered by protected areas shows temporal trends in the mean percentage of each important site for terrestrial and freshwater biodiversity (i.e., those that contribute significantly to the global persistence of biodiversity) that is covered by designated protected areas.  It is important to mention that SDG indicator 15.2.1: is composed of five sub-indicators that measure progress towards all dimensions of sustainable forest management. The environmental values of forests are covered by three sub-indicators focused on the extension of forest area, biomass within the forest area and protection and maintenance of biological diversity, and of natural and associated cultural resources. Social and economic values of forests are reconciled with environmental values through sustainable management plans. The subindicator provides further qualification to the management of forest areas, by assessing areas which are independently verified for compliance with a set of national or international standards.   The sub-indicators are: Forest area annual net change rate Above-ground biomass stock in forest Proportion of forest area located within legally established protect areas Proportion of forest area under a long term forest management plan Forest area under an independently verified forest management certification scheme According to Food and Agriculture Organization of the United Nations (FAO) -- the Custodian Agency for this indicator -- the rationale behind above-ground biomass in forest per hectare (tonnes per hectare) can be summarised as follows:  Changes in the above-ground biomass stock in forest indicate the balance between gains in biomass stock due to forest growth and losses due to wood removals, natural losses, fire, wind, pests and diseases. At country level and over a longer period, sustainable forest management would imply a stable or increasing biomass stock per hectare, while a long-term reduction of biomass stock per hectare would imply either unsustainable management of the forests and degradation or unexpected major losses due to fire, wind, pests or diseases The full official metadata for this Tier I indicator are available at UN SDG Metadata website. For more information on this data series, please visit UN SDG website.</skos:definition>
    <dct:description>The data series presented here measures the above-ground biomass in forest per hectare (tonnes per hectare). This data series contributes to the measurement of SDG Indicator 15.2.1, classified as Tier I in September 2018, which is officially defined as follows: Proportion of important sites for terrestrial and freshwater biodiversity that are covered by protected areas shows temporal trends in the mean percentage of each important site for terrestrial and freshwater biodiversity (i.e., those that contribute significantly to the global persistence of biodiversity) that is covered by designated protected areas.  It is important to mention that SDG indicator 15.2.1: is composed of five sub-indicators that measure progress towards all dimensions of sustainable forest management. The environmental values of forests are covered by three sub-indicators focused on the extension of forest area, biomass within the forest area and protection and maintenance of biological diversity, and of natural and associated cultural resources. Social and economic values of forests are reconciled with environmental values through sustainable management plans. The subindicator provides further qualification to the management of forest areas, by assessing areas which are independently verified for compliance with a set of national or international standards.   The sub-indicators are: Forest area annual net change rate Above-ground biomass stock in forest Proportion of forest area located within legally established protect areas Proportion of forest area under a long term forest management plan Forest area under an independently verified forest management certification scheme According to Food and Agriculture Organization of the United Nations (FAO) -- the Custodian Agency for this indicator -- the rationale behind above-ground biomass in forest per hectare (tonnes per hectare) can be summarised as follows:  Changes in the above-ground biomass stock in forest indicate the balance between gains in biomass stock due to forest growth and losses due to wood removals, natural losses, fire, wind, pests and diseases. At country level and over a longer period, sustainable forest management would imply a stable or increasing biomass stock per hectare, while a long-term reduction of biomass stock per hectare would imply either unsustainable management of the forests and degradation or unexpected major losses due to fire, wind, pests or diseases The full official metadata for this Tier I indicator are available at UN SDG Metadata website. For more information on this data series, please visit UN SDG website.</dct:description>
    <rdfs:comment>The data series presented here measures the above-ground biomass in forest per hectare (tonnes per hectare). This data series contributes to the measurement of SDG Indicator 15.2.1, classified as Tier I in September 2018, which is officially defined as follows: Proportion of important sites for terrestrial and freshwater biodiversity that are covered by protected areas shows temporal trends in the mean percentage of each important site for terrestrial and freshwater biodiversity (i.e., those that contribute significantly to the global persistence of biodiversity) that is covered by designated protected areas.  It is important to mention that SDG indicator 15.2.1: is composed of five sub-indicators that measure progress towards all dimensions of sustainable forest management. The environmental values of forests are covered by three sub-indicators focused on the extension of forest area, biomass within the forest area and protection and maintenance of biological diversity, and of natural and associated cultural resources. Social and economic values of forests are reconciled with environmental values through sustainable management plans. The subindicator provides further qualification to the management of forest areas, by assessing areas which are independently verified for compliance with a set of national or international standards.   The sub-indicators are: Forest area annual net change rate Above-ground biomass stock in forest Proportion of forest area located within legally established protect areas Proportion of forest area under a long term forest management plan Forest area under an independently verified forest management certification scheme According to Food and Agriculture Organization of the United Nations (FAO) -- the Custodian Agency for this indicator -- the rationale behind above-ground biomass in forest per hectare (tonnes per hectare) can be summarised as follows:  Changes in the above-ground biomass stock in forest indicate the balance between gains in biomass stock due to forest growth and losses due to wood removals, natural losses, fire, wind, pests and diseases. At country level and over a longer period, sustainable forest management would imply a stable or increasing biomass stock per hectare, while a long-term reduction of biomass stock per hectare would imply either unsustainable management of the forests and degradation or unexpected major losses due to fire, wind, pests or diseases The full official metadata for this Tier I indicator are available at UN SDG Metadata website. For more information on this data series, please visit UN SDG website.</rdfs:comment>
    <skos:inScheme rdf:resource="http://data.landportal.info/vocabulary/25"/>
    <rdfs:seeAlso rdf:resource="https://landportal.org/book/indicator/un-aglndfrstbiopha"/>
  </rdf:Description>

</rdf:RDF>