<?xml version="1.0" encoding="UTF-8"?>
<rdf:RDF xmlns:rdf="http://www.w3.org/1999/02/22-rdf-syntax-ns#"
  xmlns:dct="http://purl.org/dc/terms/"
  xmlns:schema="http://schema.org/"
  xmlns:skos="http://www.w3.org/2004/02/skos/core#"
  xmlns:sdmx-attribute="http://purl.org/linked-data/sdmx/2009/attribute#"
  xmlns:rdfs="http://www.w3.org/2000/01/rdf-schema#">

  <rdf:Description rdf:about="http://data.landportal.info/indicator/UN-AG_LND_FRSTMGT">
    <rdf:type rdf:resource="http://www.w3.org/2004/02/skos/core#Concept"/>
    <rdf:type rdf:resource="http://purl.org/weso/ontology/computex#Indicator"/>
    <dct:subject rdf:resource="http://data.landportal.info/voc/landvoc/theme/T-FLR"/>
    <dct:subject rdf:resource="http://data.landportal.info/voc/landvoc/theme/T-FOREST"/>
    <dct:subject rdf:resource="http://data.landportal.info/voc/landvoc/theme/T-ENVIR"/>
    <schema:about rdf:resource="http://data.landportal.info/voc/landvoc/theme/T-FLR"/>
    <schema:about rdf:resource="http://data.landportal.info/voc/landvoc/theme/T-FOREST"/>
    <schema:about rdf:resource="http://data.landportal.info/voc/landvoc/theme/T-ENVIR"/>
    <dct:identifier>UN-AG_LND_FRSTMGT</dct:identifier>
    <skos:notation>UN-AG_LND_FRSTMGT</skos:notation>
    <dct:source rdf:resource="http://data.landportal.info/dataset/UN-SDG_15.2.1"/>
    <sdmx-attribute:unitMeasure>Percentage (%)</sdmx-attribute:unitMeasure>
    <rdfs:label>Proportion of forest area under a long term forest management plan</rdfs:label>
    <skos:prefLabel>Proportion of forest area under a long term forest management plan</skos:prefLabel>
    <dct:title>Proportion of forest area under a long term forest management plan</dct:title>
    <skos:definition>The data series presented here measures the proportion of forest area with a long-term management plan. This data series contributes to the measurement of SDG Indicator 15.2.1, classified as Tier I in September 2018, which is officially defined as follows: Proportion of important sites for terrestrial and freshwater biodiversity that are covered by protected areas shows temporal trends in the mean percentage of each important site for terrestrial and freshwater biodiversity (i.e., those that contribute significantly to the global persistence of biodiversity) that is covered by designated protected areas.  It is important to mention that SDG indicator 15.2.1: is composed of five sub-indicators that measure progress towards all dimensions of sustainable forest management. The environmental values of forests are covered by three sub-indicators focused on the extension of forest area, biomass within the forest area and protection and maintenance of biological diversity, and of natural and associated cultural resources. Social and economic values of forests are reconciled with environmental values through sustainable management plans. The subindicator provides further qualification to the management of forest areas, by assessing areas which are independently verified for compliance with a set of national or international standards.   The sub-indicators are: Forest area annual net change rate Above-ground biomass stock in forest Proportion of forest area located within legally established protect areas Proportion of forest area under a long term forest management plan Forest area under an independently verified forest management certification scheme According to Food and Agriculture Organization of the United Nations (FAO) -- the Custodian Agency for this indicator -- the rationale behind the proportion of forest area with a long-term management plan can be summarised as follows:  The fourth sub-indicator looks at the forest area that is under a long term forest management plan. The existence of a documented forest management plan is the basis for long term and sustainable management of the forest resources for a variety of management objectives such as for wood and non-wood forest products, protection of soil and water, biodiversity conservation, social and cultural use, and a combination of two or several of these. An increasing area under forest management plan is therefore an indicator of progress towards sustainable forest management. The full official metadata for this Tier I indicator are available at UN SDG Metadata website. For more information on this data series, please visit UN SDG website.</skos:definition>
    <dct:description>The data series presented here measures the proportion of forest area with a long-term management plan. This data series contributes to the measurement of SDG Indicator 15.2.1, classified as Tier I in September 2018, which is officially defined as follows: Proportion of important sites for terrestrial and freshwater biodiversity that are covered by protected areas shows temporal trends in the mean percentage of each important site for terrestrial and freshwater biodiversity (i.e., those that contribute significantly to the global persistence of biodiversity) that is covered by designated protected areas.  It is important to mention that SDG indicator 15.2.1: is composed of five sub-indicators that measure progress towards all dimensions of sustainable forest management. The environmental values of forests are covered by three sub-indicators focused on the extension of forest area, biomass within the forest area and protection and maintenance of biological diversity, and of natural and associated cultural resources. Social and economic values of forests are reconciled with environmental values through sustainable management plans. The subindicator provides further qualification to the management of forest areas, by assessing areas which are independently verified for compliance with a set of national or international standards.   The sub-indicators are: Forest area annual net change rate Above-ground biomass stock in forest Proportion of forest area located within legally established protect areas Proportion of forest area under a long term forest management plan Forest area under an independently verified forest management certification scheme According to Food and Agriculture Organization of the United Nations (FAO) -- the Custodian Agency for this indicator -- the rationale behind the proportion of forest area with a long-term management plan can be summarised as follows:  The fourth sub-indicator looks at the forest area that is under a long term forest management plan. The existence of a documented forest management plan is the basis for long term and sustainable management of the forest resources for a variety of management objectives such as for wood and non-wood forest products, protection of soil and water, biodiversity conservation, social and cultural use, and a combination of two or several of these. An increasing area under forest management plan is therefore an indicator of progress towards sustainable forest management. The full official metadata for this Tier I indicator are available at UN SDG Metadata website. For more information on this data series, please visit UN SDG website.</dct:description>
    <rdfs:comment>The data series presented here measures the proportion of forest area with a long-term management plan. This data series contributes to the measurement of SDG Indicator 15.2.1, classified as Tier I in September 2018, which is officially defined as follows: Proportion of important sites for terrestrial and freshwater biodiversity that are covered by protected areas shows temporal trends in the mean percentage of each important site for terrestrial and freshwater biodiversity (i.e., those that contribute significantly to the global persistence of biodiversity) that is covered by designated protected areas.  It is important to mention that SDG indicator 15.2.1: is composed of five sub-indicators that measure progress towards all dimensions of sustainable forest management. The environmental values of forests are covered by three sub-indicators focused on the extension of forest area, biomass within the forest area and protection and maintenance of biological diversity, and of natural and associated cultural resources. Social and economic values of forests are reconciled with environmental values through sustainable management plans. The subindicator provides further qualification to the management of forest areas, by assessing areas which are independently verified for compliance with a set of national or international standards.   The sub-indicators are: Forest area annual net change rate Above-ground biomass stock in forest Proportion of forest area located within legally established protect areas Proportion of forest area under a long term forest management plan Forest area under an independently verified forest management certification scheme According to Food and Agriculture Organization of the United Nations (FAO) -- the Custodian Agency for this indicator -- the rationale behind the proportion of forest area with a long-term management plan can be summarised as follows:  The fourth sub-indicator looks at the forest area that is under a long term forest management plan. The existence of a documented forest management plan is the basis for long term and sustainable management of the forest resources for a variety of management objectives such as for wood and non-wood forest products, protection of soil and water, biodiversity conservation, social and cultural use, and a combination of two or several of these. An increasing area under forest management plan is therefore an indicator of progress towards sustainable forest management. The full official metadata for this Tier I indicator are available at UN SDG Metadata website. For more information on this data series, please visit UN SDG website.</rdfs:comment>
    <skos:inScheme rdf:resource="http://data.landportal.info/vocabulary/25"/>
    <rdfs:seeAlso rdf:resource="https://landportal.org/book/indicator/un-aglndfrstmgt"/>
  </rdf:Description>

</rdf:RDF>