<?xml version="1.0" encoding="UTF-8"?>
<rdf:RDF xmlns:rdf="http://www.w3.org/1999/02/22-rdf-syntax-ns#"
  xmlns:dct="http://purl.org/dc/terms/"
  xmlns:schema="http://schema.org/"
  xmlns:skos="http://www.w3.org/2004/02/skos/core#"
  xmlns:rdfs="http://www.w3.org/2000/01/rdf-schema#">

  <rdf:Description rdf:about="http://data.landportal.info/dataset/UN-SDG_15.1.2">
    <rdf:type rdf:resource="http://www.w3.org/2004/02/skos/core#Concept"/>
    <rdf:type rdf:resource="http://purl.org/linked-data/cube#DataSet"/>
    <rdf:type rdf:resource="http://www.w3.org/ns/dcat#Dataset"/>
    <dct:license rdf:resource="http://purl.org/NET/rdflicense/allrightsreserved"/>
    <schema:license rdf:resource="http://purl.org/NET/rdflicense/allrightsreserved"/>
    <dct:subject rdf:resource="http://data.landportal.info/voc/landvoc/theme/T-FLR"/>
    <dct:subject rdf:resource="http://data.landportal.info/voc/landvoc/theme/T-ENVIR"/>
    <dct:subject rdf:resource="http://data.landportal.info/voc/landvoc/theme/T-PASTOR"/>
    <schema:about rdf:resource="http://data.landportal.info/voc/landvoc/theme/T-FLR"/>
    <schema:about rdf:resource="http://data.landportal.info/voc/landvoc/theme/T-ENVIR"/>
    <schema:about rdf:resource="http://data.landportal.info/voc/landvoc/theme/T-PASTOR"/>
    <dct:publisher rdf:resource="http://data.landportal.info/organization/e82f9624-3a20-4f31-a61f-861982f6f1c5"/>
    <schema:image rdf:resource="https://landportal.org/sites/landportal.org/files/sdg15.1.2.png"/>
    <schema:logo rdf:resource="https://landportal.org/sites/landportal.org/files/sdg15.1.2.png"/>
    <dct:identifier>UN-SDG_15.1.2</dct:identifier>
    <skos:notation>UN-SDG_15.1.2</skos:notation>
    <skos:prefLabel>SDG 15.1.2 - Proportion of important sites for terrestrial and freshwater biodiversity that are covered by protected areas, by ecosystem type</skos:prefLabel>
    <rdfs:label>SDG 15.1.2 - Proportion of important sites for terrestrial and freshwater biodiversity that are covered by protected areas, by ecosystem type</rdfs:label>
    <dct:title>SDG 15.1.2 - Proportion of important sites for terrestrial and freshwater biodiversity that are covered by protected areas, by ecosystem type</dct:title>
    <skos:definition>The data included in this dataset reflects indicator 15.1.2 of the Sustainable Development Goals (SDGs), which measures the proportion of important sites for terrestrial and freshwater biodiversity that are covered by protected areas, by ecosystem type. This indicator is under &quot;Goal 15: Life on Land&quot; of the SDGs and it refers to Target 15.1, which focuses on conservation, restoration and sustainable use of ecosystems: By 2020, ensure the conservation, restoration and sustainable use of terrestrial and inland freshwater ecosystems and their services, in particular forests, wetlands, mountains and drylands, in line with obligations under international agreements. This indicator is currently classified as Tier I. Food and Agriculture Organization of the United Nations (FAO) is the Custodian agency for this indicator and official metadata are available at SDG UN Metadata website. For more information, check also this indicator's page on LandPortal SDG portfolio. Please note that according to their official formulation, several SDGs indicators needs to be disaggregated, therefore the related datasets that appear on our website might contain more than one data series for a given SDGs indicator. In particular, SDG indicator 15.1.2 is composed of two sub-indicators: Average proportion of Freshwater Key Biodiversity Areas (KBAs) covered by protected areas (%) Average proportion of Terrestrial Key Biodiversity Areas (KBAs) covered by protected areas (%)</skos:definition>
    <dct:description>The data included in this dataset reflects indicator 15.1.2 of the Sustainable Development Goals (SDGs), which measures the proportion of important sites for terrestrial and freshwater biodiversity that are covered by protected areas, by ecosystem type. This indicator is under &quot;Goal 15: Life on Land&quot; of the SDGs and it refers to Target 15.1, which focuses on conservation, restoration and sustainable use of ecosystems: By 2020, ensure the conservation, restoration and sustainable use of terrestrial and inland freshwater ecosystems and their services, in particular forests, wetlands, mountains and drylands, in line with obligations under international agreements. This indicator is currently classified as Tier I. Food and Agriculture Organization of the United Nations (FAO) is the Custodian agency for this indicator and official metadata are available at SDG UN Metadata website. For more information, check also this indicator's page on LandPortal SDG portfolio. Please note that according to their official formulation, several SDGs indicators needs to be disaggregated, therefore the related datasets that appear on our website might contain more than one data series for a given SDGs indicator. In particular, SDG indicator 15.1.2 is composed of two sub-indicators: Average proportion of Freshwater Key Biodiversity Areas (KBAs) covered by protected areas (%) Average proportion of Terrestrial Key Biodiversity Areas (KBAs) covered by protected areas (%)</dct:description>
    <rdfs:comment>The data included in this dataset reflects indicator 15.1.2 of the Sustainable Development Goals (SDGs), which measures the proportion of important sites for terrestrial and freshwater biodiversity that are covered by protected areas, by ecosystem type. This indicator is under &quot;Goal 15: Life on Land&quot; of the SDGs and it refers to Target 15.1, which focuses on conservation, restoration and sustainable use of ecosystems: By 2020, ensure the conservation, restoration and sustainable use of terrestrial and inland freshwater ecosystems and their services, in particular forests, wetlands, mountains and drylands, in line with obligations under international agreements. This indicator is currently classified as Tier I. Food and Agriculture Organization of the United Nations (FAO) is the Custodian agency for this indicator and official metadata are available at SDG UN Metadata website. For more information, check also this indicator's page on LandPortal SDG portfolio. Please note that according to their official formulation, several SDGs indicators needs to be disaggregated, therefore the related datasets that appear on our website might contain more than one data series for a given SDGs indicator. In particular, SDG indicator 15.1.2 is composed of two sub-indicators: Average proportion of Freshwater Key Biodiversity Areas (KBAs) covered by protected areas (%) Average proportion of Terrestrial Key Biodiversity Areas (KBAs) covered by protected areas (%)</rdfs:comment>
    <skos:inScheme rdf:resource="http://data.landportal.info/vocabulary/24"/>
    <rdfs:seeAlso rdf:resource="https://landportal.org/book/dataset/un-sdg1512"/>
  </rdf:Description>

</rdf:RDF>