<?xml version="1.0" encoding="UTF-8"?>
<rdf:RDF xmlns:rdf="http://www.w3.org/1999/02/22-rdf-syntax-ns#"
  xmlns:dct="http://purl.org/dc/terms/"
  xmlns:skos="http://www.w3.org/2004/02/skos/core#"
  xmlns:schema="http://schema.org/"
  xmlns:sdmx-attribute="http://purl.org/linked-data/sdmx/2009/attribute#"
  xmlns:rdfs="http://www.w3.org/2000/01/rdf-schema#">

  <rdf:Description rdf:about="http://data.landportal.info/indicator/FAO-21033-6121">
    <rdf:type rdf:resource="http://www.w3.org/2004/02/skos/core#Concept"/>
    <rdf:type rdf:resource="http://purl.org/weso/ontology/computex#Indicator"/>
    <dct:identifier>FAO-21033-6121</dct:identifier>
    <skos:notation>FAO-21033-6121</skos:notation>
    <dct:source rdf:resource="http://data.landportal.info/dataset/FAO-FS"/>
    <dct:subject rdf:resource="http://data.landportal.info/voc/landvoc/theme/T-FOOD"/>
    <dct:subject rdf:resource="http://data.landportal.info/voc/landvoc/theme/T-SOCEC"/>
    <schema:about rdf:resource="http://data.landportal.info/voc/landvoc/theme/T-FOOD"/>
    <schema:about rdf:resource="http://data.landportal.info/voc/landvoc/theme/T-SOCEC"/>
    <sdmx-attribute:unitMeasure>Percentage (3-year average)</sdmx-attribute:unitMeasure>
    <rdfs:label>Value of food imports over total merchandise exports (%) (3-year average)</rdfs:label>
    <skos:prefLabel>Value of food imports over total merchandise exports (%) (3-year average)</skos:prefLabel>
    <dct:title>Value of food imports over total merchandise exports (%) (3-year average)</dct:title>
    <skos:definition>This indicator is part of the FAO Suite of Food Security Indicators (2017) in the dimension &amp;quot;stability&amp;quot;. It is the share of the value of food (excl. fish) imports over total merchandise exports. This indicator provides a measure of vulnerability and captures the adequacy of foreign exchange reserves to pay for food imports, which has implications for national food security depending on production and trade patterns. The indicator is calculated in three year averages, from 1990-92 to 2010-11, to reduce the impact of possible errors in estimated trade flows.</skos:definition>
    <dct:description>This indicator is part of the FAO Suite of Food Security Indicators (2017) in the dimension &amp;quot;stability&amp;quot;. It is the share of the value of food (excl. fish) imports over total merchandise exports. This indicator provides a measure of vulnerability and captures the adequacy of foreign exchange reserves to pay for food imports, which has implications for national food security depending on production and trade patterns. The indicator is calculated in three year averages, from 1990-92 to 2010-11, to reduce the impact of possible errors in estimated trade flows.</dct:description>
    <rdfs:comment>This indicator is part of the FAO Suite of Food Security Indicators (2017) in the dimension &amp;quot;stability&amp;quot;. It is the share of the value of food (excl. fish) imports over total merchandise exports. This indicator provides a measure of vulnerability and captures the adequacy of foreign exchange reserves to pay for food imports, which has implications for national food security depending on production and trade patterns. The indicator is calculated in three year averages, from 1990-92 to 2010-11, to reduce the impact of possible errors in estimated trade flows.</rdfs:comment>
    <skos:inScheme rdf:resource="http://data.landportal.info/vocabulary/25"/>
    <rdfs:seeAlso rdf:resource="https://landportal.org/book/indicator/fao-21033-6121"/>
  </rdf:Description>

</rdf:RDF>