<?xml version="1.0" encoding="UTF-8"?>
<rdf:RDF xmlns:rdf="http://www.w3.org/1999/02/22-rdf-syntax-ns#"
  xmlns:dct="http://purl.org/dc/terms/"
  xmlns:skos="http://www.w3.org/2004/02/skos/core#"
  xmlns:schema="http://schema.org/"
  xmlns:sdmx-attribute="http://purl.org/linked-data/sdmx/2009/attribute#"
  xmlns:rdfs="http://www.w3.org/2000/01/rdf-schema#">

  <rdf:Description rdf:about="http://data.landportal.info/indicator/FAO-21030-6127">
    <rdf:type rdf:resource="http://www.w3.org/2004/02/skos/core#Concept"/>
    <rdf:type rdf:resource="http://purl.org/weso/ontology/computex#Indicator"/>
    <dct:identifier>FAO-21030-6127</dct:identifier>
    <skos:notation>FAO-21030-6127</skos:notation>
    <dct:source rdf:resource="http://data.landportal.info/dataset/FAO-FS"/>
    <dct:subject rdf:resource="http://data.landportal.info/voc/landvoc/theme/T-FOOD"/>
    <dct:subject rdf:resource="http://data.landportal.info/voc/landvoc/theme/T-SOCEC"/>
    <schema:about rdf:resource="http://data.landportal.info/voc/landvoc/theme/T-FOOD"/>
    <schema:about rdf:resource="http://data.landportal.info/voc/landvoc/theme/T-SOCEC"/>
    <sdmx-attribute:unitMeasure>Constant International $ per person (3-year average)</sdmx-attribute:unitMeasure>
    <rdfs:label>Per capita food production variability (I$ per person constant 2004-06)</rdfs:label>
    <skos:prefLabel>Per capita food production variability (I$ per person constant 2004-06)</skos:prefLabel>
    <dct:title>Per capita food production variability (I$ per person constant 2004-06)</dct:title>
    <skos:definition>This indicator is part of the FAO Suite of Food Security Indicators (2017) in the dimension &amp;quot;stability&amp;quot;. Per capita food production variability corresponds to the variability of the &amp;quot;food net per capita production value in constant 2004-2006 international $&amp;quot; as disseminated in FAOSTAT. The per capita food production variability compares the variations of the per capita food production across countries and time. Missing values in the food net per capita production value are interpolated using a linear trend. The series is then detrended by fitting a cubic spline by ordinary least squares to the series. The difference between the cubic fit and the acual values are then calculated. Lastly, the volatility for a specific year is defined as the standard deviation of these differences over the previous five years. The aggregates are computed applying the same methodology to the aggregates of the per capita food production variable.</skos:definition>
    <dct:description>This indicator is part of the FAO Suite of Food Security Indicators (2017) in the dimension &amp;quot;stability&amp;quot;. Per capita food production variability corresponds to the variability of the &amp;quot;food net per capita production value in constant 2004-2006 international $&amp;quot; as disseminated in FAOSTAT. The per capita food production variability compares the variations of the per capita food production across countries and time. Missing values in the food net per capita production value are interpolated using a linear trend. The series is then detrended by fitting a cubic spline by ordinary least squares to the series. The difference between the cubic fit and the acual values are then calculated. Lastly, the volatility for a specific year is defined as the standard deviation of these differences over the previous five years. The aggregates are computed applying the same methodology to the aggregates of the per capita food production variable.</dct:description>
    <rdfs:comment>This indicator is part of the FAO Suite of Food Security Indicators (2017) in the dimension &amp;quot;stability&amp;quot;. Per capita food production variability corresponds to the variability of the &amp;quot;food net per capita production value in constant 2004-2006 international $&amp;quot; as disseminated in FAOSTAT. The per capita food production variability compares the variations of the per capita food production across countries and time. Missing values in the food net per capita production value are interpolated using a linear trend. The series is then detrended by fitting a cubic spline by ordinary least squares to the series. The difference between the cubic fit and the acual values are then calculated. Lastly, the volatility for a specific year is defined as the standard deviation of these differences over the previous five years. The aggregates are computed applying the same methodology to the aggregates of the per capita food production variable.</rdfs:comment>
    <skos:inScheme rdf:resource="http://data.landportal.info/vocabulary/25"/>
    <rdfs:seeAlso rdf:resource="https://landportal.org/book/indicator/fao-21030-6127"/>
  </rdf:Description>

</rdf:RDF>