<?xml version="1.0" encoding="UTF-8"?>
<rdf:RDF xmlns:rdf="http://www.w3.org/1999/02/22-rdf-syntax-ns#"
  xmlns:dct="http://purl.org/dc/terms/"
  xmlns:skos="http://www.w3.org/2004/02/skos/core#"
  xmlns:schema="http://schema.org/"
  xmlns:sdmx-attribute="http://purl.org/linked-data/sdmx/2009/attribute#"
  xmlns:rdfs="http://www.w3.org/2000/01/rdf-schema#">

  <rdf:Description rdf:about="http://data.landportal.info/indicator/FAO-21026-6121">
    <rdf:type rdf:resource="http://www.w3.org/2004/02/skos/core#Concept"/>
    <rdf:type rdf:resource="http://purl.org/weso/ontology/computex#Indicator"/>
    <dct:identifier>FAO-21026-6121</dct:identifier>
    <skos:notation>FAO-21026-6121</skos:notation>
    <dct:source rdf:resource="http://data.landportal.info/dataset/FAO-FS"/>
    <dct:subject rdf:resource="http://data.landportal.info/voc/landvoc/theme/T-FOOD"/>
    <schema:about rdf:resource="http://data.landportal.info/voc/landvoc/theme/T-FOOD"/>
    <sdmx-attribute:unitMeasure>Percentage</sdmx-attribute:unitMeasure>
    <rdfs:label>Percentage of children under 5 years of age affected by wasting (%)</rdfs:label>
    <skos:prefLabel>Percentage of children under 5 years of age affected by wasting (%)</skos:prefLabel>
    <dct:title>Percentage of children under 5 years of age affected by wasting (%)</dct:title>
    <skos:definition>This indicator is part of the FAO Suite of Food Security Indicators (2017) in the dimension &amp;quot;utilization&amp;quot;. Wasting prevalence is the proportion of children under five whose weight for height is more than two standard deviations below the median for the international reference population ages 0-59. This indicator belongs to a set of indicators whose purpose is to measure nutritional imbalance and malnutrition resulting in undernutrition (assessed by underweight, stunting and wasting) and overweight. Child growth is the most widely used indicator of nutritional status in a community and is internationally recognized as an important public-health indicator for monitoring health in populations. In addition, children who suffer from growth retardation as a result of poor diets and/or recurrent infections tend to have a greater risk of suffering illness and death. The indicator is also included in the set of World Development Indicators by the World Bank (http://data.worldbank.org/indicator/SH.STA.WAST.ZS)</skos:definition>
    <dct:description>This indicator is part of the FAO Suite of Food Security Indicators (2017) in the dimension &amp;quot;utilization&amp;quot;. Wasting prevalence is the proportion of children under five whose weight for height is more than two standard deviations below the median for the international reference population ages 0-59. This indicator belongs to a set of indicators whose purpose is to measure nutritional imbalance and malnutrition resulting in undernutrition (assessed by underweight, stunting and wasting) and overweight. Child growth is the most widely used indicator of nutritional status in a community and is internationally recognized as an important public-health indicator for monitoring health in populations. In addition, children who suffer from growth retardation as a result of poor diets and/or recurrent infections tend to have a greater risk of suffering illness and death. The indicator is also included in the set of World Development Indicators by the World Bank (http://data.worldbank.org/indicator/SH.STA.WAST.ZS)</dct:description>
    <rdfs:comment>This indicator is part of the FAO Suite of Food Security Indicators (2017) in the dimension &amp;quot;utilization&amp;quot;. Wasting prevalence is the proportion of children under five whose weight for height is more than two standard deviations below the median for the international reference population ages 0-59. This indicator belongs to a set of indicators whose purpose is to measure nutritional imbalance and malnutrition resulting in undernutrition (assessed by underweight, stunting and wasting) and overweight. Child growth is the most widely used indicator of nutritional status in a community and is internationally recognized as an important public-health indicator for monitoring health in populations. In addition, children who suffer from growth retardation as a result of poor diets and/or recurrent infections tend to have a greater risk of suffering illness and death. The indicator is also included in the set of World Development Indicators by the World Bank (http://data.worldbank.org/indicator/SH.STA.WAST.ZS)</rdfs:comment>
    <skos:inScheme rdf:resource="http://data.landportal.info/vocabulary/25"/>
    <rdfs:seeAlso rdf:resource="https://landportal.org/book/indicator/fao-21026-6121"/>
  </rdf:Description>

</rdf:RDF>