<?xml version="1.0" encoding="UTF-8"?>
<rdf:RDF xmlns:rdf="http://www.w3.org/1999/02/22-rdf-syntax-ns#"
  xmlns:dct="http://purl.org/dc/terms/"
  xmlns:skos="http://www.w3.org/2004/02/skos/core#"
  xmlns:schema="http://schema.org/"
  xmlns:sdmx-attribute="http://purl.org/linked-data/sdmx/2009/attribute#"
  xmlns:rdfs="http://www.w3.org/2000/01/rdf-schema#">

  <rdf:Description rdf:about="http://data.landportal.info/indicator/FAO-21012-6121">
    <rdf:type rdf:resource="http://www.w3.org/2004/02/skos/core#Concept"/>
    <rdf:type rdf:resource="http://purl.org/weso/ontology/computex#Indicator"/>
    <dct:identifier>FAO-21012-6121</dct:identifier>
    <skos:notation>FAO-21012-6121</skos:notation>
    <dct:source rdf:resource="http://data.landportal.info/dataset/FAO-FS"/>
    <dct:subject rdf:resource="http://data.landportal.info/voc/landvoc/theme/T-FOOD"/>
    <schema:about rdf:resource="http://data.landportal.info/voc/landvoc/theme/T-FOOD"/>
    <sdmx-attribute:unitMeasure>Percentage (3-year average)</sdmx-attribute:unitMeasure>
    <rdfs:label>Share of dietary energy supply derived from cereals, roots and tubers (%) (3-year average)</rdfs:label>
    <skos:prefLabel>Share of dietary energy supply derived from cereals, roots and tubers (%) (3-year average)</skos:prefLabel>
    <dct:title>Share of dietary energy supply derived from cereals, roots and tubers (%) (3-year average)</dct:title>
    <skos:definition>This indicator is part of the FAO Suite of Food Security Indicators (2017) in the dimension &amp;quot;availability&amp;quot;. The indicator expresses the energy supply (in kcal/caput/day) provided by cereals, roots and tubers as a percentage of the total Dietary Energy Supply (DES) (in kcal/caput/day) calculated from the correponding countries in the FAOSTAT food balance sheets. This indicator provides information on the quality of the diet. It provides a cross country comparable measure of the share of dietary energy supply derived from cereals, roots and tubers. The indicator is calculated in three year averages, from 1990-92 to 2011-13, to reduce the impact of possible errors in estimated DES, due to the difficulties in properly accounting of stock variations in major food.</skos:definition>
    <dct:description>This indicator is part of the FAO Suite of Food Security Indicators (2017) in the dimension &amp;quot;availability&amp;quot;. The indicator expresses the energy supply (in kcal/caput/day) provided by cereals, roots and tubers as a percentage of the total Dietary Energy Supply (DES) (in kcal/caput/day) calculated from the correponding countries in the FAOSTAT food balance sheets. This indicator provides information on the quality of the diet. It provides a cross country comparable measure of the share of dietary energy supply derived from cereals, roots and tubers. The indicator is calculated in three year averages, from 1990-92 to 2011-13, to reduce the impact of possible errors in estimated DES, due to the difficulties in properly accounting of stock variations in major food.</dct:description>
    <rdfs:comment>This indicator is part of the FAO Suite of Food Security Indicators (2017) in the dimension &amp;quot;availability&amp;quot;. The indicator expresses the energy supply (in kcal/caput/day) provided by cereals, roots and tubers as a percentage of the total Dietary Energy Supply (DES) (in kcal/caput/day) calculated from the correponding countries in the FAOSTAT food balance sheets. This indicator provides information on the quality of the diet. It provides a cross country comparable measure of the share of dietary energy supply derived from cereals, roots and tubers. The indicator is calculated in three year averages, from 1990-92 to 2011-13, to reduce the impact of possible errors in estimated DES, due to the difficulties in properly accounting of stock variations in major food.</rdfs:comment>
    <skos:inScheme rdf:resource="http://data.landportal.info/vocabulary/25"/>
    <rdfs:seeAlso rdf:resource="https://landportal.org/book/indicator/fao-21012-6121"/>
  </rdf:Description>

</rdf:RDF>