<?xml version="1.0" encoding="UTF-8"?>
<rdf:RDF xmlns:rdf="http://www.w3.org/1999/02/22-rdf-syntax-ns#"
  xmlns:dct="http://purl.org/dc/terms/"
  xmlns:skos="http://www.w3.org/2004/02/skos/core#"
  xmlns:schema="http://schema.org/"
  xmlns:sdmx-attribute="http://purl.org/linked-data/sdmx/2009/attribute#"
  xmlns:rdfs="http://www.w3.org/2000/01/rdf-schema#">

  <rdf:Description rdf:about="http://data.landportal.info/indicator/FAO-21001-6132">
    <rdf:type rdf:resource="http://www.w3.org/2004/02/skos/core#Concept"/>
    <rdf:type rdf:resource="http://purl.org/weso/ontology/computex#Indicator"/>
    <dct:identifier>FAO-21001-6132</dct:identifier>
    <skos:notation>FAO-21001-6132</skos:notation>
    <dct:source rdf:resource="http://data.landportal.info/dataset/FAO-FS"/>
    <dct:subject rdf:resource="http://data.landportal.info/voc/landvoc/theme/T-FOOD"/>
    <schema:about rdf:resource="http://data.landportal.info/voc/landvoc/theme/T-FOOD"/>
    <sdmx-attribute:unitMeasure>Millions (3-year average)</sdmx-attribute:unitMeasure>
    <rdfs:label>Number of people undernourished (millions) (3-year average)</rdfs:label>
    <skos:prefLabel>Number of people undernourished (millions) (3-year average)</skos:prefLabel>
    <dct:title>Number of people undernourished (millions) (3-year average)</dct:title>
    <skos:definition>This indicator is part of the FAO Suite of Food Security Indicators (2017) as &amp;quot;Additional useful statistics&amp;quot;. This indicator estimates the number of people at risk of undernourishment. It is calculated by applying the estimated prevalence of undernourishment to total population in each period. The indicator is calculated in three year averages, from 1990-92 to 2014-16, to reduce the impact of possible errors in estimated DES, due to the difficulties in properly accounting of stock variations in major food. More details on the methodology for computing the prevalence of undernourishment are in &amp;quot;Annex 2&amp;quot; of the &amp;quot;State of Food Insecurity in the World 2015&amp;quot; Report (http://www.fao.org/publications/sofi/en/).</skos:definition>
    <dct:description>This indicator is part of the FAO Suite of Food Security Indicators (2017) as &amp;quot;Additional useful statistics&amp;quot;. This indicator estimates the number of people at risk of undernourishment. It is calculated by applying the estimated prevalence of undernourishment to total population in each period. The indicator is calculated in three year averages, from 1990-92 to 2014-16, to reduce the impact of possible errors in estimated DES, due to the difficulties in properly accounting of stock variations in major food. More details on the methodology for computing the prevalence of undernourishment are in &amp;quot;Annex 2&amp;quot; of the &amp;quot;State of Food Insecurity in the World 2015&amp;quot; Report (http://www.fao.org/publications/sofi/en/).</dct:description>
    <rdfs:comment>This indicator is part of the FAO Suite of Food Security Indicators (2017) as &amp;quot;Additional useful statistics&amp;quot;. This indicator estimates the number of people at risk of undernourishment. It is calculated by applying the estimated prevalence of undernourishment to total population in each period. The indicator is calculated in three year averages, from 1990-92 to 2014-16, to reduce the impact of possible errors in estimated DES, due to the difficulties in properly accounting of stock variations in major food. More details on the methodology for computing the prevalence of undernourishment are in &amp;quot;Annex 2&amp;quot; of the &amp;quot;State of Food Insecurity in the World 2015&amp;quot; Report (http://www.fao.org/publications/sofi/en/).</rdfs:comment>
    <skos:inScheme rdf:resource="http://data.landportal.info/vocabulary/25"/>
    <rdfs:seeAlso rdf:resource="https://landportal.org/book/indicator/fao-21001-6132"/>
  </rdf:Description>

</rdf:RDF>