<?xml version="1.0" encoding="UTF-8"?>
<rdf:RDF xmlns:rdf="http://www.w3.org/1999/02/22-rdf-syntax-ns#"
  xmlns:dct="http://purl.org/dc/terms/"
  xmlns:skos="http://www.w3.org/2004/02/skos/core#"
  xmlns:schema="http://schema.org/"
  xmlns:sdmx-attribute="http://purl.org/linked-data/sdmx/2009/attribute#"
  xmlns:rdfs="http://www.w3.org/2000/01/rdf-schema#">

  <rdf:Description rdf:about="http://data.landportal.info/indicator/FAO-21032-6125">
    <rdf:type rdf:resource="http://www.w3.org/2004/02/skos/core#Concept"/>
    <rdf:type rdf:resource="http://purl.org/weso/ontology/computex#Indicator"/>
    <dct:identifier>FAO-21032-6125</dct:identifier>
    <skos:notation>FAO-21032-6125</skos:notation>
    <sdmx-attribute:unitMeasure>Index (-2.5; 2.5)</sdmx-attribute:unitMeasure>	
    <dct:source rdf:resource="http://data.landportal.info/dataset/FAO-FS"/>
    <dct:subject rdf:resource="http://data.landportal.info/voc/landvoc/theme/T-FOOD"/>
    <dct:subject rdf:resource="http://data.landportal.info/voc/landvoc/theme/T-SOCEC"/>
    <schema:about rdf:resource="http://data.landportal.info/voc/landvoc/theme/T-FOOD"/>
    <schema:about rdf:resource="http://data.landportal.info/voc/landvoc/theme/T-SOCEC"/>
    <rdfs:label>Political stability and absence of violence/terrorism (index)</rdfs:label>
    <skos:prefLabel>Political stability and absence of violence/terrorism (index)</skos:prefLabel>
    <dct:title>Political stability and absence of violence/terrorism (index)</dct:title>
    <skos:definition>This indicator is part of the FAO Suite of Food Security Indicators (2017) in the dimension &quot;stability&quot;. Political stability and absence of violence measures perceptions of the likelihood that the government will be destabilized or overthrown by unconstitutional or violent means, including politically-motivated violence and terrorism. This indicator provides a measure of political shocks that might have implications for national food security. The WGI compile and summarize information from 30 existing data sources that report the views and experiences of citizens, entrepreneurs, and experts in the public, private and NGO sectors from around the world, on the quality of various aspects of governance.   The WGI draw on four different types of source data: 1)  Surveys of households and firms; 2) Commercial business information providers; 3) Non-governmental organizations ; 4) Public sector organizations. A summary table listing the data sources used in the current update of the WGI, and the years they are included in the WGI can be found at: http://info.worldbank.org/governance/wgi/pdf/table1.pdf The indicator reflects the statistical compilation of responses given by a large number of enterprise, citizen and expert survey respondents in industrial and developing countries, as reported by a number of survey institutes, think tanks, non-governmental organizations, and international organizations. More information at: http://www.govindicators.org,  http://info.worldbank.org/governance/wgi/pdf/pv.pdf, http://papers.ssrn.com/sol3/papers.cfm?abstract_id=1682130 and www.govindicators.org. Produced by: Brookings Institution (Daniel Kaufmann); World Bank Development Research Group (Aart Kraay); and World Bank Institute (Massimo Mastruzzi).</skos:definition>
    <dct:description>This indicator is part of the FAO Suite of Food Security Indicators (2017) in the dimension &quot;stability&quot;. Political stability and absence of violence measures perceptions of the likelihood that the government will be destabilized or overthrown by unconstitutional or violent means, including politically-motivated violence and terrorism. This indicator provides a measure of political shocks that might have implications for national food security. The WGI compile and summarize information from 30 existing data sources that report the views and experiences of citizens, entrepreneurs, and experts in the public, private and NGO sectors from around the world, on the quality of various aspects of governance.   The WGI draw on four different types of source data: 1)  Surveys of households and firms; 2) Commercial business information providers; 3) Non-governmental organizations ; 4) Public sector organizations. A summary table listing the data sources used in the current update of the WGI, and the years they are included in the WGI can be found at: http://info.worldbank.org/governance/wgi/pdf/table1.pdf The indicator reflects the statistical compilation of responses given by a large number of enterprise, citizen and expert survey respondents in industrial and developing countries, as reported by a number of survey institutes, think tanks, non-governmental organizations, and international organizations. More information at: http://www.govindicators.org,  http://info.worldbank.org/governance/wgi/pdf/pv.pdf, http://papers.ssrn.com/sol3/papers.cfm?abstract_id=1682130 and www.govindicators.org. Produced by: Brookings Institution (Daniel Kaufmann); World Bank Development Research Group (Aart Kraay); and World Bank Institute (Massimo Mastruzzi).</dct:description>
    <rdfs:comment>This indicator is part of the FAO Suite of Food Security Indicators (2017) in the dimension &quot;stability&quot;. Political stability and absence of violence measures perceptions of the likelihood that the government will be destabilized or overthrown by unconstitutional or violent means, including politically-motivated violence and terrorism. This indicator provides a measure of political shocks that might have implications for national food security. The WGI compile and summarize information from 30 existing data sources that report the views and experiences of citizens, entrepreneurs, and experts in the public, private and NGO sectors from around the world, on the quality of various aspects of governance.   The WGI draw on four different types of source data: 1)  Surveys of households and firms; 2) Commercial business information providers; 3) Non-governmental organizations ; 4) Public sector organizations. A summary table listing the data sources used in the current update of the WGI, and the years they are included in the WGI can be found at: http://info.worldbank.org/governance/wgi/pdf/table1.pdf The indicator reflects the statistical compilation of responses given by a large number of enterprise, citizen and expert survey respondents in industrial and developing countries, as reported by a number of survey institutes, think tanks, non-governmental organizations, and international organizations. More information at: http://www.govindicators.org,  http://info.worldbank.org/governance/wgi/pdf/pv.pdf, http://papers.ssrn.com/sol3/papers.cfm?abstract_id=1682130 and www.govindicators.org. Produced by: Brookings Institution (Daniel Kaufmann); World Bank Development Research Group (Aart Kraay); and World Bank Institute (Massimo Mastruzzi).</rdfs:comment>
    <skos:inScheme rdf:resource="http://data.landportal.info/vocabulary/25"/>
    <rdfs:seeAlso rdf:resource="https://landportal.org/book/indicator/fao-21032-6125"/>
  </rdf:Description>

</rdf:RDF>