<?xml version="1.0" encoding="UTF-8"?>
<rdf:RDF xmlns:rdf="http://www.w3.org/1999/02/22-rdf-syntax-ns#"
  xmlns:schema="http://schema.org/"
  xmlns:dct="http://purl.org/dc/terms/"
  xmlns:skos="http://www.w3.org/2004/02/skos/core#"
  xmlns:rdfs="http://www.w3.org/2000/01/rdf-schema#">

  <rdf:Description rdf:about="http://data.landportal.info/dataset/PRINDEX-PRINDEX2018">
    <rdf:type rdf:resource="http://www.w3.org/2004/02/skos/core#Concept"/>
    <rdf:type rdf:resource="http://purl.org/linked-data/cube#DataSet"/>
    <rdf:type rdf:resource="http://www.w3.org/ns/dcat#Dataset"/>
    <schema:image rdf:resource="https://landportal.org/sites/landportal.org/files/Prindex_CMYK_logo_horizontal_orange-black_strapline_1.png"/>
    <schema:logo rdf:resource="https://landportal.org/sites/landportal.org/files/Prindex_CMYK_logo_horizontal_orange-black_strapline_1.png"/>
    <dct:subject rdf:resource="http://aims.fao.org/aos/agrovoc/c_a1b5abd0"/>
    <dct:subject rdf:resource="http://aims.fao.org/aos/agrovoc/c_37898"/>
    <dct:subject rdf:resource="http://aims.fao.org/aos/agrovoc/c_12069"/>
    <dct:subject rdf:resource="http://aims.fao.org/aos/agrovoc/c_37942"/>
    <dct:subject rdf:resource="http://data.landportal.info/voc/landvoc/overarching-category/OA-ACCESS"/>
    <dct:subject rdf:resource="http://data.landportal.info/voc/landvoc/overarching-category/OA-LAW"/>
    <dct:subject rdf:resource="http://data.landportal.info/voc/landvoc/theme/T-SOCEC"/>
    <dct:subject rdf:resource="http://data.landportal.info/voc/landvoc/theme/T-URBAN"/>
    <schema:about rdf:resource="http://aims.fao.org/aos/agrovoc/c_a1b5abd0"/>
    <schema:about rdf:resource="http://aims.fao.org/aos/agrovoc/c_37898"/>
    <schema:about rdf:resource="http://aims.fao.org/aos/agrovoc/c_12069"/>
    <schema:about rdf:resource="http://aims.fao.org/aos/agrovoc/c_37942"/>
    <schema:about rdf:resource="http://data.landportal.info/voc/landvoc/overarching-category/OA-ACCESS"/>
    <schema:about rdf:resource="http://data.landportal.info/voc/landvoc/overarching-category/OA-LAW"/>
    <schema:about rdf:resource="http://data.landportal.info/voc/landvoc/theme/T-SOCEC"/>
    <schema:about rdf:resource="http://data.landportal.info/voc/landvoc/theme/T-URBAN"/>
    <dct:publisher rdf:resource="http://data.landportal.info/organization/ebb0ada4-d3ab-426e-b0a6-488f7e8bb965"/>
    <dct:license rdf:resource="http://purl.org/NET/rdflicense/cc-by-nc4.0"/>
    <dct:identifier>PRINDEX-PRINDEX2018</dct:identifier>
    <skos:notation>PRINDEX-PRINDEX2018</skos:notation>
    <skos:prefLabel>Prindex - Global Property Rights Index (2018)</skos:prefLabel>
    <rdfs:label>Prindex - Global Property Rights Index (2018)</rdfs:label>
    <dct:title>Prindex - Global Property Rights Index (2018)</dct:title>
    <skos:definition>Prindex stands for the Global Property Rights Index, an indicator of citizens' perceptions of the security of land and property rights. This dataset portfolio shows a selection of the key 2018 Prindex indicators for 15 countries (Burkina Faso, Cameroon, Costa Rica, Ivory Coast, Ecuador, Honduras, Liberia, Madagascar, Mozambique, Namibia, Perù, Rwanda, Senegal, Thailand and Zambia) but additional information about the methodology and the questionnaire, as well as the full data are available on the new Prindex website: https://www.prindex.net/. Results from the first 15 countries shows that 1 in 4 people feel insecure about their land and property rights. Prindex is an initiative of ODI and Land Alliance supported by Omidyar Network, DFID and other donors. It aims to fill the gap in information about individual perception of tenure security, by creating a baseline global dataset covering more than 100 countries by the end of 2019, to support the achievement of secure property rights around the world.</skos:definition>
    <dct:description>Prindex stands for the Global Property Rights Index, an indicator of citizens' perceptions of the security of land and property rights. This dataset portfolio shows a selection of the key 2018 Prindex indicators for 15 countries (Burkina Faso, Cameroon, Costa Rica, Ivory Coast, Ecuador, Honduras, Liberia, Madagascar, Mozambique, Namibia, Perù, Rwanda, Senegal, Thailand and Zambia) but additional information about the methodology and the questionnaire, as well as the full data are available on the new Prindex website: https://www.prindex.net/. Results from the first 15 countries shows that 1 in 4 people feel insecure about their land and property rights. Prindex is an initiative of ODI and Land Alliance supported by Omidyar Network, DFID and other donors. It aims to fill the gap in information about individual perception of tenure security, by creating a baseline global dataset covering more than 100 countries by the end of 2019, to support the achievement of secure property rights around the world.</dct:description>
    <rdfs:comment>Prindex stands for the Global Property Rights Index, an indicator of citizens' perceptions of the security of land and property rights. This dataset portfolio shows a selection of the key 2018 Prindex indicators for 15 countries (Burkina Faso, Cameroon, Costa Rica, Ivory Coast, Ecuador, Honduras, Liberia, Madagascar, Mozambique, Namibia, Perù, Rwanda, Senegal, Thailand and Zambia) but additional information about the methodology and the questionnaire, as well as the full data are available on the new Prindex website: https://www.prindex.net/. Results from the first 15 countries shows that 1 in 4 people feel insecure about their land and property rights. Prindex is an initiative of ODI and Land Alliance supported by Omidyar Network, DFID and other donors. It aims to fill the gap in information about individual perception of tenure security, by creating a baseline global dataset covering more than 100 countries by the end of 2019, to support the achievement of secure property rights around the world.</rdfs:comment>
    <skos:inScheme rdf:resource="http://data.landportal.info/vocabulary/24"/>
    <rdfs:seeAlso rdf:resource="https://landportal.org/book/dataset/prindex-prindex2018"/>
  </rdf:Description>

</rdf:RDF>