<?xml version="1.0" encoding="UTF-8"?>
<rdf:RDF xmlns:rdf="http://www.w3.org/1999/02/22-rdf-syntax-ns#"
  xmlns:dct="http://purl.org/dc/terms/"
  xmlns:schema="http://schema.org/"
  xmlns:skos="http://www.w3.org/2004/02/skos/core#"
  xmlns:sdmx-attribute="http://purl.org/linked-data/sdmx/2009/attribute#"
  xmlns:rdfs="http://www.w3.org/2000/01/rdf-schema#">

  <rdf:Description rdf:about="http://data.landportal.info/indicator/FAO-21022-6121">
    <rdf:type rdf:resource="http://www.w3.org/2004/02/skos/core#Concept"/>
    <rdf:type rdf:resource="http://purl.org/weso/ontology/computex#Indicator"/>
    <dct:subject rdf:resource="http://data.landportal.info/voc/landvoc/theme/T-FOOD"/>
    <dct:subject rdf:resource="http://data.landportal.info/voc/landvoc/theme/T-SOCEC"/>
    <schema:about rdf:resource="http://data.landportal.info/voc/landvoc/theme/T-FOOD"/>
    <schema:about rdf:resource="http://data.landportal.info/voc/landvoc/theme/T-SOCEC"/>
    <dct:identifier>FAO-21022-6121</dct:identifier>
    <skos:notation>FAO-21022-6121</skos:notation>
    <dct:source rdf:resource="http://data.landportal.info/dataset/FAO-FS.2011"/>
    <sdmx-attribute:unitMeasure>Percentage</sdmx-attribute:unitMeasure>
    <rdfs:label>Share of food expenditure of the poor</rdfs:label>
    <skos:prefLabel>Share of food expenditure of the poor</skos:prefLabel>
    <dct:title>Share of food expenditure of the poor</dct:title>
    <skos:definition>This indicator is part of the FAO Suite of Food Security Indicators (2011) in the dimension &quot;access&quot;. It measures the proportion of food consumption over total consumption (food and non-food) for the lowest income quintile of the population. Due to the way in which the share of food expenditures is defined in the sources of data, this indicator captures the monetary value of food obtained from all the possible food sources (purchases, own-production, gift, in-kind payment, etc.), rather than just the monetary value of purchased food. Total consumption expenditures include both food and non-food expenditures, and exclude non-consumption expenditures such as taxes, insurances, etc. According to the Engel's Law, the higher the income of a household, the lower the proportion of income spent on food. When applied at the National level, this indicator reflects the living standard of a country, as well as the vulnerability of a country to food price increases. Due to the lack/unreliability of income data, this indicator has been built as the ratio between food consumption and total consumption, hence using total consumption as a proxy income. Finally, given the higher vulnerability of the poorer households to food price increase, this indicator only encompasses the share of food consumption of the lowest income quintile of a country population.</skos:definition>
    <dct:description>This indicator is part of the FAO Suite of Food Security Indicators (2011) in the dimension &quot;access&quot;. It measures the proportion of food consumption over total consumption (food and non-food) for the lowest income quintile of the population. Due to the way in which the share of food expenditures is defined in the sources of data, this indicator captures the monetary value of food obtained from all the possible food sources (purchases, own-production, gift, in-kind payment, etc.), rather than just the monetary value of purchased food. Total consumption expenditures include both food and non-food expenditures, and exclude non-consumption expenditures such as taxes, insurances, etc. According to the Engel's Law, the higher the income of a household, the lower the proportion of income spent on food. When applied at the National level, this indicator reflects the living standard of a country, as well as the vulnerability of a country to food price increases. Due to the lack/unreliability of income data, this indicator has been built as the ratio between food consumption and total consumption, hence using total consumption as a proxy income. Finally, given the higher vulnerability of the poorer households to food price increase, this indicator only encompasses the share of food consumption of the lowest income quintile of a country population.</dct:description>
    <rdfs:comment>This indicator is part of the FAO Suite of Food Security Indicators (2011) in the dimension &quot;access&quot;. It measures the proportion of food consumption over total consumption (food and non-food) for the lowest income quintile of the population. Due to the way in which the share of food expenditures is defined in the sources of data, this indicator captures the monetary value of food obtained from all the possible food sources (purchases, own-production, gift, in-kind payment, etc.), rather than just the monetary value of purchased food. Total consumption expenditures include both food and non-food expenditures, and exclude non-consumption expenditures such as taxes, insurances, etc. According to the Engel's Law, the higher the income of a household, the lower the proportion of income spent on food. When applied at the National level, this indicator reflects the living standard of a country, as well as the vulnerability of a country to food price increases. Due to the lack/unreliability of income data, this indicator has been built as the ratio between food consumption and total consumption, hence using total consumption as a proxy income. Finally, given the higher vulnerability of the poorer households to food price increase, this indicator only encompasses the share of food consumption of the lowest income quintile of a country population.</rdfs:comment>
    <skos:inScheme rdf:resource="http://data.landportal.info/vocabulary/25"/>
    <rdfs:seeAlso rdf:resource="https://landportal.org/book/indicators/indfaofsec5"/>
  </rdf:Description>

</rdf:RDF>