<?xml version="1.0" encoding="UTF-8"?>
<rdf:RDF xmlns:rdf="http://www.w3.org/1999/02/22-rdf-syntax-ns#"
  xmlns:dct="http://purl.org/dc/terms/"
  xmlns:schema="http://schema.org/"
  xmlns:skos="http://www.w3.org/2004/02/skos/core#"
  xmlns:sdmx-attribute="http://purl.org/linked-data/sdmx/2009/attribute#"
  xmlns:rdfs="http://www.w3.org/2000/01/rdf-schema#">

  <rdf:Description rdf:about="http://data.landportal.info/indicator/FAO-21036-6121">
    <rdf:type rdf:resource="http://www.w3.org/2004/02/skos/core#Concept"/>
    <rdf:type rdf:resource="http://purl.org/weso/ontology/computex#Indicator"/>
    <dct:subject rdf:resource="http://aims.fao.org/aos/agrovoc/c_10967"/>
    <dct:subject rdf:resource="http://data.landportal.info/voc/landvoc/theme/T-FOOD"/>
    <schema:about rdf:resource="http://aims.fao.org/aos/agrovoc/c_10967"/>
    <schema:about rdf:resource="http://data.landportal.info/voc/landvoc/theme/T-FOOD"/>
    <dct:identifier>FAO-21036-6121</dct:identifier>
    <skos:notation>FAO-21036-6121</skos:notation>
    <dct:source rdf:resource="http://data.landportal.info/dataset/FAO-FS.2011"/>
    <sdmx-attribute:unitMeasure>Percentage</sdmx-attribute:unitMeasure>
    <rdfs:label>Prevalence of anaemia among children under 5 years of age (%)</rdfs:label>
    <skos:prefLabel>Prevalence of anaemia among children under 5 years of age (%)</skos:prefLabel>
    <dct:title>Prevalence of anaemia among children under 5 years of age (%)</dct:title>
    <skos:definition>This indicator is part of the FAO Suite of Food Security Indicators (2011) in the dimension &amp;quot;utilization&amp;quot;. Prevalence of anemia among children under age 5, is the percentage of children under age 5 whose hemoglobin level is less than 110 grams per liter at sea level. Anemia is a condition in which the number of red blood cells or their oxygen-carrying capacity is insufficient to meet physiologic needs, which vary by age, sex, altitude, smoking status, and pregnancy status. In its severe form it is associated with fatigue, weakness, dizziness, and drowsiness. Children under age 5 and pregnant women have the highest risk for anemia.The prevalence of anaemia is an important health indicator. Iron deficiency is thought to be the most common cause of anaemia globally, but other nutritional deficiencies (including folate, vitamin B12 and vitamin A), acute and chronic inflammation, parasitic infections, and inherited or acquired disorders that affect haemoglobin synthesis, red blood cell production or red blood cell survival, can all cause anaemia. When used with other measurements of iron status, the haemoglobin concentration can provide information about the severity of iron deficiency. The cut-off values for public health significance is 40%. A prevalence of anaemia equal or higher than this level signals a severe public health problem. This indicator -- originally calculated by Stevens et al., 2013 -- is also available on the World Bank site (http://data.worldbank.org/indicator/SH.ANM.CHLD.ZS)</skos:definition>
    <dct:description>This indicator is part of the FAO Suite of Food Security Indicators (2011) in the dimension &amp;quot;utilization&amp;quot;. Prevalence of anemia among children under age 5, is the percentage of children under age 5 whose hemoglobin level is less than 110 grams per liter at sea level. Anemia is a condition in which the number of red blood cells or their oxygen-carrying capacity is insufficient to meet physiologic needs, which vary by age, sex, altitude, smoking status, and pregnancy status. In its severe form it is associated with fatigue, weakness, dizziness, and drowsiness. Children under age 5 and pregnant women have the highest risk for anemia.The prevalence of anaemia is an important health indicator. Iron deficiency is thought to be the most common cause of anaemia globally, but other nutritional deficiencies (including folate, vitamin B12 and vitamin A), acute and chronic inflammation, parasitic infections, and inherited or acquired disorders that affect haemoglobin synthesis, red blood cell production or red blood cell survival, can all cause anaemia. When used with other measurements of iron status, the haemoglobin concentration can provide information about the severity of iron deficiency. The cut-off values for public health significance is 40%. A prevalence of anaemia equal or higher than this level signals a severe public health problem. This indicator -- originally calculated by Stevens et al., 2013 -- is also available on the World Bank site (http://data.worldbank.org/indicator/SH.ANM.CHLD.ZS)</dct:description>
    <rdfs:comment>This indicator is part of the FAO Suite of Food Security Indicators (2011) in the dimension &amp;quot;utilization&amp;quot;. Prevalence of anemia among children under age 5, is the percentage of children under age 5 whose hemoglobin level is less than 110 grams per liter at sea level. Anemia is a condition in which the number of red blood cells or their oxygen-carrying capacity is insufficient to meet physiologic needs, which vary by age, sex, altitude, smoking status, and pregnancy status. In its severe form it is associated with fatigue, weakness, dizziness, and drowsiness. Children under age 5 and pregnant women have the highest risk for anemia.The prevalence of anaemia is an important health indicator. Iron deficiency is thought to be the most common cause of anaemia globally, but other nutritional deficiencies (including folate, vitamin B12 and vitamin A), acute and chronic inflammation, parasitic infections, and inherited or acquired disorders that affect haemoglobin synthesis, red blood cell production or red blood cell survival, can all cause anaemia. When used with other measurements of iron status, the haemoglobin concentration can provide information about the severity of iron deficiency. The cut-off values for public health significance is 40%. A prevalence of anaemia equal or higher than this level signals a severe public health problem. This indicator -- originally calculated by Stevens et al., 2013 -- is also available on the World Bank site (http://data.worldbank.org/indicator/SH.ANM.CHLD.ZS)</rdfs:comment>
    <skos:inScheme rdf:resource="http://data.landportal.info/vocabulary/25"/>
    <rdfs:seeAlso rdf:resource="https://landportal.org/book/indicator/fao-21036-6121"/>
  </rdf:Description>

</rdf:RDF>