<?xml version="1.0" encoding="UTF-8"?>
<rdf:RDF xmlns:rdf="http://www.w3.org/1999/02/22-rdf-syntax-ns#"
  xmlns:dct="http://purl.org/dc/terms/"
  xmlns:skos="http://www.w3.org/2004/02/skos/core#"
  xmlns:sdmx-attribute="http://purl.org/linked-data/sdmx/2009/attribute#"
  xmlns:schema="http://schema.org/"
  xmlns:rdfs="http://www.w3.org/2000/01/rdf-schema#">

  <rdf:Description rdf:about="http://data.landportal.info/indicator/FAO-21037-6121">
    <rdf:type rdf:resource="http://www.w3.org/2004/02/skos/core#Concept"/>
    <rdf:type rdf:resource="http://purl.org/weso/ontology/computex#Indicator"/>
    <dct:source rdf:resource="http://data.landportal.info/dataset/FAO-FS.2011"/>
    <dct:identifier>FAO-21037-6121</dct:identifier>
    <skos:notation>FAO-21037-6121</skos:notation>
    <sdmx-attribute:unitMeasure>Percentage</sdmx-attribute:unitMeasure>
    <dct:subject rdf:resource="http://data.landportal.info/voc/landvoc/theme/T-FOOD"/>
    <schema:about rdf:resource="http://data.landportal.info/voc/landvoc/theme/T-FOOD"/>
    <rdfs:label>Prevalence of vitamin A deficiency in the population (%)</rdfs:label>
    <skos:prefLabel>Prevalence of vitamin A deficiency in the population (%)</skos:prefLabel>
    <dct:title>Prevalence of vitamin A deficiency in the population (%)</dct:title>
    <skos:definition>This indicator (originally measured by the WHO) is part of the FAO Suite of Food Security Indicators (2011) in the dimension &amp;quot;utilization&amp;quot;. The prevalence of vitamin A deficiency is the proportion of total population with serum retinol equal or lower than 0.70 ?mol/l. The distribution of serum retinol values in a population and the prevalence of individuals with serum retinol values below a given cut-off can provide important information on the vitamin A status of a population and may reflect the severity of vitamin A deficiency as a public health problem, especially when the degree of underlying infection or inflammation is taken into account. Serum retinol values are most often measured in young children, a group highly vulnerable to deficiency. Deficiency of vitamin A is associated with significant morbidity and mortality from common childhood infections and is the world’s leading preventable cause of childhood blindness. The cut-off values for public health significance is 20%. A prevalence of Vitamine A deficiency equal or higher than this level signals a severe public health problem</skos:definition>
    <dct:description>This indicator (originally measured by the WHO) is part of the FAO Suite of Food Security Indicators (2011) in the dimension &amp;quot;utilization&amp;quot;. The prevalence of vitamin A deficiency is the proportion of total population with serum retinol equal or lower than 0.70 ?mol/l. The distribution of serum retinol values in a population and the prevalence of individuals with serum retinol values below a given cut-off can provide important information on the vitamin A status of a population and may reflect the severity of vitamin A deficiency as a public health problem, especially when the degree of underlying infection or inflammation is taken into account. Serum retinol values are most often measured in young children, a group highly vulnerable to deficiency. Deficiency of vitamin A is associated with significant morbidity and mortality from common childhood infections and is the world’s leading preventable cause of childhood blindness. The cut-off values for public health significance is 20%. A prevalence of Vitamine A deficiency equal or higher than this level signals a severe public health problem</dct:description>
    <rdfs:comment>This indicator (originally measured by the WHO) is part of the FAO Suite of Food Security Indicators (2011) in the dimension &amp;quot;utilization&amp;quot;. The prevalence of vitamin A deficiency is the proportion of total population with serum retinol equal or lower than 0.70 ?mol/l. The distribution of serum retinol values in a population and the prevalence of individuals with serum retinol values below a given cut-off can provide important information on the vitamin A status of a population and may reflect the severity of vitamin A deficiency as a public health problem, especially when the degree of underlying infection or inflammation is taken into account. Serum retinol values are most often measured in young children, a group highly vulnerable to deficiency. Deficiency of vitamin A is associated with significant morbidity and mortality from common childhood infections and is the world’s leading preventable cause of childhood blindness. The cut-off values for public health significance is 20%. A prevalence of Vitamine A deficiency equal or higher than this level signals a severe public health problem</rdfs:comment>
    <skos:inScheme rdf:resource="http://data.landportal.info/vocabulary/25"/>
    <rdfs:seeAlso rdf:resource="https://landportal.org/book/indicator/fao-21037-6121"/>
  </rdf:Description>

</rdf:RDF>