<?xml version="1.0" encoding="UTF-8"?>
<rdf:RDF xmlns:rdf="http://www.w3.org/1999/02/22-rdf-syntax-ns#"
  xmlns:dct="http://purl.org/dc/terms/"
  xmlns:schema="http://schema.org/"
  xmlns:skos="http://www.w3.org/2004/02/skos/core#"
  xmlns:sdmx-attribute="http://purl.org/linked-data/sdmx/2009/attribute#"
  xmlns:rdfs="http://www.w3.org/2000/01/rdf-schema#">

  <rdf:Description rdf:about="http://data.landportal.info/indicator/FAO-21015-6121">
    <rdf:type rdf:resource="http://www.w3.org/2004/02/skos/core#Concept"/>
    <rdf:type rdf:resource="http://purl.org/weso/ontology/computex#Indicator"/>
    <dct:subject rdf:resource="http://data.landportal.info/voc/landvoc/theme/T-FOOD"/>
    <dct:subject rdf:resource="http://data.landportal.info/voc/landvoc/theme/T-SOCEC"/>
    <schema:about rdf:resource="http://data.landportal.info/voc/landvoc/theme/T-FOOD"/>
    <schema:about rdf:resource="http://data.landportal.info/voc/landvoc/theme/T-SOCEC"/>
    <dct:identifier>FAO-21015-6121</dct:identifier>
    <skos:notation>FAO-21015-6121</skos:notation>
    <dct:source rdf:resource="http://data.landportal.info/dataset/FAO-FS.2011"/>
    <sdmx-attribute:unitMeasure>Percentage</sdmx-attribute:unitMeasure>
    <rdfs:label>Percentage of paved roads over total roads (%)</rdfs:label>
    <skos:prefLabel>Percentage of paved roads over total roads (%)</skos:prefLabel>
    <dct:title>Percentage of paved roads over total roads (%)</dct:title>
    <skos:definition>This indicator is part of the FAO Suite of Food Security Indicators (2011) in the dimension &amp;quot;access&amp;quot;. The indicator measure the share (%) of paved roads over total road network, where paved roads are those surfaced with crushed stone (macadam) and hydrocarbon binder or bituminized agents, with concrete, or with cobblestones, as a percentage of all the country&amp;#039;s roads, measured in length. This indicator provides information on the possibility of physical access to markets. Original data comes from the International Road Federation and the World Road Statistics. The indicator was previously included in the World Bank WGI (World Governance Indicators) database (http://data.worldbank.org/indicator/IS.ROD.PAVE.ZS and http://data.worldbank.org/indicator/IS.ROD.TOTL.KM), but the series is no longer available</skos:definition>
    <dct:description>This indicator is part of the FAO Suite of Food Security Indicators (2011) in the dimension &amp;quot;access&amp;quot;. The indicator measure the share (%) of paved roads over total road network, where paved roads are those surfaced with crushed stone (macadam) and hydrocarbon binder or bituminized agents, with concrete, or with cobblestones, as a percentage of all the country&amp;#039;s roads, measured in length. This indicator provides information on the possibility of physical access to markets. Original data comes from the International Road Federation and the World Road Statistics. The indicator was previously included in the World Bank WGI (World Governance Indicators) database (http://data.worldbank.org/indicator/IS.ROD.PAVE.ZS and http://data.worldbank.org/indicator/IS.ROD.TOTL.KM), but the series is no longer available</dct:description>
    <rdfs:comment>This indicator is part of the FAO Suite of Food Security Indicators (2011) in the dimension &amp;quot;access&amp;quot;. The indicator measure the share (%) of paved roads over total road network, where paved roads are those surfaced with crushed stone (macadam) and hydrocarbon binder or bituminized agents, with concrete, or with cobblestones, as a percentage of all the country&amp;#039;s roads, measured in length. This indicator provides information on the possibility of physical access to markets. Original data comes from the International Road Federation and the World Road Statistics. The indicator was previously included in the World Bank WGI (World Governance Indicators) database (http://data.worldbank.org/indicator/IS.ROD.PAVE.ZS and http://data.worldbank.org/indicator/IS.ROD.TOTL.KM), but the series is no longer available</rdfs:comment>
    <skos:inScheme rdf:resource="http://data.landportal.info/vocabulary/25"/>
    <rdfs:seeAlso rdf:resource="https://landportal.org/book/indicator/fao-21015-6121"/>
  </rdf:Description>

</rdf:RDF>