<?xml version="1.0" encoding="UTF-8"?>
<rdf:RDF xmlns:rdf="http://www.w3.org/1999/02/22-rdf-syntax-ns#"
  xmlns:dct="http://purl.org/dc/terms/"
  xmlns:skos="http://www.w3.org/2004/02/skos/core#"
  xmlns:schema="http://schema.org/"
  xmlns:sdmx-attribute="http://purl.org/linked-data/sdmx/2009/attribute#"
  xmlns:rdfs="http://www.w3.org/2000/01/rdf-schema#">

  <rdf:Description rdf:about="http://data.landportal.info/indicator/FAO-21017-6124">
    <rdf:type rdf:resource="http://www.w3.org/2004/02/skos/core#Concept"/>
    <rdf:type rdf:resource="http://purl.org/weso/ontology/computex#Indicator"/>
    <dct:identifier>FAO-21017-6124</dct:identifier>
    <skos:notation>FAO-21017-6124</skos:notation>
    <dct:source rdf:resource="http://data.landportal.info/dataset/FAO-FS.2011"/>
    <dct:subject rdf:resource="http://data.landportal.info/voc/landvoc/theme/T-FOOD"/>
    <dct:subject rdf:resource="http://data.landportal.info/voc/landvoc/theme/T-SOCEC"/>
    <schema:about rdf:resource="http://data.landportal.info/voc/landvoc/theme/T-FOOD"/>
    <schema:about rdf:resource="http://data.landportal.info/voc/landvoc/theme/T-SOCEC"/>
    <sdmx-attribute:unitMeasure>Percentage</sdmx-attribute:unitMeasure>
    <rdfs:label>Road density (per 100 square km of land area)</rdfs:label>
    <skos:prefLabel>Road density (per 100 square km of land area)</skos:prefLabel>
    <dct:title>Road density (per 100 square km of land area)</dct:title>
    <skos:definition>This indicator is part of the FAO Suite of Food Security Indicators (2011) in the dimension &amp;quot;access&amp;quot;. The indicator measures the Km of road per 100 square km of land area, where total road network includes motorways, highways, and main or national roads, secondary or regional roads, and all other roads in a country. A motorway is a road designed and built for motor traffic that separates the traffic flowing in opposite directions. This indicator provides information on the possibility of physical access to markets. The indicator was previously included in the World Bank WGI (World Governance Indicators) database (http://data.worldbank.org/indicator/IS.ROD.PAVE.ZS and http://data.worldbank.org/indicator/IS.ROD.TOTL.KM), but the series is no longer available (Source: Faostat - http://www.fao.org/faostat/en/#data/FS).</skos:definition>
    <dct:description>This indicator is part of the FAO Suite of Food Security Indicators (2011) in the dimension &amp;quot;access&amp;quot;. The indicator measures the Km of road per 100 square km of land area, where total road network includes motorways, highways, and main or national roads, secondary or regional roads, and all other roads in a country. A motorway is a road designed and built for motor traffic that separates the traffic flowing in opposite directions. This indicator provides information on the possibility of physical access to markets. The indicator was previously included in the World Bank WGI (World Governance Indicators) database (http://data.worldbank.org/indicator/IS.ROD.PAVE.ZS and http://data.worldbank.org/indicator/IS.ROD.TOTL.KM), but the series is no longer available (Source: Faostat - http://www.fao.org/faostat/en/#data/FS).</dct:description>
    <rdfs:comment>This indicator is part of the FAO Suite of Food Security Indicators (2011) in the dimension &amp;quot;access&amp;quot;. The indicator measures the Km of road per 100 square km of land area, where total road network includes motorways, highways, and main or national roads, secondary or regional roads, and all other roads in a country. A motorway is a road designed and built for motor traffic that separates the traffic flowing in opposite directions. This indicator provides information on the possibility of physical access to markets. The indicator was previously included in the World Bank WGI (World Governance Indicators) database (http://data.worldbank.org/indicator/IS.ROD.PAVE.ZS and http://data.worldbank.org/indicator/IS.ROD.TOTL.KM), but the series is no longer available (Source: Faostat - http://www.fao.org/faostat/en/#data/FS).</rdfs:comment>
    <skos:inScheme rdf:resource="http://data.landportal.info/vocabulary/25"/>
    <rdfs:seeAlso rdf:resource="https://landportal.org/book/indicator/fao-21017-6124"/>
  </rdf:Description>

</rdf:RDF>