<?xml version="1.0" encoding="UTF-8"?>
<rdf:RDF xmlns:rdf="http://www.w3.org/1999/02/22-rdf-syntax-ns#"
  xmlns:dct="http://purl.org/dc/terms/"
  xmlns:skos="http://www.w3.org/2004/02/skos/core#"
  xmlns:schema="http://schema.org/"
  xmlns:rdfs="http://www.w3.org/2000/01/rdf-schema#">

  <rdf:Description rdf:about="http://data.landportal.info/dataset/UNEP-WCMC-DRY">
    <rdf:type rdf:resource="http://www.w3.org/2004/02/skos/core#Concept"/>
    <rdf:type rdf:resource="http://purl.org/linked-data/cube#DataSet"/>
    <rdf:type rdf:resource="http://www.w3.org/ns/dcat#Dataset"/>
    <dct:identifier>UNEP-WCMC-DRY</dct:identifier>
    <skos:notation>UNEP-WCMC-DRY</skos:notation>
    <dct:publisher rdf:resource="http://data.landportal.info/organization/0d63369c-984d-471e-9582-ff18bfaf09e0"/>
    <dct:subject rdf:resource="http://data.landportal.info/voc/landvoc/overarching-category/OA-USE"/>
    <dct:subject rdf:resource="http://data.landportal.info/voc/landvoc/theme/T-ENVIR"/>
    <dct:subject rdf:resource="http://data.landportal.info/voc/landvoc/theme/T-PASTOR"/>
    <schema:about rdf:resource="http://data.landportal.info/voc/landvoc/overarching-category/OA-USE"/>
    <schema:about rdf:resource="http://data.landportal.info/voc/landvoc/theme/T-ENVIR"/>
    <schema:about rdf:resource="http://data.landportal.info/voc/landvoc/theme/T-PASTOR"/>
    <dct:license rdf:resource="http://purl.org/NET/rdflicense/cc-by4.0"/>
    <schema:image rdf:resource="https://landportal.org/sites/landportal.org/files/UNEP_WCMC_0.png"/>
    <schema:logo rdf:resource="https://landportal.org/sites/landportal.org/files/UNEP_WCMC_0.png"/>
    <skos:prefLabel>UNEP-WCMC - Drylands</skos:prefLabel>
    <rdfs:label>UNEP-WCMC - Drylands</rdfs:label>
    <dct:title>UNEP-WCMC - Drylands</dct:title>
    <skos:definition>The UNEP-WCMC - Drylands database has been produced from the map of drylands generated by UNEP-WCMC. ILRI, in collaboration with the ILC's global rangelands initiative, aggregated the data at the country level using a map of administrative boundaries of countries. This dataset contains aggregated country-level information over the areas that can be defined as drylands, according to the United Nations Convention to Combat Desertification (UNCCD) definition of Drylands.  All indicators included in this datasets are measured in square kilometers and are aggregated at the country level, for 140 countries in total. In particular, the dataset presented here distinguish between arid, semiarid, subhumid and additional drylands areas. Additional drylands area include areas that might not fall - based on the ratio of precipitation to potential evapotranspiration (P/PET) - within the intervals traditionally used to identify arid (0.06 - 0.20 P/PET), semiarid (0.21 - 0.50 P/PET) and subhumid areas (0.51 - 0.65 P/PET), and yet are likely to include dryland and dry-subhumid features. The original micro-data used to calculate these indicators, which are not available on the Land Portal, come from the follwing source: UNEP-WCMC (2007): A spatial analysis approach to the global delineation of dryland areas of relevance to the CBD Programme of Work on Dry and Subhumid Lands. Dataset based on spatial analysis between WWF terrestrial ecoregions (WWF-US, 2004) and aridity zones (CRU/UEA; UNEPGRID, 1991). Dataset checked and refined to remove many gaps, overlaps and slivers (July 2014).</skos:definition>
    <dct:description>The UNEP-WCMC - Drylands database has been produced from the map of drylands generated by UNEP-WCMC. ILRI, in collaboration with the ILC's global rangelands initiative, aggregated the data at the country level using a map of administrative boundaries of countries. This dataset contains aggregated country-level information over the areas that can be defined as drylands, according to the United Nations Convention to Combat Desertification (UNCCD) definition of Drylands.  All indicators included in this datasets are measured in square kilometers and are aggregated at the country level, for 140 countries in total. In particular, the dataset presented here distinguish between arid, semiarid, subhumid and additional drylands areas. Additional drylands area include areas that might not fall - based on the ratio of precipitation to potential evapotranspiration (P/PET) - within the intervals traditionally used to identify arid (0.06 - 0.20 P/PET), semiarid (0.21 - 0.50 P/PET) and subhumid areas (0.51 - 0.65 P/PET), and yet are likely to include dryland and dry-subhumid features. The original micro-data used to calculate these indicators, which are not available on the Land Portal, come from the follwing source: UNEP-WCMC (2007): A spatial analysis approach to the global delineation of dryland areas of relevance to the CBD Programme of Work on Dry and Subhumid Lands. Dataset based on spatial analysis between WWF terrestrial ecoregions (WWF-US, 2004) and aridity zones (CRU/UEA; UNEPGRID, 1991). Dataset checked and refined to remove many gaps, overlaps and slivers (July 2014).</dct:description>
    <rdfs:comment>The UNEP-WCMC - Drylands database has been produced from the map of drylands generated by UNEP-WCMC. ILRI, in collaboration with the ILC's global rangelands initiative, aggregated the data at the country level using a map of administrative boundaries of countries. This dataset contains aggregated country-level information over the areas that can be defined as drylands, according to the United Nations Convention to Combat Desertification (UNCCD) definition of Drylands.  All indicators included in this datasets are measured in square kilometers and are aggregated at the country level, for 140 countries in total. In particular, the dataset presented here distinguish between arid, semiarid, subhumid and additional drylands areas. Additional drylands area include areas that might not fall - based on the ratio of precipitation to potential evapotranspiration (P/PET) - within the intervals traditionally used to identify arid (0.06 - 0.20 P/PET), semiarid (0.21 - 0.50 P/PET) and subhumid areas (0.51 - 0.65 P/PET), and yet are likely to include dryland and dry-subhumid features. The original micro-data used to calculate these indicators, which are not available on the Land Portal, come from the follwing source: UNEP-WCMC (2007): A spatial analysis approach to the global delineation of dryland areas of relevance to the CBD Programme of Work on Dry and Subhumid Lands. Dataset based on spatial analysis between WWF terrestrial ecoregions (WWF-US, 2004) and aridity zones (CRU/UEA; UNEPGRID, 1991). Dataset checked and refined to remove many gaps, overlaps and slivers (July 2014).</rdfs:comment>
    <skos:inScheme rdf:resource="http://data.landportal.info/vocabulary/24"/>
    <rdfs:seeAlso rdf:resource="https://landportal.org/book/dataset/unep-wcmc-dry"/>
  </rdf:Description>

</rdf:RDF>