<?xml version="1.0" encoding="UTF-8"?>
<rdf:RDF xmlns:rdf="http://www.w3.org/1999/02/22-rdf-syntax-ns#"
  xmlns:dct="http://purl.org/dc/terms/"
  xmlns:schema="http://schema.org/"
  xmlns:skos="http://www.w3.org/2004/02/skos/core#"
  xmlns:sdmx-attribute="http://purl.org/linked-data/sdmx/2009/attribute#"
  xmlns:rdfs="http://www.w3.org/2000/01/rdf-schema#">

  <rdf:Description rdf:about="http://data.landportal.info/indicator/UN-SP_GNP_WNOWNS">
    <rdf:type rdf:resource="http://www.w3.org/2004/02/skos/core#Concept"/>
    <rdf:type rdf:resource="http://purl.org/weso/ontology/computex#Indicator"/>
    <dct:subject rdf:resource="http://aims.fao.org/aos/agrovoc/c_f29f3106"/>
    <dct:subject rdf:resource="http://aims.fao.org/aos/agrovoc/c_1dfe5bfe"/>
    <dct:subject rdf:resource="http://aims.fao.org/aos/agrovoc/c_4bd6790a"/>
    <dct:subject rdf:resource="http://aims.fao.org/aos/agrovoc/c_28718"/>
    <dct:subject rdf:resource="http://aims.fao.org/aos/agrovoc/c_8420"/>
    <dct:subject rdf:resource="http://data.landportal.info/voc/landvoc/theme/T-FOOD"/>
    <dct:subject rdf:resource="http://data.landportal.info/voc/landvoc/theme/T-GENDER"/>
    <schema:about rdf:resource="http://aims.fao.org/aos/agrovoc/c_f29f3106"/>
    <schema:about rdf:resource="http://aims.fao.org/aos/agrovoc/c_1dfe5bfe"/>
    <schema:about rdf:resource="http://aims.fao.org/aos/agrovoc/c_4bd6790a"/>
    <schema:about rdf:resource="http://aims.fao.org/aos/agrovoc/c_28718"/>
    <schema:about rdf:resource="http://aims.fao.org/aos/agrovoc/c_8420"/>
    <schema:about rdf:resource="http://data.landportal.info/voc/landvoc/theme/T-FOOD"/>
    <schema:about rdf:resource="http://data.landportal.info/voc/landvoc/theme/T-GENDER"/>
    <dct:identifier>UN-SP_GNP_WNOWNS</dct:identifier>
    <skos:notation>UN-SP_GNP_WNOWNS</skos:notation>
    <dct:source rdf:resource="http://data.landportal.info/dataset/UN-SDG_5.A.1"/>
    <sdmx-attribute:unitMeasure>Percentage (%)</sdmx-attribute:unitMeasure>
    <rdfs:label>Share of women among agricultural land owners or rights-bearers (%)</rdfs:label>
    <skos:prefLabel>Share of women among agricultural land owners or rights-bearers (%)</skos:prefLabel>
    <dct:title>Share of women among agricultural land owners or rights-bearers (%)</dct:title>
    <skos:definition>Share of women among owners or rights-bearers of agricultural land, by type of tenure (%). This indicator focusses on the gender parity, measuring the extent to which women are disadvantaged in ownership / tenure rights over agricultural land.</skos:definition>
    <dct:description>Share of women among owners or rights-bearers of agricultural land, by type of tenure (%). This indicator focusses on the gender parity, measuring the extent to which women are disadvantaged in ownership / tenure rights over agricultural land.</dct:description>
    <rdfs:comment>Share of women among owners or rights-bearers of agricultural land, by type of tenure (%). This indicator focusses on the gender parity, measuring the extent to which women are disadvantaged in ownership / tenure rights over agricultural land.</rdfs:comment>
    <skos:inScheme rdf:resource="http://data.landportal.info/vocabulary/25"/>
    <rdfs:seeAlso rdf:resource="https://landportal.org/book/indicator/un-spgnpwnowns"/>
  </rdf:Description>

</rdf:RDF>