<?xml version="1.0" encoding="UTF-8"?>
<rdf:RDF xmlns:rdf="http://www.w3.org/1999/02/22-rdf-syntax-ns#"
  xmlns:dct="http://purl.org/dc/terms/"
  xmlns:schema="http://schema.org/"
  xmlns:skos="http://www.w3.org/2004/02/skos/core#"
  xmlns:rdfs="http://www.w3.org/2000/01/rdf-schema#">

  <rdf:Description rdf:about="http://data.landportal.info/dataset/SEDAC-ABW">
    <rdf:type rdf:resource="http://www.w3.org/2004/02/skos/core#Concept"/>
    <rdf:type rdf:resource="http://purl.org/linked-data/cube#DataSet"/>
    <rdf:type rdf:resource="http://www.w3.org/ns/dcat#Dataset"/>
    <dct:subject rdf:resource="http://data.landportal.info/voc/landvoc/overarching-category/OA-USE"/>
    <dct:subject rdf:resource="http://data.landportal.info/voc/landvoc/theme/T-ENVIR"/>
    <dct:subject rdf:resource="http://data.landportal.info/voc/landvoc/theme/T-PASTOR"/>
    <schema:about rdf:resource="http://data.landportal.info/voc/landvoc/overarching-category/OA-USE"/>
    <schema:about rdf:resource="http://data.landportal.info/voc/landvoc/theme/T-ENVIR"/>
    <schema:about rdf:resource="http://data.landportal.info/voc/landvoc/theme/T-PASTOR"/>
    <dct:identifier>SEDAC-ABW</dct:identifier>
    <skos:notation>SEDAC-ABW</skos:notation>
    <dct:publisher rdf:resource="http://data.landportal.info/organization/f5bb7338-c0ac-415e-ad8d-f3c324ea3341"/>
    <skos:prefLabel>SEDAC - Anthropogenic Biomes of the World</skos:prefLabel>
    <rdfs:label>SEDAC - Anthropogenic Biomes of the World</rdfs:label>
    <dct:title>SEDAC - Anthropogenic Biomes of the World</dct:title>
    <skos:definition>The indicators included in this dataset are part of the Anthropogenic Biomes of the World (Version 2). This dataset describes anthropogenic transformations within the terrestrial biosphere caused by sustained direct human interaction with ecosystems, including agriculture and urbanization. According to Ellis et Al., (2011), anthrome classes ranges from wildlands - with little antrhropogenic impact on the ecosystem - to dense human settlements - in which the anthropogenic impact is maximum. We present here a subset of indicators measuring country-level extension (in sq. Km) of biomes that are relevant to rangelands and pastoralism, namely pastoral villages, residential rangelands, populated rangelands and remote rangelands. Full data and additional information are available via this link: http://sedac.ciesin.columbia.edu/data/set/anthromes-anthropogenic-biomes... Full citation for the data included here is: Ellis, E.C., K.K. Goldewijk, S. Siebert, D. Lightman, and N. Ramankutty. 2013. Anthropogenic Biomes of the World, Version 2: 2000. Palisades, NY: NASA Socioeconomic Data and Applications Center (SEDAC). http://dx.doi.org/10.7927/H4D798B9. For more information about anthrome classes, please visit: http://ecotope.org/anthromes/v2/ or consult: Ellis, E. C., K. Klein Goldewijk, S. Siebert, D. Lightman, and N. Ramankutty. 2010. Anthropogenic transformation of the biomes, 1700 to 2000. Global Ecology and Biogeography 19(5):589-606. Available at: http://ecotope.org/people/ellis/papers/ellis_2010.pdf</skos:definition>
    <dct:description>The indicators included in this dataset are part of the Anthropogenic Biomes of the World (Version 2). This dataset describes anthropogenic transformations within the terrestrial biosphere caused by sustained direct human interaction with ecosystems, including agriculture and urbanization. According to Ellis et Al., (2011), anthrome classes ranges from wildlands - with little antrhropogenic impact on the ecosystem - to dense human settlements - in which the anthropogenic impact is maximum. We present here a subset of indicators measuring country-level extension (in sq. Km) of biomes that are relevant to rangelands and pastoralism, namely pastoral villages, residential rangelands, populated rangelands and remote rangelands. Full data and additional information are available via this link: http://sedac.ciesin.columbia.edu/data/set/anthromes-anthropogenic-biomes... Full citation for the data included here is: Ellis, E.C., K.K. Goldewijk, S. Siebert, D. Lightman, and N. Ramankutty. 2013. Anthropogenic Biomes of the World, Version 2: 2000. Palisades, NY: NASA Socioeconomic Data and Applications Center (SEDAC). http://dx.doi.org/10.7927/H4D798B9. For more information about anthrome classes, please visit: http://ecotope.org/anthromes/v2/ or consult: Ellis, E. C., K. Klein Goldewijk, S. Siebert, D. Lightman, and N. Ramankutty. 2010. Anthropogenic transformation of the biomes, 1700 to 2000. Global Ecology and Biogeography 19(5):589-606. Available at: http://ecotope.org/people/ellis/papers/ellis_2010.pdf</dct:description>
    <rdfs:comment>The indicators included in this dataset are part of the Anthropogenic Biomes of the World (Version 2). This dataset describes anthropogenic transformations within the terrestrial biosphere caused by sustained direct human interaction with ecosystems, including agriculture and urbanization. According to Ellis et Al., (2011), anthrome classes ranges from wildlands - with little antrhropogenic impact on the ecosystem - to dense human settlements - in which the anthropogenic impact is maximum. We present here a subset of indicators measuring country-level extension (in sq. Km) of biomes that are relevant to rangelands and pastoralism, namely pastoral villages, residential rangelands, populated rangelands and remote rangelands. Full data and additional information are available via this link: http://sedac.ciesin.columbia.edu/data/set/anthromes-anthropogenic-biomes... Full citation for the data included here is: Ellis, E.C., K.K. Goldewijk, S. Siebert, D. Lightman, and N. Ramankutty. 2013. Anthropogenic Biomes of the World, Version 2: 2000. Palisades, NY: NASA Socioeconomic Data and Applications Center (SEDAC). http://dx.doi.org/10.7927/H4D798B9. For more information about anthrome classes, please visit: http://ecotope.org/anthromes/v2/ or consult: Ellis, E. C., K. Klein Goldewijk, S. Siebert, D. Lightman, and N. Ramankutty. 2010. Anthropogenic transformation of the biomes, 1700 to 2000. Global Ecology and Biogeography 19(5):589-606. Available at: http://ecotope.org/people/ellis/papers/ellis_2010.pdf</rdfs:comment>
    <skos:inScheme rdf:resource="http://data.landportal.info/vocabulary/24"/>
    <rdfs:seeAlso rdf:resource="https://landportal.org/book/dataset/sedac-abw"/>
  </rdf:Description>

</rdf:RDF>