<?xml version="1.0" encoding="UTF-8"?>
<rdf:RDF xmlns:rdf="http://www.w3.org/1999/02/22-rdf-syntax-ns#"
  xmlns:schema="http://schema.org/"
  xmlns:dct="http://purl.org/dc/terms/"
  xmlns:skos="http://www.w3.org/2004/02/skos/core#"
  xmlns:rdfs="http://www.w3.org/2000/01/rdf-schema#">

  <rdf:Description rdf:about="http://data.landportal.info/dataset/UN-SDG_15.3.1">
    <rdf:type rdf:resource="http://www.w3.org/2004/02/skos/core#Concept"/>
    <rdf:type rdf:resource="http://purl.org/linked-data/cube#DataSet"/>
    <rdf:type rdf:resource="http://www.w3.org/ns/dcat#Dataset"/>
    <schema:image rdf:resource="https://landportal.org/sites/landportal.org/files/sdg15.3.1.png"/>
    <schema:logo rdf:resource="https://landportal.org/sites/landportal.org/files/sdg15.3.1.png"/>
    <dct:subject rdf:resource="http://data.landportal.info/voc/landvoc/theme/T-FLR"/>
    <dct:subject rdf:resource="http://data.landportal.info/voc/landvoc/theme/T-ENVIR"/>
    <dct:subject rdf:resource="http://data.landportal.info/voc/landvoc/theme/T-PASTOR"/>
    <schema:about rdf:resource="http://data.landportal.info/voc/landvoc/theme/T-FLR"/>
    <schema:about rdf:resource="http://data.landportal.info/voc/landvoc/theme/T-ENVIR"/>
    <schema:about rdf:resource="http://data.landportal.info/voc/landvoc/theme/T-PASTOR"/>
    <dct:license rdf:resource="http://purl.org/NET/rdflicense/allrightsreserved"/>
    <schema:license rdf:resource="http://purl.org/NET/rdflicense/allrightsreserved"/>
    <dct:publisher rdf:resource="http://data.landportal.info/organization/e82f9624-3a20-4f31-a61f-861982f6f1c5"/>
    <dct:identifier>UN-SDG_15.3.1</dct:identifier>
    <skos:notation>UN-SDG_15.3.1</skos:notation>
    <skos:prefLabel>SDG 15.3.1 - Proportion of land that is degraded over total land area</skos:prefLabel>
    <rdfs:label>SDG 15.3.1 - Proportion of land that is degraded over total land area</rdfs:label>
    <dct:title>SDG 15.3.1 - Proportion of land that is degraded over total land area</dct:title>
    <skos:definition>The data included in this dataset reflects indicator 15.3.1 of the Sustainable Development Goals (SDGs), which measures the proportion of land that is degraded over the total land area. This indicator is under &quot;Goal 15: Life on Land&quot; of the SDGs and it refers to Target 15.3, which focuses on combatting desertification and restoring degraded land: By 2030, combat desertification, restore degraded land and soil, including land affected by desertification, drought and floods, and strive to achieve a land degradation-neutral world. This indicator is currently classified as Tier II. United Nations Convention to Combat Desertification (UNCCD) is the Custodian agency for this indicator and official metadata are available at SDG UN Metadata website. For more information, check also this indicator's page on LandPortal SDG portfolio. Please note that according to their official formulation, several SDGs indicators needs to be disaggregated, therefore the related datasets that appear on our website might contain more than one data series for a given SDGs indicator. In particular, SDG indicator 15.3.1 is composed by the following data series: Proportion of land that is degraded over total land area (%)</skos:definition>
    <dct:description>The data included in this dataset reflects indicator 15.3.1 of the Sustainable Development Goals (SDGs), which measures the proportion of land that is degraded over the total land area. This indicator is under &quot;Goal 15: Life on Land&quot; of the SDGs and it refers to Target 15.3, which focuses on combatting desertification and restoring degraded land: By 2030, combat desertification, restore degraded land and soil, including land affected by desertification, drought and floods, and strive to achieve a land degradation-neutral world. This indicator is currently classified as Tier II. United Nations Convention to Combat Desertification (UNCCD) is the Custodian agency for this indicator and official metadata are available at SDG UN Metadata website. For more information, check also this indicator's page on LandPortal SDG portfolio. Please note that according to their official formulation, several SDGs indicators needs to be disaggregated, therefore the related datasets that appear on our website might contain more than one data series for a given SDGs indicator. In particular, SDG indicator 15.3.1 is composed by the following data series: Proportion of land that is degraded over total land area (%)</dct:description>
    <rdfs:comment>The data included in this dataset reflects indicator 15.3.1 of the Sustainable Development Goals (SDGs), which measures the proportion of land that is degraded over the total land area. This indicator is under &quot;Goal 15: Life on Land&quot; of the SDGs and it refers to Target 15.3, which focuses on combatting desertification and restoring degraded land: By 2030, combat desertification, restore degraded land and soil, including land affected by desertification, drought and floods, and strive to achieve a land degradation-neutral world. This indicator is currently classified as Tier II. United Nations Convention to Combat Desertification (UNCCD) is the Custodian agency for this indicator and official metadata are available at SDG UN Metadata website. For more information, check also this indicator's page on LandPortal SDG portfolio. Please note that according to their official formulation, several SDGs indicators needs to be disaggregated, therefore the related datasets that appear on our website might contain more than one data series for a given SDGs indicator. In particular, SDG indicator 15.3.1 is composed by the following data series: Proportion of land that is degraded over total land area (%)</rdfs:comment>
    <skos:inScheme rdf:resource="http://data.landportal.info/vocabulary/24"/>
    <rdfs:seeAlso rdf:resource="https://landportal.org/book/dataset/un-sdg1531"/>
  </rdf:Description>

</rdf:RDF>