<?xml version="1.0" encoding="UTF-8"?>
<rdf:RDF xmlns:rdf="http://www.w3.org/1999/02/22-rdf-syntax-ns#"
  xmlns:schema="http://schema.org/"
  xmlns:dct="http://purl.org/dc/terms/"
  xmlns:skos="http://www.w3.org/2004/02/skos/core#"
  xmlns:rdfs="http://www.w3.org/2000/01/rdf-schema#">

  <rdf:Description rdf:about="http://data.landportal.info/dataset/WB-DB">
    <rdf:type rdf:resource="http://www.w3.org/2004/02/skos/core#Concept"/>
    <rdf:type rdf:resource="http://purl.org/linked-data/cube#DataSet"/>
    <rdf:type rdf:resource="http://www.w3.org/ns/dcat#Dataset"/>
    <schema:image rdf:resource="https://landportal.org/sites/landportal.org/files/doingbusiness-logo.png"/>
    <schema:logo rdf:resource="https://landportal.org/sites/landportal.org/files/doingbusiness-logo.png"/>
    <dct:subject rdf:resource="http://aims.fao.org/aos/agrovoc/c_9000091"/>
    <dct:subject rdf:resource="http://aims.fao.org/aos/agrovoc/c_9000098"/>
    <dct:subject rdf:resource="http://data.landportal.info/voc/landvoc/overarching-category/OA-USE"/>
    <dct:subject rdf:resource="http://data.landportal.info/voc/landvoc/theme/T-INVEST"/>
    <dct:subject rdf:resource="http://data.landportal.info/voc/landvoc/theme/T-SOCEC"/>
    <schema:about rdf:resource="http://aims.fao.org/aos/agrovoc/c_9000091"/>
    <schema:about rdf:resource="http://aims.fao.org/aos/agrovoc/c_9000098"/>
    <schema:about rdf:resource="http://data.landportal.info/voc/landvoc/overarching-category/OA-USE"/>
    <schema:about rdf:resource="http://data.landportal.info/voc/landvoc/theme/T-INVEST"/>
    <schema:about rdf:resource="http://data.landportal.info/voc/landvoc/theme/T-SOCEC"/>
    <dct:license rdf:resource="http://purl.org/NET/rdflicense/cc-by4.0"/>
    <dct:publisher rdf:resource="http://data.landportal.info/organization/78e2ad5a-ed53-4bc5-aafe-2d39f19da353"/>
    <dct:identifier>WB-DB</dct:identifier>
    <skos:notation>WB-DB</skos:notation>
    <skos:prefLabel>WB - Doing Business</skos:prefLabel>
    <rdfs:label>WB - Doing Business</rdfs:label>
    <dct:title>WB - Doing Business</dct:title>
    <skos:definition>The Doing Business project provides objective measures of business regulations and their enforcement across 190 economies and selected cities at the subnational and regional level. The Doing Business project, launched in 2002, looks at domestic small and medium-size companies and measures the regulations applying to them through their life cycle. By gathering and analyzing comprehensive quantitative data to compare business regulation environments across economies and over time, Doing Business encourages economies to compete towards more efficient regulation; offers measurable benchmarks for reform; and serves as a resource for academics, journalists, private sector researchers and others interested in the business climate of each economy. Doing Business covers 11 areas of business regulation across 190 economies. Ten of these areas—starting a business, dealing with construction permits, getting electricity, registering property, getting credit, protecting minority investors, paying taxes, trading across borders, enforcing contracts and resolving insolvency—are included in the distance to frontier score and ease of doing business ranking. Doing Business also measures features of labor market regulation, which is not included in these two measures. Doing Business relies on four main sources of information: the relevant laws and regulations, Doing Business respondents, the governments of the economies covered and the World Bank Group regional staff. More than 43,000 professionals in 190 economies have assisted in providing the data that inform the Doing Business indicators over the past 15 years.  On the Land Portal, we only display a selection of all indicators included in the Doing Business project. In particular, we have focused our attention on land-related indicators. Thus, we have included all available measures related to the quality of the land administration index, including all its sub-components (reliability of infrastructure index, transparency of information index, geographic coverage index, land dispute resolution index, equal access to property rights index) and measures for the registering property index (procedures, time, cost and quality of the land administration index). In order to offer a clear picture of the general regulatory and business context in which these land-related indicators are calculated, we have also included the ease of doing business distance to frontier and score, which are based on all the 10 regulation areas assessed by the Doing Business.                     Find more information at the Doing Business website.   </skos:definition>
    <dct:description>The Doing Business project provides objective measures of business regulations and their enforcement across 190 economies and selected cities at the subnational and regional level. The Doing Business project, launched in 2002, looks at domestic small and medium-size companies and measures the regulations applying to them through their life cycle. By gathering and analyzing comprehensive quantitative data to compare business regulation environments across economies and over time, Doing Business encourages economies to compete towards more efficient regulation; offers measurable benchmarks for reform; and serves as a resource for academics, journalists, private sector researchers and others interested in the business climate of each economy. Doing Business covers 11 areas of business regulation across 190 economies. Ten of these areas—starting a business, dealing with construction permits, getting electricity, registering property, getting credit, protecting minority investors, paying taxes, trading across borders, enforcing contracts and resolving insolvency—are included in the distance to frontier score and ease of doing business ranking. Doing Business also measures features of labor market regulation, which is not included in these two measures. Doing Business relies on four main sources of information: the relevant laws and regulations, Doing Business respondents, the governments of the economies covered and the World Bank Group regional staff. More than 43,000 professionals in 190 economies have assisted in providing the data that inform the Doing Business indicators over the past 15 years.  On the Land Portal, we only display a selection of all indicators included in the Doing Business project. In particular, we have focused our attention on land-related indicators. Thus, we have included all available measures related to the quality of the land administration index, including all its sub-components (reliability of infrastructure index, transparency of information index, geographic coverage index, land dispute resolution index, equal access to property rights index) and measures for the registering property index (procedures, time, cost and quality of the land administration index). In order to offer a clear picture of the general regulatory and business context in which these land-related indicators are calculated, we have also included the ease of doing business distance to frontier and score, which are based on all the 10 regulation areas assessed by the Doing Business.                     Find more information at the Doing Business website.   </dct:description>
    <rdfs:comment>The Doing Business project provides objective measures of business regulations and their enforcement across 190 economies and selected cities at the subnational and regional level. The Doing Business project, launched in 2002, looks at domestic small and medium-size companies and measures the regulations applying to them through their life cycle. By gathering and analyzing comprehensive quantitative data to compare business regulation environments across economies and over time, Doing Business encourages economies to compete towards more efficient regulation; offers measurable benchmarks for reform; and serves as a resource for academics, journalists, private sector researchers and others interested in the business climate of each economy. Doing Business covers 11 areas of business regulation across 190 economies. Ten of these areas—starting a business, dealing with construction permits, getting electricity, registering property, getting credit, protecting minority investors, paying taxes, trading across borders, enforcing contracts and resolving insolvency—are included in the distance to frontier score and ease of doing business ranking. Doing Business also measures features of labor market regulation, which is not included in these two measures. Doing Business relies on four main sources of information: the relevant laws and regulations, Doing Business respondents, the governments of the economies covered and the World Bank Group regional staff. More than 43,000 professionals in 190 economies have assisted in providing the data that inform the Doing Business indicators over the past 15 years.  On the Land Portal, we only display a selection of all indicators included in the Doing Business project. In particular, we have focused our attention on land-related indicators. Thus, we have included all available measures related to the quality of the land administration index, including all its sub-components (reliability of infrastructure index, transparency of information index, geographic coverage index, land dispute resolution index, equal access to property rights index) and measures for the registering property index (procedures, time, cost and quality of the land administration index). In order to offer a clear picture of the general regulatory and business context in which these land-related indicators are calculated, we have also included the ease of doing business distance to frontier and score, which are based on all the 10 regulation areas assessed by the Doing Business.                     Find more information at the Doing Business website.   </rdfs:comment>
    <skos:inScheme rdf:resource="http://data.landportal.info/vocabulary/24"/>
    <rdfs:seeAlso rdf:resource="https://landportal.org/book/dataset/wb-db"/>
  </rdf:Description>

</rdf:RDF>