<?xml version="1.0" encoding="UTF-8"?>
<rdf:RDF xmlns:rdf="http://www.w3.org/1999/02/22-rdf-syntax-ns#"
  xmlns:dct="http://purl.org/dc/terms/"
  xmlns:schema="http://schema.org/"
  xmlns:skos="http://www.w3.org/2004/02/skos/core#"
  xmlns:rdfs="http://www.w3.org/2000/01/rdf-schema#">

  <rdf:Description rdf:about="http://data.landportal.info/dataset/NDGAIN-CI">
    <rdf:type rdf:resource="http://www.w3.org/2004/02/skos/core#Concept"/>
    <rdf:type rdf:resource="http://purl.org/linked-data/cube#DataSet"/>
    <rdf:type rdf:resource="http://www.w3.org/ns/dcat#Dataset"/>
    <dct:license rdf:resource="http://purl.org/NET/rdflicense/cc-by4.0"/>
    <schema:license rdf:resource="http://purl.org/NET/rdflicense/cc-by4.0"/>
    <dct:subject rdf:resource="http://aims.fao.org/aos/agrovoc/c_1666"/>
    <dct:subject rdf:resource="http://data.landportal.info/voc/landvoc/theme/T-ENVIR"/>
    <schema:about rdf:resource="http://aims.fao.org/aos/agrovoc/c_1666"/>
    <schema:about rdf:resource="http://data.landportal.info/voc/landvoc/theme/T-ENVIR"/>
    <dct:publisher rdf:resource="http://data.landportal.info/organization/36b4ff30-6a58-4eeb-9841-03e6c0bd983d"/>
    <schema:image rdf:resource="https://landportal.org/sites/landportal.org/files/nd_gain.jpg"/>
    <schema:logo rdf:resource="https://landportal.org/sites/landportal.org/files/nd_gain.jpg"/>
    <dct:identifier>NDGAIN-CI</dct:identifier>
    <skos:notation>NDGAIN-CI</skos:notation>
    <skos:prefLabel>Notre Dame Global Adaptation Initiative</skos:prefLabel>
    <rdfs:label>Notre Dame Global Adaptation Initiative</rdfs:label>
    <dct:title>Notre Dame Global Adaptation Initiative</dct:title>
    <skos:definition>The Notre Dame-Global Adaptation Index (ND-GAIN) Country Index is a free opensource index that shows a country’s current vulnerability to climate disruptions. It also assesses a country’s readiness to leverage private and public sector investment for adaptive actions. ND-GAIN brings together over 74 variables to form 45 core indicators to measure vulnerability and readiness of 192 UN countries from 1995 to the present (Due to data availability, ND-GAIN measures vulnerability of 182 countries and readiness of 184 countries). Corporate, NGO, government, and development decision-makers use ND-GAIN’s country-level rankings and underlying data to make informed strategic operational and reputational decisions regarding supply chains, capital projects, policy changes and community engagements. Notre Dame Global Adaptation Index moved to the University of Notre Dame in April 2013. It was formerly housed in the Global Adaptation Institute in Washington, D.C. It now resides within the Climate Change Adaptation Program of the University of Notre Dame’s Environmental Change Initiative (ND-ECI), a Strategic Research Initiative focused on “science serving society” and draws on resources from both inside and outside of the university. Adaptation is an evolving concept. ND-GAIN understanding of climate change and the risks it presents is constantly improving through ongoing research. ND-GAIN strives to estimate adaptation risk and opportunity using the best available research outputs, data, and tools. To this end, the index keeps updating whenever it is necessary, and highlights of each release can be found at http://index.gain.org/about/reference.</skos:definition>
    <dct:description>The Notre Dame-Global Adaptation Index (ND-GAIN) Country Index is a free opensource index that shows a country’s current vulnerability to climate disruptions. It also assesses a country’s readiness to leverage private and public sector investment for adaptive actions. ND-GAIN brings together over 74 variables to form 45 core indicators to measure vulnerability and readiness of 192 UN countries from 1995 to the present (Due to data availability, ND-GAIN measures vulnerability of 182 countries and readiness of 184 countries). Corporate, NGO, government, and development decision-makers use ND-GAIN’s country-level rankings and underlying data to make informed strategic operational and reputational decisions regarding supply chains, capital projects, policy changes and community engagements. Notre Dame Global Adaptation Index moved to the University of Notre Dame in April 2013. It was formerly housed in the Global Adaptation Institute in Washington, D.C. It now resides within the Climate Change Adaptation Program of the University of Notre Dame’s Environmental Change Initiative (ND-ECI), a Strategic Research Initiative focused on “science serving society” and draws on resources from both inside and outside of the university. Adaptation is an evolving concept. ND-GAIN understanding of climate change and the risks it presents is constantly improving through ongoing research. ND-GAIN strives to estimate adaptation risk and opportunity using the best available research outputs, data, and tools. To this end, the index keeps updating whenever it is necessary, and highlights of each release can be found at http://index.gain.org/about/reference.</dct:description>
    <rdfs:comment>The Notre Dame-Global Adaptation Index (ND-GAIN) Country Index is a free opensource index that shows a country’s current vulnerability to climate disruptions. It also assesses a country’s readiness to leverage private and public sector investment for adaptive actions. ND-GAIN brings together over 74 variables to form 45 core indicators to measure vulnerability and readiness of 192 UN countries from 1995 to the present (Due to data availability, ND-GAIN measures vulnerability of 182 countries and readiness of 184 countries). Corporate, NGO, government, and development decision-makers use ND-GAIN’s country-level rankings and underlying data to make informed strategic operational and reputational decisions regarding supply chains, capital projects, policy changes and community engagements. Notre Dame Global Adaptation Index moved to the University of Notre Dame in April 2013. It was formerly housed in the Global Adaptation Institute in Washington, D.C. It now resides within the Climate Change Adaptation Program of the University of Notre Dame’s Environmental Change Initiative (ND-ECI), a Strategic Research Initiative focused on “science serving society” and draws on resources from both inside and outside of the university. Adaptation is an evolving concept. ND-GAIN understanding of climate change and the risks it presents is constantly improving through ongoing research. ND-GAIN strives to estimate adaptation risk and opportunity using the best available research outputs, data, and tools. To this end, the index keeps updating whenever it is necessary, and highlights of each release can be found at http://index.gain.org/about/reference.</rdfs:comment>
    <skos:inScheme rdf:resource="http://data.landportal.info/vocabulary/24"/>
    <rdfs:seeAlso rdf:resource="https://landportal.org/book/dataset/nd-gain"/>
  </rdf:Description>

</rdf:RDF>