<?xml version="1.0" encoding="utf-8" ?>
<rdf:RDF
	xmlns:rdf="http://www.w3.org/1999/02/22-rdf-syntax-ns#"
	xmlns:rdfs="http://www.w3.org/2000/01/rdf-schema#"
	xmlns:skos="http://www.w3.org/2004/02/skos/core#"
	xmlns:dct="http://purl.org/dc/terms/"
	xmlns:schema="http://schema.org/"
	xmlns:sdmx-attribute="http://purl.org/linked-data/sdmx/2009/attribute#" >
  <rdf:Description rdf:about="http://data.landportal.info/indicator/WB-DB-RP-QLA-EAPR.INDEX">
    <rdf:type rdf:resource="http://www.w3.org/2004/02/skos/core#Concept" />
    <rdf:type rdf:resource="http://purl.org/weso/ontology/computex#Indicator" />
    <rdfs:label>Equal access to property rights index (Quality of land administration index - Doing Business)</rdfs:label>
    <rdfs:comment>The equal access to property rights index has two components: Whether unmarried men and unmarried women have equal ownership rights to property. A score of -1 is assigned if there are unequal ownership rights to property; 0 if there is equality. Whether married men and married women have equal ownership rights to property. A score of -1 is assigned if there are unequal ownership rights to property; 0 if there is equality. Ownership rights cover the ability to manage, control, administer, access, encumber, receive, dispose of and transfer property. Each restriction is considered if there is a differential treatment for men and women in the law considering the default marital property regime. For customary land systems, equality is assumed unless there is a general legal provision stating a differential treatment. The index ranges from -2 to 0, with higher values indicating greater inclusiveness of property rights. In Mali, for example, unmarried men and unmarried women have equal ownership rights to property (a score of 0). The same applies to married men and women who can use their property in the same way (a score of 0). Adding these numbers gives Mali a score of 0 on the equal access to property rights indexwhich indicates equal property rights between men and women. On the contrary in Tonga, unmarried men and unmarried women do not have equal ownership rights to property according to the Land Act [Cap 132], Sections 7, 45 and 82 (a score of -1). The same applies to married men and women who are not permitted to use their property in the same way according to the Land Act [Cap 132], Sections 7, 45 and 82 (a score of -1). Adding these numbers gives Tonga a score of -2 on the equal access to property rights indexwhich indicates unequal property rights between men and women. Read more aboutthe &quot;Equal access to property rights index Methodology&quot;</rdfs:comment>
    <rdfs:seeAlso rdf:resource="https://landportal.org/book/indicator/wb-db-rp-qla-eaprindex" />
    <skos:notation>WB-DB-RP-QLA-EAPR.INDEX</skos:notation>
    <skos:inScheme rdf:resource="http://data.landportal.info/vocabulary/25" />
    <skos:prefLabel>Equal access to property rights index (Quality of land administration index - Doing Business)</skos:prefLabel>
    <dct:subject rdf:resource="http://aims.fao.org/aos/agrovoc/c_9000098" />
    <dct:subject rdf:resource="http://data.landportal.info/voc/landvoc/theme/T-INST" />
    <dct:subject rdf:resource="http://data.landportal.info/voc/landvoc/overarching-category/OA-USE" />
    <dct:subject rdf:resource="http://data.landportal.info/voc/landvoc/theme/T-INVEST" />
    <dct:title>Equal access to property rights index (Quality of land administration index - Doing Business)</dct:title>
    <dct:description>The equal access to property rights index has two components: Whether unmarried men and unmarried women have equal ownership rights to property. A score of -1 is assigned if there are unequal ownership rights to property; 0 if there is equality. Whether married men and married women have equal ownership rights to property. A score of -1 is assigned if there are unequal ownership rights to property; 0 if there is equality. Ownership rights cover the ability to manage, control, administer, access, encumber, receive, dispose of and transfer property. Each restriction is considered if there is a differential treatment for men and women in the law considering the default marital property regime. For customary land systems, equality is assumed unless there is a general legal provision stating a differential treatment. The index ranges from -2 to 0, with higher values indicating greater inclusiveness of property rights. In Mali, for example, unmarried men and unmarried women have equal ownership rights to property (a score of 0). The same applies to married men and women who can use their property in the same way (a score of 0). Adding these numbers gives Mali a score of 0 on the equal access to property rights indexwhich indicates equal property rights between men and women. On the contrary in Tonga, unmarried men and unmarried women do not have equal ownership rights to property according to the Land Act [Cap 132], Sections 7, 45 and 82 (a score of -1). The same applies to married men and women who are not permitted to use their property in the same way according to the Land Act [Cap 132], Sections 7, 45 and 82 (a score of -1). Adding these numbers gives Tonga a score of -2 on the equal access to property rights indexwhich indicates unequal property rights between men and women. Read more aboutthe &quot;Equal access to property rights index Methodology&quot;</dct:description>
    <dct:identifier>WB-DB-RP-QLA-EAPR.INDEX</dct:identifier>
    <schema:about rdf:resource="http://aims.fao.org/aos/agrovoc/c_9000098" />
    <schema:about rdf:resource="http://data.landportal.info/voc/landvoc/theme/T-INST" />
    <schema:about rdf:resource="http://data.landportal.info/voc/landvoc/theme/T-INVEST" />
    <schema:about rdf:resource="http://data.landportal.info/voc/landvoc/overarching-category/OA-USE" />
    <dct:source rdf:resource="http://data.landportal.info/dataset/WB-DB" />
    <skos:definition>The equal access to property rights index has two components: Whether unmarried men and unmarried women have equal ownership rights to property. A score of -1 is assigned if there are unequal ownership rights to property; 0 if there is equality. Whether married men and married women have equal ownership rights to property. A score of -1 is assigned if there are unequal ownership rights to property; 0 if there is equality. Ownership rights cover the ability to manage, control, administer, access, encumber, receive, dispose of and transfer property. Each restriction is considered if there is a differential treatment for men and women in the law considering the default marital property regime. For customary land systems, equality is assumed unless there is a general legal provision stating a differential treatment. The index ranges from -2 to 0, with higher values indicating greater inclusiveness of property rights. In Mali, for example, unmarried men and unmarried women have equal ownership rights to property (a score of 0). The same applies to married men and women who can use their property in the same way (a score of 0). Adding these numbers gives Mali a score of 0 on the equal access to property rights indexwhich indicates equal property rights between men and women. On the contrary in Tonga, unmarried men and unmarried women do not have equal ownership rights to property according to the Land Act [Cap 132], Sections 7, 45 and 82 (a score of -1). The same applies to married men and women who are not permitted to use their property in the same way according to the Land Act [Cap 132], Sections 7, 45 and 82 (a score of -1). Adding these numbers gives Tonga a score of -2 on the equal access to property rights indexwhich indicates unequal property rights between men and women. Read more aboutthe &quot;Equal access to property rights index Methodology&quot;</skos:definition>
    <sdmx-attribute:unitMeasure>Index (-2; 0)</sdmx-attribute:unitMeasure>
  </rdf:Description>
  <rdf:Description rdf:about="http://data.landportal.info/indicator/WB-DB-RP-QLA-GEOCOVER.INDEX">
    <rdf:type rdf:resource="http://www.w3.org/2004/02/skos/core#Concept" />
    <rdf:type rdf:resource="http://purl.org/weso/ontology/computex#Indicator" />
    <rdfs:label>Geographic coverage index (Quality of land administration index - Doing Business)</rdfs:label>
    <rdfs:comment>The geographic coverage index has four components: How complete the coverage of the land registry is at the level of the largest business city. A score of 2 is assigned if all privately held land plots in the city are formally registered at the land registry; 0 if not. How complete the coverage of the land registry is at the level of the economy. A score of 2 is assigned if all privately held land plots in the economy are formally registered at the land registry; 0 if not. How complete the coverage of the mapping agency is at the level of the largest business city. A score of 2 is assigned if all privately held land plots in the city are mapped; 0 if not. How complete the coverage of the mapping agency is at the level of the economy. A score of 2 is assigned if all privately held land plots in the economy are mapped; 0 if not. The index ranges from 0 to 8, with higher values indicating greater geographic coverage in land ownership registration and cadastral mapping. In the Republic of Korea, for example, all privately held land plots are formally registered at the land registry in Seoul (a score of 2) and in the economy as a whole (a score of 2). In addition, all privately held land plots are mapped in Seoul (a score of 2) and in the economy as a whole (a score of 2). Adding these numbers gives Korea a score of 8 on the geographic coverage index.  Read more aboutthe &quot;Geographic coverage indexMethodology&quot;</rdfs:comment>
    <rdfs:seeAlso rdf:resource="https://landportal.org/book/indicator/wb-db-rp-qla-geocoverindex" />
    <skos:notation>WB-DB-RP-QLA-GEOCOVER.INDEX</skos:notation>
    <skos:inScheme rdf:resource="http://data.landportal.info/vocabulary/25" />
    <skos:prefLabel>Geographic coverage index (Quality of land administration index - Doing Business)</skos:prefLabel>
    <dct:subject rdf:resource="http://aims.fao.org/aos/agrovoc/c_9000098" />
    <dct:subject rdf:resource="http://data.landportal.info/voc/landvoc/theme/T-INST" />
    <dct:subject rdf:resource="http://data.landportal.info/voc/landvoc/overarching-category/OA-USE" />
    <dct:subject rdf:resource="http://data.landportal.info/voc/landvoc/theme/T-INVEST" />
    <dct:title>Geographic coverage index (Quality of land administration index - Doing Business)</dct:title>
    <dct:description>The geographic coverage index has four components: How complete the coverage of the land registry is at the level of the largest business city. A score of 2 is assigned if all privately held land plots in the city are formally registered at the land registry; 0 if not. How complete the coverage of the land registry is at the level of the economy. A score of 2 is assigned if all privately held land plots in the economy are formally registered at the land registry; 0 if not. How complete the coverage of the mapping agency is at the level of the largest business city. A score of 2 is assigned if all privately held land plots in the city are mapped; 0 if not. How complete the coverage of the mapping agency is at the level of the economy. A score of 2 is assigned if all privately held land plots in the economy are mapped; 0 if not. The index ranges from 0 to 8, with higher values indicating greater geographic coverage in land ownership registration and cadastral mapping. In the Republic of Korea, for example, all privately held land plots are formally registered at the land registry in Seoul (a score of 2) and in the economy as a whole (a score of 2). In addition, all privately held land plots are mapped in Seoul (a score of 2) and in the economy as a whole (a score of 2). Adding these numbers gives Korea a score of 8 on the geographic coverage index.  Read more aboutthe &quot;Geographic coverage indexMethodology&quot;</dct:description>
    <dct:identifier>WB-DB-RP-QLA-GEOCOVER.INDEX</dct:identifier>
    <schema:about rdf:resource="http://aims.fao.org/aos/agrovoc/c_9000098" />
    <schema:about rdf:resource="http://data.landportal.info/voc/landvoc/theme/T-INST" />
    <schema:about rdf:resource="http://data.landportal.info/voc/landvoc/theme/T-INVEST" />
    <schema:about rdf:resource="http://data.landportal.info/voc/landvoc/overarching-category/OA-USE" />
    <dct:source rdf:resource="http://data.landportal.info/dataset/WB-DB" />
    <skos:definition>The geographic coverage index has four components: How complete the coverage of the land registry is at the level of the largest business city. A score of 2 is assigned if all privately held land plots in the city are formally registered at the land registry; 0 if not. How complete the coverage of the land registry is at the level of the economy. A score of 2 is assigned if all privately held land plots in the economy are formally registered at the land registry; 0 if not. How complete the coverage of the mapping agency is at the level of the largest business city. A score of 2 is assigned if all privately held land plots in the city are mapped; 0 if not. How complete the coverage of the mapping agency is at the level of the economy. A score of 2 is assigned if all privately held land plots in the economy are mapped; 0 if not. The index ranges from 0 to 8, with higher values indicating greater geographic coverage in land ownership registration and cadastral mapping. In the Republic of Korea, for example, all privately held land plots are formally registered at the land registry in Seoul (a score of 2) and in the economy as a whole (a score of 2). In addition, all privately held land plots are mapped in Seoul (a score of 2) and in the economy as a whole (a score of 2). Adding these numbers gives Korea a score of 8 on the geographic coverage index.  Read more aboutthe &quot;Geographic coverage indexMethodology&quot;</skos:definition>
    <sdmx-attribute:unitMeasure>Index (0; 8)</sdmx-attribute:unitMeasure>
  </rdf:Description>
  <rdf:Description rdf:about="http://data.landportal.info/indicator/WB-DB-RP-QLA-INFRA.INDEX">
    <rdf:type rdf:resource="http://purl.org/weso/ontology/computex#Indicator" />
    <rdf:type rdf:resource="http://www.w3.org/2004/02/skos/core#Concept" />
    <rdfs:label>Reliability of infrastructure index (Quality of land administration index - Doing Business)</rdfs:label>
    <rdfs:comment>The reliability of infrastructure index has six components: How land titles are kept at the registry of the largest business city of the economy. A score of 2 is assigned if the majority of land titles are fully digital; 1 if the majority are scanned; 0 if the majority are kept in paper format. Whether there is an electronic database for checking for encumbrances. A score of 1 is assigned if yes; 0 if no. How maps of land plots are kept at the mapping agency of the largest business city of the economy. A score of 2 is assigned if the majority of maps are fully digital; 1 if the majority are scanned; 0 if the majority are kept in paper format. Whether there is a geographic information systeman electronic database for recording boundaries, checking plans and providing cadastral information. A score of 1 is assigned if yes; 0 if no. How the land ownership registry and mapping agency are linked. A score of 1 is assigned if information about land ownership and maps are kept in a single database or in linked databases; 0 if there is no connection between the different databases. How immovable property is identified. A score of 1 is assigned if there is a unique number to identify properties for the majority of land plots; 0 if there are multiple identifiers. The index ranges from 0 to 8, with higher values indicating a higher quality of infrastructure for ensuring the reliability of information on property titles and boundaries. In Turkey, for example, the land registry offices in Istanbul maintain titles in a fully digital format (a score of 2) and have a fully electronic database to check for encumbrances (a score of 1). The Cadastral Directorate offices in Istanbul have digital maps (a score of 2), and the Geographical Information Directorate has a public portal allowing users to check the plans and cadastral information on parcels along with satellite images (a score of 1). Databases about land ownership and maps are linked to each other through the TAKBIS system, an integrated information system for the land registry offices and cadastral offices (a score of 1). Finally, there is a unique identifying number for properties (a score of 1). Adding these numbers gives Turkey a score of 8 on the reliability of infrastructure index.  Read more aboutthe &quot;Reliability of infrastructure index Methodology&quot;</rdfs:comment>
    <rdfs:seeAlso rdf:resource="https://landportal.org/book/indicator/wb-db-rp-qla-infraindex" />
    <skos:notation>WB-DB-RP-QLA-INFRA.INDEX</skos:notation>
    <skos:inScheme rdf:resource="http://data.landportal.info/vocabulary/25" />
    <skos:prefLabel>Reliability of infrastructure index (Quality of land administration index - Doing Business)</skos:prefLabel>
    <dct:subject rdf:resource="http://aims.fao.org/aos/agrovoc/c_9000098" />
    <dct:subject rdf:resource="http://data.landportal.info/voc/landvoc/overarching-category/OA-USE" />
    <dct:subject rdf:resource="http://data.landportal.info/voc/landvoc/theme/T-INVEST" />
    <dct:subject rdf:resource="http://data.landportal.info/voc/landvoc/theme/T-INST" />
    <dct:title>Reliability of infrastructure index (Quality of land administration index - Doing Business)</dct:title>
    <dct:description>The reliability of infrastructure index has six components: How land titles are kept at the registry of the largest business city of the economy. A score of 2 is assigned if the majority of land titles are fully digital; 1 if the majority are scanned; 0 if the majority are kept in paper format. Whether there is an electronic database for checking for encumbrances. A score of 1 is assigned if yes; 0 if no. How maps of land plots are kept at the mapping agency of the largest business city of the economy. A score of 2 is assigned if the majority of maps are fully digital; 1 if the majority are scanned; 0 if the majority are kept in paper format. Whether there is a geographic information systeman electronic database for recording boundaries, checking plans and providing cadastral information. A score of 1 is assigned if yes; 0 if no. How the land ownership registry and mapping agency are linked. A score of 1 is assigned if information about land ownership and maps are kept in a single database or in linked databases; 0 if there is no connection between the different databases. How immovable property is identified. A score of 1 is assigned if there is a unique number to identify properties for the majority of land plots; 0 if there are multiple identifiers. The index ranges from 0 to 8, with higher values indicating a higher quality of infrastructure for ensuring the reliability of information on property titles and boundaries. In Turkey, for example, the land registry offices in Istanbul maintain titles in a fully digital format (a score of 2) and have a fully electronic database to check for encumbrances (a score of 1). The Cadastral Directorate offices in Istanbul have digital maps (a score of 2), and the Geographical Information Directorate has a public portal allowing users to check the plans and cadastral information on parcels along with satellite images (a score of 1). Databases about land ownership and maps are linked to each other through the TAKBIS system, an integrated information system for the land registry offices and cadastral offices (a score of 1). Finally, there is a unique identifying number for properties (a score of 1). Adding these numbers gives Turkey a score of 8 on the reliability of infrastructure index.  Read more aboutthe &quot;Reliability of infrastructure index Methodology&quot;</dct:description>
    <dct:identifier>WB-DB-RP-QLA-INFRA.INDEX</dct:identifier>
    <schema:about rdf:resource="http://aims.fao.org/aos/agrovoc/c_9000098" />
    <schema:about rdf:resource="http://data.landportal.info/voc/landvoc/theme/T-INVEST" />
    <schema:about rdf:resource="http://data.landportal.info/voc/landvoc/overarching-category/OA-USE" />
    <schema:about rdf:resource="http://data.landportal.info/voc/landvoc/theme/T-INST" />
    <dct:source rdf:resource="http://data.landportal.info/dataset/WB-DB" />
    <skos:definition>The reliability of infrastructure index has six components: How land titles are kept at the registry of the largest business city of the economy. A score of 2 is assigned if the majority of land titles are fully digital; 1 if the majority are scanned; 0 if the majority are kept in paper format. Whether there is an electronic database for checking for encumbrances. A score of 1 is assigned if yes; 0 if no. How maps of land plots are kept at the mapping agency of the largest business city of the economy. A score of 2 is assigned if the majority of maps are fully digital; 1 if the majority are scanned; 0 if the majority are kept in paper format. Whether there is a geographic information systeman electronic database for recording boundaries, checking plans and providing cadastral information. A score of 1 is assigned if yes; 0 if no. How the land ownership registry and mapping agency are linked. A score of 1 is assigned if information about land ownership and maps are kept in a single database or in linked databases; 0 if there is no connection between the different databases. How immovable property is identified. A score of 1 is assigned if there is a unique number to identify properties for the majority of land plots; 0 if there are multiple identifiers. The index ranges from 0 to 8, with higher values indicating a higher quality of infrastructure for ensuring the reliability of information on property titles and boundaries. In Turkey, for example, the land registry offices in Istanbul maintain titles in a fully digital format (a score of 2) and have a fully electronic database to check for encumbrances (a score of 1). The Cadastral Directorate offices in Istanbul have digital maps (a score of 2), and the Geographical Information Directorate has a public portal allowing users to check the plans and cadastral information on parcels along with satellite images (a score of 1). Databases about land ownership and maps are linked to each other through the TAKBIS system, an integrated information system for the land registry offices and cadastral offices (a score of 1). Finally, there is a unique identifying number for properties (a score of 1). Adding these numbers gives Turkey a score of 8 on the reliability of infrastructure index.  Read more aboutthe &quot;Reliability of infrastructure index Methodology&quot;</skos:definition>
    <sdmx-attribute:unitMeasure>Index (0; 8)</sdmx-attribute:unitMeasure>
  </rdf:Description>
  <rdf:Description rdf:about="http://data.landportal.info/indicator/WB-DB-RP-QLA-LDR.INDEX">
    <rdf:type rdf:resource="http://purl.org/weso/ontology/computex#Indicator" />
    <rdf:type rdf:resource="http://www.w3.org/2004/02/skos/core#Concept" />
    <rdfs:label>Land dispute resolution index (Quality of land administration index - Doing Business)</rdfs:label>
    <rdfs:comment>The land dispute resolution index assesses the legal framework for immovable property registration and the accessibility of dispute resolution mechanisms. The index has eight components: Whether the law requires that all property sale transactions be registered at the immovable property registry to make them opposable to third parties. A score of 1.5 is assigned if yes; 0 if no. Whether the formal system of immovable property registration is subject to a guarantee. A score of 0.5 is assigned if either a state or private guarantee over immovable property registration is required by law; 0 if no such guarantee is required. Whether there is a specific compensation mechanism to cover for losses incurred by parties who engaged in good faith in a property transaction based on erroneous information certified by the immovable property registry. A score of 0.5 is assigned if yes; 0 if no. Whether the legal system requires verification of the legal validity of the documents necessary for a property transaction. A score of 0.5 is assigned if there is a review of legal validity, either by the registrar or by a professional (such as a notary or alawyer); 0 if there is no review. Whether the legal system requires verification of the identity of the parties to a property transaction. A score of 0.5 is assigned if there is verification of identity, either by the registrar or by a professional (such as a notary or a lawyer); 0 if there is no verification. Whether there is a national database to verify the accuracy of identity documents. A score of 1 is assigned if such a national database is available; 0 if not. How much time it takes to obtain a decision from a court of first instance (without an appeal) in a standard land dispute between two local businesses over tenure rights worth 50 times income per capita and located in the largest business city. A score of 3 is assigned if it takes less than one year; 2 if it takes between one and two years; 1 if it takes between two and three years; 0 if it takes more than three years. Whether there are publicly available statistics on the number of land disputes in the first instance. A score of 0.5 is assigned if statistics are published about land disputes in the economy in the past calendar year; 0 if no such statistics are made publicly available. The index ranges from 0 to 8, with higher values indicating greater protection against land disputes. In Lithuania, for example, according to the Civil Code and the Law on the Real Property Register, property transactions must be registered at the land registry to make them opposable to third parties (a score of 1.5). The property transfer system is guaranteed by the state (a score of 0.5) and has a compensation mechanism to coverlosses incurred by parties who engaged in good faith in a property transaction based on an error by the registry (a score of 0.5). A notary verifies the legal validity of the documents in a property transaction (a score of 0.5) and the identity of the parties (a score of 0.5), in accordance with the Law on the Notary Office (Law I-2882). Lithuania has a national database to verify the accuracy of identity documents (a score of 1). In a land dispute between two Lithuanian companies over the tenure rights of a property worth $770,000, the Vilnius District Court gives a decision in less than one year (a score of 3). Finally, statistics about land disputes are collected and published; there were a total of 549 land disputes in the country in 2016 (a score of 0.5). Adding these numbers gives Lithuania a score of 8 on the land dispute resolution index. Read more aboutthe &quot;Land dispute resolution indexMethodology&quot;</rdfs:comment>
    <rdfs:seeAlso rdf:resource="https://landportal.org/book/indicator/wb-db-rp-qla-ldrindex" />
    <skos:notation>WB-DB-RP-QLA-LDR.INDEX</skos:notation>
    <skos:inScheme rdf:resource="http://data.landportal.info/vocabulary/25" />
    <skos:prefLabel>Land dispute resolution index (Quality of land administration index - Doing Business)</skos:prefLabel>
    <dct:subject rdf:resource="http://aims.fao.org/aos/agrovoc/c_9000098" />
    <dct:subject rdf:resource="http://data.landportal.info/voc/landvoc/overarching-category/OA-USE" />
    <dct:subject rdf:resource="http://data.landportal.info/voc/landvoc/theme/T-INVEST" />
    <dct:subject rdf:resource="http://data.landportal.info/voc/landvoc/theme/T-INST" />
    <dct:title>Land dispute resolution index (Quality of land administration index - Doing Business)</dct:title>
    <dct:description>The land dispute resolution index assesses the legal framework for immovable property registration and the accessibility of dispute resolution mechanisms. The index has eight components: Whether the law requires that all property sale transactions be registered at the immovable property registry to make them opposable to third parties. A score of 1.5 is assigned if yes; 0 if no. Whether the formal system of immovable property registration is subject to a guarantee. A score of 0.5 is assigned if either a state or private guarantee over immovable property registration is required by law; 0 if no such guarantee is required. Whether there is a specific compensation mechanism to cover for losses incurred by parties who engaged in good faith in a property transaction based on erroneous information certified by the immovable property registry. A score of 0.5 is assigned if yes; 0 if no. Whether the legal system requires verification of the legal validity of the documents necessary for a property transaction. A score of 0.5 is assigned if there is a review of legal validity, either by the registrar or by a professional (such as a notary or alawyer); 0 if there is no review. Whether the legal system requires verification of the identity of the parties to a property transaction. A score of 0.5 is assigned if there is verification of identity, either by the registrar or by a professional (such as a notary or a lawyer); 0 if there is no verification. Whether there is a national database to verify the accuracy of identity documents. A score of 1 is assigned if such a national database is available; 0 if not. How much time it takes to obtain a decision from a court of first instance (without an appeal) in a standard land dispute between two local businesses over tenure rights worth 50 times income per capita and located in the largest business city. A score of 3 is assigned if it takes less than one year; 2 if it takes between one and two years; 1 if it takes between two and three years; 0 if it takes more than three years. Whether there are publicly available statistics on the number of land disputes in the first instance. A score of 0.5 is assigned if statistics are published about land disputes in the economy in the past calendar year; 0 if no such statistics are made publicly available. The index ranges from 0 to 8, with higher values indicating greater protection against land disputes. In Lithuania, for example, according to the Civil Code and the Law on the Real Property Register, property transactions must be registered at the land registry to make them opposable to third parties (a score of 1.5). The property transfer system is guaranteed by the state (a score of 0.5) and has a compensation mechanism to coverlosses incurred by parties who engaged in good faith in a property transaction based on an error by the registry (a score of 0.5). A notary verifies the legal validity of the documents in a property transaction (a score of 0.5) and the identity of the parties (a score of 0.5), in accordance with the Law on the Notary Office (Law I-2882). Lithuania has a national database to verify the accuracy of identity documents (a score of 1). In a land dispute between two Lithuanian companies over the tenure rights of a property worth $770,000, the Vilnius District Court gives a decision in less than one year (a score of 3). Finally, statistics about land disputes are collected and published; there were a total of 549 land disputes in the country in 2016 (a score of 0.5). Adding these numbers gives Lithuania a score of 8 on the land dispute resolution index. Read more aboutthe &quot;Land dispute resolution indexMethodology&quot;</dct:description>
    <dct:identifier>WB-DB-RP-QLA-LDR.INDEX</dct:identifier>
    <schema:about rdf:resource="http://aims.fao.org/aos/agrovoc/c_9000098" />
    <schema:about rdf:resource="http://data.landportal.info/voc/landvoc/theme/T-INVEST" />
    <schema:about rdf:resource="http://data.landportal.info/voc/landvoc/overarching-category/OA-USE" />
    <schema:about rdf:resource="http://data.landportal.info/voc/landvoc/theme/T-INST" />
    <dct:source rdf:resource="http://data.landportal.info/dataset/WB-DB" />
    <skos:definition>The land dispute resolution index assesses the legal framework for immovable property registration and the accessibility of dispute resolution mechanisms. The index has eight components: Whether the law requires that all property sale transactions be registered at the immovable property registry to make them opposable to third parties. A score of 1.5 is assigned if yes; 0 if no. Whether the formal system of immovable property registration is subject to a guarantee. A score of 0.5 is assigned if either a state or private guarantee over immovable property registration is required by law; 0 if no such guarantee is required. Whether there is a specific compensation mechanism to cover for losses incurred by parties who engaged in good faith in a property transaction based on erroneous information certified by the immovable property registry. A score of 0.5 is assigned if yes; 0 if no. Whether the legal system requires verification of the legal validity of the documents necessary for a property transaction. A score of 0.5 is assigned if there is a review of legal validity, either by the registrar or by a professional (such as a notary or alawyer); 0 if there is no review. Whether the legal system requires verification of the identity of the parties to a property transaction. A score of 0.5 is assigned if there is verification of identity, either by the registrar or by a professional (such as a notary or a lawyer); 0 if there is no verification. Whether there is a national database to verify the accuracy of identity documents. A score of 1 is assigned if such a national database is available; 0 if not. How much time it takes to obtain a decision from a court of first instance (without an appeal) in a standard land dispute between two local businesses over tenure rights worth 50 times income per capita and located in the largest business city. A score of 3 is assigned if it takes less than one year; 2 if it takes between one and two years; 1 if it takes between two and three years; 0 if it takes more than three years. Whether there are publicly available statistics on the number of land disputes in the first instance. A score of 0.5 is assigned if statistics are published about land disputes in the economy in the past calendar year; 0 if no such statistics are made publicly available. The index ranges from 0 to 8, with higher values indicating greater protection against land disputes. In Lithuania, for example, according to the Civil Code and the Law on the Real Property Register, property transactions must be registered at the land registry to make them opposable to third parties (a score of 1.5). The property transfer system is guaranteed by the state (a score of 0.5) and has a compensation mechanism to coverlosses incurred by parties who engaged in good faith in a property transaction based on an error by the registry (a score of 0.5). A notary verifies the legal validity of the documents in a property transaction (a score of 0.5) and the identity of the parties (a score of 0.5), in accordance with the Law on the Notary Office (Law I-2882). Lithuania has a national database to verify the accuracy of identity documents (a score of 1). In a land dispute between two Lithuanian companies over the tenure rights of a property worth $770,000, the Vilnius District Court gives a decision in less than one year (a score of 3). Finally, statistics about land disputes are collected and published; there were a total of 549 land disputes in the country in 2016 (a score of 0.5). Adding these numbers gives Lithuania a score of 8 on the land dispute resolution index. Read more aboutthe &quot;Land dispute resolution indexMethodology&quot;</skos:definition>
    <sdmx-attribute:unitMeasure>Index (0; 8)</sdmx-attribute:unitMeasure>
  </rdf:Description>
  <rdf:Description rdf:about="http://data.landportal.info/indicator/WB-DB-RP-QLA-TRANSP.INDEX">
    <rdf:type rdf:resource="http://purl.org/weso/ontology/computex#Indicator" />
    <rdf:type rdf:resource="http://www.w3.org/2004/02/skos/core#Concept" />
    <rdfs:label>Transparency of information index (Quality of land administration index - Doing Business)</rdfs:label>
    <rdfs:comment>The transparency of information index has 10 components: Whether information on land ownership is made publicly available. A score of 1 is assigned if information on land ownership is accessible by anyone; 0 if access is restricted.  Whether the list of documents required for completingthe registration ofproperty transactions is made publicly available. A score of 0.5 is assigned if the list of documents is accessible online or on a public board; 0 if it is not made available to the public or if it can be obtained only in person. Whether the fee schedule for completing the registration of property transactions is made publicly available. A score of 0.5 is assigned if the fee schedule is accessible online or on a public board or is free of charge; 0 if it is not made available to the public or if it can be obtained only in person. Whether the agency in charge of immovable property registration commits to delivering a legally binding document that proves property ownership within a specific time frame. A score of 0.5 is assigned if the service standard is accessible online or on a public board; 0 if it is not made available to the public or if it can be obtained only in person. Whether there is a specific and separate mechanism for filing complaints about a problem that occurred at the agency in charge of immovable property registration. A score of 1 is assigned if there is a specific and separate mechanism for filing a complaint; 0 if there is only a general mechanism or no mechanism. Whether there are publicly available official statistics tracking the number of transactions at the immovable property registration agency. A score of 0.5 is assigned if statistics are published about property transfers in the largest business city in the past calendar year at the latest on June 1st of the following year; 0 if no such statistics are made publicly available. Whether maps of land plots are made publicly available. A score of 0.5 is assigned if maps are accessible by anyone; 0 if access is restricted. Whether the fee schedule for accessing maps is made publicly available. A score of 0.5 is assigned if the fee schedule is accessible online or on a public board or free of charge; 0 if it is not made available to the public or if it can be obtained only in person. Whether the mapping agency commits to delivering an updated map within a specific time frame. A score of 0.5 is assigned if the service standard is accessible online or on a public board; 0 if it is not made available to the public or if it can be obtained only in person. Whether there is a specific and separate mechanism for filing complaints about a problem that occurred at the mapping agency. A score of 0.5 is assigned if there is a specific and separate mechanism for filing a complaint; 0 if there is only a general mechanism or no mechanism. The index ranges from 0 to 6, with higher values indicating greater transparency in the land administration system. In the Netherlands, for example, anyone who pays a fee can consult the land ownership database (a score of 1). Information can be obtained at the office, by mail or online using the Kadaster website (http://www.kadaster.nl). Anyone can also get information online about the list of documents to submit for property registration (a score of 0.5), the fee schedule for registration (a score of 0.5) and the service standards (a score of 0.5). And anyone facing a problem at the land registry can file a complaint or report an error by filling out a specific form online (a score of 1). In addition, the Kadaster makes statistics about land transactions available to the public, reporting a total of 214,793 property transfers in Amsterdam in 2016 (a score of 0.5). Moreover, anyone who pays a fee can consult online cadastral maps (a score of 0.5). It is also possible to get public access to the fee schedule for map consultation (a score of 0.5), the service standards for delivery of an updated plan (a score of 0.5) and a specific mechanism for filing a complaint about a map (a score of 0.5). Adding these numbers gives the Netherlands a score of 6 on the transparency of information index.  Read more aboutthe &quot;Transparency of information index Methodology&quot;</rdfs:comment>
    <rdfs:seeAlso rdf:resource="https://landportal.org/book/indicator/wb-db-rp-qla-transpindex" />
    <skos:notation>WB-DB-RP-QLA-TRANSP.INDEX</skos:notation>
    <skos:inScheme rdf:resource="http://data.landportal.info/vocabulary/25" />
    <skos:prefLabel>Transparency of information index (Quality of land administration index - Doing Business)</skos:prefLabel>
    <dct:subject rdf:resource="http://aims.fao.org/aos/agrovoc/c_9000098" />
    <dct:subject rdf:resource="http://data.landportal.info/voc/landvoc/overarching-category/OA-USE" />
    <dct:subject rdf:resource="http://data.landportal.info/voc/landvoc/theme/T-INVEST" />
    <dct:subject rdf:resource="http://data.landportal.info/voc/landvoc/theme/T-INST" />
    <dct:title>Transparency of information index (Quality of land administration index - Doing Business)</dct:title>
    <dct:description>The transparency of information index has 10 components: Whether information on land ownership is made publicly available. A score of 1 is assigned if information on land ownership is accessible by anyone; 0 if access is restricted.  Whether the list of documents required for completingthe registration ofproperty transactions is made publicly available. A score of 0.5 is assigned if the list of documents is accessible online or on a public board; 0 if it is not made available to the public or if it can be obtained only in person. Whether the fee schedule for completing the registration of property transactions is made publicly available. A score of 0.5 is assigned if the fee schedule is accessible online or on a public board or is free of charge; 0 if it is not made available to the public or if it can be obtained only in person. Whether the agency in charge of immovable property registration commits to delivering a legally binding document that proves property ownership within a specific time frame. A score of 0.5 is assigned if the service standard is accessible online or on a public board; 0 if it is not made available to the public or if it can be obtained only in person. Whether there is a specific and separate mechanism for filing complaints about a problem that occurred at the agency in charge of immovable property registration. A score of 1 is assigned if there is a specific and separate mechanism for filing a complaint; 0 if there is only a general mechanism or no mechanism. Whether there are publicly available official statistics tracking the number of transactions at the immovable property registration agency. A score of 0.5 is assigned if statistics are published about property transfers in the largest business city in the past calendar year at the latest on June 1st of the following year; 0 if no such statistics are made publicly available. Whether maps of land plots are made publicly available. A score of 0.5 is assigned if maps are accessible by anyone; 0 if access is restricted. Whether the fee schedule for accessing maps is made publicly available. A score of 0.5 is assigned if the fee schedule is accessible online or on a public board or free of charge; 0 if it is not made available to the public or if it can be obtained only in person. Whether the mapping agency commits to delivering an updated map within a specific time frame. A score of 0.5 is assigned if the service standard is accessible online or on a public board; 0 if it is not made available to the public or if it can be obtained only in person. Whether there is a specific and separate mechanism for filing complaints about a problem that occurred at the mapping agency. A score of 0.5 is assigned if there is a specific and separate mechanism for filing a complaint; 0 if there is only a general mechanism or no mechanism. The index ranges from 0 to 6, with higher values indicating greater transparency in the land administration system. In the Netherlands, for example, anyone who pays a fee can consult the land ownership database (a score of 1). Information can be obtained at the office, by mail or online using the Kadaster website (http://www.kadaster.nl). Anyone can also get information online about the list of documents to submit for property registration (a score of 0.5), the fee schedule for registration (a score of 0.5) and the service standards (a score of 0.5). And anyone facing a problem at the land registry can file a complaint or report an error by filling out a specific form online (a score of 1). In addition, the Kadaster makes statistics about land transactions available to the public, reporting a total of 214,793 property transfers in Amsterdam in 2016 (a score of 0.5). Moreover, anyone who pays a fee can consult online cadastral maps (a score of 0.5). It is also possible to get public access to the fee schedule for map consultation (a score of 0.5), the service standards for delivery of an updated plan (a score of 0.5) and a specific mechanism for filing a complaint about a map (a score of 0.5). Adding these numbers gives the Netherlands a score of 6 on the transparency of information index.  Read more aboutthe &quot;Transparency of information index Methodology&quot;</dct:description>
    <dct:identifier>WB-DB-RP-QLA-TRANSP.INDEX</dct:identifier>
    <schema:about rdf:resource="http://aims.fao.org/aos/agrovoc/c_9000098" />
    <schema:about rdf:resource="http://data.landportal.info/voc/landvoc/theme/T-INVEST" />
    <schema:about rdf:resource="http://data.landportal.info/voc/landvoc/overarching-category/OA-USE" />
    <schema:about rdf:resource="http://data.landportal.info/voc/landvoc/theme/T-INST" />
    <dct:source rdf:resource="http://data.landportal.info/dataset/WB-DB" />
    <skos:definition>The transparency of information index has 10 components: Whether information on land ownership is made publicly available. A score of 1 is assigned if information on land ownership is accessible by anyone; 0 if access is restricted.  Whether the list of documents required for completingthe registration ofproperty transactions is made publicly available. A score of 0.5 is assigned if the list of documents is accessible online or on a public board; 0 if it is not made available to the public or if it can be obtained only in person. Whether the fee schedule for completing the registration of property transactions is made publicly available. A score of 0.5 is assigned if the fee schedule is accessible online or on a public board or is free of charge; 0 if it is not made available to the public or if it can be obtained only in person. Whether the agency in charge of immovable property registration commits to delivering a legally binding document that proves property ownership within a specific time frame. A score of 0.5 is assigned if the service standard is accessible online or on a public board; 0 if it is not made available to the public or if it can be obtained only in person. Whether there is a specific and separate mechanism for filing complaints about a problem that occurred at the agency in charge of immovable property registration. A score of 1 is assigned if there is a specific and separate mechanism for filing a complaint; 0 if there is only a general mechanism or no mechanism. Whether there are publicly available official statistics tracking the number of transactions at the immovable property registration agency. A score of 0.5 is assigned if statistics are published about property transfers in the largest business city in the past calendar year at the latest on June 1st of the following year; 0 if no such statistics are made publicly available. Whether maps of land plots are made publicly available. A score of 0.5 is assigned if maps are accessible by anyone; 0 if access is restricted. Whether the fee schedule for accessing maps is made publicly available. A score of 0.5 is assigned if the fee schedule is accessible online or on a public board or free of charge; 0 if it is not made available to the public or if it can be obtained only in person. Whether the mapping agency commits to delivering an updated map within a specific time frame. A score of 0.5 is assigned if the service standard is accessible online or on a public board; 0 if it is not made available to the public or if it can be obtained only in person. Whether there is a specific and separate mechanism for filing complaints about a problem that occurred at the mapping agency. A score of 0.5 is assigned if there is a specific and separate mechanism for filing a complaint; 0 if there is only a general mechanism or no mechanism. The index ranges from 0 to 6, with higher values indicating greater transparency in the land administration system. In the Netherlands, for example, anyone who pays a fee can consult the land ownership database (a score of 1). Information can be obtained at the office, by mail or online using the Kadaster website (http://www.kadaster.nl). Anyone can also get information online about the list of documents to submit for property registration (a score of 0.5), the fee schedule for registration (a score of 0.5) and the service standards (a score of 0.5). And anyone facing a problem at the land registry can file a complaint or report an error by filling out a specific form online (a score of 1). In addition, the Kadaster makes statistics about land transactions available to the public, reporting a total of 214,793 property transfers in Amsterdam in 2016 (a score of 0.5). Moreover, anyone who pays a fee can consult online cadastral maps (a score of 0.5). It is also possible to get public access to the fee schedule for map consultation (a score of 0.5), the service standards for delivery of an updated plan (a score of 0.5) and a specific mechanism for filing a complaint about a map (a score of 0.5). Adding these numbers gives the Netherlands a score of 6 on the transparency of information index.  Read more aboutthe &quot;Transparency of information index Methodology&quot;</skos:definition>
    <sdmx-attribute:unitMeasure>Index (0; 6)</sdmx-attribute:unitMeasure>
  </rdf:Description>
  <rdf:Description rdf:about="http://data.landportal.info/indicator/WB-DB-RP-QLA.DTF">
    <rdf:type rdf:resource="http://purl.org/weso/ontology/computex#Indicator" />
    <rdf:type rdf:resource="http://www.w3.org/2004/02/skos/core#Concept" />
    <rdfs:label>Quality of land administration index (Doing Business) - Distance To Frontier</rdfs:label>
    <rdfs:comment>This is thedistance to frontier score of the indicator Quality of land administration index(thatranges from 0 to 30, with higher values indicating better quality of the land administration system) The distance to frontier score helps assess the absolute level of regulatory performance over time. It measures the distance of each economy to the frontier, which represents the best performance observed on each of the indicators across all economies in the Doing Business sample since 2005. One can both see the gap between a particular economys performance and the best performance at any point in time and assess the absolute change in the economys regulatory environment over time as measured by Doing Business. An economys distance to frontier is reflected on a scale from 0 to 100, where 0 represents the lowest performance and 100 represents the frontier. Read more aboutthe &quot;Quality of land administration index Methodology&quot;</rdfs:comment>
    <rdfs:seeAlso rdf:resource="https://landportal.org/book/indicator/wb-db-rp-qladtf" />
    <skos:notation>WB-DB-RP-QLA.DTF</skos:notation>
    <skos:inScheme rdf:resource="http://data.landportal.info/vocabulary/25" />
    <skos:prefLabel>Quality of land administration index (Doing Business) - Distance To Frontier</skos:prefLabel>
    <dct:subject rdf:resource="http://aims.fao.org/aos/agrovoc/c_9000098" />
    <dct:subject rdf:resource="http://data.landportal.info/voc/landvoc/overarching-category/OA-USE" />
    <dct:subject rdf:resource="http://data.landportal.info/voc/landvoc/theme/T-INVEST" />
    <dct:subject rdf:resource="http://data.landportal.info/voc/landvoc/theme/T-INST" />
    <dct:title>Quality of land administration index (Doing Business) - Distance To Frontier</dct:title>
    <dct:description>This is thedistance to frontier score of the indicator Quality of land administration index(thatranges from 0 to 30, with higher values indicating better quality of the land administration system) The distance to frontier score helps assess the absolute level of regulatory performance over time. It measures the distance of each economy to the frontier, which represents the best performance observed on each of the indicators across all economies in the Doing Business sample since 2005. One can both see the gap between a particular economys performance and the best performance at any point in time and assess the absolute change in the economys regulatory environment over time as measured by Doing Business. An economys distance to frontier is reflected on a scale from 0 to 100, where 0 represents the lowest performance and 100 represents the frontier. Read more aboutthe &quot;Quality of land administration index Methodology&quot;</dct:description>
    <dct:identifier>WB-DB-RP-QLA.DTF</dct:identifier>
    <schema:about rdf:resource="http://aims.fao.org/aos/agrovoc/c_9000098" />
    <schema:about rdf:resource="http://data.landportal.info/voc/landvoc/theme/T-INVEST" />
    <schema:about rdf:resource="http://data.landportal.info/voc/landvoc/overarching-category/OA-USE" />
    <schema:about rdf:resource="http://data.landportal.info/voc/landvoc/theme/T-INST" />
    <dct:source rdf:resource="http://data.landportal.info/dataset/WB-DB" />
    <skos:definition>This is thedistance to frontier score of the indicator Quality of land administration index(thatranges from 0 to 30, with higher values indicating better quality of the land administration system) The distance to frontier score helps assess the absolute level of regulatory performance over time. It measures the distance of each economy to the frontier, which represents the best performance observed on each of the indicators across all economies in the Doing Business sample since 2005. One can both see the gap between a particular economys performance and the best performance at any point in time and assess the absolute change in the economys regulatory environment over time as measured by Doing Business. An economys distance to frontier is reflected on a scale from 0 to 100, where 0 represents the lowest performance and 100 represents the frontier. Read more aboutthe &quot;Quality of land administration index Methodology&quot;</skos:definition>
    <sdmx-attribute:unitMeasure>Index (0; 100)</sdmx-attribute:unitMeasure>
  </rdf:Description>
  <rdf:Description rdf:about="http://data.landportal.info/indicator/WB-DB-RP-QLA.INDEX">
    <rdf:type rdf:resource="http://purl.org/weso/ontology/computex#Indicator" />
    <rdf:type rdf:resource="http://www.w3.org/2004/02/skos/core#Concept" />
    <rdfs:label>Quality of land administration index (Doing Business)</rdfs:label>
    <rdfs:comment>The quality of land administration index is composed of five other indices: the reliability of infrastructure transparency of information geographic coverage land dispute resolution equal access to property rights. Data are collected for each economys largest business city. For 11 economies the data are also collected for the second largest business city. The index ranges from 0 to 30, with higher values indicating better quality of the land administration system. If private sector entities were unable to register property transfers in an economy between June 2016 and June 2017, the economy receives a no practice mark on the procedures, time and cost indicators. A no practice economy receives a score of 0 on the quality of land administration index even if its legal framework includes provisions related to land administration. Read more aboutthe &quot;Quality of land administration index Methodology&quot;</rdfs:comment>
    <rdfs:seeAlso rdf:resource="https://landportal.org/book/indicator/wb-db-rp-qlaindex" />
    <skos:notation>WB-DB-RP-QLA.INDEX</skos:notation>
    <skos:inScheme rdf:resource="http://data.landportal.info/vocabulary/25" />
    <skos:prefLabel>Quality of land administration index (Doing Business)</skos:prefLabel>
    <dct:subject rdf:resource="http://aims.fao.org/aos/agrovoc/c_9000098" />
    <dct:subject rdf:resource="http://data.landportal.info/voc/landvoc/theme/T-INST" />
    <dct:subject rdf:resource="http://data.landportal.info/voc/landvoc/overarching-category/OA-USE" />
    <dct:subject rdf:resource="http://data.landportal.info/voc/landvoc/theme/T-INVEST" />
    <dct:title>Quality of land administration index (Doing Business)</dct:title>
    <dct:description>The quality of land administration index is composed of five other indices: the reliability of infrastructure transparency of information geographic coverage land dispute resolution equal access to property rights. Data are collected for each economys largest business city. For 11 economies the data are also collected for the second largest business city. The index ranges from 0 to 30, with higher values indicating better quality of the land administration system. If private sector entities were unable to register property transfers in an economy between June 2016 and June 2017, the economy receives a no practice mark on the procedures, time and cost indicators. A no practice economy receives a score of 0 on the quality of land administration index even if its legal framework includes provisions related to land administration. Read more aboutthe &quot;Quality of land administration index Methodology&quot;</dct:description>
    <dct:identifier>WB-DB-RP-QLA.INDEX</dct:identifier>
    <schema:about rdf:resource="http://aims.fao.org/aos/agrovoc/c_9000098" />
    <schema:about rdf:resource="http://data.landportal.info/voc/landvoc/theme/T-INST" />
    <schema:about rdf:resource="http://data.landportal.info/voc/landvoc/theme/T-INVEST" />
    <schema:about rdf:resource="http://data.landportal.info/voc/landvoc/overarching-category/OA-USE" />
    <dct:source rdf:resource="http://data.landportal.info/dataset/WB-DB" />
    <skos:definition>The quality of land administration index is composed of five other indices: the reliability of infrastructure transparency of information geographic coverage land dispute resolution equal access to property rights. Data are collected for each economys largest business city. For 11 economies the data are also collected for the second largest business city. The index ranges from 0 to 30, with higher values indicating better quality of the land administration system. If private sector entities were unable to register property transfers in an economy between June 2016 and June 2017, the economy receives a no practice mark on the procedures, time and cost indicators. A no practice economy receives a score of 0 on the quality of land administration index even if its legal framework includes provisions related to land administration. Read more aboutthe &quot;Quality of land administration index Methodology&quot;</skos:definition>
    <sdmx-attribute:unitMeasure>Index (0; 30)</sdmx-attribute:unitMeasure>
  </rdf:Description>
  <rdf:Description rdf:about="http://data.landportal.info/indicator/WB-DB-RP.DTF">
    <rdf:type rdf:resource="http://purl.org/weso/ontology/computex#Indicator" />
    <rdf:type rdf:resource="http://www.w3.org/2004/02/skos/core#Concept" />
    <rdfs:label>Registering property (Doing Business) - Distance To Frontier</rdfs:label>
    <rdfs:comment>Doing Business records the full sequence of procedures necessary for a business (the buyer) to purchase a property from another business (the seller) and to transfer the property title to the buyers name so that the buyer can use the property for expanding its business, use the property as collateral in taking new loans or, if necessary, sell the property to another business. It also measures the time and cost to complete each of these procedures. Doing Business also measures the quality of the land administration system in each economy. The quality of land administration index has five dimensions: reliability of infrastructure, transparency of information, geographic coverage, land dispute resolution and equal access to property rights. The ranking of economies on the ease of registering property is determined by sorting their distance to frontier scores for registering property. These scores are the simple average of the distance to frontier scores for each of the component indicators. The distance to frontier score helps assess the absolute level of regulatory performance over time. It measures the distance of each economy to the frontier, which represents the best performance observed on each of the indicators across all economies in the Doing Business sample since 2005. One can both see the gap between a particular economys performance and the best performance at any point in time and assess the absolute change in the economys regulatory environment over time as measured by Doing Business. An economys distance to frontier is reflected on a scale from 0 to 100, where 0 represents the lowest performance and 100 represents the frontier. Read more aboutthe &quot;Registering Property Methodology&quot;</rdfs:comment>
    <rdfs:seeAlso rdf:resource="https://landportal.org/book/indicator/wb-db-rpdtf" />
    <skos:notation>WB-DB-RP.DTF</skos:notation>
    <skos:inScheme rdf:resource="http://data.landportal.info/vocabulary/25" />
    <skos:prefLabel>Registering property (Doing Business) - Distance To Frontier</skos:prefLabel>
    <dct:subject rdf:resource="http://aims.fao.org/aos/agrovoc/c_9000098" />
    <dct:subject rdf:resource="http://data.landportal.info/voc/landvoc/theme/T-INST" />
    <dct:subject rdf:resource="http://data.landportal.info/voc/landvoc/overarching-category/OA-USE" />
    <dct:subject rdf:resource="http://data.landportal.info/voc/landvoc/theme/T-INVEST" />
    <dct:title>Registering property (Doing Business) - Distance To Frontier</dct:title>
    <dct:description>Doing Business records the full sequence of procedures necessary for a business (the buyer) to purchase a property from another business (the seller) and to transfer the property title to the buyers name so that the buyer can use the property for expanding its business, use the property as collateral in taking new loans or, if necessary, sell the property to another business. It also measures the time and cost to complete each of these procedures. Doing Business also measures the quality of the land administration system in each economy. The quality of land administration index has five dimensions: reliability of infrastructure, transparency of information, geographic coverage, land dispute resolution and equal access to property rights. The ranking of economies on the ease of registering property is determined by sorting their distance to frontier scores for registering property. These scores are the simple average of the distance to frontier scores for each of the component indicators. The distance to frontier score helps assess the absolute level of regulatory performance over time. It measures the distance of each economy to the frontier, which represents the best performance observed on each of the indicators across all economies in the Doing Business sample since 2005. One can both see the gap between a particular economys performance and the best performance at any point in time and assess the absolute change in the economys regulatory environment over time as measured by Doing Business. An economys distance to frontier is reflected on a scale from 0 to 100, where 0 represents the lowest performance and 100 represents the frontier. Read more aboutthe &quot;Registering Property Methodology&quot;</dct:description>
    <dct:identifier>WB-DB-RP.DTF</dct:identifier>
    <schema:about rdf:resource="http://aims.fao.org/aos/agrovoc/c_9000098" />
    <schema:about rdf:resource="http://data.landportal.info/voc/landvoc/theme/T-INST" />
    <schema:about rdf:resource="http://data.landportal.info/voc/landvoc/theme/T-INVEST" />
    <schema:about rdf:resource="http://data.landportal.info/voc/landvoc/overarching-category/OA-USE" />
    <dct:source rdf:resource="http://data.landportal.info/dataset/WB-DB" />
    <skos:definition>Doing Business records the full sequence of procedures necessary for a business (the buyer) to purchase a property from another business (the seller) and to transfer the property title to the buyers name so that the buyer can use the property for expanding its business, use the property as collateral in taking new loans or, if necessary, sell the property to another business. It also measures the time and cost to complete each of these procedures. Doing Business also measures the quality of the land administration system in each economy. The quality of land administration index has five dimensions: reliability of infrastructure, transparency of information, geographic coverage, land dispute resolution and equal access to property rights. The ranking of economies on the ease of registering property is determined by sorting their distance to frontier scores for registering property. These scores are the simple average of the distance to frontier scores for each of the component indicators. The distance to frontier score helps assess the absolute level of regulatory performance over time. It measures the distance of each economy to the frontier, which represents the best performance observed on each of the indicators across all economies in the Doing Business sample since 2005. One can both see the gap between a particular economys performance and the best performance at any point in time and assess the absolute change in the economys regulatory environment over time as measured by Doing Business. An economys distance to frontier is reflected on a scale from 0 to 100, where 0 represents the lowest performance and 100 represents the frontier. Read more aboutthe &quot;Registering Property Methodology&quot;</skos:definition>
    <sdmx-attribute:unitMeasure>Index (0; 100)</sdmx-attribute:unitMeasure>
  </rdf:Description>
  <rdf:Description rdf:about="http://data.landportal.info/indicator/WB-DB-RP.RANKING">
    <rdf:type rdf:resource="http://purl.org/weso/ontology/computex#Indicator" />
    <rdf:type rdf:resource="http://www.w3.org/2004/02/skos/core#Concept" />
    <rdfs:label>Registering property (Doing Business) - Ranking</rdfs:label>
    <rdfs:comment>Doing Business records the full sequence of procedures necessary for a business (the buyer) to purchase a property from another business (the seller) and to transfer the property title to the buyers name so that the buyer can use the property for expanding its business, use the property as collateral in taking new loans or, if necessary, sell the property to another business. It also measures the time and cost to complete each of these procedures. Doing Business also measures the quality of the land administration system in each economy. The quality of land administration index has five dimensions: reliability of infrastructure, transparency of information, geographic coverage, land dispute resolution and equal access to property rights. The ranking of economies on the ease of registering property is determined by sorting their distance to frontier scores for registering property. These scores are the simple average of the distance to frontier scores for each of the component indicators. Read more aboutthe &quot;Registering Property Methodology&quot;</rdfs:comment>
    <rdfs:seeAlso rdf:resource="https://landportal.org/book/indicator/wb-db-rpranking" />
    <skos:notation>WB-DB-RP.RANKING</skos:notation>
    <skos:inScheme rdf:resource="http://data.landportal.info/vocabulary/25" />
    <skos:prefLabel>Registering property (Doing Business) - Ranking</skos:prefLabel>
    <dct:subject rdf:resource="http://aims.fao.org/aos/agrovoc/c_9000098" />
    <dct:subject rdf:resource="http://data.landportal.info/voc/landvoc/theme/T-INST" />
    <dct:subject rdf:resource="http://data.landportal.info/voc/landvoc/overarching-category/OA-USE" />
    <dct:subject rdf:resource="http://data.landportal.info/voc/landvoc/theme/T-INVEST" />
    <dct:title>Registering property (Doing Business) - Ranking</dct:title>
    <dct:description>Doing Business records the full sequence of procedures necessary for a business (the buyer) to purchase a property from another business (the seller) and to transfer the property title to the buyers name so that the buyer can use the property for expanding its business, use the property as collateral in taking new loans or, if necessary, sell the property to another business. It also measures the time and cost to complete each of these procedures. Doing Business also measures the quality of the land administration system in each economy. The quality of land administration index has five dimensions: reliability of infrastructure, transparency of information, geographic coverage, land dispute resolution and equal access to property rights. The ranking of economies on the ease of registering property is determined by sorting their distance to frontier scores for registering property. These scores are the simple average of the distance to frontier scores for each of the component indicators. Read more aboutthe &quot;Registering Property Methodology&quot;</dct:description>
    <dct:identifier>WB-DB-RP.RANKING</dct:identifier>
    <schema:about rdf:resource="http://aims.fao.org/aos/agrovoc/c_9000098" />
    <schema:about rdf:resource="http://data.landportal.info/voc/landvoc/theme/T-INST" />
    <schema:about rdf:resource="http://data.landportal.info/voc/landvoc/theme/T-INVEST" />
    <schema:about rdf:resource="http://data.landportal.info/voc/landvoc/overarching-category/OA-USE" />
    <dct:source rdf:resource="http://data.landportal.info/dataset/WB-DB" />
    <skos:definition>Doing Business records the full sequence of procedures necessary for a business (the buyer) to purchase a property from another business (the seller) and to transfer the property title to the buyers name so that the buyer can use the property for expanding its business, use the property as collateral in taking new loans or, if necessary, sell the property to another business. It also measures the time and cost to complete each of these procedures. Doing Business also measures the quality of the land administration system in each economy. The quality of land administration index has five dimensions: reliability of infrastructure, transparency of information, geographic coverage, land dispute resolution and equal access to property rights. The ranking of economies on the ease of registering property is determined by sorting their distance to frontier scores for registering property. These scores are the simple average of the distance to frontier scores for each of the component indicators. Read more aboutthe &quot;Registering Property Methodology&quot;</skos:definition>
    <sdmx-attribute:unitMeasure>Rank</sdmx-attribute:unitMeasure>
  </rdf:Description>
  <rdf:Description rdf:about="http://data.landportal.info/indicator/WB-DB.DTF">
    <rdf:type rdf:resource="http://purl.org/weso/ontology/computex#Indicator" />
    <rdf:type rdf:resource="http://www.w3.org/2004/02/skos/core#Concept" />
    <rdfs:label>Ease of Doing Business - Distance To Frontier</rdfs:label>
    <rdfs:comment>The distance to frontier score helps assess the absolute level of regulatory performance over time. It measures the distance of each economy to the frontier, which represents the best performance observed on each of the indicators across all economies in the Doing Business sample since 2005. One can both see the gap between a particular economys performance and the best performance at any point in time and assess the absolute change in the economys regulatory environment over time as measured by Doing Business. An economys distance to frontier is reflected on a scale from 0 to 100, where 0 represents the lowest performance and 100 represents the frontier.  For example, a score of 75 in 2017 means an economy was 25 percentage points away from the frontier constructed from the best performances across all economies and across time. A score of 80 in 2018 would indicate the economy is improving.  Read the methodology, explaining how the ease of doing business rankings and the distance to frontier measure are calculated (PDF).</rdfs:comment>
    <rdfs:seeAlso rdf:resource="https://landportal.org/book/indicator/wb-dbdtf" />
    <skos:notation>WB-DB.DTF</skos:notation>
    <skos:inScheme rdf:resource="http://data.landportal.info/vocabulary/25" />
    <skos:prefLabel>Ease of Doing Business - Distance To Frontier</skos:prefLabel>
    <dct:subject rdf:resource="http://aims.fao.org/aos/agrovoc/c_9000098" />
    <dct:subject rdf:resource="http://data.landportal.info/voc/landvoc/theme/T-INST" />
    <dct:subject rdf:resource="http://data.landportal.info/voc/landvoc/overarching-category/OA-USE" />
    <dct:subject rdf:resource="http://data.landportal.info/voc/landvoc/theme/T-INVEST" />
    <dct:title>Ease of Doing Business - Distance To Frontier</dct:title>
    <dct:description>The distance to frontier score helps assess the absolute level of regulatory performance over time. It measures the distance of each economy to the frontier, which represents the best performance observed on each of the indicators across all economies in the Doing Business sample since 2005. One can both see the gap between a particular economys performance and the best performance at any point in time and assess the absolute change in the economys regulatory environment over time as measured by Doing Business. An economys distance to frontier is reflected on a scale from 0 to 100, where 0 represents the lowest performance and 100 represents the frontier.  For example, a score of 75 in 2017 means an economy was 25 percentage points away from the frontier constructed from the best performances across all economies and across time. A score of 80 in 2018 would indicate the economy is improving.  Read the methodology, explaining how the ease of doing business rankings and the distance to frontier measure are calculated (PDF).</dct:description>
    <dct:identifier>WB-DB.DTF</dct:identifier>
    <schema:about rdf:resource="http://aims.fao.org/aos/agrovoc/c_9000098" />
    <schema:about rdf:resource="http://data.landportal.info/voc/landvoc/theme/T-INST" />
    <schema:about rdf:resource="http://data.landportal.info/voc/landvoc/theme/T-INVEST" />
    <schema:about rdf:resource="http://data.landportal.info/voc/landvoc/overarching-category/OA-USE" />
    <dct:source rdf:resource="http://data.landportal.info/dataset/WB-DB" />
    <skos:definition>The distance to frontier score helps assess the absolute level of regulatory performance over time. It measures the distance of each economy to the frontier, which represents the best performance observed on each of the indicators across all economies in the Doing Business sample since 2005. One can both see the gap between a particular economys performance and the best performance at any point in time and assess the absolute change in the economys regulatory environment over time as measured by Doing Business. An economys distance to frontier is reflected on a scale from 0 to 100, where 0 represents the lowest performance and 100 represents the frontier.  For example, a score of 75 in 2017 means an economy was 25 percentage points away from the frontier constructed from the best performances across all economies and across time. A score of 80 in 2018 would indicate the economy is improving.  Read the methodology, explaining how the ease of doing business rankings and the distance to frontier measure are calculated (PDF).</skos:definition>
    <sdmx-attribute:unitMeasure>Index (0; 100)</sdmx-attribute:unitMeasure>
  </rdf:Description>
  <rdf:Description rdf:about="http://data.landportal.info/indicator/WB-DB.RANKING">
    <rdf:type rdf:resource="http://purl.org/weso/ontology/computex#Indicator" />
    <rdf:type rdf:resource="http://www.w3.org/2004/02/skos/core#Concept" />
    <rdfs:label>Ease of Doing Business - Ranking</rdfs:label>
    <rdfs:comment>Economies are ranked on their ease of doing business. A high ease of doing business ranking means the regulatory environment is more conducive to the starting and operation of a local firm. The ranking of economies is determined by sorting the aggregate distance to frontier scores, rounded to two decimals,on 10 topics, each consisting of several indicators, giving equal weight to each topic. The list of topics is: Starting a Business Dealing with Construction Permits Getting Electricity Registering Property Getting Credit Protecting Minority Investors Paying Taxes Trading across Borders Enforcing Contracts Resolving Insolvency  Read the methodology, explaininghow the ease of doing business rankings and the distance to frontier measure are calculated (PDF)</rdfs:comment>
    <rdfs:seeAlso rdf:resource="https://landportal.org/book/indicator/wb-dbranking" />
    <skos:notation>WB-DB.RANKING</skos:notation>
    <skos:inScheme rdf:resource="http://data.landportal.info/vocabulary/25" />
    <skos:prefLabel>Ease of Doing Business - Ranking</skos:prefLabel>
    <dct:subject rdf:resource="http://aims.fao.org/aos/agrovoc/c_9000098" />
    <dct:subject rdf:resource="http://data.landportal.info/voc/landvoc/overarching-category/OA-USE" />
    <dct:subject rdf:resource="http://data.landportal.info/voc/landvoc/theme/T-INVEST" />
    <dct:subject rdf:resource="http://data.landportal.info/voc/landvoc/theme/T-INST" />
    <dct:title>Ease of Doing Business - Ranking</dct:title>
    <dct:description>Economies are ranked on their ease of doing business. A high ease of doing business ranking means the regulatory environment is more conducive to the starting and operation of a local firm. The ranking of economies is determined by sorting the aggregate distance to frontier scores, rounded to two decimals,on 10 topics, each consisting of several indicators, giving equal weight to each topic. The list of topics is: Starting a Business Dealing with Construction Permits Getting Electricity Registering Property Getting Credit Protecting Minority Investors Paying Taxes Trading across Borders Enforcing Contracts Resolving Insolvency  Read the methodology, explaininghow the ease of doing business rankings and the distance to frontier measure are calculated (PDF)</dct:description>
    <dct:identifier>WB-DB.RANKING</dct:identifier>
    <schema:about rdf:resource="http://aims.fao.org/aos/agrovoc/c_9000098" />
    <schema:about rdf:resource="http://data.landportal.info/voc/landvoc/theme/T-INVEST" />
    <schema:about rdf:resource="http://data.landportal.info/voc/landvoc/overarching-category/OA-USE" />
    <schema:about rdf:resource="http://data.landportal.info/voc/landvoc/theme/T-INST" />
    <dct:source rdf:resource="http://data.landportal.info/dataset/WB-DB" />
    <skos:definition>Economies are ranked on their ease of doing business. A high ease of doing business ranking means the regulatory environment is more conducive to the starting and operation of a local firm. The ranking of economies is determined by sorting the aggregate distance to frontier scores, rounded to two decimals,on 10 topics, each consisting of several indicators, giving equal weight to each topic. The list of topics is: Starting a Business Dealing with Construction Permits Getting Electricity Registering Property Getting Credit Protecting Minority Investors Paying Taxes Trading across Borders Enforcing Contracts Resolving Insolvency  Read the methodology, explaininghow the ease of doing business rankings and the distance to frontier measure are calculated (PDF)</skos:definition>
    <sdmx-attribute:unitMeasure>Rank</sdmx-attribute:unitMeasure>
  </rdf:Description>
  <rdf:Description rdf:about="http://data.landportal.info/indicator/WB-DB-RP.COST.DTF">
    <rdf:type rdf:resource="http://www.w3.org/2004/02/skos/core#Concept" />
    <rdf:type rdf:resource="http://purl.org/weso/ontology/computex#Indicator" />
    <rdfs:label>Cost - Registering property (Doing Business) - Distance To Frontier</rdfs:label>
    <rdfs:comment>This is the distance to frontier score of the indicator &quot;Cost - Registering property (Doing Business)&quot;. The distance to frontier score helps assess the absolute level of regulatory performance over time. It measures the distance of each economy to the frontier, which represents the best performance observed on each of the indicators across all economies in the Doing Business sample since 2005. One can both see the gap between a particular economys performance and the best performance at any point in time and assess the absolute change in the economys regulatory environment over time as measured by Doing Business. An economys distance to frontier is reflected on a scale from 0 to 100, where 0 represents the lowest performance and 100 represents the frontier. Doing Business records the full sequence of procedures necessary for a business (the buyer) to purchase a property from another business (the seller) and to transfer the property title to the buyers name so that the buyer can use the property for expanding its business, use the property as collateral in taking new loans or, if necessary, sell the property to another business. It also measures the time and cost to complete each of these procedures. Doing Business also measures the quality of the land administration system in each economy. Cost is recorded as a percentage of the property value, assumed to be equivalent to 50 times income per capita. Only official costs required by law are recorded, including fees, transfer taxes, stamp duties and any other payment to the property registry, notaries, public agencies or lawyers. Other taxes, such as capital gains tax or value added tax, are excluded from the cost measure. Both costs borne by the buyer and the seller are included. If cost estimates differ among sources, the median reported value is used.</rdfs:comment>
    <rdfs:seeAlso rdf:resource="https://landportal.org/book/indicator/wb-db-rpcostdtf" />
    <skos:notation>WB-DB-RP.COST.DTF</skos:notation>
    <skos:inScheme rdf:resource="http://data.landportal.info/vocabulary/25" />
    <skos:prefLabel>Cost - Registering property (Doing Business) - Distance To Frontier</skos:prefLabel>
    <dct:subject rdf:resource="http://data.landportal.info/voc/landvoc/overarching-category/OA-USE" />
    <dct:subject rdf:resource="http://data.landportal.info/voc/landvoc/theme/T-INVEST" />
    <dct:subject rdf:resource="http://data.landportal.info/voc/landvoc/theme/T-INST" />
    <dct:subject rdf:resource="http://aims.fao.org/aos/agrovoc/c_9000098" />
    <dct:title>Cost - Registering property (Doing Business) - Distance To Frontier</dct:title>
    <dct:description>This is the distance to frontier score of the indicator &quot;Cost - Registering property (Doing Business)&quot;. The distance to frontier score helps assess the absolute level of regulatory performance over time. It measures the distance of each economy to the frontier, which represents the best performance observed on each of the indicators across all economies in the Doing Business sample since 2005. One can both see the gap between a particular economys performance and the best performance at any point in time and assess the absolute change in the economys regulatory environment over time as measured by Doing Business. An economys distance to frontier is reflected on a scale from 0 to 100, where 0 represents the lowest performance and 100 represents the frontier. Doing Business records the full sequence of procedures necessary for a business (the buyer) to purchase a property from another business (the seller) and to transfer the property title to the buyers name so that the buyer can use the property for expanding its business, use the property as collateral in taking new loans or, if necessary, sell the property to another business. It also measures the time and cost to complete each of these procedures. Doing Business also measures the quality of the land administration system in each economy. Cost is recorded as a percentage of the property value, assumed to be equivalent to 50 times income per capita. Only official costs required by law are recorded, including fees, transfer taxes, stamp duties and any other payment to the property registry, notaries, public agencies or lawyers. Other taxes, such as capital gains tax or value added tax, are excluded from the cost measure. Both costs borne by the buyer and the seller are included. If cost estimates differ among sources, the median reported value is used.</dct:description>
    <dct:identifier>WB-DB-RP.COST.DTF</dct:identifier>
    <schema:about rdf:resource="http://data.landportal.info/voc/landvoc/theme/T-INVEST" />
    <schema:about rdf:resource="http://data.landportal.info/voc/landvoc/overarching-category/OA-USE" />
    <schema:about rdf:resource="http://data.landportal.info/voc/landvoc/theme/T-INST" />
    <schema:about rdf:resource="http://aims.fao.org/aos/agrovoc/c_9000098" />
    <dct:source rdf:resource="http://data.landportal.info/dataset/WB-DB" />
    <skos:definition>This is the distance to frontier score of the indicator &quot;Cost - Registering property (Doing Business)&quot;. The distance to frontier score helps assess the absolute level of regulatory performance over time. It measures the distance of each economy to the frontier, which represents the best performance observed on each of the indicators across all economies in the Doing Business sample since 2005. One can both see the gap between a particular economys performance and the best performance at any point in time and assess the absolute change in the economys regulatory environment over time as measured by Doing Business. An economys distance to frontier is reflected on a scale from 0 to 100, where 0 represents the lowest performance and 100 represents the frontier. Doing Business records the full sequence of procedures necessary for a business (the buyer) to purchase a property from another business (the seller) and to transfer the property title to the buyers name so that the buyer can use the property for expanding its business, use the property as collateral in taking new loans or, if necessary, sell the property to another business. It also measures the time and cost to complete each of these procedures. Doing Business also measures the quality of the land administration system in each economy. Cost is recorded as a percentage of the property value, assumed to be equivalent to 50 times income per capita. Only official costs required by law are recorded, including fees, transfer taxes, stamp duties and any other payment to the property registry, notaries, public agencies or lawyers. Other taxes, such as capital gains tax or value added tax, are excluded from the cost measure. Both costs borne by the buyer and the seller are included. If cost estimates differ among sources, the median reported value is used.</skos:definition>
    <sdmx-attribute:unitMeasure>Index (0; 100)</sdmx-attribute:unitMeasure>
  </rdf:Description>
  <rdf:Description rdf:about="http://data.landportal.info/indicator/WB-DB-RP.PROC.DTF">
    <rdf:type rdf:resource="http://www.w3.org/2004/02/skos/core#Concept" />
    <rdf:type rdf:resource="http://purl.org/weso/ontology/computex#Indicator" />
    <rdfs:label>Procedures - Registering property (Doing Business) - Distance To Frontier</rdfs:label>
    <rdfs:comment>This is the distance to frontier score of the indicator &quot;Procedures - Registering property (Doing Business)&quot;. The distance to frontier score helps assess the absolute level of regulatory performance over time. It measures the distance of each economy to the frontier, which represents the best performance observed on each of the indicators across all economies in the Doing Business sample since 2005. One can both see the gap between a particular economys performance and the best performance at any point in time and assess the absolute change in the economys regulatory environment over time as measured by Doing Business. An economys distance to frontier is reflected on a scale from 0 to 100, where 0 represents the lowest performance and 100 represents the frontier. Doing Business records the full sequence of procedures necessary for a business (the buyer) to purchase a property from another business (the seller) and to transfer the property title to the buyers name so that the buyer can use the property for expanding its business, use the property as collateral in taking new loans or, if necessary, sell the property to another business. It also measures the time and cost to complete each of these procedures. Doing Business also measures the quality of the land administration system in each economy. A procedure is defined as any interaction of the buyer or the seller, their agents (if an agent is legally or in practice required) with external parties, including government agencies, inspectors, notaries and lawyers. Interactions between company officers and employees are not considered. All procedures that are legally or in practice required for registering property are recorded, even if they may be avoided in exceptional cases (table 1). If a procedure can be accelerated legally for an additional cost, the fastest procedure is chosen if that option is more benecial to the economys distance to frontier score and if is used by the majority of property owners. Although the buyer may use lawyers or other professionals where necessary in the registration process, it is assumed that the buyer does not employ an outside facilitator in the registration process unless legally or in practice required to do so.</rdfs:comment>
    <rdfs:seeAlso rdf:resource="https://landportal.org/book/indicator/wb-db-rpprocdtf" />
    <skos:notation>WB-DB-RP.PROC.DTF</skos:notation>
    <skos:inScheme rdf:resource="http://data.landportal.info/vocabulary/25" />
    <skos:prefLabel>Procedures - Registering property (Doing Business) - Distance To Frontier</skos:prefLabel>
    <dct:subject rdf:resource="http://data.landportal.info/voc/landvoc/overarching-category/OA-USE" />
    <dct:subject rdf:resource="http://data.landportal.info/voc/landvoc/theme/T-INVEST" />
    <dct:subject rdf:resource="http://data.landportal.info/voc/landvoc/theme/T-INST" />
    <dct:subject rdf:resource="http://aims.fao.org/aos/agrovoc/c_9000098" />
    <dct:title>Procedures - Registering property (Doing Business) - Distance To Frontier</dct:title>
    <dct:description>This is the distance to frontier score of the indicator &quot;Procedures - Registering property (Doing Business)&quot;. The distance to frontier score helps assess the absolute level of regulatory performance over time. It measures the distance of each economy to the frontier, which represents the best performance observed on each of the indicators across all economies in the Doing Business sample since 2005. One can both see the gap between a particular economys performance and the best performance at any point in time and assess the absolute change in the economys regulatory environment over time as measured by Doing Business. An economys distance to frontier is reflected on a scale from 0 to 100, where 0 represents the lowest performance and 100 represents the frontier. Doing Business records the full sequence of procedures necessary for a business (the buyer) to purchase a property from another business (the seller) and to transfer the property title to the buyers name so that the buyer can use the property for expanding its business, use the property as collateral in taking new loans or, if necessary, sell the property to another business. It also measures the time and cost to complete each of these procedures. Doing Business also measures the quality of the land administration system in each economy. A procedure is defined as any interaction of the buyer or the seller, their agents (if an agent is legally or in practice required) with external parties, including government agencies, inspectors, notaries and lawyers. Interactions between company officers and employees are not considered. All procedures that are legally or in practice required for registering property are recorded, even if they may be avoided in exceptional cases (table 1). If a procedure can be accelerated legally for an additional cost, the fastest procedure is chosen if that option is more benecial to the economys distance to frontier score and if is used by the majority of property owners. Although the buyer may use lawyers or other professionals where necessary in the registration process, it is assumed that the buyer does not employ an outside facilitator in the registration process unless legally or in practice required to do so.</dct:description>
    <dct:identifier>WB-DB-RP.PROC.DTF</dct:identifier>
    <schema:about rdf:resource="http://aims.fao.org/aos/agrovoc/c_9000098" />
    <schema:about rdf:resource="http://data.landportal.info/voc/landvoc/theme/T-INVEST" />
    <schema:about rdf:resource="http://data.landportal.info/voc/landvoc/overarching-category/OA-USE" />
    <schema:about rdf:resource="http://data.landportal.info/voc/landvoc/theme/T-INST" />
    <dct:source rdf:resource="http://data.landportal.info/dataset/WB-DB" />
    <skos:definition>This is the distance to frontier score of the indicator &quot;Procedures - Registering property (Doing Business)&quot;. The distance to frontier score helps assess the absolute level of regulatory performance over time. It measures the distance of each economy to the frontier, which represents the best performance observed on each of the indicators across all economies in the Doing Business sample since 2005. One can both see the gap between a particular economys performance and the best performance at any point in time and assess the absolute change in the economys regulatory environment over time as measured by Doing Business. An economys distance to frontier is reflected on a scale from 0 to 100, where 0 represents the lowest performance and 100 represents the frontier. Doing Business records the full sequence of procedures necessary for a business (the buyer) to purchase a property from another business (the seller) and to transfer the property title to the buyers name so that the buyer can use the property for expanding its business, use the property as collateral in taking new loans or, if necessary, sell the property to another business. It also measures the time and cost to complete each of these procedures. Doing Business also measures the quality of the land administration system in each economy. A procedure is defined as any interaction of the buyer or the seller, their agents (if an agent is legally or in practice required) with external parties, including government agencies, inspectors, notaries and lawyers. Interactions between company officers and employees are not considered. All procedures that are legally or in practice required for registering property are recorded, even if they may be avoided in exceptional cases (table 1). If a procedure can be accelerated legally for an additional cost, the fastest procedure is chosen if that option is more benecial to the economys distance to frontier score and if is used by the majority of property owners. Although the buyer may use lawyers or other professionals where necessary in the registration process, it is assumed that the buyer does not employ an outside facilitator in the registration process unless legally or in practice required to do so.</skos:definition>
    <sdmx-attribute:unitMeasure>Index (0; 100)</sdmx-attribute:unitMeasure>
  </rdf:Description>
  <rdf:Description rdf:about="http://data.landportal.info/indicator/WB-DB-RP.TIME">
    <rdf:type rdf:resource="http://www.w3.org/2004/02/skos/core#Concept" />
    <rdf:type rdf:resource="http://purl.org/weso/ontology/computex#Indicator" />
    <rdfs:label>Time - Registering property (Doing Business)</rdfs:label>
    <rdfs:comment>This indicator measures the median duration that property lawyers, notaries or registry officials indicate is necessary to complete a procedure. Doing Business records the full sequence of procedures necessary for a business (the buyer) to purchase a property from another business (the seller) and to transfer the property title to the buyers name so that the buyer can use the property for expanding its business, use the property as collateral in taking new loans or, if necessary, sell the property to another business. It also measures the time and cost to complete each of these procedures. Doing Business also measures the quality of the land administration system in each economy. Time is recorded in calendar days. The measure captures the median duration that property lawyers, notaries or registry officials indicate is necessary to complete a procedure. It is assumed that the minimum time required for each procedure is one day, except for procedures that can be fully completed online, for which the time required is recorded as half a day. Although procedures may take place simultaneously, they cannot start on the same day, again with the exception of procedures that can be fully completed online. It is assumed that the buyer does not waste time and commits to completing each remaining procedure without delay. If a procedure can be accelerated for an additional cost, the fastest legal procedure available and used by the majority of property owners is chosen. If procedures can be undertaken simultaneously, it is assumed that they are. It is assumed that the parties involved are aware of all requirements and their sequence from the beginning. Time spent on gathering information is not considered. If time estimates differ among sources, the median reported value is used.</rdfs:comment>
    <rdfs:seeAlso rdf:resource="https://landportal.org/book/indicator/wb-db-rptime" />
    <skos:notation>WB-DB-RP.TIME</skos:notation>
    <skos:inScheme rdf:resource="http://data.landportal.info/vocabulary/25" />
    <skos:prefLabel>Time - Registering property (Doing Business)</skos:prefLabel>
    <dct:subject rdf:resource="http://data.landportal.info/voc/landvoc/overarching-category/OA-USE" />
    <dct:subject rdf:resource="http://data.landportal.info/voc/landvoc/theme/T-INVEST" />
    <dct:subject rdf:resource="http://data.landportal.info/voc/landvoc/theme/T-INST" />
    <dct:subject rdf:resource="http://aims.fao.org/aos/agrovoc/c_9000098" />
    <dct:title>Time - Registering property (Doing Business)</dct:title>
    <dct:description>This indicator measures the median duration that property lawyers, notaries or registry officials indicate is necessary to complete a procedure. Doing Business records the full sequence of procedures necessary for a business (the buyer) to purchase a property from another business (the seller) and to transfer the property title to the buyers name so that the buyer can use the property for expanding its business, use the property as collateral in taking new loans or, if necessary, sell the property to another business. It also measures the time and cost to complete each of these procedures. Doing Business also measures the quality of the land administration system in each economy. Time is recorded in calendar days. The measure captures the median duration that property lawyers, notaries or registry officials indicate is necessary to complete a procedure. It is assumed that the minimum time required for each procedure is one day, except for procedures that can be fully completed online, for which the time required is recorded as half a day. Although procedures may take place simultaneously, they cannot start on the same day, again with the exception of procedures that can be fully completed online. It is assumed that the buyer does not waste time and commits to completing each remaining procedure without delay. If a procedure can be accelerated for an additional cost, the fastest legal procedure available and used by the majority of property owners is chosen. If procedures can be undertaken simultaneously, it is assumed that they are. It is assumed that the parties involved are aware of all requirements and their sequence from the beginning. Time spent on gathering information is not considered. If time estimates differ among sources, the median reported value is used.</dct:description>
    <dct:identifier>WB-DB-RP.TIME</dct:identifier>
    <schema:about rdf:resource="http://aims.fao.org/aos/agrovoc/c_9000098" />
    <schema:about rdf:resource="http://data.landportal.info/voc/landvoc/theme/T-INVEST" />
    <schema:about rdf:resource="http://data.landportal.info/voc/landvoc/overarching-category/OA-USE" />
    <schema:about rdf:resource="http://data.landportal.info/voc/landvoc/theme/T-INST" />
    <dct:source rdf:resource="http://data.landportal.info/dataset/WB-DB" />
    <skos:definition>This indicator measures the median duration that property lawyers, notaries or registry officials indicate is necessary to complete a procedure. Doing Business records the full sequence of procedures necessary for a business (the buyer) to purchase a property from another business (the seller) and to transfer the property title to the buyers name so that the buyer can use the property for expanding its business, use the property as collateral in taking new loans or, if necessary, sell the property to another business. It also measures the time and cost to complete each of these procedures. Doing Business also measures the quality of the land administration system in each economy. Time is recorded in calendar days. The measure captures the median duration that property lawyers, notaries or registry officials indicate is necessary to complete a procedure. It is assumed that the minimum time required for each procedure is one day, except for procedures that can be fully completed online, for which the time required is recorded as half a day. Although procedures may take place simultaneously, they cannot start on the same day, again with the exception of procedures that can be fully completed online. It is assumed that the buyer does not waste time and commits to completing each remaining procedure without delay. If a procedure can be accelerated for an additional cost, the fastest legal procedure available and used by the majority of property owners is chosen. If procedures can be undertaken simultaneously, it is assumed that they are. It is assumed that the parties involved are aware of all requirements and their sequence from the beginning. Time spent on gathering information is not considered. If time estimates differ among sources, the median reported value is used.</skos:definition>
    <sdmx-attribute:unitMeasure>Days</sdmx-attribute:unitMeasure>
  </rdf:Description>
  <rdf:Description rdf:about="http://data.landportal.info/indicator/WB-DB-RP.TIME.DTF">
    <rdf:type rdf:resource="http://www.w3.org/2004/02/skos/core#Concept" />
    <rdf:type rdf:resource="http://purl.org/weso/ontology/computex#Indicator" />
    <rdfs:label>Time - Registering property (Doing Business) - Distance To Frontier</rdfs:label>
    <rdfs:comment>This is the distance to frontier score of the indicator &quot;Time - Registering property (Doing Business)&quot;. The distance to frontier score helps assess the absolute level of regulatory performance over time. It measures the distance of each economy to the frontier, which represents the best performance observed on each of the indicators across all economies in the Doing Business sample since 2005. One can both see the gap between a particular economys performance and the best performance at any point in time and assess the absolute change in the economys regulatory environment over time as measured by Doing Business. An economys distance to frontier is reflected on a scale from 0 to 100, where 0 represents the lowest performance and 100 represents the frontier. Doing Business records the full sequence of procedures necessary for a business (the buyer) to purchase a property from another business (the seller) and to transfer the property title to the buyers name so that the buyer can use the property for expanding its business, use the property as collateral in taking new loans or, if necessary, sell the property to another business. It also measures the time and cost to complete each of these procedures. Doing Business also measures the quality of the land administration system in each economy. Time is recorded in calendar days. The measure captures the median duration that property lawyers, notaries or registry officials indicate is necessary to complete a procedure. It is assumed that the minimum time required for each procedure is one day, except for procedures that can be fully completed online, for which the time required is recorded as half a day. Although procedures may take place simultaneously, they cannot start on the same day, again with the exception of procedures that can be fully completed online. It is assumed that the buyer does not waste time and commits to completing each remaining procedure without delay. If a procedure can be accelerated for an additional cost, the fastest legal procedure available and used by the majority of property owners is chosen. If procedures can be undertaken simultaneously, it is assumed that they are. It is assumed that the parties involved are aware of all requirements and their sequence from the beginning. Time spent on gathering information is not considered. If time estimates differ among sources, the median reported value is used.</rdfs:comment>
    <rdfs:seeAlso rdf:resource="https://landportal.org/book/indicator/wb-db-rptimedtf" />
    <skos:notation>WB-DB-RP.TIME.DTF</skos:notation>
    <skos:inScheme rdf:resource="http://data.landportal.info/vocabulary/25" />
    <skos:prefLabel>Time - Registering property (Doing Business) - Distance To Frontier</skos:prefLabel>
    <dct:subject rdf:resource="http://data.landportal.info/voc/landvoc/overarching-category/OA-USE" />
    <dct:subject rdf:resource="http://data.landportal.info/voc/landvoc/theme/T-INVEST" />
    <dct:subject rdf:resource="http://data.landportal.info/voc/landvoc/theme/T-INST" />
    <dct:subject rdf:resource="http://aims.fao.org/aos/agrovoc/c_9000098" />
    <dct:title>Time - Registering property (Doing Business) - Distance To Frontier</dct:title>
    <dct:description>This is the distance to frontier score of the indicator &quot;Time - Registering property (Doing Business)&quot;. The distance to frontier score helps assess the absolute level of regulatory performance over time. It measures the distance of each economy to the frontier, which represents the best performance observed on each of the indicators across all economies in the Doing Business sample since 2005. One can both see the gap between a particular economys performance and the best performance at any point in time and assess the absolute change in the economys regulatory environment over time as measured by Doing Business. An economys distance to frontier is reflected on a scale from 0 to 100, where 0 represents the lowest performance and 100 represents the frontier. Doing Business records the full sequence of procedures necessary for a business (the buyer) to purchase a property from another business (the seller) and to transfer the property title to the buyers name so that the buyer can use the property for expanding its business, use the property as collateral in taking new loans or, if necessary, sell the property to another business. It also measures the time and cost to complete each of these procedures. Doing Business also measures the quality of the land administration system in each economy. Time is recorded in calendar days. The measure captures the median duration that property lawyers, notaries or registry officials indicate is necessary to complete a procedure. It is assumed that the minimum time required for each procedure is one day, except for procedures that can be fully completed online, for which the time required is recorded as half a day. Although procedures may take place simultaneously, they cannot start on the same day, again with the exception of procedures that can be fully completed online. It is assumed that the buyer does not waste time and commits to completing each remaining procedure without delay. If a procedure can be accelerated for an additional cost, the fastest legal procedure available and used by the majority of property owners is chosen. If procedures can be undertaken simultaneously, it is assumed that they are. It is assumed that the parties involved are aware of all requirements and their sequence from the beginning. Time spent on gathering information is not considered. If time estimates differ among sources, the median reported value is used.</dct:description>
    <dct:identifier>WB-DB-RP.TIME.DTF</dct:identifier>
    <schema:about rdf:resource="http://aims.fao.org/aos/agrovoc/c_9000098" />
    <schema:about rdf:resource="http://data.landportal.info/voc/landvoc/theme/T-INVEST" />
    <schema:about rdf:resource="http://data.landportal.info/voc/landvoc/overarching-category/OA-USE" />
    <schema:about rdf:resource="http://data.landportal.info/voc/landvoc/theme/T-INST" />
    <dct:source rdf:resource="http://data.landportal.info/dataset/WB-DB" />
    <skos:definition>This is the distance to frontier score of the indicator &quot;Time - Registering property (Doing Business)&quot;. The distance to frontier score helps assess the absolute level of regulatory performance over time. It measures the distance of each economy to the frontier, which represents the best performance observed on each of the indicators across all economies in the Doing Business sample since 2005. One can both see the gap between a particular economys performance and the best performance at any point in time and assess the absolute change in the economys regulatory environment over time as measured by Doing Business. An economys distance to frontier is reflected on a scale from 0 to 100, where 0 represents the lowest performance and 100 represents the frontier. Doing Business records the full sequence of procedures necessary for a business (the buyer) to purchase a property from another business (the seller) and to transfer the property title to the buyers name so that the buyer can use the property for expanding its business, use the property as collateral in taking new loans or, if necessary, sell the property to another business. It also measures the time and cost to complete each of these procedures. Doing Business also measures the quality of the land administration system in each economy. Time is recorded in calendar days. The measure captures the median duration that property lawyers, notaries or registry officials indicate is necessary to complete a procedure. It is assumed that the minimum time required for each procedure is one day, except for procedures that can be fully completed online, for which the time required is recorded as half a day. Although procedures may take place simultaneously, they cannot start on the same day, again with the exception of procedures that can be fully completed online. It is assumed that the buyer does not waste time and commits to completing each remaining procedure without delay. If a procedure can be accelerated for an additional cost, the fastest legal procedure available and used by the majority of property owners is chosen. If procedures can be undertaken simultaneously, it is assumed that they are. It is assumed that the parties involved are aware of all requirements and their sequence from the beginning. Time spent on gathering information is not considered. If time estimates differ among sources, the median reported value is used.</skos:definition>
    <sdmx-attribute:unitMeasure>Index (0; 100)</sdmx-attribute:unitMeasure>
  </rdf:Description>
  <rdf:Description rdf:about="http://data.landportal.info/indicator/WB-DB-RP.COST">
    <rdf:type rdf:resource="http://purl.org/weso/ontology/computex#Indicator" />
    <rdf:type rdf:resource="http://www.w3.org/2004/02/skos/core#Concept" />
    <rdfs:label>Cost - Registering property (Doing Business)</rdfs:label>
    <rdfs:comment>This indicator measures the cost required to complete each procedure (% of property value). Doing Business records the full sequence of procedures necessary for a business (the buyer) to purchase a property from another business (the seller) and to transfer the property title to the buyers name. This,so that the buyer can use the property for expanding its business, use the property as collateral in taking new loans or, if necessary, sell the property to another business. It also measures the time and cost to complete each of these procedures. Doing Business also measures the quality of the land administration system in each economy. Cost is recorded as a percentage of the property value, assumed to be equivalent to 50 times income per capita. Only official costs required by law are recorded, including fees, transfer taxes, stamp duties and any other payment to the property registry, notaries, public agencies or lawyers. Other taxes, such as capital gains tax or value added tax, are excluded from the cost measure. Both costs borne by the buyer and the seller are included. If cost estimates differ among sources, the median reported value is used.</rdfs:comment>
    <rdfs:seeAlso rdf:resource="https://landportal.org/book/indicator/wb-db-rpcost" />
    <skos:notation>WB-DB-RP.COST</skos:notation>
    <skos:inScheme rdf:resource="http://data.landportal.info/vocabulary/25" />
    <skos:prefLabel>Cost - Registering property (Doing Business)</skos:prefLabel>
    <dct:subject rdf:resource="http://aims.fao.org/aos/agrovoc/c_9000098" />
    <dct:subject rdf:resource="http://data.landportal.info/voc/landvoc/overarching-category/OA-USE" />
    <dct:subject rdf:resource="http://data.landportal.info/voc/landvoc/theme/T-INVEST" />
    <dct:subject rdf:resource="http://data.landportal.info/voc/landvoc/theme/T-INST" />
    <dct:title>Cost - Registering property (Doing Business)</dct:title>
    <dct:description>This indicator measures the cost required to complete each procedure (% of property value). Doing Business records the full sequence of procedures necessary for a business (the buyer) to purchase a property from another business (the seller) and to transfer the property title to the buyers name. This,so that the buyer can use the property for expanding its business, use the property as collateral in taking new loans or, if necessary, sell the property to another business. It also measures the time and cost to complete each of these procedures. Doing Business also measures the quality of the land administration system in each economy. Cost is recorded as a percentage of the property value, assumed to be equivalent to 50 times income per capita. Only official costs required by law are recorded, including fees, transfer taxes, stamp duties and any other payment to the property registry, notaries, public agencies or lawyers. Other taxes, such as capital gains tax or value added tax, are excluded from the cost measure. Both costs borne by the buyer and the seller are included. If cost estimates differ among sources, the median reported value is used.</dct:description>
    <dct:identifier>WB-DB-RP.COST</dct:identifier>
    <schema:about rdf:resource="http://data.landportal.info/voc/landvoc/theme/T-INVEST" />
    <schema:about rdf:resource="http://data.landportal.info/voc/landvoc/overarching-category/OA-USE" />
    <schema:about rdf:resource="http://data.landportal.info/voc/landvoc/theme/T-INST" />
    <schema:about rdf:resource="http://aims.fao.org/aos/agrovoc/c_9000098" />
    <dct:source rdf:resource="http://data.landportal.info/dataset/WB-DB" />
    <skos:definition>This indicator measures the cost required to complete each procedure (% of property value). Doing Business records the full sequence of procedures necessary for a business (the buyer) to purchase a property from another business (the seller) and to transfer the property title to the buyers name. This,so that the buyer can use the property for expanding its business, use the property as collateral in taking new loans or, if necessary, sell the property to another business. It also measures the time and cost to complete each of these procedures. Doing Business also measures the quality of the land administration system in each economy. Cost is recorded as a percentage of the property value, assumed to be equivalent to 50 times income per capita. Only official costs required by law are recorded, including fees, transfer taxes, stamp duties and any other payment to the property registry, notaries, public agencies or lawyers. Other taxes, such as capital gains tax or value added tax, are excluded from the cost measure. Both costs borne by the buyer and the seller are included. If cost estimates differ among sources, the median reported value is used.</skos:definition>
    <sdmx-attribute:unitMeasure>Percentage</sdmx-attribute:unitMeasure>
  </rdf:Description>
  <rdf:Description rdf:about="http://data.landportal.info/indicator/WB-DB-RP.PROC">
    <rdf:type rdf:resource="http://www.w3.org/2004/02/skos/core#Concept" />
    <rdf:type rdf:resource="http://purl.org/weso/ontology/computex#Indicator" />
    <rdfs:label>Procedures - Registering property (Doing Business)</rdfs:label>
    <rdfs:comment>This indicator measures the number of proceduresnecessary for a business. Doing Business records the full sequence of procedures necessary for a business (the buyer) to purchase a property from another business (the seller) and to transfer the property title to the buyers name so that the buyer can use the property for expanding its business, use the property as collateral in taking new loans or, if necessary, sell the property to another business. It also measures the time and cost to complete each of these procedures. Doing Business also measures the quality of the land administration system in each economy. A procedure is defined as any interaction of the buyer or the seller, their agents (if an agent is legally or in practice required) with external parties, including government agencies, inspectors, notaries and lawyers. Interactions between company officers and employees are not considered. All procedures that are legally or in practice required for registering property are recorded, even if they may be avoided in exceptional cases (table 1). If a procedure can be accelerated legally for an additional cost, the fastest procedure is chosen if that option is more benecial to the economys distance to frontier score and if is used by the majority of property owners. Although the buyer may use lawyers or other professionals where necessary in the registration process, it is assumed that the buyer does not employ an outside facilitator in the registration process unless legally or in practice required to do so.</rdfs:comment>
    <rdfs:seeAlso rdf:resource="https://landportal.org/book/indicator/wb-db-rpproc" />
    <skos:notation>WB-DB-RP.PROC</skos:notation>
    <skos:inScheme rdf:resource="http://data.landportal.info/vocabulary/25" />
    <skos:prefLabel>Procedures - Registering property (Doing Business)</skos:prefLabel>
    <dct:subject rdf:resource="http://data.landportal.info/voc/landvoc/theme/T-INST" />
    <dct:subject rdf:resource="http://aims.fao.org/aos/agrovoc/c_9000098" />
    <dct:subject rdf:resource="http://data.landportal.info/voc/landvoc/overarching-category/OA-USE" />
    <dct:subject rdf:resource="http://data.landportal.info/voc/landvoc/theme/T-INVEST" />
    <dct:title>Procedures - Registering property (Doing Business)</dct:title>
    <dct:description>This indicator measures the number of proceduresnecessary for a business. Doing Business records the full sequence of procedures necessary for a business (the buyer) to purchase a property from another business (the seller) and to transfer the property title to the buyers name so that the buyer can use the property for expanding its business, use the property as collateral in taking new loans or, if necessary, sell the property to another business. It also measures the time and cost to complete each of these procedures. Doing Business also measures the quality of the land administration system in each economy. A procedure is defined as any interaction of the buyer or the seller, their agents (if an agent is legally or in practice required) with external parties, including government agencies, inspectors, notaries and lawyers. Interactions between company officers and employees are not considered. All procedures that are legally or in practice required for registering property are recorded, even if they may be avoided in exceptional cases (table 1). If a procedure can be accelerated legally for an additional cost, the fastest procedure is chosen if that option is more benecial to the economys distance to frontier score and if is used by the majority of property owners. Although the buyer may use lawyers or other professionals where necessary in the registration process, it is assumed that the buyer does not employ an outside facilitator in the registration process unless legally or in practice required to do so.</dct:description>
    <dct:identifier>WB-DB-RP.PROC</dct:identifier>
    <schema:about rdf:resource="http://aims.fao.org/aos/agrovoc/c_9000098" />
    <schema:about rdf:resource="http://data.landportal.info/voc/landvoc/theme/T-INST" />
    <schema:about rdf:resource="http://data.landportal.info/voc/landvoc/theme/T-INVEST" />
    <schema:about rdf:resource="http://data.landportal.info/voc/landvoc/overarching-category/OA-USE" />
    <dct:source rdf:resource="http://data.landportal.info/dataset/WB-DB" />
    <skos:definition>This indicator measures the number of proceduresnecessary for a business. Doing Business records the full sequence of procedures necessary for a business (the buyer) to purchase a property from another business (the seller) and to transfer the property title to the buyers name so that the buyer can use the property for expanding its business, use the property as collateral in taking new loans or, if necessary, sell the property to another business. It also measures the time and cost to complete each of these procedures. Doing Business also measures the quality of the land administration system in each economy. A procedure is defined as any interaction of the buyer or the seller, their agents (if an agent is legally or in practice required) with external parties, including government agencies, inspectors, notaries and lawyers. Interactions between company officers and employees are not considered. All procedures that are legally or in practice required for registering property are recorded, even if they may be avoided in exceptional cases (table 1). If a procedure can be accelerated legally for an additional cost, the fastest procedure is chosen if that option is more benecial to the economys distance to frontier score and if is used by the majority of property owners. Although the buyer may use lawyers or other professionals where necessary in the registration process, it is assumed that the buyer does not employ an outside facilitator in the registration process unless legally or in practice required to do so.</skos:definition>
    <sdmx-attribute:unitMeasure>Number</sdmx-attribute:unitMeasure>
  </rdf:Description>
</rdf:RDF>