<?xml version="1.0" encoding="utf-8" ?>
<rdf:RDF
	xmlns:rdf="http://www.w3.org/1999/02/22-rdf-syntax-ns#"
	xmlns:rdfs="http://www.w3.org/2000/01/rdf-schema#"
	xmlns:skos="http://www.w3.org/2004/02/skos/core#"
	xmlns:dct="http://purl.org/dc/terms/"
	xmlns:schema="http://schema.org/"
	xmlns:sdmx-attribute="http://purl.org/linked-data/sdmx/2009/attribute#" >
  <rdf:Description rdf:about="http://data.landportal.info/indicator/TI-GCB-IBL">
    <rdf:type rdf:resource="http://purl.org/weso/ontology/computex#Indicator" />
    <rdf:type rdf:resource="http://www.w3.org/2004/02/skos/core#Concept" />
    <rdfs:label>Incidence of bribes paid for land services</rdfs:label>
    <rdfs:comment>This indicator measures the weghted proportion (%) of respondants who have been requested to paid a bribe, among those who contacted land services. In particular, the indicator is obtained aggregating at the country level for each year the responses to the following question: &amp;quot;In the past 12 months have you or anyone living in your household paid a bribe in any form to each of the following institutions/organizations [Land Services]?&amp;quot; We only considered the share of those replying YES to the previous question, among those who reported that they (or anyone in the household) had contacted insitutions or organizations for land services in the last 12 months. We used the weights provided in the original dataset provided by TI. This question has been included in 4 waves of the Global Curruption Barometer survey: 2009, 2010, 2011, 2012. For more information around the TI&amp;#039;s GCB please visit: https://www.transparency.org/news/feature/global_corruption_barometer_ci....</rdfs:comment>
    <rdfs:seeAlso rdf:resource="https://landportal.org/book/indicator/ti-gcb-ibl" />
    <skos:notation>TI-GCB-IBL</skos:notation>
    <skos:inScheme rdf:resource="http://data.landportal.info/vocabulary/25" />
    <skos:prefLabel>Incidence of bribes paid for land services</skos:prefLabel>
    <dct:subject rdf:resource="http://data.landportal.info/voc/landvoc/overarching-category/OA-LAW" />
    <dct:subject rdf:resource="http://data.landportal.info/voc/landvoc/theme/T-INST" />
    <dct:title>Incidence of bribes paid for land services</dct:title>
    <dct:description>This indicator measures the weghted proportion (%) of respondants who have been requested to paid a bribe, among those who contacted land services. In particular, the indicator is obtained aggregating at the country level for each year the responses to the following question: &amp;quot;In the past 12 months have you or anyone living in your household paid a bribe in any form to each of the following institutions/organizations [Land Services]?&amp;quot; We only considered the share of those replying YES to the previous question, among those who reported that they (or anyone in the household) had contacted insitutions or organizations for land services in the last 12 months. We used the weights provided in the original dataset provided by TI. This question has been included in 4 waves of the Global Curruption Barometer survey: 2009, 2010, 2011, 2012. For more information around the TI&amp;#039;s GCB please visit: https://www.transparency.org/news/feature/global_corruption_barometer_ci....</dct:description>
    <dct:identifier>TI-GCB-IBL</dct:identifier>
    <schema:about rdf:resource="http://data.landportal.info/voc/landvoc/overarching-category/OA-LAW" />
    <schema:about rdf:resource="http://data.landportal.info/voc/landvoc/theme/T-INST" />
    <dct:source rdf:resource="http://data.landportal.info/dataset/TI-GCB" />
    <skos:definition>This indicator measures the weghted proportion (%) of respondants who have been requested to paid a bribe, among those who contacted land services. In particular, the indicator is obtained aggregating at the country level for each year the responses to the following question: &amp;quot;In the past 12 months have you or anyone living in your household paid a bribe in any form to each of the following institutions/organizations [Land Services]?&amp;quot; We only considered the share of those replying YES to the previous question, among those who reported that they (or anyone in the household) had contacted insitutions or organizations for land services in the last 12 months. We used the weights provided in the original dataset provided by TI. This question has been included in 4 waves of the Global Curruption Barometer survey: 2009, 2010, 2011, 2012. For more information around the TI&amp;#039;s GCB please visit: https://www.transparency.org/news/feature/global_corruption_barometer_ci....</skos:definition>
    <sdmx-attribute:unitMeasure>1&#39;000 Ha</sdmx-attribute:unitMeasure>
  </rdf:Description>
  <rdf:Description rdf:about="http://data.landportal.info/indicator/TI-GCB-PPCL.a">
    <rdf:type rdf:resource="http://purl.org/weso/ontology/computex#Indicator" />
    <rdf:type rdf:resource="http://www.w3.org/2004/02/skos/core#Concept" />
    <rdfs:label>Perception of &#39;&#39;petty&#39;&#39; corruption for land services - Average problem</rdfs:label>
    <rdfs:comment>This indicator measures the weghted proportion (%) of respondants who percevied petty corruption for land services as a AVERAGE PROBLEM. In particuar, the 2009 round of the Global Corruption Barometer included the following question: &amp;quot;How serious do you think is in this country the problem of bribes being paid to land authorities to obtain favourable decisions in selling, buying, leasing, inheriting and registering land, or in land tax declaration, or in handling land disputes?&amp;quot; Possible answers were the followings: - Not a problem at all - Moderate - Average - Serious - Very serious problem - Dont know / No Answer (NA) We used the weights provided in the original dataset provided by TI. For more information around the TI&amp;#039;s GCB please visit: https://www.transparency.org/news/feature/global_corruption_barometer_ci...</rdfs:comment>
    <rdfs:seeAlso rdf:resource="https://landportal.org/book/indicator/ti-gcb-ppcla" />
    <skos:notation>TI-GCB-PPCL.a</skos:notation>
    <skos:inScheme rdf:resource="http://data.landportal.info/vocabulary/25" />
    <skos:prefLabel>Perception of &#39;&#39;petty&#39;&#39; corruption for land services - Average problem</skos:prefLabel>
    <dct:subject rdf:resource="http://data.landportal.info/voc/landvoc/overarching-category/OA-LAW" />
    <dct:subject rdf:resource="http://data.landportal.info/voc/landvoc/theme/T-INST" />
    <dct:title>Perception of &#39;&#39;petty&#39;&#39; corruption for land services - Average problem</dct:title>
    <dct:description>This indicator measures the weghted proportion (%) of respondants who percevied petty corruption for land services as a AVERAGE PROBLEM. In particuar, the 2009 round of the Global Corruption Barometer included the following question: &amp;quot;How serious do you think is in this country the problem of bribes being paid to land authorities to obtain favourable decisions in selling, buying, leasing, inheriting and registering land, or in land tax declaration, or in handling land disputes?&amp;quot; Possible answers were the followings: - Not a problem at all - Moderate - Average - Serious - Very serious problem - Dont know / No Answer (NA) We used the weights provided in the original dataset provided by TI. For more information around the TI&amp;#039;s GCB please visit: https://www.transparency.org/news/feature/global_corruption_barometer_ci...</dct:description>
    <dct:identifier>TI-GCB-PPCL.a</dct:identifier>
    <schema:about rdf:resource="http://data.landportal.info/voc/landvoc/overarching-category/OA-LAW" />
    <schema:about rdf:resource="http://data.landportal.info/voc/landvoc/theme/T-INST" />
    <dct:source rdf:resource="http://data.landportal.info/dataset/TI-GCB" />
    <skos:definition>This indicator measures the weghted proportion (%) of respondants who percevied petty corruption for land services as a AVERAGE PROBLEM. In particuar, the 2009 round of the Global Corruption Barometer included the following question: &amp;quot;How serious do you think is in this country the problem of bribes being paid to land authorities to obtain favourable decisions in selling, buying, leasing, inheriting and registering land, or in land tax declaration, or in handling land disputes?&amp;quot; Possible answers were the followings: - Not a problem at all - Moderate - Average - Serious - Very serious problem - Dont know / No Answer (NA) We used the weights provided in the original dataset provided by TI. For more information around the TI&amp;#039;s GCB please visit: https://www.transparency.org/news/feature/global_corruption_barometer_ci...</skos:definition>
    <sdmx-attribute:unitMeasure>1&#39;000 Ha</sdmx-attribute:unitMeasure>
  </rdf:Description>
  <rdf:Description rdf:about="http://data.landportal.info/indicator/TI-GCB-PPCL.dk">
    <rdf:type rdf:resource="http://purl.org/weso/ontology/computex#Indicator" />
    <rdf:type rdf:resource="http://www.w3.org/2004/02/skos/core#Concept" />
    <rdfs:label>Perception of &#39;&#39;petty&#39;&#39; corruption for land services - Don&#39;t know / NA</rdfs:label>
    <rdfs:comment>This indicator measures the weghted proportion (%) of respondants who DID NOT KNOW or DID NOT ANSWER to what extent petty corruption for land services was a problem. In particuar, the 2009 round of the Global Corruption Barometer included the following question: &amp;quot;How serious do you think is in this country the problem of bribes being paid to land authorities to obtain favourable decisions in selling, buying, leasing, inheriting and registering land, or in land tax declaration, or in handling land disputes?&amp;quot; Possible answers were the followings: - Not a problem at all - Moderate - Average - Serious - Very serious problem - Dont know / No Answer (NA) We used the weights provided in the original dataset provided by TI. For more information around the TI&amp;#039;s GCB please visit: https://www.transparency.org/news/feature/global_corruption_barometer_ci...</rdfs:comment>
    <rdfs:seeAlso rdf:resource="https://landportal.org/book/indicator/ti-gcb-ppcldk" />
    <skos:notation>TI-GCB-PPCL.dk</skos:notation>
    <skos:inScheme rdf:resource="http://data.landportal.info/vocabulary/25" />
    <skos:prefLabel>Perception of &#39;&#39;petty&#39;&#39; corruption for land services - Don&#39;t know / NA</skos:prefLabel>
    <dct:subject rdf:resource="http://data.landportal.info/voc/landvoc/overarching-category/OA-LAW" />
    <dct:subject rdf:resource="http://data.landportal.info/voc/landvoc/theme/T-INST" />
    <dct:title>Perception of &#39;&#39;petty&#39;&#39; corruption for land services - Don&#39;t know / NA</dct:title>
    <dct:description>This indicator measures the weghted proportion (%) of respondants who DID NOT KNOW or DID NOT ANSWER to what extent petty corruption for land services was a problem. In particuar, the 2009 round of the Global Corruption Barometer included the following question: &amp;quot;How serious do you think is in this country the problem of bribes being paid to land authorities to obtain favourable decisions in selling, buying, leasing, inheriting and registering land, or in land tax declaration, or in handling land disputes?&amp;quot; Possible answers were the followings: - Not a problem at all - Moderate - Average - Serious - Very serious problem - Dont know / No Answer (NA) We used the weights provided in the original dataset provided by TI. For more information around the TI&amp;#039;s GCB please visit: https://www.transparency.org/news/feature/global_corruption_barometer_ci...</dct:description>
    <dct:identifier>TI-GCB-PPCL.dk</dct:identifier>
    <schema:about rdf:resource="http://data.landportal.info/voc/landvoc/overarching-category/OA-LAW" />
    <schema:about rdf:resource="http://data.landportal.info/voc/landvoc/theme/T-INST" />
    <dct:source rdf:resource="http://data.landportal.info/dataset/TI-GCB" />
    <skos:definition>This indicator measures the weghted proportion (%) of respondants who DID NOT KNOW or DID NOT ANSWER to what extent petty corruption for land services was a problem. In particuar, the 2009 round of the Global Corruption Barometer included the following question: &amp;quot;How serious do you think is in this country the problem of bribes being paid to land authorities to obtain favourable decisions in selling, buying, leasing, inheriting and registering land, or in land tax declaration, or in handling land disputes?&amp;quot; Possible answers were the followings: - Not a problem at all - Moderate - Average - Serious - Very serious problem - Dont know / No Answer (NA) We used the weights provided in the original dataset provided by TI. For more information around the TI&amp;#039;s GCB please visit: https://www.transparency.org/news/feature/global_corruption_barometer_ci...</skos:definition>
    <sdmx-attribute:unitMeasure>1&#39;000 Ha</sdmx-attribute:unitMeasure>
  </rdf:Description>
  <rdf:Description rdf:about="http://data.landportal.info/indicator/TI-GCB-PPCL.m">
    <rdf:type rdf:resource="http://www.w3.org/2004/02/skos/core#Concept" />
    <rdf:type rdf:resource="http://purl.org/weso/ontology/computex#Indicator" />
    <rdfs:label>Perception of &#39;&#39;petty&#39;&#39; corruption for land services - Moderate problem</rdfs:label>
    <rdfs:comment>This indicator measures the weghted proportion (%) of respondants who percevied petty corruption for land services as a MODERATE PROBLEM. In particuar, the 2009 round of the Global Corruption Barometer included the following question: &amp;quot;How serious do you think is in this country the problem of bribes being paid to land authorities to obtain favourable decisions in selling, buying, leasing, inheriting and registering land, or in land tax declaration, or in handling land disputes?&amp;quot; Possible answers were the followings: - Not a problem at all - Moderate - Average - Serious - Very serious problem - Dont know / No Answer (NA) We used the weights provided in the original dataset provided by TI. For more information around the TI&amp;#039;s GCB please visit: https://www.transparency.org/news/feature/global_corruption_barometer_ci...</rdfs:comment>
    <rdfs:seeAlso rdf:resource="https://landportal.org/book/indicator/ti-gcb-ppclm" />
    <skos:notation>TI-GCB-PPCL.m</skos:notation>
    <skos:inScheme rdf:resource="http://data.landportal.info/vocabulary/25" />
    <skos:prefLabel>Perception of &#39;&#39;petty&#39;&#39; corruption for land services - Moderate problem</skos:prefLabel>
    <dct:subject rdf:resource="http://data.landportal.info/voc/landvoc/theme/T-INST" />
    <dct:subject rdf:resource="http://data.landportal.info/voc/landvoc/overarching-category/OA-LAW" />
    <dct:title>Perception of &#39;&#39;petty&#39;&#39; corruption for land services - Moderate problem</dct:title>
    <dct:description>This indicator measures the weghted proportion (%) of respondants who percevied petty corruption for land services as a MODERATE PROBLEM. In particuar, the 2009 round of the Global Corruption Barometer included the following question: &amp;quot;How serious do you think is in this country the problem of bribes being paid to land authorities to obtain favourable decisions in selling, buying, leasing, inheriting and registering land, or in land tax declaration, or in handling land disputes?&amp;quot; Possible answers were the followings: - Not a problem at all - Moderate - Average - Serious - Very serious problem - Dont know / No Answer (NA) We used the weights provided in the original dataset provided by TI. For more information around the TI&amp;#039;s GCB please visit: https://www.transparency.org/news/feature/global_corruption_barometer_ci...</dct:description>
    <dct:identifier>TI-GCB-PPCL.m</dct:identifier>
    <schema:about rdf:resource="http://data.landportal.info/voc/landvoc/theme/T-INST" />
    <schema:about rdf:resource="http://data.landportal.info/voc/landvoc/overarching-category/OA-LAW" />
    <dct:source rdf:resource="http://data.landportal.info/dataset/TI-GCB" />
    <skos:definition>This indicator measures the weghted proportion (%) of respondants who percevied petty corruption for land services as a MODERATE PROBLEM. In particuar, the 2009 round of the Global Corruption Barometer included the following question: &amp;quot;How serious do you think is in this country the problem of bribes being paid to land authorities to obtain favourable decisions in selling, buying, leasing, inheriting and registering land, or in land tax declaration, or in handling land disputes?&amp;quot; Possible answers were the followings: - Not a problem at all - Moderate - Average - Serious - Very serious problem - Dont know / No Answer (NA) We used the weights provided in the original dataset provided by TI. For more information around the TI&amp;#039;s GCB please visit: https://www.transparency.org/news/feature/global_corruption_barometer_ci...</skos:definition>
    <sdmx-attribute:unitMeasure>1&#39;000 Ha</sdmx-attribute:unitMeasure>
  </rdf:Description>
  <rdf:Description rdf:about="http://data.landportal.info/indicator/TI-GCB-PPCL.n">
    <rdf:type rdf:resource="http://www.w3.org/2004/02/skos/core#Concept" />
    <rdf:type rdf:resource="http://purl.org/weso/ontology/computex#Indicator" />
    <rdfs:label>Perception of &#39;&#39;petty&#39;&#39; corruption for land services - Not a problem</rdfs:label>
    <rdfs:comment>This indicator measures the weghted proportion (%) of respondants who percevied that petty corruption for land services was NOT A PROBLEM. In particuar, the 2009 round of the Global Corruption Barometer included the following question: &amp;quot;How serious do you think is in this country the problem of bribes being paid to land authorities to obtain favourable decisions in selling, buying, leasing, inheriting and registering land, or in land tax declaration, or in handling land disputes?&amp;quot; Possible answers were the followings: - Not a problem at all - Moderate - Average - Serious - Very serious problem - Dont know / No Answer (NA) We used the weights provided in the original dataset provided by TI. For more information around the TI&amp;#039;s GCB please visit: https://www.transparency.org/news/feature/global_corruption_barometer_ci...</rdfs:comment>
    <rdfs:seeAlso rdf:resource="https://landportal.org/book/indicator/ti-gcb-ppcln" />
    <skos:notation>TI-GCB-PPCL.n</skos:notation>
    <skos:inScheme rdf:resource="http://data.landportal.info/vocabulary/25" />
    <skos:prefLabel>Perception of &#39;&#39;petty&#39;&#39; corruption for land services - Not a problem</skos:prefLabel>
    <dct:subject rdf:resource="http://data.landportal.info/voc/landvoc/theme/T-INST" />
    <dct:subject rdf:resource="http://data.landportal.info/voc/landvoc/overarching-category/OA-LAW" />
    <dct:title>Perception of &#39;&#39;petty&#39;&#39; corruption for land services - Not a problem</dct:title>
    <dct:description>This indicator measures the weghted proportion (%) of respondants who percevied that petty corruption for land services was NOT A PROBLEM. In particuar, the 2009 round of the Global Corruption Barometer included the following question: &amp;quot;How serious do you think is in this country the problem of bribes being paid to land authorities to obtain favourable decisions in selling, buying, leasing, inheriting and registering land, or in land tax declaration, or in handling land disputes?&amp;quot; Possible answers were the followings: - Not a problem at all - Moderate - Average - Serious - Very serious problem - Dont know / No Answer (NA) We used the weights provided in the original dataset provided by TI. For more information around the TI&amp;#039;s GCB please visit: https://www.transparency.org/news/feature/global_corruption_barometer_ci...</dct:description>
    <dct:identifier>TI-GCB-PPCL.n</dct:identifier>
    <schema:about rdf:resource="http://data.landportal.info/voc/landvoc/theme/T-INST" />
    <schema:about rdf:resource="http://data.landportal.info/voc/landvoc/overarching-category/OA-LAW" />
    <dct:source rdf:resource="http://data.landportal.info/dataset/TI-GCB" />
    <skos:definition>This indicator measures the weghted proportion (%) of respondants who percevied that petty corruption for land services was NOT A PROBLEM. In particuar, the 2009 round of the Global Corruption Barometer included the following question: &amp;quot;How serious do you think is in this country the problem of bribes being paid to land authorities to obtain favourable decisions in selling, buying, leasing, inheriting and registering land, or in land tax declaration, or in handling land disputes?&amp;quot; Possible answers were the followings: - Not a problem at all - Moderate - Average - Serious - Very serious problem - Dont know / No Answer (NA) We used the weights provided in the original dataset provided by TI. For more information around the TI&amp;#039;s GCB please visit: https://www.transparency.org/news/feature/global_corruption_barometer_ci...</skos:definition>
    <sdmx-attribute:unitMeasure>1&#39;000 Ha</sdmx-attribute:unitMeasure>
  </rdf:Description>
  <rdf:Description rdf:about="http://data.landportal.info/indicator/TI-GCB-PPCL.s">
    <rdf:type rdf:resource="http://purl.org/weso/ontology/computex#Indicator" />
    <rdf:type rdf:resource="http://www.w3.org/2004/02/skos/core#Concept" />
    <rdfs:label>Perception of &#39;&#39;petty&#39;&#39; corruption for land services - Serious problem</rdfs:label>
    <rdfs:comment>This indicator measures the weghted proportion (%) of respondants who percevied petty corruption for land services as a SERIOUS PROBLEM. In particuar, the 2009 round of the Global Corruption Barometer included the following question: &amp;quot;How serious do you think is in this country the problem of bribes being paid to land authorities to obtain favourable decisions in selling, buying, leasing, inheriting and registering land, or in land tax declaration, or in handling land disputes?&amp;quot; Possible answers were the followings: - Not a problem at all - Moderate - Average - Serious - Very serious problem - Dont know / No Answer (NA) We used the weights provided in the original dataset provided by TI. For more information around the TI&amp;#039;s GCB please visit: https://www.transparency.org/news/feature/global_corruption_barometer_ci...</rdfs:comment>
    <rdfs:seeAlso rdf:resource="https://landportal.org/book/indicator/ti-gcb-ppcls" />
    <skos:notation>TI-GCB-PPCL.s</skos:notation>
    <skos:inScheme rdf:resource="http://data.landportal.info/vocabulary/25" />
    <skos:prefLabel>Perception of &#39;&#39;petty&#39;&#39; corruption for land services - Serious problem</skos:prefLabel>
    <dct:subject rdf:resource="http://data.landportal.info/voc/landvoc/theme/T-INST" />
    <dct:subject rdf:resource="http://data.landportal.info/voc/landvoc/overarching-category/OA-LAW" />
    <dct:title>Perception of &#39;&#39;petty&#39;&#39; corruption for land services - Serious problem</dct:title>
    <dct:description>This indicator measures the weghted proportion (%) of respondants who percevied petty corruption for land services as a SERIOUS PROBLEM. In particuar, the 2009 round of the Global Corruption Barometer included the following question: &amp;quot;How serious do you think is in this country the problem of bribes being paid to land authorities to obtain favourable decisions in selling, buying, leasing, inheriting and registering land, or in land tax declaration, or in handling land disputes?&amp;quot; Possible answers were the followings: - Not a problem at all - Moderate - Average - Serious - Very serious problem - Dont know / No Answer (NA) We used the weights provided in the original dataset provided by TI. For more information around the TI&amp;#039;s GCB please visit: https://www.transparency.org/news/feature/global_corruption_barometer_ci...</dct:description>
    <dct:identifier>TI-GCB-PPCL.s</dct:identifier>
    <schema:about rdf:resource="http://data.landportal.info/voc/landvoc/theme/T-INST" />
    <schema:about rdf:resource="http://data.landportal.info/voc/landvoc/overarching-category/OA-LAW" />
    <dct:source rdf:resource="http://data.landportal.info/dataset/TI-GCB" />
    <skos:definition>This indicator measures the weghted proportion (%) of respondants who percevied petty corruption for land services as a SERIOUS PROBLEM. In particuar, the 2009 round of the Global Corruption Barometer included the following question: &amp;quot;How serious do you think is in this country the problem of bribes being paid to land authorities to obtain favourable decisions in selling, buying, leasing, inheriting and registering land, or in land tax declaration, or in handling land disputes?&amp;quot; Possible answers were the followings: - Not a problem at all - Moderate - Average - Serious - Very serious problem - Dont know / No Answer (NA) We used the weights provided in the original dataset provided by TI. For more information around the TI&amp;#039;s GCB please visit: https://www.transparency.org/news/feature/global_corruption_barometer_ci...</skos:definition>
    <sdmx-attribute:unitMeasure>1&#39;000 Ha</sdmx-attribute:unitMeasure>
  </rdf:Description>
  <rdf:Description rdf:about="http://data.landportal.info/indicator/TI-GCB-PPCL.vs">
    <rdf:type rdf:resource="http://purl.org/weso/ontology/computex#Indicator" />
    <rdf:type rdf:resource="http://www.w3.org/2004/02/skos/core#Concept" />
    <rdfs:label>Perception of &#39;&#39;petty&#39;&#39; corruption for land services - Very serious problem</rdfs:label>
    <rdfs:comment>This indicator measures the weghted proportion (%) of respondants who percevied petty corruption for land services as a VERY SERIOUS PROBLEM. In particuar, the 2009 round of the Global Corruption Barometer included the following question: &amp;quot;How serious do you think is in this country the problem of bribes being paid to land authorities to obtain favourable decisions in selling, buying, leasing, inheriting and registering land, or in land tax declaration, or in handling land disputes?&amp;quot; Possible answers were the followings: - Not a problem at all - Moderate - Average - Serious - Very serious problem - Dont know / No Answer (NA) We used the weights provided in the original dataset provided by TI. For more information around the TI&amp;#039;s GCB please visit: https://www.transparency.org/news/feature/global_corruption_barometer_ci...</rdfs:comment>
    <rdfs:seeAlso rdf:resource="https://landportal.org/book/indicator/ti-gcb-ppclvs" />
    <skos:notation>TI-GCB-PPCL.vs</skos:notation>
    <skos:inScheme rdf:resource="http://data.landportal.info/vocabulary/25" />
    <skos:prefLabel>Perception of &#39;&#39;petty&#39;&#39; corruption for land services - Very serious problem</skos:prefLabel>
    <dct:subject rdf:resource="http://data.landportal.info/voc/landvoc/theme/T-INST" />
    <dct:subject rdf:resource="http://data.landportal.info/voc/landvoc/overarching-category/OA-LAW" />
    <dct:title>Perception of &#39;&#39;petty&#39;&#39; corruption for land services - Very serious problem</dct:title>
    <dct:description>This indicator measures the weghted proportion (%) of respondants who percevied petty corruption for land services as a VERY SERIOUS PROBLEM. In particuar, the 2009 round of the Global Corruption Barometer included the following question: &amp;quot;How serious do you think is in this country the problem of bribes being paid to land authorities to obtain favourable decisions in selling, buying, leasing, inheriting and registering land, or in land tax declaration, or in handling land disputes?&amp;quot; Possible answers were the followings: - Not a problem at all - Moderate - Average - Serious - Very serious problem - Dont know / No Answer (NA) We used the weights provided in the original dataset provided by TI. For more information around the TI&amp;#039;s GCB please visit: https://www.transparency.org/news/feature/global_corruption_barometer_ci...</dct:description>
    <dct:identifier>TI-GCB-PPCL.vs</dct:identifier>
    <schema:about rdf:resource="http://data.landportal.info/voc/landvoc/theme/T-INST" />
    <schema:about rdf:resource="http://data.landportal.info/voc/landvoc/overarching-category/OA-LAW" />
    <dct:source rdf:resource="http://data.landportal.info/dataset/TI-GCB" />
    <skos:definition>This indicator measures the weghted proportion (%) of respondants who percevied petty corruption for land services as a VERY SERIOUS PROBLEM. In particuar, the 2009 round of the Global Corruption Barometer included the following question: &amp;quot;How serious do you think is in this country the problem of bribes being paid to land authorities to obtain favourable decisions in selling, buying, leasing, inheriting and registering land, or in land tax declaration, or in handling land disputes?&amp;quot; Possible answers were the followings: - Not a problem at all - Moderate - Average - Serious - Very serious problem - Dont know / No Answer (NA) We used the weights provided in the original dataset provided by TI. For more information around the TI&amp;#039;s GCB please visit: https://www.transparency.org/news/feature/global_corruption_barometer_ci...</skos:definition>
    <sdmx-attribute:unitMeasure>1&#39;000 Ha</sdmx-attribute:unitMeasure>
  </rdf:Description>
  <rdf:Description rdf:about="http://data.landportal.info/indicator/TI-GCB-GPCL.dk">
    <rdf:type rdf:resource="http://purl.org/weso/ontology/computex#Indicator" />
    <rdf:type rdf:resource="http://www.w3.org/2004/02/skos/core#Concept" />
    <rdfs:label>Perception of &quot;grand&quot; or political corruption in land matters - Don&#39;t know / NA</rdfs:label>
    <rdfs:comment>This indicator measures the weghted proportion (%) of respondants who DID NOT KNOW or DID NOT ANSWER to what extent grand or politcal corruption for land services was a problem. In particuar, the 2009 round of the Global Corruption Barometer included the following question: &amp;quot;How serious do you think the problem of grand or political corruption in land matters is in this country?&amp;quot; Possible answers were the followings: - Not a problem at all - Moderate - Average - Serious - Very serious problem - Dont know / No Answer (NA) We used the weights provided in the original dataset provided by TI. For more information around the TI&amp;#039;s GCB please visit: https://www.transparency.org/news/feature/global_corruption_barometer_ci...</rdfs:comment>
    <rdfs:seeAlso rdf:resource="https://landportal.org/book/indicator/ti-gcb-gpcldk" />
    <skos:notation>TI-GCB-GPCL.dk</skos:notation>
    <skos:inScheme rdf:resource="http://data.landportal.info/vocabulary/25" />
    <skos:prefLabel>Perception of &quot;grand&quot; or political corruption in land matters - Don&#39;t know / NA</skos:prefLabel>
    <dct:subject rdf:resource="http://data.landportal.info/voc/landvoc/overarching-category/OA-LAW" />
    <dct:subject rdf:resource="http://data.landportal.info/voc/landvoc/theme/T-INST" />
    <dct:title>Perception of &quot;grand&quot; or political corruption in land matters - Don&#39;t know / NA</dct:title>
    <dct:description>This indicator measures the weghted proportion (%) of respondants who DID NOT KNOW or DID NOT ANSWER to what extent grand or politcal corruption for land services was a problem. In particuar, the 2009 round of the Global Corruption Barometer included the following question: &amp;quot;How serious do you think the problem of grand or political corruption in land matters is in this country?&amp;quot; Possible answers were the followings: - Not a problem at all - Moderate - Average - Serious - Very serious problem - Dont know / No Answer (NA) We used the weights provided in the original dataset provided by TI. For more information around the TI&amp;#039;s GCB please visit: https://www.transparency.org/news/feature/global_corruption_barometer_ci...</dct:description>
    <dct:identifier>TI-GCB-GPCL.dk</dct:identifier>
    <schema:about rdf:resource="http://data.landportal.info/voc/landvoc/overarching-category/OA-LAW" />
    <schema:about rdf:resource="http://data.landportal.info/voc/landvoc/theme/T-INST" />
    <dct:source rdf:resource="http://data.landportal.info/dataset/TI-GCB" />
    <skos:definition>This indicator measures the weghted proportion (%) of respondants who DID NOT KNOW or DID NOT ANSWER to what extent grand or politcal corruption for land services was a problem. In particuar, the 2009 round of the Global Corruption Barometer included the following question: &amp;quot;How serious do you think the problem of grand or political corruption in land matters is in this country?&amp;quot; Possible answers were the followings: - Not a problem at all - Moderate - Average - Serious - Very serious problem - Dont know / No Answer (NA) We used the weights provided in the original dataset provided by TI. For more information around the TI&amp;#039;s GCB please visit: https://www.transparency.org/news/feature/global_corruption_barometer_ci...</skos:definition>
    <sdmx-attribute:unitMeasure>1&#39;000 Ha</sdmx-attribute:unitMeasure>
  </rdf:Description>
  <rdf:Description rdf:about="http://data.landportal.info/indicator/TI-GCB-GPCL.vs">
    <rdf:type rdf:resource="http://purl.org/weso/ontology/computex#Indicator" />
    <rdf:type rdf:resource="http://www.w3.org/2004/02/skos/core#Concept" />
    <rdfs:label>Perception of &quot;grand&quot; or political corruption in land matters - Very serious problem</rdfs:label>
    <rdfs:comment>This indicator measures the weghted proportion (%) of respondants who percevied grand or political corruption for land services as a VERY SERIOUS PROBLEM. In particuar, the 2009 round of the Global Corruption Barometer included the following question: How serious do you think the problem of grand or political corruption in land matters is in this country? Possible answer were the followings: - Not a problem at all - Moderate - Average - Serious - Very serious problem - Dont know/ No answer (NA) We used the weights provided in the original dataset provided by TI. For more information around the TI&amp;#039;s GCB please visit: https://www.transparency.org/news/feature/global_corruption_barometer_ci...</rdfs:comment>
    <rdfs:seeAlso rdf:resource="https://landportal.org/book/indicator/ti-gcb-gpclvs" />
    <skos:notation>TI-GCB-GPCL.vs</skos:notation>
    <skos:inScheme rdf:resource="http://data.landportal.info/vocabulary/25" />
    <skos:prefLabel>Perception of &quot;grand&quot; or political corruption in land matters - Very serious problem</skos:prefLabel>
    <dct:subject rdf:resource="http://data.landportal.info/voc/landvoc/overarching-category/OA-LAW" />
    <dct:subject rdf:resource="http://data.landportal.info/voc/landvoc/theme/T-INST" />
    <dct:title>Perception of &quot;grand&quot; or political corruption in land matters - Very serious problem</dct:title>
    <dct:description>This indicator measures the weghted proportion (%) of respondants who percevied grand or political corruption for land services as a VERY SERIOUS PROBLEM. In particuar, the 2009 round of the Global Corruption Barometer included the following question: How serious do you think the problem of grand or political corruption in land matters is in this country? Possible answer were the followings: - Not a problem at all - Moderate - Average - Serious - Very serious problem - Dont know/ No answer (NA) We used the weights provided in the original dataset provided by TI. For more information around the TI&amp;#039;s GCB please visit: https://www.transparency.org/news/feature/global_corruption_barometer_ci...</dct:description>
    <dct:identifier>TI-GCB-GPCL.vs</dct:identifier>
    <schema:about rdf:resource="http://data.landportal.info/voc/landvoc/overarching-category/OA-LAW" />
    <schema:about rdf:resource="http://data.landportal.info/voc/landvoc/theme/T-INST" />
    <dct:source rdf:resource="http://data.landportal.info/dataset/TI-GCB" />
    <skos:definition>This indicator measures the weghted proportion (%) of respondants who percevied grand or political corruption for land services as a VERY SERIOUS PROBLEM. In particuar, the 2009 round of the Global Corruption Barometer included the following question: How serious do you think the problem of grand or political corruption in land matters is in this country? Possible answer were the followings: - Not a problem at all - Moderate - Average - Serious - Very serious problem - Dont know/ No answer (NA) We used the weights provided in the original dataset provided by TI. For more information around the TI&amp;#039;s GCB please visit: https://www.transparency.org/news/feature/global_corruption_barometer_ci...</skos:definition>
    <sdmx-attribute:unitMeasure>1&#39;000 Ha</sdmx-attribute:unitMeasure>
  </rdf:Description>
  <rdf:Description rdf:about="http://data.landportal.info/indicator/TI-GCB-GPCL.a">
    <rdf:type rdf:resource="http://purl.org/weso/ontology/computex#Indicator" />
    <rdf:type rdf:resource="http://www.w3.org/2004/02/skos/core#Concept" />
    <rdfs:label>Perception of &quot;grand&quot; or political corruption in land matters - Average problem</rdfs:label>
    <rdfs:comment>This indicator measures the weghted proportion (%) of respondants who percevied grand or political corruption for land services as a AVERAGE PROBLEM. In particuar, the 2009 round of the Global Corruption Barometer included the following question: How serious do you think the problem of grand or political corruption in land matters is in this country? Possible answers were the followings: - Not a problem at all - Moderate - Average - Serious - Very serious problem - Dont know/ No answer (NA) We used the weights provided in the original dataset provided by TI. For more information around the TI&amp;#039;s GCB please visit: https://www.transparency.org/news/feature/global_corruption_barometer_ci...</rdfs:comment>
    <rdfs:seeAlso rdf:resource="https://landportal.org/book/indicator/ti-gcb-gpcla" />
    <skos:notation>TI-GCB-GPCL.a</skos:notation>
    <skos:inScheme rdf:resource="http://data.landportal.info/vocabulary/25" />
    <skos:prefLabel>Perception of &quot;grand&quot; or political corruption in land matters - Average problem</skos:prefLabel>
    <dct:subject rdf:resource="http://data.landportal.info/voc/landvoc/overarching-category/OA-LAW" />
    <dct:subject rdf:resource="http://data.landportal.info/voc/landvoc/theme/T-INST" />
    <dct:title>Perception of &quot;grand&quot; or political corruption in land matters - Average problem</dct:title>
    <dct:description>This indicator measures the weghted proportion (%) of respondants who percevied grand or political corruption for land services as a AVERAGE PROBLEM. In particuar, the 2009 round of the Global Corruption Barometer included the following question: How serious do you think the problem of grand or political corruption in land matters is in this country? Possible answers were the followings: - Not a problem at all - Moderate - Average - Serious - Very serious problem - Dont know/ No answer (NA) We used the weights provided in the original dataset provided by TI. For more information around the TI&amp;#039;s GCB please visit: https://www.transparency.org/news/feature/global_corruption_barometer_ci...</dct:description>
    <dct:identifier>TI-GCB-GPCL.a</dct:identifier>
    <schema:about rdf:resource="http://data.landportal.info/voc/landvoc/overarching-category/OA-LAW" />
    <schema:about rdf:resource="http://data.landportal.info/voc/landvoc/theme/T-INST" />
    <dct:source rdf:resource="http://data.landportal.info/dataset/TI-GCB" />
    <skos:definition>This indicator measures the weghted proportion (%) of respondants who percevied grand or political corruption for land services as a AVERAGE PROBLEM. In particuar, the 2009 round of the Global Corruption Barometer included the following question: How serious do you think the problem of grand or political corruption in land matters is in this country? Possible answers were the followings: - Not a problem at all - Moderate - Average - Serious - Very serious problem - Dont know/ No answer (NA) We used the weights provided in the original dataset provided by TI. For more information around the TI&amp;#039;s GCB please visit: https://www.transparency.org/news/feature/global_corruption_barometer_ci...</skos:definition>
    <sdmx-attribute:unitMeasure>1&#39;000 Ha</sdmx-attribute:unitMeasure>
  </rdf:Description>
  <rdf:Description rdf:about="http://data.landportal.info/indicator/TI-GCB-GPCL.m">
    <rdf:type rdf:resource="http://purl.org/weso/ontology/computex#Indicator" />
    <rdf:type rdf:resource="http://www.w3.org/2004/02/skos/core#Concept" />
    <rdfs:label>Perception of &quot;grand&quot; or political corruption in land matters - Moderate problem</rdfs:label>
    <rdfs:comment>This indicator measures the weghted proportion (%) of respondants who percevied grand or political corruption for land services as a MODERATE PROBLEM. In particuar, the 2009 round of the Global Corruption Barometer included the following question: How serious do you think the problem of grand or political corruption in land matters is in this country? Possible answers were the followings: - Not a problem at all - Moderate - Average - Serious - Very serious problem - Dont know/ No answer (NA) We used the weights provided in the original dataset provided by TI. For more information around the TI&amp;#039;s GCB please visit: https://www.transparency.org/news/feature/global_corruption_barometer_ci...</rdfs:comment>
    <rdfs:seeAlso rdf:resource="https://landportal.org/book/indicator/ti-gcb-gpclm" />
    <skos:notation>TI-GCB-GPCL.m</skos:notation>
    <skos:inScheme rdf:resource="http://data.landportal.info/vocabulary/25" />
    <skos:prefLabel>Perception of &quot;grand&quot; or political corruption in land matters - Moderate problem</skos:prefLabel>
    <dct:subject rdf:resource="http://data.landportal.info/voc/landvoc/overarching-category/OA-LAW" />
    <dct:subject rdf:resource="http://data.landportal.info/voc/landvoc/theme/T-INST" />
    <dct:title>Perception of &quot;grand&quot; or political corruption in land matters - Moderate problem</dct:title>
    <dct:description>This indicator measures the weghted proportion (%) of respondants who percevied grand or political corruption for land services as a MODERATE PROBLEM. In particuar, the 2009 round of the Global Corruption Barometer included the following question: How serious do you think the problem of grand or political corruption in land matters is in this country? Possible answers were the followings: - Not a problem at all - Moderate - Average - Serious - Very serious problem - Dont know/ No answer (NA) We used the weights provided in the original dataset provided by TI. For more information around the TI&amp;#039;s GCB please visit: https://www.transparency.org/news/feature/global_corruption_barometer_ci...</dct:description>
    <dct:identifier>TI-GCB-GPCL.m</dct:identifier>
    <schema:about rdf:resource="http://data.landportal.info/voc/landvoc/overarching-category/OA-LAW" />
    <schema:about rdf:resource="http://data.landportal.info/voc/landvoc/theme/T-INST" />
    <dct:source rdf:resource="http://data.landportal.info/dataset/TI-GCB" />
    <skos:definition>This indicator measures the weghted proportion (%) of respondants who percevied grand or political corruption for land services as a MODERATE PROBLEM. In particuar, the 2009 round of the Global Corruption Barometer included the following question: How serious do you think the problem of grand or political corruption in land matters is in this country? Possible answers were the followings: - Not a problem at all - Moderate - Average - Serious - Very serious problem - Dont know/ No answer (NA) We used the weights provided in the original dataset provided by TI. For more information around the TI&amp;#039;s GCB please visit: https://www.transparency.org/news/feature/global_corruption_barometer_ci...</skos:definition>
    <sdmx-attribute:unitMeasure>1&#39;000 Ha</sdmx-attribute:unitMeasure>
  </rdf:Description>
  <rdf:Description rdf:about="http://data.landportal.info/indicator/TI-GCB-GPCL.n">
    <rdf:type rdf:resource="http://purl.org/weso/ontology/computex#Indicator" />
    <rdf:type rdf:resource="http://www.w3.org/2004/02/skos/core#Concept" />
    <rdfs:label>Perception of &quot;grand&quot; or political corruption in land matters - Not a problem</rdfs:label>
    <rdfs:comment>This indicator measures the weghted proportion (%) of respondants who percevied that grand or political corruption for land services was NOT A PROBLEM. In particuar, the 2009 round of the Global Corruption Barometer included the following question: How serious do you think the problem of grand or political corruption in land matters is in this country? Possible answers were the followings: - Not a problem at all - Moderate - Average - Serious - Very serious problem - Dont know/ No answer (NA) We used the weights provided in the original dataset provided by TI. For more information around the TI&amp;#039;s GCB please visit: https://www.transparency.org/news/feature/global_corruption_barometer_ci...</rdfs:comment>
    <rdfs:seeAlso rdf:resource="https://landportal.org/book/indicator/ti-gcb-gpcln" />
    <skos:notation>TI-GCB-GPCL.n</skos:notation>
    <skos:inScheme rdf:resource="http://data.landportal.info/vocabulary/25" />
    <skos:prefLabel>Perception of &quot;grand&quot; or political corruption in land matters - Not a problem</skos:prefLabel>
    <dct:subject rdf:resource="http://data.landportal.info/voc/landvoc/overarching-category/OA-LAW" />
    <dct:subject rdf:resource="http://data.landportal.info/voc/landvoc/theme/T-INST" />
    <dct:title>Perception of &quot;grand&quot; or political corruption in land matters - Not a problem</dct:title>
    <dct:description>This indicator measures the weghted proportion (%) of respondants who percevied that grand or political corruption for land services was NOT A PROBLEM. In particuar, the 2009 round of the Global Corruption Barometer included the following question: How serious do you think the problem of grand or political corruption in land matters is in this country? Possible answers were the followings: - Not a problem at all - Moderate - Average - Serious - Very serious problem - Dont know/ No answer (NA) We used the weights provided in the original dataset provided by TI. For more information around the TI&amp;#039;s GCB please visit: https://www.transparency.org/news/feature/global_corruption_barometer_ci...</dct:description>
    <dct:identifier>TI-GCB-GPCL.n</dct:identifier>
    <schema:about rdf:resource="http://data.landportal.info/voc/landvoc/theme/T-INST" />
    <schema:about rdf:resource="http://data.landportal.info/voc/landvoc/overarching-category/OA-LAW" />
    <dct:source rdf:resource="http://data.landportal.info/dataset/TI-GCB" />
    <skos:definition>This indicator measures the weghted proportion (%) of respondants who percevied that grand or political corruption for land services was NOT A PROBLEM. In particuar, the 2009 round of the Global Corruption Barometer included the following question: How serious do you think the problem of grand or political corruption in land matters is in this country? Possible answers were the followings: - Not a problem at all - Moderate - Average - Serious - Very serious problem - Dont know/ No answer (NA) We used the weights provided in the original dataset provided by TI. For more information around the TI&amp;#039;s GCB please visit: https://www.transparency.org/news/feature/global_corruption_barometer_ci...</skos:definition>
    <sdmx-attribute:unitMeasure>1&#39;000 Ha</sdmx-attribute:unitMeasure>
  </rdf:Description>
  <rdf:Description rdf:about="http://data.landportal.info/indicator/TI-GCB-GPCL.s">
    <rdf:type rdf:resource="http://purl.org/weso/ontology/computex#Indicator" />
    <rdf:type rdf:resource="http://www.w3.org/2004/02/skos/core#Concept" />
    <rdfs:label>Perception of &quot;grand&quot; or political corruption in land matters - Serious problem</rdfs:label>
    <rdfs:comment>This indicator measures the weghted proportion (%) of respondants who percevied grand or political corruption for land services as a SERIOUS PROBLEM. In particuar, the 2009 round of the Global Corruption Barometer included the following question: How serious do you think the problem of grand or political corruption in land matters is in this country? Possible answers were the followings: - Not a problem at all - Moderate - Average - Serious - Very serious problem - Dont know/ No answer (NA) We used the weights provided in the original dataset provided by TI. For more information around the TI&amp;#039;s GCB please visit: https://www.transparency.org/news/feature/global_corruption_barometer_ci...</rdfs:comment>
    <rdfs:seeAlso rdf:resource="https://landportal.org/book/indicator/ti-gcb-gpcls" />
    <skos:notation>TI-GCB-GPCL.s</skos:notation>
    <skos:inScheme rdf:resource="http://data.landportal.info/vocabulary/25" />
    <skos:prefLabel>Perception of &quot;grand&quot; or political corruption in land matters - Serious problem</skos:prefLabel>
    <dct:subject rdf:resource="http://data.landportal.info/voc/landvoc/theme/T-INST" />
    <dct:subject rdf:resource="http://data.landportal.info/voc/landvoc/overarching-category/OA-LAW" />
    <dct:title>Perception of &quot;grand&quot; or political corruption in land matters - Serious problem</dct:title>
    <dct:description>This indicator measures the weghted proportion (%) of respondants who percevied grand or political corruption for land services as a SERIOUS PROBLEM. In particuar, the 2009 round of the Global Corruption Barometer included the following question: How serious do you think the problem of grand or political corruption in land matters is in this country? Possible answers were the followings: - Not a problem at all - Moderate - Average - Serious - Very serious problem - Dont know/ No answer (NA) We used the weights provided in the original dataset provided by TI. For more information around the TI&amp;#039;s GCB please visit: https://www.transparency.org/news/feature/global_corruption_barometer_ci...</dct:description>
    <dct:identifier>TI-GCB-GPCL.s</dct:identifier>
    <schema:about rdf:resource="http://data.landportal.info/voc/landvoc/theme/T-INST" />
    <schema:about rdf:resource="http://data.landportal.info/voc/landvoc/overarching-category/OA-LAW" />
    <dct:source rdf:resource="http://data.landportal.info/dataset/TI-GCB" />
    <skos:definition>This indicator measures the weghted proportion (%) of respondants who percevied grand or political corruption for land services as a SERIOUS PROBLEM. In particuar, the 2009 round of the Global Corruption Barometer included the following question: How serious do you think the problem of grand or political corruption in land matters is in this country? Possible answers were the followings: - Not a problem at all - Moderate - Average - Serious - Very serious problem - Dont know/ No answer (NA) We used the weights provided in the original dataset provided by TI. For more information around the TI&amp;#039;s GCB please visit: https://www.transparency.org/news/feature/global_corruption_barometer_ci...</skos:definition>
    <sdmx-attribute:unitMeasure>1&#39;000 Ha</sdmx-attribute:unitMeasure>
  </rdf:Description>
</rdf:RDF>