<?xml version="1.0" encoding="UTF-8"?>
<rdf:RDF xmlns:rdf="http://www.w3.org/1999/02/22-rdf-syntax-ns#"
  xmlns:dct="http://purl.org/dc/terms/"
  xmlns:schema="http://schema.org/"
  xmlns:skos="http://www.w3.org/2004/02/skos/core#"
  xmlns:sdmx-attribute="http://purl.org/linked-data/sdmx/2009/attribute#"
  xmlns:rdfs="http://www.w3.org/2000/01/rdf-schema#">

  <rdf:Description rdf:about="http://data.landportal.info/indicator/PRINDEX-PRINDEX2018.PR.KHD">
    <rdf:type rdf:resource="http://www.w3.org/2004/02/skos/core#Concept"/>
    <rdf:type rdf:resource="http://purl.org/weso/ontology/computex#Indicator"/>
    <dct:subject rdf:resource="http://data.landportal.info/voc/landvoc/overarching-category/OA-ACCESS"/>
    <dct:subject rdf:resource="http://data.landportal.info/voc/landvoc/theme/T-INST"/>
    <schema:about rdf:resource="http://data.landportal.info/voc/landvoc/overarching-category/OA-ACCESS"/>
    <schema:about rdf:resource="http://data.landportal.info/voc/landvoc/theme/T-INST"/>
    <dct:identifier>PRINDEX-PRINDEX2018.PR.KHD</dct:identifier>
    <skos:notation>PRINDEX-PRINDEX2018.PR.KHD</skos:notation>
    <dct:source rdf:resource="http://data.landportal.info/dataset/PRINDEX-PRINDEX2018"/>
    <sdmx-attribute:unitMeasure>Percentage</sdmx-attribute:unitMeasure>
    <rdfs:label>Prindex - Property rights - Know how to defend their property rights (%)</rdfs:label>
    <skos:prefLabel>Prindex - Property rights - Know how to defend their property rights (%)</skos:prefLabel>
    <dct:title>Prindex - Property rights - Know how to defend their property rights (%)</dct:title>
    <skos:definition>Percentage of people who, if challenged, know how to defend their rights to live in or otherwise use their properties</skos:definition>
    <dct:description>Percentage of people who, if challenged, know how to defend their rights to live in or otherwise use their properties</dct:description>
    <rdfs:comment>Percentage of people who, if challenged, know how to defend their rights to live in or otherwise use their properties</rdfs:comment>
    <skos:inScheme rdf:resource="http://data.landportal.info/vocabulary/25"/>
    <rdfs:seeAlso rdf:resource="https://landportal.org/book/indicator/prindex-prindex2018prkhd"/>
  </rdf:Description>

</rdf:RDF>