<?xml version="1.0" encoding="UTF-8"?>
<rdf:RDF xmlns:rdf="http://www.w3.org/1999/02/22-rdf-syntax-ns#"
  xmlns:dct="http://purl.org/dc/terms/"
  xmlns:schema="http://schema.org/"
  xmlns:skos="http://www.w3.org/2004/02/skos/core#"
  xmlns:sdmx-attribute="http://purl.org/linked-data/sdmx/2009/attribute#"
  xmlns:rdfs="http://www.w3.org/2000/01/rdf-schema#">

  <rdf:Description rdf:about="http://data.landportal.info/indicator/NDGAIN-COUNTRY_INDEX">
    <rdf:type rdf:resource="http://www.w3.org/2004/02/skos/core#Concept"/>
    <rdf:type rdf:resource="http://purl.org/weso/ontology/computex#Indicator"/>
    <dct:subject rdf:resource="http://aims.fao.org/aos/agrovoc/c_1666"/>
    <dct:subject rdf:resource="http://data.landportal.info/voc/landvoc/theme/T-ENVIR"/>
    <schema:about rdf:resource="http://aims.fao.org/aos/agrovoc/c_1666"/>
    <schema:about rdf:resource="http://data.landportal.info/voc/landvoc/theme/T-ENVIR"/>
    <dct:identifier>NDGAIN-COUNTRY_INDEX</dct:identifier>
    <skos:notation>NDGAIN-COUNTRY_INDEX</skos:notation>
    <dct:source rdf:resource="http://data.landportal.info/dataset/NDGAIN-CI"/>
    <sdmx-attribute:unitMeasure>Index</sdmx-attribute:unitMeasure>
    <rdfs:label>ND-GAIN Country Index</rdfs:label>
    <skos:prefLabel>ND-GAIN Country Index</skos:prefLabel>
    <dct:title>ND-GAIN Country Index</dct:title>
    <skos:definition>The ND-GAIN Country Index summarizes a country's vulnerability to climate change and other global challenges in combination with its readiness to improve resilience. It aims to help governments, businesses and communities better prioritize investments for a more efficient response to the immediate global challenges ahead.   More information at https://gain.nd.edu/our-work/country-index/</skos:definition>
    <dct:description>The ND-GAIN Country Index summarizes a country's vulnerability to climate change and other global challenges in combination with its readiness to improve resilience. It aims to help governments, businesses and communities better prioritize investments for a more efficient response to the immediate global challenges ahead.   More information at https://gain.nd.edu/our-work/country-index/</dct:description>
    <rdfs:comment>The ND-GAIN Country Index summarizes a country's vulnerability to climate change and other global challenges in combination with its readiness to improve resilience. It aims to help governments, businesses and communities better prioritize investments for a more efficient response to the immediate global challenges ahead.   More information at https://gain.nd.edu/our-work/country-index/</rdfs:comment>
    <skos:inScheme rdf:resource="http://data.landportal.info/vocabulary/25"/>
    <rdfs:seeAlso rdf:resource="https://landportal.org/book/indicator/ndgain-countryindex"/>
  </rdf:Description>

</rdf:RDF>