<?xml version="1.0" encoding="UTF-8"?>
<rdf:RDF xmlns:rdf="http://www.w3.org/1999/02/22-rdf-syntax-ns#"
  xmlns:dct="http://purl.org/dc/terms/"
  xmlns:schema="http://schema.org/"
  xmlns:skos="http://www.w3.org/2004/02/skos/core#"
  xmlns:sdmx-attribute="http://purl.org/linked-data/sdmx/2009/attribute#"
  xmlns:rdfs="http://www.w3.org/2000/01/rdf-schema#">

  <rdf:Description rdf:about="http://data.landportal.info/indicator/WB-EN.CLC.DRSK.XQ">
    <rdf:type rdf:resource="http://www.w3.org/2004/02/skos/core#Concept"/>
    <rdf:type rdf:resource="http://purl.org/weso/ontology/computex#Indicator"/>
    <dct:subject rdf:resource="http://aims.fao.org/aos/agrovoc/c_10391"/>
    <dct:subject rdf:resource="http://data.landportal.info/voc/landvoc/theme/T-ENVIR"/>
    <schema:about rdf:resource="http://aims.fao.org/aos/agrovoc/c_10391"/>
    <schema:about rdf:resource="http://data.landportal.info/voc/landvoc/theme/T-ENVIR"/>
    <dct:identifier>WB-EN.CLC.DRSK.XQ</dct:identifier>
    <skos:notation>WB-EN.CLC.DRSK.XQ</skos:notation>
    <dct:source rdf:resource="http://data.landportal.info/dataset/WB-CC"/>
    <sdmx-attribute:unitMeasure>Index (1;5)</sdmx-attribute:unitMeasure>
    <rdfs:label>Disaster risk reduction progress score (1-5 scale; 5=best)</rdfs:label>
    <skos:prefLabel>Disaster risk reduction progress score (1-5 scale; 5=best)</skos:prefLabel>
    <dct:title>Disaster risk reduction progress score (1-5 scale; 5=best)</dct:title>
    <skos:definition>Disaster risk reduction progress score is an average of self-assessment scores, ranging from 1 to 5 (where 5 = best) submitted by countries under Priority 1 of the Hyogo Framework National Progress Reports. The Hyogo Framework is a global blueprint for disaster risk reduction efforts that was adopted by 168 countries in 2005. Assessments of &quot;Priority 1&quot; include four indicators that reflect the degree to which countries have prioritized disaster risk reduction and the strengthening of relevant institutions. (Source: http://databank.worldbank.org/data/reports.aspx?source=2&amp;amp;type=metadata&amp;amp;series=EN.CLC.DRSK.XQ)</skos:definition>
    <dct:description>Disaster risk reduction progress score is an average of self-assessment scores, ranging from 1 to 5 (where 5 = best) submitted by countries under Priority 1 of the Hyogo Framework National Progress Reports. The Hyogo Framework is a global blueprint for disaster risk reduction efforts that was adopted by 168 countries in 2005. Assessments of &quot;Priority 1&quot; include four indicators that reflect the degree to which countries have prioritized disaster risk reduction and the strengthening of relevant institutions. (Source: http://databank.worldbank.org/data/reports.aspx?source=2&amp;amp;type=metadata&amp;amp;series=EN.CLC.DRSK.XQ)</dct:description>
    <rdfs:comment>Disaster risk reduction progress score is an average of self-assessment scores, ranging from 1 to 5 (where 5 = best) submitted by countries under Priority 1 of the Hyogo Framework National Progress Reports. The Hyogo Framework is a global blueprint for disaster risk reduction efforts that was adopted by 168 countries in 2005. Assessments of &quot;Priority 1&quot; include four indicators that reflect the degree to which countries have prioritized disaster risk reduction and the strengthening of relevant institutions. (Source: http://databank.worldbank.org/data/reports.aspx?source=2&amp;amp;type=metadata&amp;amp;series=EN.CLC.DRSK.XQ)</rdfs:comment>
    <skos:inScheme rdf:resource="http://data.landportal.info/vocabulary/25"/>
    <rdfs:seeAlso rdf:resource="https://landportal.org/book/indicator/wb-enclcdrskxq"/>
  </rdf:Description>

</rdf:RDF>