<?xml version="1.0" encoding="UTF-8"?>
<rdf:RDF xmlns:rdf="http://www.w3.org/1999/02/22-rdf-syntax-ns#"
  xmlns:dct="http://purl.org/dc/terms/"
  xmlns:schema="http://schema.org/"
  xmlns:skos="http://www.w3.org/2004/02/skos/core#"
  xmlns:sdmx-attribute="http://purl.org/linked-data/sdmx/2009/attribute#"
  xmlns:rdfs="http://www.w3.org/2000/01/rdf-schema#">

  <rdf:Description rdf:about="http://data.landportal.info/indicator/WB-EN.ATM.METH.AG.KT.CE">
    <rdf:type rdf:resource="http://www.w3.org/2004/02/skos/core#Concept"/>
    <rdf:type rdf:resource="http://purl.org/weso/ontology/computex#Indicator"/>
    <dct:subject rdf:resource="http://aims.fao.org/aos/agrovoc/c_203"/>
    <dct:subject rdf:resource="http://aims.fao.org/aos/agrovoc/c_1666"/>
    <dct:subject rdf:resource="http://aims.fao.org/aos/agrovoc/c_4182"/>
    <dct:subject rdf:resource="http://data.landportal.info/voc/landvoc/theme/T-ENVIR"/>
    <schema:about rdf:resource="http://aims.fao.org/aos/agrovoc/c_203"/>
    <schema:about rdf:resource="http://aims.fao.org/aos/agrovoc/c_1666"/>
    <schema:about rdf:resource="http://aims.fao.org/aos/agrovoc/c_4182"/>
    <schema:about rdf:resource="http://data.landportal.info/voc/landvoc/theme/T-ENVIR"/>
    <dct:identifier>WB-EN.ATM.METH.AG.KT.CE</dct:identifier>
    <skos:notation>WB-EN.ATM.METH.AG.KT.CE</skos:notation>
    <dct:source rdf:resource="http://data.landportal.info/dataset/WB-CC"/>
    <sdmx-attribute:unitMeasure>Kiloton of CO2 equivalent</sdmx-attribute:unitMeasure>
    <rdfs:label>Agricultural methane emissions (thousand metric tons of CO2 equivalent)</rdfs:label>
    <skos:prefLabel>Agricultural methane emissions (thousand metric tons of CO2 equivalent)</skos:prefLabel>
    <dct:title>Agricultural methane emissions (thousand metric tons of CO2 equivalent)</dct:title>
    <skos:definition>This indicator measures agricultural methane emissions (CH4) in terms of thousand metric tons of CO2 equivalent. Agricultural methane emissions are methane emissions from animals, animal waste, rice production, agricultural waste burning (nonenergy, on-site), and savannah burning. The carbon dioxide emissions of a country are only an indicator of one greenhouse gas. For a more complete idea of how a country influences climate change, gases such as methane and nitrous oxide should be taken into account. This is particularly important in agricultural economies. (Source: http://databank.worldbank.org/data/reports.aspx?source=2&amp;amp;type=metadata&amp;amp;series=EN.ATM.METH.AG.KT.CE)</skos:definition>
    <dct:description>This indicator measures agricultural methane emissions (CH4) in terms of thousand metric tons of CO2 equivalent. Agricultural methane emissions are methane emissions from animals, animal waste, rice production, agricultural waste burning (nonenergy, on-site), and savannah burning. The carbon dioxide emissions of a country are only an indicator of one greenhouse gas. For a more complete idea of how a country influences climate change, gases such as methane and nitrous oxide should be taken into account. This is particularly important in agricultural economies. (Source: http://databank.worldbank.org/data/reports.aspx?source=2&amp;amp;type=metadata&amp;amp;series=EN.ATM.METH.AG.KT.CE)</dct:description>
    <rdfs:comment>This indicator measures agricultural methane emissions (CH4) in terms of thousand metric tons of CO2 equivalent. Agricultural methane emissions are methane emissions from animals, animal waste, rice production, agricultural waste burning (nonenergy, on-site), and savannah burning. The carbon dioxide emissions of a country are only an indicator of one greenhouse gas. For a more complete idea of how a country influences climate change, gases such as methane and nitrous oxide should be taken into account. This is particularly important in agricultural economies. (Source: http://databank.worldbank.org/data/reports.aspx?source=2&amp;amp;type=metadata&amp;amp;series=EN.ATM.METH.AG.KT.CE)</rdfs:comment>
    <skos:inScheme rdf:resource="http://data.landportal.info/vocabulary/25"/>
    <rdfs:seeAlso rdf:resource="https://landportal.org/book/indicator/wb-enatmmethagktce"/>
  </rdf:Description>

</rdf:RDF>