<?xml version="1.0" encoding="UTF-8"?>
<rdf:RDF xmlns:rdf="http://www.w3.org/1999/02/22-rdf-syntax-ns#"
  xmlns:dct="http://purl.org/dc/terms/"
  xmlns:schema="http://schema.org/"
  xmlns:skos="http://www.w3.org/2004/02/skos/core#"
  xmlns:sdmx-attribute="http://purl.org/linked-data/sdmx/2009/attribute#"
  xmlns:rdfs="http://www.w3.org/2000/01/rdf-schema#">

  <rdf:Description rdf:about="http://data.landportal.info/indicator/FAO-LG.1T">
    <rdf:type rdf:resource="http://www.w3.org/2004/02/skos/core#Concept"/>
    <rdf:type rdf:resource="http://purl.org/weso/ontology/computex#Indicator"/>
    <dct:subject rdf:resource="http://aims.fao.org/aos/agrovoc/c_1dfe5bfe"/>
    <dct:subject rdf:resource="http://aims.fao.org/aos/agrovoc/c_28718"/>
    <dct:subject rdf:resource="http://aims.fao.org/aos/agrovoc/c_4184"/>
    <dct:subject rdf:resource="http://data.landportal.info/voc/landvoc/theme/T-INST"/>
    <schema:about rdf:resource="http://aims.fao.org/aos/agrovoc/c_1dfe5bfe"/>
    <schema:about rdf:resource="http://aims.fao.org/aos/agrovoc/c_28718"/>
    <schema:about rdf:resource="http://aims.fao.org/aos/agrovoc/c_4184"/>
    <schema:about rdf:resource="http://data.landportal.info/voc/landvoc/theme/T-INST"/>
    <dct:identifier>FAO-LG.1T</dct:identifier>
    <skos:notation>FAO-LG.1T</skos:notation>
    <dct:source rdf:resource="http://data.landportal.info/dataset/FAO-LG"/>
    <sdmx-attribute:unitMeasure>Number</sdmx-attribute:unitMeasure>
    <rdfs:label>Total number of agricultural holders</rdfs:label>
    <skos:prefLabel>Total number of agricultural holders</skos:prefLabel>
    <dct:title>Total number of agricultural holders</dct:title>
    <skos:definition>Is the total number of Agricultural holders in a given country in a given year. The agricultural holder is defined as the person who makes the major decisions regarding resource use and exercises management control over the agricultural holding operation. The agricultural holder has technical and economic responsibility for the holding. The agricultural holding can be under single management or there may be more than one joint holder in a holding. A joint holder is a person making the major decisions regarding resource use and exercising management control over the agricultural holding operations, in conjunction with another person (Numbers of Holdings under Women and Men Co-Ownership).</skos:definition>
    <dct:description>Is the total number of Agricultural holders in a given country in a given year. The agricultural holder is defined as the person who makes the major decisions regarding resource use and exercises management control over the agricultural holding operation. The agricultural holder has technical and economic responsibility for the holding. The agricultural holding can be under single management or there may be more than one joint holder in a holding. A joint holder is a person making the major decisions regarding resource use and exercising management control over the agricultural holding operations, in conjunction with another person (Numbers of Holdings under Women and Men Co-Ownership).</dct:description>
    <rdfs:comment>Is the total number of Agricultural holders in a given country in a given year. The agricultural holder is defined as the person who makes the major decisions regarding resource use and exercises management control over the agricultural holding operation. The agricultural holder has technical and economic responsibility for the holding. The agricultural holding can be under single management or there may be more than one joint holder in a holding. A joint holder is a person making the major decisions regarding resource use and exercising management control over the agricultural holding operations, in conjunction with another person (Numbers of Holdings under Women and Men Co-Ownership).</rdfs:comment>
    <skos:inScheme rdf:resource="http://data.landportal.info/vocabulary/25"/>
    <rdfs:seeAlso rdf:resource="https://landportal.org/book/indicators/indfaogender3"/>
  </rdf:Description>

</rdf:RDF>