<?xml version="1.0" encoding="UTF-8"?>
<rdf:RDF xmlns:rdf="http://www.w3.org/1999/02/22-rdf-syntax-ns#"
  xmlns:dct="http://purl.org/dc/terms/"
  xmlns:schema="http://schema.org/"
  xmlns:skos="http://www.w3.org/2004/02/skos/core#"
  xmlns:sdmx-attribute="http://purl.org/linked-data/sdmx/2009/attribute#"
  xmlns:rdfs="http://www.w3.org/2000/01/rdf-schema#">

  <rdf:Description rdf:about="http://data.landportal.info/indicator/FAO-LG.1MA">
    <rdf:type rdf:resource="http://www.w3.org/2004/02/skos/core#Concept"/>
    <rdf:type rdf:resource="http://purl.org/weso/ontology/computex#Indicator"/>
    <dct:subject rdf:resource="http://aims.fao.org/aos/agrovoc/c_1dfe5bfe"/>
    <dct:subject rdf:resource="http://aims.fao.org/aos/agrovoc/c_9000090"/>
    <dct:subject rdf:resource="http://aims.fao.org/aos/agrovoc/c_28718"/>
    <dct:subject rdf:resource="http://aims.fao.org/aos/agrovoc/c_12069"/>
    <dct:subject rdf:resource="http://data.landportal.info/voc/landvoc/theme/T-GENDER"/>
    <schema:about rdf:resource="http://aims.fao.org/aos/agrovoc/c_1dfe5bfe"/>
    <schema:about rdf:resource="http://aims.fao.org/aos/agrovoc/c_9000090"/>
    <schema:about rdf:resource="http://aims.fao.org/aos/agrovoc/c_28718"/>
    <schema:about rdf:resource="http://aims.fao.org/aos/agrovoc/c_12069"/>
    <schema:about rdf:resource="http://data.landportal.info/voc/landvoc/theme/T-GENDER"/>
    <dct:identifier>FAO-LG.1MA</dct:identifier>
    <skos:notation>FAO-LG.1MA</skos:notation>
    <dct:source rdf:resource="http://data.landportal.info/dataset/FAO-LG"/>
    <sdmx-attribute:unitMeasure>Number</sdmx-attribute:unitMeasure>
    <rdfs:label>Agricultural holders by sex (male - total n)</rdfs:label>
    <skos:prefLabel>Agricultural holders by sex (male - total n)</skos:prefLabel>
    <dct:title>Agricultural holders by sex (male - total n)</dct:title>
    <skos:definition>Agricultural holders by sex (male - total n) according to the FAO Land and Gender Database.</skos:definition>
    <dct:description>Agricultural holders by sex (male - total n) according to the FAO Land and Gender Database.</dct:description>
    <rdfs:comment>Agricultural holders by sex (male - total n) according to the FAO Land and Gender Database.</rdfs:comment>
    <skos:inScheme rdf:resource="http://data.landportal.info/vocabulary/25"/>
    <rdfs:seeAlso rdf:resource="https://landportal.org/book/indicators/fao-lg1ma"/>
  </rdf:Description>

</rdf:RDF>