<?xml version="1.0" encoding="UTF-8"?>
<rdf:RDF xmlns:rdf="http://www.w3.org/1999/02/22-rdf-syntax-ns#"
  xmlns:dct="http://purl.org/dc/terms/"
  xmlns:schema="http://schema.org/"
  xmlns:skos="http://www.w3.org/2004/02/skos/core#"
  xmlns:sdmx-attribute="http://purl.org/linked-data/sdmx/2009/attribute#"
  xmlns:rdfs="http://www.w3.org/2000/01/rdf-schema#">

  <rdf:Description rdf:about="http://data.landportal.info/indicator/RRI-FTD-DGOV">
    <rdf:type rdf:resource="http://www.w3.org/2004/02/skos/core#Concept"/>
    <rdf:type rdf:resource="http://purl.org/weso/ontology/computex#Indicator"/>
    <dct:subject rdf:resource="http://aims.fao.org/aos/agrovoc/c_ff890f6b"/>
    <dct:subject rdf:resource="http://aims.fao.org/aos/agrovoc/c_24843"/>
    <dct:subject rdf:resource="http://aims.fao.org/aos/agrovoc/c_1374155312641"/>
    <dct:subject rdf:resource="http://aims.fao.org/aos/agrovoc/c_331524"/>
    <dct:subject rdf:resource="http://aims.fao.org/aos/agrovoc/c_aca7ac6d"/>
    <dct:subject rdf:resource="http://aims.fao.org/aos/agrovoc/c_45cd8441"/>
    <dct:subject rdf:resource="http://data.landportal.info/voc/landvoc/theme/T-FOREST"/>
    <dct:subject rdf:resource="http://data.landportal.info/voc/landvoc/theme/T-INDIG"/>
    <schema:about rdf:resource="http://aims.fao.org/aos/agrovoc/c_ff890f6b"/>
    <schema:about rdf:resource="http://aims.fao.org/aos/agrovoc/c_24843"/>
    <schema:about rdf:resource="http://aims.fao.org/aos/agrovoc/c_1374155312641"/>
    <schema:about rdf:resource="http://aims.fao.org/aos/agrovoc/c_331524"/>
    <schema:about rdf:resource="http://aims.fao.org/aos/agrovoc/c_aca7ac6d"/>
    <schema:about rdf:resource="http://aims.fao.org/aos/agrovoc/c_45cd8441"/>
    <schema:about rdf:resource="http://data.landportal.info/voc/landvoc/theme/T-FOREST"/>
    <schema:about rdf:resource="http://data.landportal.info/voc/landvoc/theme/T-INDIG"/>
    <dct:identifier>RRI-FTD-DGOV</dct:identifier>
    <skos:notation>RRI-FTD-DGOV</skos:notation>
    <dct:source rdf:resource="http://data.landportal.info/dataset/RRI-FTD"/>
    <sdmx-attribute:unitMeasure>Million ha</sdmx-attribute:unitMeasure>
    <rdfs:label>Forest land designated by governments for Indigenous Peoples and local communities</rdfs:label>
    <skos:prefLabel>Forest land designated by governments for Indigenous Peoples and local communities</skos:prefLabel>
    <dct:title>Forest land designated by governments for Indigenous Peoples and local communities</dct:title>
    <skos:definition>Forest land designated by governments for Indigenous Peoples and local communities: Ownership of forest land under this category remains claimed by the state but some rights have been recognized by governments on a conditional basis for Indigenous Peoples and local communities. While rights-holders have some level of “control” exercised through management and/or exclusion rights over forests, they lack the full legal means to ensure the security of their claims to forests (i.e. having all three rights to exclude, to due process and compensation, and to retain rights for an unlimited duration). Data are in million ha. See more at: http://rightsandresources.org/en/resources/tenure-data/the-four-categori...</skos:definition>
    <dct:description>Forest land designated by governments for Indigenous Peoples and local communities: Ownership of forest land under this category remains claimed by the state but some rights have been recognized by governments on a conditional basis for Indigenous Peoples and local communities. While rights-holders have some level of “control” exercised through management and/or exclusion rights over forests, they lack the full legal means to ensure the security of their claims to forests (i.e. having all three rights to exclude, to due process and compensation, and to retain rights for an unlimited duration). Data are in million ha. See more at: http://rightsandresources.org/en/resources/tenure-data/the-four-categori...</dct:description>
    <rdfs:comment>Forest land designated by governments for Indigenous Peoples and local communities: Ownership of forest land under this category remains claimed by the state but some rights have been recognized by governments on a conditional basis for Indigenous Peoples and local communities. While rights-holders have some level of “control” exercised through management and/or exclusion rights over forests, they lack the full legal means to ensure the security of their claims to forests (i.e. having all three rights to exclude, to due process and compensation, and to retain rights for an unlimited duration). Data are in million ha. See more at: http://rightsandresources.org/en/resources/tenure-data/the-four-categori...</rdfs:comment>
    <skos:inScheme rdf:resource="http://data.landportal.info/vocabulary/25"/>
    <rdfs:seeAlso rdf:resource="https://landportal.org/book/indicator/rri-ftd-dgov"/>
  </rdf:Description>

</rdf:RDF>