<?xml version="1.0" encoding="UTF-8"?>
<rdf:RDF xmlns:rdf="http://www.w3.org/1999/02/22-rdf-syntax-ns#"
  xmlns:dct="http://purl.org/dc/terms/"
  xmlns:schema="http://schema.org/"
  xmlns:skos="http://www.w3.org/2004/02/skos/core#"
  xmlns:sdmx-attribute="http://purl.org/linked-data/sdmx/2009/attribute#"
  xmlns:rdfs="http://www.w3.org/2000/01/rdf-schema#">

  <rdf:Description rdf:about="http://data.landportal.info/indicator/RRI-FTD-OWCOM">
    <rdf:type rdf:resource="http://www.w3.org/2004/02/skos/core#Concept"/>
    <rdf:type rdf:resource="http://purl.org/weso/ontology/computex#Indicator"/>
    <dct:subject rdf:resource="http://aims.fao.org/aos/agrovoc/c_24843"/>
    <dct:subject rdf:resource="http://aims.fao.org/aos/agrovoc/c_331524"/>
    <dct:subject rdf:resource="http://aims.fao.org/aos/agrovoc/c_aca7ac6d"/>
    <dct:subject rdf:resource="http://aims.fao.org/aos/agrovoc/c_28718"/>
    <dct:subject rdf:resource="http://aims.fao.org/aos/agrovoc/c_45cd8441"/>
    <dct:subject rdf:resource="http://aims.fao.org/aos/agrovoc/c_13609"/>
    <dct:subject rdf:resource="http://data.landportal.info/voc/landvoc/theme/T-FOREST"/>
    <dct:subject rdf:resource="http://data.landportal.info/voc/landvoc/theme/T-INDIG"/>
    <schema:about rdf:resource="http://aims.fao.org/aos/agrovoc/c_24843"/>
    <schema:about rdf:resource="http://aims.fao.org/aos/agrovoc/c_331524"/>
    <schema:about rdf:resource="http://aims.fao.org/aos/agrovoc/c_aca7ac6d"/>
    <schema:about rdf:resource="http://aims.fao.org/aos/agrovoc/c_28718"/>
    <schema:about rdf:resource="http://aims.fao.org/aos/agrovoc/c_45cd8441"/>
    <schema:about rdf:resource="http://aims.fao.org/aos/agrovoc/c_13609"/>
    <schema:about rdf:resource="http://data.landportal.info/voc/landvoc/theme/T-FOREST"/>
    <schema:about rdf:resource="http://data.landportal.info/voc/landvoc/theme/T-INDIG"/>
    <dct:identifier>RRI-FTD-OWCOM</dct:identifier>
    <skos:notation>RRI-FTD-OWCOM</skos:notation>
    <dct:source rdf:resource="http://data.landportal.info/dataset/RRI-FTD"/>
    <sdmx-attribute:unitMeasure>Million ha</sdmx-attribute:unitMeasure>
    <rdfs:label>Forest land owned by Indigenous Peoples and local communities</rdfs:label>
    <skos:prefLabel>Forest land owned by Indigenous Peoples and local communities</skos:prefLabel>
    <dct:title>Forest land owned by Indigenous Peoples and local communities</dct:title>
    <skos:definition>Forest land owned by Indigenous Peoples and local communities: Forests are considered to be “owned” where communities have full legal rights to secure their claims to forests, defined in RRI’s research as areas where community tenure is unlimited in duration, they have the legal right to exclude outsiders from using their resources, and they are entitled to due process and compensation in the face of potential extinguishment by the state of some or all of their rights. RRI does not consider alienation rights to be essential for community ownership. Data are in million ha. See more at: http://rightsandresources.org/en/resources/tenure-data/the-four-categori...</skos:definition>
    <dct:description>Forest land owned by Indigenous Peoples and local communities: Forests are considered to be “owned” where communities have full legal rights to secure their claims to forests, defined in RRI’s research as areas where community tenure is unlimited in duration, they have the legal right to exclude outsiders from using their resources, and they are entitled to due process and compensation in the face of potential extinguishment by the state of some or all of their rights. RRI does not consider alienation rights to be essential for community ownership. Data are in million ha. See more at: http://rightsandresources.org/en/resources/tenure-data/the-four-categori...</dct:description>
    <rdfs:comment>Forest land owned by Indigenous Peoples and local communities: Forests are considered to be “owned” where communities have full legal rights to secure their claims to forests, defined in RRI’s research as areas where community tenure is unlimited in duration, they have the legal right to exclude outsiders from using their resources, and they are entitled to due process and compensation in the face of potential extinguishment by the state of some or all of their rights. RRI does not consider alienation rights to be essential for community ownership. Data are in million ha. See more at: http://rightsandresources.org/en/resources/tenure-data/the-four-categori...</rdfs:comment>
    <skos:inScheme rdf:resource="http://data.landportal.info/vocabulary/25"/>
    <rdfs:seeAlso rdf:resource="https://landportal.org/book/indicator/rri-ftd-owcom"/>
  </rdf:Description>

</rdf:RDF>