<?xml version="1.0" encoding="UTF-8"?>
<rdf:RDF xmlns:rdf="http://www.w3.org/1999/02/22-rdf-syntax-ns#"
  xmlns:dct="http://purl.org/dc/terms/"
  xmlns:schema="http://schema.org/"
  xmlns:skos="http://www.w3.org/2004/02/skos/core#"
  xmlns:sdmx-attribute="http://purl.org/linked-data/sdmx/2009/attribute#"
  xmlns:rdfs="http://www.w3.org/2000/01/rdf-schema#">

  <rdf:Description rdf:about="http://data.landportal.info/indicator/UNEP-WCMC-DRY.ADD.DRYAREAS">
    <rdf:type rdf:resource="http://www.w3.org/2004/02/skos/core#Concept"/>
    <rdf:type rdf:resource="http://purl.org/weso/ontology/computex#Indicator"/>
    <dct:subject rdf:resource="http://aims.fao.org/aos/agrovoc/c_16112"/>
    <dct:subject rdf:resource="http://aims.fao.org/aos/agrovoc/c_8e487587"/>
    <dct:subject rdf:resource="http://aims.fao.org/aos/agrovoc/c_6448"/>
    <dct:subject rdf:resource="http://data.landportal.info/voc/landvoc/theme/T-ENVIR"/>
    <dct:subject rdf:resource="http://data.landportal.info/voc/landvoc/theme/T-PASTOR"/>
    <schema:about rdf:resource="http://aims.fao.org/aos/agrovoc/c_16112"/>
    <schema:about rdf:resource="http://aims.fao.org/aos/agrovoc/c_8e487587"/>
    <schema:about rdf:resource="http://aims.fao.org/aos/agrovoc/c_6448"/>
    <schema:about rdf:resource="http://data.landportal.info/voc/landvoc/theme/T-ENVIR"/>
    <schema:about rdf:resource="http://data.landportal.info/voc/landvoc/theme/T-PASTOR"/>
    <dct:identifier>UNEP-WCMC-DRY.ADD.DRYAREAS</dct:identifier>
    <skos:notation>UNEP-WCMC-DRY.ADD.DRYAREAS</skos:notation>
    <dct:source rdf:resource="http://data.landportal.info/dataset/UNEP-WCMC-DRY"/>
    <sdmx-attribute:unitMeasure>Sq Km</sdmx-attribute:unitMeasure>
    <rdfs:label>Drylands - Additional dryland areas</rdfs:label>
    <skos:prefLabel>Drylands - Additional dryland areas</skos:prefLabel>
    <dct:title>Drylands - Additional dryland areas</dct:title>
    <skos:definition>This indicator measures the total dryland area (in sq. km) that can be defined as additional dryland area, in a given country. Additional drylands areas include areas that might not fall - based on the ratio of precipitation to potential evapotranspiration (P/PET) - within the intervals traditionally used to identify arid (0.06 - 0.20 P/PET), semiarid (0.21 - 0.50 P/PET) and subhumid areas (0.51 - 0.65 P/PET). Based on expert knowledge, the following ecoregions are likely to include dryland and dry-subhumid features: Selenge-Orkhon forest steppe Tian Shan montane steppe and meadows Northwestern Himalayan alpine shrub and meadows Central Tibetan Plateau alpine steppe Southeast Tibet shrublands and meadows Pamir alpine desert and tundra Yarlung Tsangpo arid steppe Hawaii tropical low shrublands North Tibetan Plateau-Kunlun Mountains alpine desert Hawaii tropical high shrublands, Maputaland-Pondoland bushland and thickets Ascension scrub and grasslands Drakensberg alti-montane grasslands and woodlands   The values of this indicator have been aggregated at the country level by ILRI, in collaboration with the ILC's Rangelands initiative, based on: UNEP-WCMC (2007): A spatial analysis approach to the global delineation of dryland areas of relevance to the CBD Programme of Work on Dry and Subhumid Lands. Dataset based on spatial analysis between WWF terrestrial ecoregions (WWF-US, 2004) and aridity zones (CRU/UEA; UNEPGRID, 1991). Dataset checked and refined to remove many gaps, overlaps and slivers (July 2014).</skos:definition>
    <dct:description>This indicator measures the total dryland area (in sq. km) that can be defined as additional dryland area, in a given country. Additional drylands areas include areas that might not fall - based on the ratio of precipitation to potential evapotranspiration (P/PET) - within the intervals traditionally used to identify arid (0.06 - 0.20 P/PET), semiarid (0.21 - 0.50 P/PET) and subhumid areas (0.51 - 0.65 P/PET). Based on expert knowledge, the following ecoregions are likely to include dryland and dry-subhumid features: Selenge-Orkhon forest steppe Tian Shan montane steppe and meadows Northwestern Himalayan alpine shrub and meadows Central Tibetan Plateau alpine steppe Southeast Tibet shrublands and meadows Pamir alpine desert and tundra Yarlung Tsangpo arid steppe Hawaii tropical low shrublands North Tibetan Plateau-Kunlun Mountains alpine desert Hawaii tropical high shrublands, Maputaland-Pondoland bushland and thickets Ascension scrub and grasslands Drakensberg alti-montane grasslands and woodlands   The values of this indicator have been aggregated at the country level by ILRI, in collaboration with the ILC's Rangelands initiative, based on: UNEP-WCMC (2007): A spatial analysis approach to the global delineation of dryland areas of relevance to the CBD Programme of Work on Dry and Subhumid Lands. Dataset based on spatial analysis between WWF terrestrial ecoregions (WWF-US, 2004) and aridity zones (CRU/UEA; UNEPGRID, 1991). Dataset checked and refined to remove many gaps, overlaps and slivers (July 2014).</dct:description>
    <rdfs:comment>This indicator measures the total dryland area (in sq. km) that can be defined as additional dryland area, in a given country. Additional drylands areas include areas that might not fall - based on the ratio of precipitation to potential evapotranspiration (P/PET) - within the intervals traditionally used to identify arid (0.06 - 0.20 P/PET), semiarid (0.21 - 0.50 P/PET) and subhumid areas (0.51 - 0.65 P/PET). Based on expert knowledge, the following ecoregions are likely to include dryland and dry-subhumid features: Selenge-Orkhon forest steppe Tian Shan montane steppe and meadows Northwestern Himalayan alpine shrub and meadows Central Tibetan Plateau alpine steppe Southeast Tibet shrublands and meadows Pamir alpine desert and tundra Yarlung Tsangpo arid steppe Hawaii tropical low shrublands North Tibetan Plateau-Kunlun Mountains alpine desert Hawaii tropical high shrublands, Maputaland-Pondoland bushland and thickets Ascension scrub and grasslands Drakensberg alti-montane grasslands and woodlands   The values of this indicator have been aggregated at the country level by ILRI, in collaboration with the ILC's Rangelands initiative, based on: UNEP-WCMC (2007): A spatial analysis approach to the global delineation of dryland areas of relevance to the CBD Programme of Work on Dry and Subhumid Lands. Dataset based on spatial analysis between WWF terrestrial ecoregions (WWF-US, 2004) and aridity zones (CRU/UEA; UNEPGRID, 1991). Dataset checked and refined to remove many gaps, overlaps and slivers (July 2014).</rdfs:comment>
    <skos:inScheme rdf:resource="http://data.landportal.info/vocabulary/25"/>
    <rdfs:seeAlso rdf:resource="https://landportal.org/book/indicator/unep-wcmc-dryadddryareas"/>
  </rdf:Description>

</rdf:RDF>