<?xml version="1.0" encoding="UTF-8"?>
<rdf:RDF xmlns:rdf="http://www.w3.org/1999/02/22-rdf-syntax-ns#"
  xmlns:dct="http://purl.org/dc/terms/"
  xmlns:schema="http://schema.org/"
  xmlns:skos="http://www.w3.org/2004/02/skos/core#"
  xmlns:sdmx-attribute="http://purl.org/linked-data/sdmx/2009/attribute#"
  xmlns:rdfs="http://www.w3.org/2000/01/rdf-schema#">

  <rdf:Description rdf:about="http://data.landportal.info/indicator/WF-ODB.RANKING">
    <rdf:type rdf:resource="http://www.w3.org/2004/02/skos/core#Concept"/>
    <rdf:type rdf:resource="http://purl.org/weso/ontology/computex#Indicator"/>
    <dct:subject rdf:resource="https://landportal.org/voc/landvoc/concept/open-data"/>
    <dct:subject rdf:resource="http://data.landportal.info/voc/landvoc/theme/T-SOCEC"/>
    <schema:about rdf:resource="https://landportal.org/voc/landvoc/concept/open-data"/>
    <schema:about rdf:resource="http://data.landportal.info/voc/landvoc/theme/T-SOCEC"/>
    <dct:identifier>WF-ODB.RANKING</dct:identifier>
    <skos:notation>WF-ODB.RANKING</skos:notation>
    <dct:source rdf:resource="http://data.landportal.info/dataset/WF-ODB"/>
    <sdmx-attribute:unitMeasure>Rank</sdmx-attribute:unitMeasure>
    <rdfs:label>Open Data Barometer - Ranking</rdfs:label>
    <skos:prefLabel>Open Data Barometer - Ranking</skos:prefLabel>
    <dct:title>Open Data Barometer - Ranking</dct:title>
    <skos:definition>The Open Data Barometer (ODB) aggregates data from a number of different sources that uncover the true prevalence and impact of open data initiatives around the world. This indicator uses the ODB scores calculated every year to rank countries based on the level of how governments are publishing and using open data for accountability, innovation and social impact (the country with the best level is ranked number one).</skos:definition>
    <dct:description>The Open Data Barometer (ODB) aggregates data from a number of different sources that uncover the true prevalence and impact of open data initiatives around the world. This indicator uses the ODB scores calculated every year to rank countries based on the level of how governments are publishing and using open data for accountability, innovation and social impact (the country with the best level is ranked number one).</dct:description>
    <rdfs:comment>The Open Data Barometer (ODB) aggregates data from a number of different sources that uncover the true prevalence and impact of open data initiatives around the world. This indicator uses the ODB scores calculated every year to rank countries based on the level of how governments are publishing and using open data for accountability, innovation and social impact (the country with the best level is ranked number one).</rdfs:comment>
    <skos:inScheme rdf:resource="http://data.landportal.info/vocabulary/25"/>
    <rdfs:seeAlso rdf:resource="https://landportal.org/book/indicator/wf-odbranking"/>
  </rdf:Description>

</rdf:RDF>