<?xml version="1.0" encoding="UTF-8"?>
<rdf:RDF xmlns:rdf="http://www.w3.org/1999/02/22-rdf-syntax-ns#"
  xmlns:dct="http://purl.org/dc/terms/"
  xmlns:schema="http://schema.org/"
  xmlns:skos="http://www.w3.org/2004/02/skos/core#"
  xmlns:sdmx-attribute="http://purl.org/linked-data/sdmx/2009/attribute#"
  xmlns:rdfs="http://www.w3.org/2000/01/rdf-schema#">

  <rdf:Description rdf:about="http://data.landportal.info/indicator/WF-ODB.SCORE">
    <rdf:type rdf:resource="http://www.w3.org/2004/02/skos/core#Concept"/>
    <rdf:type rdf:resource="http://purl.org/weso/ontology/computex#Indicator"/>
    <dct:subject rdf:resource="http://data.landportal.info/voc/landvoc/theme/T-SOCEC"/>
    <dct:subject rdf:resource="https://landportal.org/voc/landvoc/concept/open-data"/>
    <schema:about rdf:resource="http://data.landportal.info/voc/landvoc/theme/T-SOCEC"/>
    <schema:about rdf:resource="https://landportal.org/voc/landvoc/concept/open-data"/>
    <dct:identifier>WF-ODB.SCORE</dct:identifier>
    <skos:notation>WF-ODB.SCORE</skos:notation>
    <dct:source rdf:resource="http://data.landportal.info/dataset/WF-ODB"/>
    <sdmx-attribute:unitMeasure>Index (0; 100)</sdmx-attribute:unitMeasure>
    <rdfs:label>Open Data Barometer - Score</rdfs:label>
    <skos:prefLabel>Open Data Barometer - Score</skos:prefLabel>
    <dct:title>Open Data Barometer - Score</dct:title>
    <skos:definition>The Open Data Barometer (ODB) aggregates data from a number of different sources that uncover the true prevalence and impact of open data initiatives around the world.  The indicator ranges from 0 (worst possible score) to 100 (best possible score) how governments are publishing and using open data for accountability, innovation and social impact.</skos:definition>
    <dct:description>The Open Data Barometer (ODB) aggregates data from a number of different sources that uncover the true prevalence and impact of open data initiatives around the world.  The indicator ranges from 0 (worst possible score) to 100 (best possible score) how governments are publishing and using open data for accountability, innovation and social impact.</dct:description>
    <rdfs:comment>The Open Data Barometer (ODB) aggregates data from a number of different sources that uncover the true prevalence and impact of open data initiatives around the world.  The indicator ranges from 0 (worst possible score) to 100 (best possible score) how governments are publishing and using open data for accountability, innovation and social impact.</rdfs:comment>
    <skos:inScheme rdf:resource="http://data.landportal.info/vocabulary/25"/>
    <rdfs:seeAlso rdf:resource="https://landportal.org/book/indicator/wf-odbscore"/>
  </rdf:Description>

</rdf:RDF>