<?xml version="1.0" encoding="UTF-8"?>
<rdf:RDF xmlns:rdf="http://www.w3.org/1999/02/22-rdf-syntax-ns#"
  xmlns:dct="http://purl.org/dc/terms/"
  xmlns:skos="http://www.w3.org/2004/02/skos/core#"
  xmlns:sdmx-attribute="http://purl.org/linked-data/sdmx/2009/attribute#"
  xmlns:schema="http://schema.org/"
  xmlns:rdfs="http://www.w3.org/2000/01/rdf-schema#">

  <rdf:Description rdf:about="http://data.landportal.info/indicator/UN-PD_AGR_SSFP">
    <rdf:type rdf:resource="http://www.w3.org/2004/02/skos/core#Concept"/>
    <rdf:type rdf:resource="http://purl.org/weso/ontology/computex#Indicator"/>
    <dct:source rdf:resource="http://data.landportal.info/dataset/UN-SDG_2.3.1"/>
    <dct:identifier>UN-PD_AGR_SSFP</dct:identifier>
    <skos:notation>UN-PD_AGR_SSFP</skos:notation>
    <sdmx-attribute:unitMeasure>Constant 2011 international $</sdmx-attribute:unitMeasure>
    <dct:subject rdf:resource="http://data.landportal.info/voc/landvoc/theme/T-FOOD"/>
    <dct:subject rdf:resource="http://data.landportal.info/voc/landvoc/theme/T-INST"/>
    <dct:subject rdf:resource="http://data.landportal.info/voc/landvoc/theme/T-SOCEC"/>
    <schema:about rdf:resource="http://data.landportal.info/voc/landvoc/theme/T-FOOD"/>
    <schema:about rdf:resource="http://data.landportal.info/voc/landvoc/theme/T-INST"/>
    <schema:about rdf:resource="http://data.landportal.info/voc/landvoc/theme/T-SOCEC"/>
    <rdfs:label>Productivity of small-scale food producers (agricultural output per labour day, PPP) (constant 2011 international $)</rdfs:label>
    <skos:prefLabel>Productivity of small-scale food producers (agricultural output per labour day, PPP) (constant 2011 international $)</skos:prefLabel>
    <dct:title>Productivity of small-scale food producers (agricultural output per labour day, PPP) (constant 2011 international $)</dct:title>
    <skos:definition>/*--&gt;*/ The data series presented here measures the average productivity of small-scale food producers (agricultural output per labour day, PPP) (constant 2011 international $). This data series contributes to the measurement of SDG Indicator 2.3.1, classified as Tier II in September 2018, which is officially defined as the &quot;Volume of agricultural production of small-scale food producer in crop, livestock, fisheries, and forestry activities per number of days. The indicator is computed as a ratio of annual output to the number of working days in one year&quot;. According to FAO -- the Custodian Agency for this indicator -- the rationale behind this indicator can be summarised as follows: The 2030 Sustainable Development Agenda has emphasized the importance of enhancing productivity of small-scale food producers, as these producers play an important role in the global production of food.The indicator monitors progress in this area, where the target is to double productivity by year 2030. The enhancement of labour productivity in small-scale production units also has implications on poverty reduction, as small-scale food producers are often poor, and are frequently found to be close to subsistence conditions. The full official metadata for this Tier II indicator are available at UN SDG Metadata website. For more information, check also this indicator's page on Land Portal SDG porfolio. For more information on this data series, please visit UN SDG website.</skos:definition>
    <dct:description>/*--&gt;*/ The data series presented here measures the average productivity of small-scale food producers (agricultural output per labour day, PPP) (constant 2011 international $). This data series contributes to the measurement of SDG Indicator 2.3.1, classified as Tier II in September 2018, which is officially defined as the &quot;Volume of agricultural production of small-scale food producer in crop, livestock, fisheries, and forestry activities per number of days. The indicator is computed as a ratio of annual output to the number of working days in one year&quot;. According to FAO -- the Custodian Agency for this indicator -- the rationale behind this indicator can be summarised as follows: The 2030 Sustainable Development Agenda has emphasized the importance of enhancing productivity of small-scale food producers, as these producers play an important role in the global production of food.The indicator monitors progress in this area, where the target is to double productivity by year 2030. The enhancement of labour productivity in small-scale production units also has implications on poverty reduction, as small-scale food producers are often poor, and are frequently found to be close to subsistence conditions. The full official metadata for this Tier II indicator are available at UN SDG Metadata website. For more information, check also this indicator's page on Land Portal SDG porfolio. For more information on this data series, please visit UN SDG website.</dct:description>
    <rdfs:comment>/*--&gt;*/ The data series presented here measures the average productivity of small-scale food producers (agricultural output per labour day, PPP) (constant 2011 international $). This data series contributes to the measurement of SDG Indicator 2.3.1, classified as Tier II in September 2018, which is officially defined as the &quot;Volume of agricultural production of small-scale food producer in crop, livestock, fisheries, and forestry activities per number of days. The indicator is computed as a ratio of annual output to the number of working days in one year&quot;. According to FAO -- the Custodian Agency for this indicator -- the rationale behind this indicator can be summarised as follows: The 2030 Sustainable Development Agenda has emphasized the importance of enhancing productivity of small-scale food producers, as these producers play an important role in the global production of food.The indicator monitors progress in this area, where the target is to double productivity by year 2030. The enhancement of labour productivity in small-scale production units also has implications on poverty reduction, as small-scale food producers are often poor, and are frequently found to be close to subsistence conditions. The full official metadata for this Tier II indicator are available at UN SDG Metadata website. For more information, check also this indicator's page on Land Portal SDG porfolio. For more information on this data series, please visit UN SDG website.</rdfs:comment>
    <skos:inScheme rdf:resource="http://data.landportal.info/vocabulary/25"/>
    <rdfs:seeAlso rdf:resource="https://landportal.org/book/indicator/un-pdagrssfp"/>
  </rdf:Description>

</rdf:RDF>