<?xml version="1.0" encoding="UTF-8"?>
<rdf:RDF xmlns:rdf="http://www.w3.org/1999/02/22-rdf-syntax-ns#"
  xmlns:dct="http://purl.org/dc/terms/"
  xmlns:schema="http://schema.org/"
  xmlns:skos="http://www.w3.org/2004/02/skos/core#"
  xmlns:sdmx-attribute="http://purl.org/linked-data/sdmx/2009/attribute#"
  xmlns:rdfs="http://www.w3.org/2000/01/rdf-schema#">

  <rdf:Description rdf:about="http://data.landportal.info/indicator/UN-ER_PTD_TERRS">
    <rdf:type rdf:resource="http://www.w3.org/2004/02/skos/core#Concept"/>
    <rdf:type rdf:resource="http://purl.org/weso/ontology/computex#Indicator"/>
    <dct:subject rdf:resource="http://data.landportal.info/voc/landvoc/theme/T-FLR"/>
    <dct:subject rdf:resource="http://data.landportal.info/voc/landvoc/theme/T-ENVIR"/>
    <schema:about rdf:resource="http://data.landportal.info/voc/landvoc/theme/T-FLR"/>
    <schema:about rdf:resource="http://data.landportal.info/voc/landvoc/theme/T-ENVIR"/>
    <dct:identifier>UN-ER_PTD_TERRS</dct:identifier>
    <skos:notation>UN-ER_PTD_TERRS</skos:notation>
    <dct:source rdf:resource="http://data.landportal.info/dataset/UN-SDG_15.1.2"/>
    <sdmx-attribute:unitMeasure>Percentage (%)</sdmx-attribute:unitMeasure>
    <rdfs:label>Average proportion of Terrestrial Key Biodiversity Areas (KBAs) covered by protected areas (%)</rdfs:label>
    <skos:prefLabel>Average proportion of Terrestrial Key Biodiversity Areas (KBAs) covered by protected areas (%)</skos:prefLabel>
    <dct:title>Average proportion of Terrestrial Key Biodiversity Areas (KBAs) covered by protected areas (%)</dct:title>
    <skos:definition>The data series presented here measures the average proportion of Terrestrial Key Biodiversity Areas (KBAs) covered by protected areas (%). This data series contributes to the measurement of SDG Indicator 15.1.2, classified as Tier I in September 2018, which is officially defined as follows: Proportion of important sites for terrestrial and freshwater biodiversity that are covered by protected areas shows temporal trends in the mean percentage of each important site for terrestrial and freshwater biodiversity (i.e., those that contribute significantly to the global persistence of biodiversity) that is covered by designated protected areas.  According to Food and Agriculture Organization of the United Nations (FAO) -- the Custodian Agency for this indicator -- the rationale behind this indicator can be summarised as follows:  The safeguard of important sites is vital for stemming the decline in biodiversity and ensuring long term and sustainable use of terrestrial and freshwater natural resources. The establishment of protected areas is an important mechanism for achieving this aim, and this indicator serves as a means of measuring progress toward the conservation, restoration and sustainable use of terrestrial and freshwater ecosystems and their services, in particular forests, wetlands, mountains and drylands, in line with obligations under international agreements. Importantly, while it can be disaggregated to report on any given single ecosystem of interest (e.g., forests), it is not restricted to any single ecosystem type, and so faithfully reflects the intent of SDG target 15.1 The full official metadata for this Tier I indicator are available at UN SDG Metadata website. For more information, check also this indicator's page on Land Portal SDG porfolio. For more information on this data series, please visit UN SDG website.</skos:definition>
    <dct:description>The data series presented here measures the average proportion of Terrestrial Key Biodiversity Areas (KBAs) covered by protected areas (%). This data series contributes to the measurement of SDG Indicator 15.1.2, classified as Tier I in September 2018, which is officially defined as follows: Proportion of important sites for terrestrial and freshwater biodiversity that are covered by protected areas shows temporal trends in the mean percentage of each important site for terrestrial and freshwater biodiversity (i.e., those that contribute significantly to the global persistence of biodiversity) that is covered by designated protected areas.  According to Food and Agriculture Organization of the United Nations (FAO) -- the Custodian Agency for this indicator -- the rationale behind this indicator can be summarised as follows:  The safeguard of important sites is vital for stemming the decline in biodiversity and ensuring long term and sustainable use of terrestrial and freshwater natural resources. The establishment of protected areas is an important mechanism for achieving this aim, and this indicator serves as a means of measuring progress toward the conservation, restoration and sustainable use of terrestrial and freshwater ecosystems and their services, in particular forests, wetlands, mountains and drylands, in line with obligations under international agreements. Importantly, while it can be disaggregated to report on any given single ecosystem of interest (e.g., forests), it is not restricted to any single ecosystem type, and so faithfully reflects the intent of SDG target 15.1 The full official metadata for this Tier I indicator are available at UN SDG Metadata website. For more information, check also this indicator's page on Land Portal SDG porfolio. For more information on this data series, please visit UN SDG website.</dct:description>
    <rdfs:comment>The data series presented here measures the average proportion of Terrestrial Key Biodiversity Areas (KBAs) covered by protected areas (%). This data series contributes to the measurement of SDG Indicator 15.1.2, classified as Tier I in September 2018, which is officially defined as follows: Proportion of important sites for terrestrial and freshwater biodiversity that are covered by protected areas shows temporal trends in the mean percentage of each important site for terrestrial and freshwater biodiversity (i.e., those that contribute significantly to the global persistence of biodiversity) that is covered by designated protected areas.  According to Food and Agriculture Organization of the United Nations (FAO) -- the Custodian Agency for this indicator -- the rationale behind this indicator can be summarised as follows:  The safeguard of important sites is vital for stemming the decline in biodiversity and ensuring long term and sustainable use of terrestrial and freshwater natural resources. The establishment of protected areas is an important mechanism for achieving this aim, and this indicator serves as a means of measuring progress toward the conservation, restoration and sustainable use of terrestrial and freshwater ecosystems and their services, in particular forests, wetlands, mountains and drylands, in line with obligations under international agreements. Importantly, while it can be disaggregated to report on any given single ecosystem of interest (e.g., forests), it is not restricted to any single ecosystem type, and so faithfully reflects the intent of SDG target 15.1 The full official metadata for this Tier I indicator are available at UN SDG Metadata website. For more information, check also this indicator's page on Land Portal SDG porfolio. For more information on this data series, please visit UN SDG website.</rdfs:comment>
    <skos:inScheme rdf:resource="http://data.landportal.info/vocabulary/25"/>
    <rdfs:seeAlso rdf:resource="https://landportal.org/book/indicator/un-erptdterrs"/>
  </rdf:Description>

</rdf:RDF>